<?xml version="1.0"?>
<rdf:RDF xmlns="https://w3id.org/def/propaphen/"
     xml:base="https://w3id.org/def/propaphen/"
     xmlns:dc="http://purl.org/dc/elements/1.1/"
     xmlns:ns="http://creativecommons.org/ns#"
     xmlns:ns1="http://www.w3.org/2003/06/sw-vocab-status/ns#"
     xmlns:owl="http://www.w3.org/2002/07/owl#"
     xmlns:rdf="http://www.w3.org/1999/02/22-rdf-syntax-ns#"
     xmlns:xml="http://www.w3.org/XML/1998/namespace"
     xmlns:xsd="http://www.w3.org/2001/XMLSchema#"
     xmlns:adms="http://www.w3.org/ns/adms#"
     xmlns:gufo="http://purl.org/nemo/gufo#"
     xmlns:rdfs="http://www.w3.org/2000/01/rdf-schema#"
     xmlns:seas="https://w3id.org/seas/"
     xmlns:skos="http://www.w3.org/2004/02/skos/core#"
     xmlns:swrl="http://www.w3.org/2003/11/swrl#"
     xmlns:time="http://www.w3.org/2006/time#"
     xmlns:vann="http://purl.org/vocab/vann/"
     xmlns:swrla="http://swrl.stanford.edu/ontologies/3.3/swrla.owl#"
     xmlns:swrlb="http://www.w3.org/2003/11/swrlb#"
     xmlns:terms="http://purl.org/dc/terms/"
     xmlns:geosparql="http://www.opengis.net/ont/geosparql#"
     xmlns:propaphen="https://w3id.org/def/propaphen#"
     xmlns:wgs84_pos="http://www.w3.org/2003/01/geo/wgs84_pos#">
    <owl:Ontology rdf:about="https://w3id.org/def/propaphen">
        <owl:versionIRI rdf:resource="https://w3id.org/def/propaphen/1.0.0"/>
        <owl:imports rdf:resource="http://purl.org/nemo/gufo#/1.0.0"/>
        <owl:imports rdf:resource="http://www.opengis.net/ont/geosparql"/>
        <owl:imports rdf:resource="http://www.opengis.net/ont/sf"/>
        <owl:imports rdf:resource="http://www.w3.org/2006/time#2016"/>
        <owl:imports rdf:resource="https://w3id.org/seas/SystemOntology-1.1"/>
        <dc:creator>Alencar Medeiros, Gabriel H.</dc:creator>
        <dc:creator>Soualmia, Lina F.</dc:creator>
        <dc:creator>Zanni-Merk, Cecilia</dc:creator>
        <dc:title>PropaPhen : Core Propagation Phenomenon Ontology</dc:title>
        <terms:contributor>mailto:gabriel-henrique.alencar-medeiros@univ-rouen.fr</terms:contributor>
        <terms:created>Wed November 22, 2023</terms:created>
        <terms:creator rdf:resource="https://orcid.org/0000-0002-4594-5492"/>
        <terms:license>https://opensource.org/license/mit/</terms:license>
        <terms:modified>Wed November 28, 2023</terms:modified>
        <vann:preferredNamespacePrefix>propaphen</vann:preferredNamespacePrefix>
        <vann:preferredNamespaceUri>https://w3id.org/def/propaphen</vann:preferredNamespaceUri>
        <rdfs:comment>The Core Propagation Phenomenon Ontology (PropaPhen) is designed to represent the propagation of any phenomenon in a network, leveraging the spatiotemporal characteristics of propagation from different observation points, with the participation of multiple entities in the process. This ontology will be used in the future in a broader framework for describing, detecting, and predicting the spread of health risks in a network based on heterogeneous textual data.</rdfs:comment>
        <owl:priorVersion>1.0.0</owl:priorVersion>
        <owl:versionInfo>1.0.0</owl:versionInfo>
    </owl:Ontology>
    


    <!-- 
    ///////////////////////////////////////////////////////////////////////////////////////
    //
    // Annotation properties
    //
    ///////////////////////////////////////////////////////////////////////////////////////
     -->

    


    <!-- http://purl.org/dc/elements/1.1/contributor -->

    <owl:AnnotationProperty rdf:about="http://purl.org/dc/elements/1.1/contributor"/>
    


    <!-- http://purl.org/dc/elements/1.1/creator -->

    <owl:AnnotationProperty rdf:about="http://purl.org/dc/elements/1.1/creator"/>
    


    <!-- http://purl.org/dc/elements/1.1/date -->

    <owl:AnnotationProperty rdf:about="http://purl.org/dc/elements/1.1/date"/>
    


    <!-- http://purl.org/dc/elements/1.1/description -->

    <owl:AnnotationProperty rdf:about="http://purl.org/dc/elements/1.1/description"/>
    


    <!-- http://purl.org/dc/elements/1.1/source -->

    <owl:AnnotationProperty rdf:about="http://purl.org/dc/elements/1.1/source"/>
    


    <!-- http://purl.org/dc/elements/1.1/title -->

    <owl:AnnotationProperty rdf:about="http://purl.org/dc/elements/1.1/title"/>
    


    <!-- http://purl.org/dc/terms/bibliographicCitation -->

    <owl:AnnotationProperty rdf:about="http://purl.org/dc/terms/bibliographicCitation"/>
    


    <!-- http://purl.org/dc/terms/contributor -->

    <owl:AnnotationProperty rdf:about="http://purl.org/dc/terms/contributor"/>
    


    <!-- http://purl.org/dc/terms/created -->

    <owl:AnnotationProperty rdf:about="http://purl.org/dc/terms/created"/>
    


    <!-- http://purl.org/dc/terms/creator -->

    <owl:AnnotationProperty rdf:about="http://purl.org/dc/terms/creator"/>
    


    <!-- http://purl.org/dc/terms/description -->

    <owl:AnnotationProperty rdf:about="http://purl.org/dc/terms/description"/>
    


    <!-- http://purl.org/dc/terms/isVersionOf -->

    <owl:AnnotationProperty rdf:about="http://purl.org/dc/terms/isVersionOf"/>
    


    <!-- http://purl.org/dc/terms/issued -->

    <owl:AnnotationProperty rdf:about="http://purl.org/dc/terms/issued"/>
    


    <!-- http://purl.org/dc/terms/license -->

    <owl:AnnotationProperty rdf:about="http://purl.org/dc/terms/license"/>
    


    <!-- http://purl.org/dc/terms/modified -->

    <owl:AnnotationProperty rdf:about="http://purl.org/dc/terms/modified"/>
    


    <!-- http://purl.org/dc/terms/rights -->

    <owl:AnnotationProperty rdf:about="http://purl.org/dc/terms/rights"/>
    


    <!-- http://purl.org/dc/terms/title -->

    <owl:AnnotationProperty rdf:about="http://purl.org/dc/terms/title"/>
    


    <!-- http://purl.org/vocab/vann/preferredNamespacePrefix -->

    <owl:AnnotationProperty rdf:about="http://purl.org/vocab/vann/preferredNamespacePrefix"/>
    


    <!-- http://purl.org/vocab/vann/preferredNamespaceUri -->

    <owl:AnnotationProperty rdf:about="http://purl.org/vocab/vann/preferredNamespaceUri"/>
    


    <!-- http://swrl.stanford.edu/ontologies/3.3/swrla.owl#isRuleEnabled -->

    <owl:AnnotationProperty rdf:about="http://swrl.stanford.edu/ontologies/3.3/swrla.owl#isRuleEnabled"/>
    


    <!-- http://www.w3.org/2001/XMLSchema#pattern -->

    <owl:AnnotationProperty rdf:about="http://www.w3.org/2001/XMLSchema#pattern"/>
    


    <!-- http://www.w3.org/2003/06/sw-vocab-status/ns#term_status -->

    <owl:AnnotationProperty rdf:about="http://www.w3.org/2003/06/sw-vocab-status/ns#term_status"/>
    


    <!-- http://www.w3.org/2004/02/skos/core#altLabel -->

    <owl:AnnotationProperty rdf:about="http://www.w3.org/2004/02/skos/core#altLabel">
        <rdfs:comment xml:lang="en">The range of skos:altLabel is the class of RDF plain literals.</rdfs:comment>
        <rdfs:comment xml:lang="en">skos:prefLabel, skos:altLabel and skos:hiddenLabel are pairwise disjoint properties.</rdfs:comment>
        <rdfs:isDefinedBy rdf:resource="http://www.w3.org/2004/02/skos/core"/>
        <rdfs:label xml:lang="en">alternative label</rdfs:label>
        <skos:definition xml:lang="en">An alternative lexical label for a resource.</skos:definition>
        <skos:example xml:lang="en">Acronyms, abbreviations, spelling variants, and irregular plural/singular forms may be included among the alternative labels for a concept. Mis-spelled terms are normally included as hidden labels (see skos:hiddenLabel).</skos:example>
        <rdfs:subPropertyOf rdf:resource="http://www.w3.org/2000/01/rdf-schema#label"/>
    </owl:AnnotationProperty>
    


    <!-- http://www.w3.org/2004/02/skos/core#changeNote -->

    <owl:AnnotationProperty rdf:about="http://www.w3.org/2004/02/skos/core#changeNote">
        <rdfs:isDefinedBy rdf:resource="http://www.w3.org/2004/02/skos/core"/>
        <rdfs:label xml:lang="en">change note</rdfs:label>
        <skos:definition xml:lang="en">A note about a modification to a concept.</skos:definition>
        <rdfs:subPropertyOf rdf:resource="http://www.w3.org/2004/02/skos/core#note"/>
    </owl:AnnotationProperty>
    


    <!-- http://www.w3.org/2004/02/skos/core#definition -->

    <owl:AnnotationProperty rdf:about="http://www.w3.org/2004/02/skos/core#definition">
        <rdfs:isDefinedBy rdf:resource="http://www.w3.org/2004/02/skos/core"/>
        <rdfs:label xml:lang="en">definition</rdfs:label>
        <skos:definition xml:lang="en">A statement or formal explanation of the meaning of a concept.</skos:definition>
        <rdfs:subPropertyOf rdf:resource="http://www.w3.org/2004/02/skos/core#note"/>
    </owl:AnnotationProperty>
    


    <!-- http://www.w3.org/2004/02/skos/core#editorialNote -->

    <owl:AnnotationProperty rdf:about="http://www.w3.org/2004/02/skos/core#editorialNote">
        <rdfs:isDefinedBy rdf:resource="http://www.w3.org/2004/02/skos/core"/>
        <rdfs:label xml:lang="en">editorial note</rdfs:label>
        <skos:definition xml:lang="en">A note for an editor, translator or maintainer of the vocabulary.</skos:definition>
        <rdfs:subPropertyOf rdf:resource="http://www.w3.org/2004/02/skos/core#note"/>
    </owl:AnnotationProperty>
    


    <!-- http://www.w3.org/2004/02/skos/core#example -->

    <owl:AnnotationProperty rdf:about="http://www.w3.org/2004/02/skos/core#example">
        <rdfs:isDefinedBy rdf:resource="http://www.w3.org/2004/02/skos/core"/>
        <rdfs:label xml:lang="en">example</rdfs:label>
        <skos:definition xml:lang="en">An example of the use of a concept.</skos:definition>
        <rdfs:subPropertyOf rdf:resource="http://www.w3.org/2004/02/skos/core#note"/>
    </owl:AnnotationProperty>
    


    <!-- http://www.w3.org/2004/02/skos/core#hiddenLabel -->

    <owl:AnnotationProperty rdf:about="http://www.w3.org/2004/02/skos/core#hiddenLabel">
        <rdfs:comment xml:lang="en">The range of skos:hiddenLabel is the class of RDF plain literals.</rdfs:comment>
        <rdfs:comment xml:lang="en">skos:prefLabel, skos:altLabel and skos:hiddenLabel are pairwise disjoint properties.</rdfs:comment>
        <rdfs:isDefinedBy rdf:resource="http://www.w3.org/2004/02/skos/core"/>
        <rdfs:label xml:lang="en">hidden label</rdfs:label>
        <skos:definition xml:lang="en">A lexical label for a resource that should be hidden when generating visual displays of the resource, but should still be accessible to free text search operations.</skos:definition>
        <rdfs:subPropertyOf rdf:resource="http://www.w3.org/2000/01/rdf-schema#label"/>
    </owl:AnnotationProperty>
    


    <!-- http://www.w3.org/2004/02/skos/core#historyNote -->

    <owl:AnnotationProperty rdf:about="http://www.w3.org/2004/02/skos/core#historyNote">
        <rdfs:isDefinedBy rdf:resource="http://www.w3.org/2004/02/skos/core"/>
        <rdfs:label xml:lang="en">history note</rdfs:label>
        <skos:definition xml:lang="en">A note about the past state/use/meaning of a concept.</skos:definition>
        <rdfs:subPropertyOf rdf:resource="http://www.w3.org/2004/02/skos/core#note"/>
    </owl:AnnotationProperty>
    


    <!-- http://www.w3.org/2004/02/skos/core#note -->

    <owl:AnnotationProperty rdf:about="http://www.w3.org/2004/02/skos/core#note">
        <rdfs:isDefinedBy rdf:resource="http://www.w3.org/2004/02/skos/core"/>
        <rdfs:label xml:lang="en">note</rdfs:label>
        <skos:definition xml:lang="en">A general note, for any purpose.</skos:definition>
        <skos:scopeNote xml:lang="en">This property may be used directly, or as a super-property for more specific note types.</skos:scopeNote>
    </owl:AnnotationProperty>
    


    <!-- http://www.w3.org/2004/02/skos/core#prefLabel -->

    <owl:AnnotationProperty rdf:about="http://www.w3.org/2004/02/skos/core#prefLabel">
        <rdfs:comment xml:lang="en">A resource has no more than one value of skos:prefLabel per language tag, and no more than one value of skos:prefLabel without language tag.</rdfs:comment>
        <rdfs:comment xml:lang="en">The range of skos:prefLabel is the class of RDF plain literals.</rdfs:comment>
        <rdfs:comment xml:lang="en">skos:prefLabel, skos:altLabel and skos:hiddenLabel are pairwise
      disjoint properties.</rdfs:comment>
        <rdfs:isDefinedBy rdf:resource="http://www.w3.org/2004/02/skos/core"/>
        <rdfs:label xml:lang="en">preferred label</rdfs:label>
        <skos:definition xml:lang="en">The preferred lexical label for a resource, in a given language.</skos:definition>
        <rdfs:subPropertyOf rdf:resource="http://www.w3.org/2000/01/rdf-schema#label"/>
    </owl:AnnotationProperty>
    


    <!-- http://www.w3.org/2004/02/skos/core#scopeNote -->

    <owl:AnnotationProperty rdf:about="http://www.w3.org/2004/02/skos/core#scopeNote">
        <rdfs:isDefinedBy rdf:resource="http://www.w3.org/2004/02/skos/core"/>
        <rdfs:label xml:lang="en">scope note</rdfs:label>
        <skos:definition xml:lang="en">A note that helps to clarify the meaning and/or the use of a concept.</skos:definition>
        <rdfs:subPropertyOf rdf:resource="http://www.w3.org/2004/02/skos/core#note"/>
    </owl:AnnotationProperty>
    


    <!-- 
    ///////////////////////////////////////////////////////////////////////////////////////
    //
    // Datatypes
    //
    ///////////////////////////////////////////////////////////////////////////////////////
     -->

    


    <!-- http://www.opengis.net/ont/geosparql#gmlLiteral -->

    <rdfs:Datatype rdf:about="http://www.opengis.net/ont/geosparql#gmlLiteral">
        <dc:contributor>Matthew Perry</dc:contributor>
        <dc:creator>OGC GeoSPARQL 1.0 Standard Working Group</dc:creator>
        <dc:date rdf:datatype="http://www.w3.org/2001/XMLSchema#date">2011-06-16</dc:date>
        <dc:description xml:lang="en">
      A GML serialization of a geometry object.
    </dc:description>
        <rdfs:comment xml:lang="en">
      A GML serialization of a geometry object.
    </rdfs:comment>
        <rdfs:isDefinedBy rdf:resource="http://www.opengis.net/ont/geosparql"/>
        <rdfs:isDefinedBy rdf:resource="http://www.opengis.net/spec/geosparql/1.0"/>
        <rdfs:label xml:lang="en">GML Literal</rdfs:label>
        <skos:definition xml:lang="en">
      A GML serialization of a geometry object.
    </skos:definition>
        <skos:prefLabel xml:lang="en">GML Literal</skos:prefLabel>
    </rdfs:Datatype>
    


    <!-- http://www.opengis.net/ont/geosparql#wktLiteral -->

    <rdfs:Datatype rdf:about="http://www.opengis.net/ont/geosparql#wktLiteral">
        <dc:contributor>Matthew Perry</dc:contributor>
        <dc:creator>OGC GeoSPARQL 1.0 Standard Working Group</dc:creator>
        <dc:date rdf:datatype="http://www.w3.org/2001/XMLSchema#date">2011-06-16</dc:date>
        <dc:description xml:lang="en">
      A Well-known Text serialization of a geometry object.
    </dc:description>
        <rdfs:comment xml:lang="en">
      A Well-known Text serialization of a geometry object.
    </rdfs:comment>
        <rdfs:isDefinedBy rdf:resource="http://www.opengis.net/ont/geosparql"/>
        <rdfs:isDefinedBy rdf:resource="http://www.opengis.net/spec/geosparql/1.0"/>
        <rdfs:label xml:lang="en">Well-known Text Literal</rdfs:label>
        <skos:definition xml:lang="en">
      A Well-known Text serialization of a geometry object.
    </skos:definition>
        <skos:prefLabel xml:lang="en">Well-known Text Literal</skos:prefLabel>
    </rdfs:Datatype>
    


    <!-- http://www.w3.org/2001/XMLSchema#date -->

    <rdfs:Datatype rdf:about="http://www.w3.org/2001/XMLSchema#date"/>
    


    <!-- http://www.w3.org/2001/XMLSchema#dateTimeStamp -->

    <rdf:Description rdf:about="http://www.w3.org/2001/XMLSchema#dateTimeStamp">
        <rdfs:label xml:lang="es">sello de tiempo</rdfs:label>
    </rdf:Description>
    


    <!-- http://www.w3.org/2001/XMLSchema#duration -->

    <rdfs:Datatype rdf:about="http://www.w3.org/2001/XMLSchema#duration"/>
    


    <!-- http://www.w3.org/2001/XMLSchema#gDay -->

    <rdfs:Datatype rdf:about="http://www.w3.org/2001/XMLSchema#gDay"/>
    


    <!-- http://www.w3.org/2001/XMLSchema#gMonth -->

    <rdfs:Datatype rdf:about="http://www.w3.org/2001/XMLSchema#gMonth"/>
    


    <!-- http://www.w3.org/2001/XMLSchema#gYear -->

    <rdfs:Datatype rdf:about="http://www.w3.org/2001/XMLSchema#gYear"/>
    


    <!-- http://www.w3.org/2001/XMLSchema#gYearMonth -->

    <rdfs:Datatype rdf:about="http://www.w3.org/2001/XMLSchema#gYearMonth"/>
    


    <!-- http://www.w3.org/2006/time#generalDay -->

    <rdfs:Datatype rdf:about="http://www.w3.org/2006/time#generalDay">
        <rdfs:comment xml:lang="en">Day of month - formulated as a text string with a pattern constraint to reproduce the same lexical form as gDay, except that values up to 99 are permitted, in order to support calendars with more than 31 days in a month. 
Note that the value-space is not defined, so a generic OWL2 processor cannot compute ordering relationships of values of this type.</rdfs:comment>
        <rdfs:comment xml:lang="es">Día del mes - formulado como una cadena de texto con una restricción patrón para reproducir la misma forma léxica que gDay, excepto que se permiten valores hasta el 99, con el propósito de proporcionar soporte a calendarios con meses con más de 31 días.
            Nótese que el espacio de valores no está definido, por tanto, un procesador genérico de OWL2 no puede computar relaciones de orden de valores de este tipo.</rdfs:comment>
        <rdfs:label xml:lang="es">Día generalizado</rdfs:label>
        <rdfs:label xml:lang="en">Generalized day</rdfs:label>
        <skos:definition xml:lang="en">Day of month - formulated as a text string with a pattern constraint to reproduce the same lexical form as gDay, except that values up to 99 are permitted, in order to support calendars with more than 31 days in a month. 
Note that the value-space is not defined, so a generic OWL2 processor cannot compute ordering relationships of values of this type.</skos:definition>
        <skos:definition xml:lang="es">Día del mes - formulado como una cadena de texto con una restricción patrón para reproducir la misma forma léxica que gDay, excepto que se permiten valores hasta el 99, con el propósito de proporcionar soporte a calendarios con meses con más de 31 días.
            Nótese que el espacio de valores no está definido, por tanto, un procesador genérico de OWL2 no puede computar relaciones de orden de valores de este tipo.</skos:definition>
    </rdfs:Datatype>
    


    <!-- http://www.w3.org/2006/time#generalMonth -->

    <rdfs:Datatype rdf:about="http://www.w3.org/2006/time#generalMonth">
        <rdfs:comment xml:lang="es">Mes del año - formulado como una cadena de texto con una restricción patrón para reproducir la misma forma léxica que gMonth, excepto que se permiten valores hasta el 20, con el propósito de proporcionar soporte a calendarios con años con más de 12 meses.
            Nótese que el espacio de valores no está definido, por tanto, un procesador genérico de OWL2 no puede computar relaciones de orden de valores de este tipo.</rdfs:comment>
        <rdfs:comment xml:lang="en">Month of year - formulated as a text string with a pattern constraint to reproduce the same lexical form as gMonth, except that values up to 20 are permitted, in order to support calendars with more than 12 months in the year. 
Note that the value-space is not defined, so a generic OWL2 processor cannot compute ordering relationships of values of this type.</rdfs:comment>
        <rdfs:label xml:lang="en">Generalized month</rdfs:label>
        <rdfs:label xml:lang="es">Mes generalizado</rdfs:label>
        <skos:definition xml:lang="es">Mes del año - formulado como una cadena de texto con una restricción patrón para reproducir la misma forma léxica que gMonth, excepto que se permiten valores hasta el 20, con el propósito de proporcionar soporte a calendarios con años con más de 12 meses.
            Nótese que el espacio de valores no está definido, por tanto, un procesador genérico de OWL2 no puede computar relaciones de orden de valores de este tipo.</skos:definition>
        <skos:definition xml:lang="en">Month of year - formulated as a text string with a pattern constraint to reproduce the same lexical form as gMonth, except that values up to 20 are permitted, in order to support calendars with more than 12 months in the year. 
Note that the value-space is not defined, so a generic OWL2 processor cannot compute ordering relationships of values of this type.</skos:definition>
    </rdfs:Datatype>
    


    <!-- http://www.w3.org/2006/time#generalYear -->

    <rdfs:Datatype rdf:about="http://www.w3.org/2006/time#generalYear">
        <rdfs:comment xml:lang="es">Número de año - formulado como una cadena de texto con una restricción patrón para reproducir la misma forma léxica que gYear, aunque no está restringido a valores del calendario gregoriano.
            Nótese que el espacio de valores no está definido, por tanto, un procesador genérico de OWL2 no puede computar relaciones de orden de valores de este tipo.</rdfs:comment>
        <rdfs:comment xml:lang="en">Year number - formulated as a text string with a pattern constraint to reproduce the same lexical form as gYear, but not restricted to values from the Gregorian calendar. 
Note that the value-space is not defined, so a generic OWL2 processor cannot compute ordering relationships of values of this type.</rdfs:comment>
        <rdfs:label xml:lang="es">Año generalizado</rdfs:label>
        <rdfs:label xml:lang="en">Generalized year</rdfs:label>
        <skos:definition xml:lang="es">Número de año - formulado como una cadena de texto con una restricción patrón para reproducir la misma forma léxica que gYear, aunque no está restringido a valores del calendario gregoriano.
            Nótese que el espacio de valores no está definido, por tanto, un procesador genérico de OWL2 no puede computar relaciones de orden de valores de este tipo.</skos:definition>
        <skos:definition xml:lang="en">Year number - formulated as a text string with a pattern constraint to reproduce the same lexical form as gYear, but not restricted to values from the Gregorian calendar. 
Note that the value-space is not defined, so a generic OWL2 processor cannot compute ordering relationships of values of this type.</skos:definition>
    </rdfs:Datatype>
    


    <!-- 
    ///////////////////////////////////////////////////////////////////////////////////////
    //
    // Object Properties
    //
    ///////////////////////////////////////////////////////////////////////////////////////
     -->

    


    <!-- http://purl.org/nemo/gufo#broughtAbout -->

    <owl:ObjectProperty rdf:about="http://purl.org/nemo/gufo#broughtAbout">
        <rdfs:domain rdf:resource="http://purl.org/nemo/gufo#Event"/>
        <rdfs:range rdf:resource="http://purl.org/nemo/gufo#Situation"/>
        <rdfs:comment xml:lang="en">Identifies a gufo:Situation that is brought about by the gufo:Event.

Guizzardi et al. (2013) included a notion of &quot;brings-about&quot; that related events to a single (&quot;maximal&quot;) situation, embodying all the effects of the event at the time it ends. This implementation of gufo:broughtAbout diverges from &quot;brings-about&quot; in that work because gufo:broughtAbout can be used to relate events to more than one gufo:Situation. Each gufo:Situation identified through gufo:broughtAbout should be understood as an (improper) part of the maximal situation.</rdfs:comment>
        <rdfs:label xml:lang="en">broughtAbout</rdfs:label>
    </owl:ObjectProperty>
    


    <!-- http://purl.org/nemo/gufo#categorizes -->

    <owl:ObjectProperty rdf:about="http://purl.org/nemo/gufo#categorizes">
        <rdfs:domain>
            <owl:Class>
                <owl:intersectionOf rdf:parseType="Collection">
                    <rdf:Description rdf:about="http://purl.org/nemo/gufo#Type"/>
                    <owl:Class>
                        <owl:complementOf rdf:resource="http://purl.org/nemo/gufo#AbstractEntityType"/>
                    </owl:Class>
                    <owl:Class>
                        <owl:complementOf rdf:resource="http://purl.org/nemo/gufo#ConcreteEntityType"/>
                    </owl:Class>
                </owl:intersectionOf>
            </owl:Class>
        </rdfs:domain>
        <rdfs:range rdf:resource="http://purl.org/nemo/gufo#Type"/>
        <rdfs:comment xml:lang="en">Identifies a gufo:Type whose instances may be classified by instances of the categorizing higher-order type.

For example, &quot;ShipType&quot; gufo:categorizes &quot;Ship&quot;. Instances of &quot;ShipType&quot; such as &quot;Supercarrier&quot; and &quot;Cargoship&quot; should be declared subclasses of &quot;Ship&quot;. OWL 2 punning should be used to capture the two facets of &quot;Supercarrier&quot; and &quot;Cargoship&quot; in this example: (i) as instances of &quot;ShipType&quot;, and (ii) as subclasses of &quot;Ship&quot;.

The categorized type is termed the &quot;base type&quot; in the &quot;powertype pattern&quot; see Carvalho et al (2017), the higher-order type is often called the &quot;powertype&quot;.  

gufo:categorizes is the general (unspecific) form of categorization. See  gufo:partitions for a more specific form, in which instances of the categorized type are classified by exactly one instance of the higher-order type. 

The domain is gufo:Type excluding gufo:AbstractIndividualType as well as gufo:ConcreteIndividualTypes because those types are first-order types (their instances are individuals). Only instances of gufo:Type representing higher-order types can categorize a base type.

For further details and formalization of &quot;categorization&quot;, see Carvalho et al (2017) which combines UFO with MLT (a multi-level modeling theory).  

V. A. Carvalho, J. P. A. Almeida, C. M. Fonseca, and G. Guizzardi, “Multi-level ontology-based conceptual modeling,” Data &amp; Knowledge Engineering, vol. 109, p. 3–24, 2017. &lt;http://dx.doi.org/10.1016/j.datak.2017.03.002&gt;</rdfs:comment>
        <rdfs:label xml:lang="en">categorizes</rdfs:label>
    </owl:ObjectProperty>
    


    <!-- http://purl.org/nemo/gufo#concernsConstitutedEndurant -->

    <owl:ObjectProperty rdf:about="http://purl.org/nemo/gufo#concernsConstitutedEndurant">
        <rdfs:domain rdf:resource="http://purl.org/nemo/gufo#TemporaryConstitutionSituation"/>
        <rdfs:range rdf:resource="http://purl.org/nemo/gufo#Endurant"/>
        <rdfs:comment xml:lang="en">Identifies the constituted gufo:Endurant in the gufo:TemporaryConstitutionSituation.</rdfs:comment>
        <rdfs:label xml:lang="en">concernsConstitutedEndurant</rdfs:label>
    </owl:ObjectProperty>
    


    <!-- http://purl.org/nemo/gufo#concernsNonRigidType -->

    <owl:ObjectProperty rdf:about="http://purl.org/nemo/gufo#concernsNonRigidType">
        <rdf:type rdf:resource="http://www.w3.org/2002/07/owl#FunctionalProperty"/>
        <rdfs:domain rdf:resource="http://purl.org/nemo/gufo#TemporaryInstantiationSituation"/>
        <rdfs:range rdf:resource="http://purl.org/nemo/gufo#NonRigidType"/>
        <rdfs:comment xml:lang="en">Identifies the gufo:NonRigidType that is instantiated by the endurant that stands in a gufo:TemporaryInstantiationSituation.</rdfs:comment>
        <rdfs:label xml:lang="en">concernsNonRigidType</rdfs:label>
    </owl:ObjectProperty>
    


    <!-- http://purl.org/nemo/gufo#concernsQualityType -->

    <owl:ObjectProperty rdf:about="http://purl.org/nemo/gufo#concernsQualityType">
        <rdf:type rdf:resource="http://www.w3.org/2002/07/owl#FunctionalProperty"/>
        <rdfs:domain rdf:resource="http://purl.org/nemo/gufo#QualityValueAttributionSituation"/>
        <rdfs:range rdf:resource="http://purl.org/nemo/gufo#EndurantType"/>
        <rdfs:comment xml:lang="en">Identifies the quality type (a gufo:EndurantType subclassing gufo:Quality) whose value is attributed in the gufo:QualityValueAttributionSituation.</rdfs:comment>
        <rdfs:label xml:lang="en">concernsQualityType</rdfs:label>
    </owl:ObjectProperty>
    


    <!-- http://purl.org/nemo/gufo#concernsReifiedQualityValue -->

    <owl:ObjectProperty rdf:about="http://purl.org/nemo/gufo#concernsReifiedQualityValue">
        <rdf:type rdf:resource="http://www.w3.org/2002/07/owl#FunctionalProperty"/>
        <rdfs:domain rdf:resource="http://purl.org/nemo/gufo#QualityValueAttributionSituation"/>
        <rdfs:range rdf:resource="http://purl.org/nemo/gufo#QualityValue"/>
        <rdfs:comment rdf:resource="http://purl.org/nemo/gufo#concernsQualityValue"/>
        <rdfs:comment xml:lang="en">Identifies the gufo:QualityValue (i.e., the reified quality value) associated with the endurant that stands in the gufo:QualityValueAttributionSituation.</rdfs:comment>
        <rdfs:label xml:lang="en">concernsReifiedQualityValue</rdfs:label>
    </owl:ObjectProperty>
    


    <!-- http://purl.org/nemo/gufo#concernsRelatedEndurant -->

    <owl:ObjectProperty rdf:about="http://purl.org/nemo/gufo#concernsRelatedEndurant">
        <rdf:type rdf:resource="http://www.w3.org/2002/07/owl#FunctionalProperty"/>
        <rdfs:domain rdf:resource="http://purl.org/nemo/gufo#TemporaryRelationshipSituation"/>
        <rdfs:range rdf:resource="http://purl.org/nemo/gufo#Endurant"/>
        <rdfs:comment xml:lang="en">Identifies the related gufo:Endurant in the gufo:TemporaryRelationshipSituation.</rdfs:comment>
        <rdfs:label xml:lang="en">concernsRelatedEndurant</rdfs:label>
    </owl:ObjectProperty>
    


    <!-- http://purl.org/nemo/gufo#concernsRelationshipType -->

    <owl:ObjectProperty rdf:about="http://purl.org/nemo/gufo#concernsRelationshipType">
        <rdf:type rdf:resource="http://www.w3.org/2002/07/owl#FunctionalProperty"/>
        <rdfs:domain rdf:resource="http://purl.org/nemo/gufo#TemporaryRelationshipSituation"/>
        <rdfs:range rdf:resource="http://purl.org/nemo/gufo#RelationshipType"/>
        <rdfs:comment xml:lang="en">Identifies the gufo:RelationshipType instantiated in the gufo:TemporaryRelationshipSituation.</rdfs:comment>
        <rdfs:label xml:lang="en">concernsRelationshipType</rdfs:label>
    </owl:ObjectProperty>
    


    <!-- http://purl.org/nemo/gufo#concernsTemporaryWhole -->

    <owl:ObjectProperty rdf:about="http://purl.org/nemo/gufo#concernsTemporaryWhole">
        <rdf:type rdf:resource="http://www.w3.org/2002/07/owl#FunctionalProperty"/>
        <rdfs:domain rdf:resource="http://purl.org/nemo/gufo#TemporaryParthoodSituation"/>
        <rdfs:range rdf:resource="http://purl.org/nemo/gufo#Endurant"/>
        <rdfs:comment xml:lang="en">Identifies the whole (a gufo:Endurant) of which the endurant that stands in the gufo:TemporaryParthoodSituation is part.</rdfs:comment>
        <rdfs:label xml:lang="en">concernsTemporaryWhole</rdfs:label>
    </owl:ObjectProperty>
    


    <!-- http://purl.org/nemo/gufo#constitutes -->

    <owl:ObjectProperty rdf:about="http://purl.org/nemo/gufo#constitutes">
        <rdfs:domain rdf:resource="http://purl.org/nemo/gufo#ConcreteEntity"/>
        <rdfs:range rdf:resource="http://purl.org/nemo/gufo#ConcreteEntity"/>
        <rdfs:comment xml:lang="en">Identifies a gufo:ConcreteIndividual that is constituted (partially) by the constituent individual.

For example, the gufo:Collection of persons whose members are John, Paul, George, Ringo constituted the beatles, the gufo:Quantity of marble that constitutes the statue of Venus de Milo, and the gufo:Event of Paul raising his arm in a meeting that constitutes his voting (also a gufo:Event).

In case constitution changes in time, see gufo:standsInQualifiedConstitution.</rdfs:comment>
        <rdfs:label xml:lang="en">constitutes</rdfs:label>
        <rdfs:seeAlso rdf:resource="http://purl.org/nemo/gufo#standsInQualifiedConstitution"/>
    </owl:ObjectProperty>
    


    <!-- http://purl.org/nemo/gufo#contributedToTrigger -->

    <owl:ObjectProperty rdf:about="http://purl.org/nemo/gufo#contributedToTrigger">
        <rdfs:domain rdf:resource="http://purl.org/nemo/gufo#Situation"/>
        <rdfs:range rdf:resource="http://purl.org/nemo/gufo#Event"/>
        <rdfs:comment xml:lang="en">Identifies a gufo:Event that the gufo:Situation contributed to trigger.

Guizzardi et al. (2013) defined a notion of &quot;triggers&quot; to relate the situation satisfying all the sufficient and necessary conditions with the triggered  event. This implementation differs from  &quot;triggers&quot; as defined in that work because gufo:contributedToTrigger can be used to relate more than one gufo:Situation to a gufo:Event. Each gufo:Situation identified through gufo:contributedToTrigger should be understood as an (improper) part of the situation that triggered the event.</rdfs:comment>
        <rdfs:label xml:lang="en">contributedToTrigger</rdfs:label>
    </owl:ObjectProperty>
    


    <!-- http://purl.org/nemo/gufo#emergesFrom -->

    <owl:ObjectProperty rdf:about="http://purl.org/nemo/gufo#emergesFrom">
        <rdfs:domain rdf:resource="http://purl.org/nemo/gufo#Event"/>
        <rdfs:range rdf:resource="http://purl.org/nemo/gufo#Scene"/>
        <rdfs:comment>A gufo:Event is restricted to an area and an interval, both being conteined in a convex spatio-temporal region. In other words, a gufo;Events emerges from within a gufo:Scene.

(i.e. &quot;Lebron James becoming NBA&apos;s all-time top scorer&quot; gufo:Event hapened in the &quot;7th February, 2023 in Crypto.com Arena&quot; gufo:Scene.)</rdfs:comment>
        <rdfs:label>emergesFrom</rdfs:label>
    </owl:ObjectProperty>
    


    <!-- http://purl.org/nemo/gufo#externallyDependsOn -->

    <owl:ObjectProperty rdf:about="http://purl.org/nemo/gufo#externallyDependsOn">
        <rdf:type rdf:resource="http://www.w3.org/2002/07/owl#IrreflexiveProperty"/>
        <rdfs:domain rdf:resource="http://purl.org/nemo/gufo#ExtrinsicMode"/>
        <rdfs:range rdf:resource="http://purl.org/nemo/gufo#Endurant"/>
        <rdfs:comment xml:lang="en">Identifies a gufo:Endurant on which the gufo:ExtrinsicMode depends.

For example, John&apos;s duty to return the book he borrowed from Mary (a gufo:ExtrinsicMode) depends externally on Mary.

The identifed gufo:Endurant should  be external to the bearer of the extrinsic mode (see Guizzardi, 2005, p. 239). In other words, the identified endurant should not be a part or an intrisic aspect of the bearer of the extrinsic mode.</rdfs:comment>
        <rdfs:label xml:lang="en">externallyDependsOn</rdfs:label>
    </owl:ObjectProperty>
    


    <!-- http://purl.org/nemo/gufo#hasAssociatedQualityValueType -->

    <owl:ObjectProperty rdf:about="http://purl.org/nemo/gufo#hasAssociatedQualityValueType">
        <rdfs:domain rdf:resource="http://purl.org/nemo/gufo#EndurantType"/>
        <rdfs:range rdf:resource="http://purl.org/nemo/gufo#AbstractEntityType"/>
        <rdfs:comment xml:lang="en">Identifies a quality value type to which the quality type is associated. 

For example, a &quot;Color&quot; quality type may be associated with a &quot;ColorValueInRGB&quot; quality value type.

It relates a specialization of gufo:Quality (an instance of gufo:EndurantType) to a specialization of gufo:QualityValue  (an instance of gufo:AbstractIndividualType).

To be used only when quality values are reified.</rdfs:comment>
        <rdfs:label xml:lang="en">hasAssociatedQualityValueType</rdfs:label>
    </owl:ObjectProperty>
    


    <!-- http://purl.org/nemo/gufo#hasBeginPoint -->

    <owl:ObjectProperty rdf:about="http://purl.org/nemo/gufo#hasBeginPoint">
        <rdfs:domain rdf:resource="http://purl.org/nemo/gufo#ConcreteEntity"/>
        <rdfs:range rdf:resource="http://www.w3.org/2006/time#Instant"/>
        <rdfs:comment xml:lang="en">Identifies the begin point for a gufo:ConcreteIndividual, in the case in which time instants are reified. 

In the case of endurants, this identifies the time point when the endurant comes into existence. In the case of events, this identifies the time point when the event starts to take place. In the case of situation, this identifies the time point when the situation begins to hold.

If time instants are not reified, use gufo:hasBeginPointInXSDDate or gufo:hasBeginPointInXSDDateTimeStamp.</rdfs:comment>
        <rdfs:label xml:lang="en">hasBeginPoint</rdfs:label>
        <rdfs:seeAlso rdf:resource="http://purl.org/nemo/gufo#hasBeginPointInXSDDate"/>
        <rdfs:seeAlso rdf:resource="http://purl.org/nemo/gufo#hasBeginPointInXSDDateTimeStamp"/>
    </owl:ObjectProperty>
    


    <!-- http://purl.org/nemo/gufo#hasEndPoint -->

    <owl:ObjectProperty rdf:about="http://purl.org/nemo/gufo#hasEndPoint">
        <rdfs:domain rdf:resource="http://purl.org/nemo/gufo#ConcreteEntity"/>
        <rdfs:range rdf:resource="http://www.w3.org/2006/time#Instant"/>
        <rdfs:comment xml:lang="en">Identifies the end point for a gufo:ConcreteIndividual, in the case in which time instants are reified.

In the case of endurants, this identifies the time point when the endurant ceases to exist. In the case of events, this identifies the time point when the event ends. In the case of situation, this identifies the time point when the situation ceases to hold.</rdfs:comment>
        <rdfs:label xml:lang="en">hasEndPoint</rdfs:label>
        <rdfs:seeAlso rdf:resource="http://purl.org/nemo/gufo#hasEndPointInXSDDate"/>
        <rdfs:seeAlso rdf:resource="http://purl.org/nemo/gufo#hasEndPointInXSDDateTimeStamp"/>
    </owl:ObjectProperty>
    


    <!-- http://purl.org/nemo/gufo#hasReifiedQualityValue -->

    <owl:ObjectProperty rdf:about="http://purl.org/nemo/gufo#hasReifiedQualityValue">
        <rdfs:domain rdf:resource="http://purl.org/nemo/gufo#ConcreteEntity"/>
        <rdfs:range rdf:resource="http://purl.org/nemo/gufo#QualityValue"/>
        <rdfs:comment xml:lang="en">Identifies an instance of gufo:QualityValue to reflect the perception or conception of a quality in a certain value space. 

Use this property only for quality values that are to be reified in the A-box and associated with a gufo:ConcreteIndividual. Otherwise, use the gufo:hasQualityValue data property and a literal to determine the quality value.

The full representation pattern for quality values involves first identifying a gufo:Quality that inheres in a concrete individual and then associating it with a reified quality value. For example, let us consider the color of Yves Klein&apos;s &quot;Blue Monochrome&quot; painting made in 1961 (MoMA&apos;s object with number 618.1967). In the full pattern, an instance of gufo:Quality that inheres in the physical object (the color of that painting) is associated with a gufo:QualityValue (say the triplet &lt;0, 47, 167&gt; for that painting) through gufo:hasReifiedQualityValue. The full pattern is recommended when different quality spaces are expected to be used for the same quality. For example, the color of that painting could also be associated with a quadruple &lt;100, 72, 0, 35&gt; representing the same color in a CMYK space.

When the full pattern is not required, gufo:hasReifiedQualityValue can also be used to directly associate a concrete individual (without identifying the quality) with a quality value.</rdfs:comment>
        <rdfs:label xml:lang="en">hasReifiedQualityValue</rdfs:label>
        <rdfs:seeAlso rdf:resource="http://purl.org/nemo/gufo#hasQualityValue"/>
    </owl:ObjectProperty>
    


    <!-- http://purl.org/nemo/gufo#historicallyDependsOn -->

    <owl:ObjectProperty rdf:about="http://purl.org/nemo/gufo#historicallyDependsOn">
        <rdf:type rdf:resource="http://www.w3.org/2002/07/owl#TransitiveProperty"/>
        <rdfs:domain rdf:resource="http://purl.org/nemo/gufo#ConcreteEntity"/>
        <rdfs:range rdf:resource="http://purl.org/nemo/gufo#ConcreteEntity"/>
        <rdfs:comment xml:lang="en">Identifies a gufo:ConcreteIndividual on which the concrete individual depends historically. 

For example, a person is historically dependent on his/her ancestors.

When used between events, historical dependence encompasses causation (when the event is caused by the other), but also other cases where there is dependence but not causation (when the event brings about a situation that is either insufficient or more than sufficient to trigger the historically dependent event).

For example, Real Madrid&apos;s goal in the 60th minute of the 2016 FIFA Club World Cup Final is historically dependent on (and in this case caused by) a penalty kick by Cristiano Ronaldo. The penalty kick itself is historically dependent on (but not caused by) a penalty (the occurrence of the penalty is necessary but not sufficient to cause the penalty kick as authorization of the referee is required). 

Historical dependence is transitive. Hence, in the example above, Real Madrid&apos;s goal is historically dependent on the penalty.</rdfs:comment>
        <rdfs:label xml:lang="en">historicallyDependsOn</rdfs:label>
    </owl:ObjectProperty>
    


    <!-- http://purl.org/nemo/gufo#inheresIn -->

    <owl:ObjectProperty rdf:about="http://purl.org/nemo/gufo#inheresIn">
        <rdf:type rdf:resource="http://www.w3.org/2002/07/owl#FunctionalProperty"/>
        <rdf:type rdf:resource="http://www.w3.org/2002/07/owl#AsymmetricProperty"/>
        <rdf:type rdf:resource="http://www.w3.org/2002/07/owl#IrreflexiveProperty"/>
        <rdfs:domain rdf:resource="http://purl.org/nemo/gufo#Aspect"/>
        <rdfs:range rdf:resource="http://purl.org/nemo/gufo#ConcreteEntity"/>
        <rdfs:comment xml:lang="en">Identifies the gufo:ConcreteIndividual in which the gufo:Aspect inheres. Inherence is a sort of existential dependence. The identified concrete individual is the &quot;bearer&quot; of the aspect.

For example, the color of an object inheres in the object and the average speed of a flight inheres in the flight.</rdfs:comment>
        <rdfs:label xml:lang="en">inheresIn</rdfs:label>
    </owl:ObjectProperty>
    


    <!-- http://purl.org/nemo/gufo#isAspectProperPartOf -->

    <owl:ObjectProperty rdf:about="http://purl.org/nemo/gufo#isAspectProperPartOf">
        <rdfs:subPropertyOf rdf:resource="http://purl.org/nemo/gufo#isProperPartOf"/>
        <rdf:type rdf:resource="http://www.w3.org/2002/07/owl#TransitiveProperty"/>
        <rdfs:domain rdf:resource="http://purl.org/nemo/gufo#Aspect"/>
        <rdfs:range rdf:resource="http://purl.org/nemo/gufo#Aspect"/>
        <rdfs:comment xml:lang="en">Identifies a gufo:Aspect of which the aspect is a proper part.

For example, John&apos;s obligations towards Mary in the scope of their marriage is an aspect proper part of their marriage  (and same can be said of Mary&apos;s extrinsic aspects in the scope of their marriage.)

This property can be used to represent the composition of a relator from extrisinc aspects, but also to represent complex extrisinc aspects.

gufo:isAspectProperPartOf is transitive.</rdfs:comment>
        <rdfs:label xml:lang="en">isAspectProperPartOf</rdfs:label>
    </owl:ObjectProperty>
    


    <!-- http://purl.org/nemo/gufo#isCollectionMemberOf -->

    <owl:ObjectProperty rdf:about="http://purl.org/nemo/gufo#isCollectionMemberOf">
        <rdfs:subPropertyOf rdf:resource="http://purl.org/nemo/gufo#isObjectProperPartOf"/>
        <rdfs:domain rdf:resource="http://purl.org/nemo/gufo#Object"/>
        <rdfs:range rdf:resource="http://purl.org/nemo/gufo#Collection"/>
        <rdfs:comment xml:lang="en">Identifies a gufo:Collection of which the object is a member. 

This is the relation between John and a group of persons, and between a cow and its herd.

gufo:isCollectionMemberOf is intransitive (Guizzardi, 2005, p. 185).

For membership in a gufo:VariableCollection, see gufo:standsInQualifiedParthood.</rdfs:comment>
        <rdfs:label xml:lang="en">isCollectionMemberOf</rdfs:label>
        <rdfs:seeAlso rdf:resource="http://purl.org/nemo/gufo#standsInQualifiedParthood"/>
    </owl:ObjectProperty>
    


    <!-- http://purl.org/nemo/gufo#isComponentOf -->

    <owl:ObjectProperty rdf:about="http://purl.org/nemo/gufo#isComponentOf">
        <rdfs:subPropertyOf rdf:resource="http://purl.org/nemo/gufo#isObjectProperPartOf"/>
        <rdfs:domain rdf:resource="http://purl.org/nemo/gufo#Object"/>
        <rdfs:range rdf:resource="http://purl.org/nemo/gufo#FunctionalComplex"/>
        <rdfs:comment xml:lang="en">Identifies a gufo:FunctionalComplex of which the object is a component.

For example, the habitation module is a component of the International Space Station, and so are each of the solar panels; Obama&apos;s brain is a component of his body, and so is his heart; the engine is a component of the HMS Queen Elizabeth (R08).

gufo:isComponentOf is not transitive in the general case. Particular sub-properties may be transitive (Guizzardi, 2005, p. 183).

When a component may change its relation to be whole, see gufo:standsInQualifiedParthood.</rdfs:comment>
        <rdfs:label xml:lang="en">isComponentOf</rdfs:label>
        <rdfs:seeAlso rdf:resource="http://purl.org/nemo/gufo#standsInQualifiedParthood"/>
    </owl:ObjectProperty>
    


    <!-- http://purl.org/nemo/gufo#isDerivedFrom -->

    <owl:ObjectProperty rdf:about="http://purl.org/nemo/gufo#isDerivedFrom">
        <rdfs:domain>
            <owl:Class>
                <owl:unionOf rdf:parseType="Collection">
                    <rdf:Description rdf:about="http://purl.org/nemo/gufo#ComparativeRelationshipType"/>
                    <rdf:Description rdf:about="http://purl.org/nemo/gufo#MaterialRelationshipType"/>
                </owl:unionOf>
            </owl:Class>
        </rdfs:domain>
        <rdfs:range rdf:resource="http://purl.org/nemo/gufo#EndurantType"/>
        <rdfs:comment xml:lang="en">Identifies a gufo:EndurantType from which the material or comparative relation can be derived. The identified gufo:EndurantType should be a subclass of gufo:Aspect, more specifically a subclass of gufo:ExtrinsicAspect in the case of a gufo:MaterialRelationshipType, and a subclass of gufo:IntrinsicAspect in the case of a gufo:ComparativeRelationshipType.

For example, &quot;marriedWith&quot; can be derived from &quot;Marriage&quot;, &quot;heavierThan&quot; can be derived from &quot;Weight&quot;.

See Fonseca et al. (2019).</rdfs:comment>
        <rdfs:label xml:lang="en">isDerivedFrom</rdfs:label>
    </owl:ObjectProperty>
    


    <!-- http://purl.org/nemo/gufo#isEventProperPartOf -->

    <owl:ObjectProperty rdf:about="http://purl.org/nemo/gufo#isEventProperPartOf">
        <rdfs:subPropertyOf rdf:resource="http://purl.org/nemo/gufo#isProperPartOf"/>
        <rdf:type rdf:resource="http://www.w3.org/2002/07/owl#TransitiveProperty"/>
        <rdfs:domain rdf:resource="http://purl.org/nemo/gufo#AtomicEvent"/>
        <rdfs:domain rdf:resource="http://purl.org/nemo/gufo#ComplexEvent"/>
        <rdfs:range rdf:resource="http://purl.org/nemo/gufo#ComplexEvent"/>
        <rdfs:comment xml:lang="en">Identifies a gufo:Event of which the event is part. 

For example, Cristiano Ronaldo&apos;s penalty kick is an event proper part of the 2016 FIFA Club World Cup Final, having ocurred in the 60th minute of that match. That match is itself an event proper part of the 2016 FIFA Club World Cup.

The match can be decomposed in different ways. For example, we can identify the participation of each player in the match (instances of gufo:Participation that are proper parts of the match) or decomposed the match using some temporal segmentation (each minute of the match, each of which is a proper part of the match).

gufo:isEventProperPartOf is transitive.</rdfs:comment>
        <rdfs:label xml:lang="en">isEventProperPartOf</rdfs:label>
    </owl:ObjectProperty>
    


    <!-- http://purl.org/nemo/gufo#isObjectProperPartOf -->

    <owl:ObjectProperty rdf:about="http://purl.org/nemo/gufo#isObjectProperPartOf">
        <rdfs:subPropertyOf rdf:resource="http://purl.org/nemo/gufo#isProperPartOf"/>
        <rdf:type rdf:resource="http://www.w3.org/2002/07/owl#TransitiveProperty"/>
        <rdfs:domain rdf:resource="http://purl.org/nemo/gufo#Object"/>
        <rdfs:range rdf:resource="http://purl.org/nemo/gufo#Object"/>
        <rdfs:comment xml:lang="en">Identifies a gufo:Object of which the object is a part.

This is a general parthood relation between objects. Use the various sub-properties provided in order to represent specific types of parthood, each of which has specialized semantics (and different formal properties in this implementation, in particular, transitivity (Guizzardi, 2005, section 5.6).</rdfs:comment>
        <rdfs:label xml:lang="en">isObjectProperPartOf</rdfs:label>
    </owl:ObjectProperty>
    


    <!-- http://purl.org/nemo/gufo#isProperPartOf -->

    <owl:ObjectProperty rdf:about="http://purl.org/nemo/gufo#isProperPartOf">
        <rdf:type rdf:resource="http://www.w3.org/2002/07/owl#TransitiveProperty"/>
        <rdfs:domain rdf:resource="http://www.w3.org/2002/07/owl#Thing"/>
        <rdfs:range rdf:resource="http://www.w3.org/2002/07/owl#Thing"/>
        <rdfs:comment xml:lang="en">Identifies a whole of which the entity is a proper part.

gufo:isProperPartOf is the most generic parthood relation in this implementation. Use the various sub-properties provided in order to represent specific types of parthood.

Proper parthood (and each of its sub-properties) is asymmetric and irreflexive. Nevertheless, these characteristics are not declared in this implementation since that would violate rules of OWL 2 DL that guarantee decidability of reasoning. Instead, we have focused only on declaring transitivity where applicable.

Note that gufo:isProperPartOf (as the most general notion of parthood) is transitive, although the various sub-properties may not be transitive.</rdfs:comment>
        <rdfs:label xml:lang="en">isProperPartOf</rdfs:label>
    </owl:ObjectProperty>
    


    <!-- http://purl.org/nemo/gufo#isSituationProperPartOf -->

    <owl:ObjectProperty rdf:about="http://purl.org/nemo/gufo#isSituationProperPartOf">
        <rdfs:subPropertyOf rdf:resource="http://purl.org/nemo/gufo#isProperPartOf"/>
        <rdfs:domain rdf:resource="http://purl.org/nemo/gufo#Situation"/>
        <rdfs:range rdf:resource="http://purl.org/nemo/gufo#Situation"/>
        <rdfs:comment xml:lang="en">Identifies a gufo:Situation of which the situation is a part.

Examples include: the situation in which John has influenza is part of the situation in which John has influenza and he is tired; the situation in which John is friends with Mary is part of the situation in which he is friends with Mary and Alice; the situation in which John is married to Alice is part of the situation in which John is married to Alice, while she works at the Free University of Bozen-Bolzano.</rdfs:comment>
        <rdfs:label xml:lang="en">isSituationProperPartOf</rdfs:label>
    </owl:ObjectProperty>
    


    <!-- http://purl.org/nemo/gufo#isSubCollectionOf -->

    <owl:ObjectProperty rdf:about="http://purl.org/nemo/gufo#isSubCollectionOf">
        <rdfs:subPropertyOf rdf:resource="http://purl.org/nemo/gufo#isObjectProperPartOf"/>
        <rdf:type rdf:resource="http://www.w3.org/2002/07/owl#TransitiveProperty"/>
        <rdfs:domain rdf:resource="http://purl.org/nemo/gufo#Collection"/>
        <rdfs:range rdf:resource="http://purl.org/nemo/gufo#Collection"/>
        <rdfs:comment xml:lang="en">Identifies a gufo:Collection of which the collection is a sub-collection. All members of the sub-collection are members of the identified super-collection.

gufo:isSubCollectionOf is transitive (Guizzardi, 2005, p. 186).

For parthood involving one or more varied collections, see gufo:standsInQualifiedParthood.</rdfs:comment>
        <rdfs:label xml:lang="en">isSubCollectionOf</rdfs:label>
        <rdfs:seeAlso rdf:resource="http://purl.org/nemo/gufo#standsInQualifiedParthood"/>
    </owl:ObjectProperty>
    


    <!-- http://purl.org/nemo/gufo#isSubQuantityOf -->

    <owl:ObjectProperty rdf:about="http://purl.org/nemo/gufo#isSubQuantityOf">
        <rdfs:subPropertyOf rdf:resource="http://purl.org/nemo/gufo#isObjectProperPartOf"/>
        <rdf:type rdf:resource="http://www.w3.org/2002/07/owl#TransitiveProperty"/>
        <rdfs:domain rdf:resource="http://purl.org/nemo/gufo#Quantity"/>
        <rdfs:range rdf:resource="http://purl.org/nemo/gufo#Quantity"/>
        <rdfs:comment xml:lang="en">Identifies a gufo:Quantity of which the quantity is a part.

For example, the quantity of water in a wine glass is a sub-quantity of the wine in that glass.

gufo:isSubQuantityOf is transitive (Guizzardi, 2005, p. 184).

Sub-quantities are always essential parts of their wholes. Thus, gufo:standsInQualifiedParthood is not applicable for sub-quantities.</rdfs:comment>
        <rdfs:label xml:lang="en">isSubQuantityOf</rdfs:label>
    </owl:ObjectProperty>
    


    <!-- http://purl.org/nemo/gufo#manifestedIn -->

    <owl:ObjectProperty rdf:about="http://purl.org/nemo/gufo#manifestedIn">
        <rdfs:domain rdf:resource="http://purl.org/nemo/gufo#Aspect"/>
        <rdfs:range rdf:resource="http://purl.org/nemo/gufo#Event"/>
        <rdfs:comment xml:lang="en">Identifies a gufo:Event in which the gufo:Aspect is manifested.

For example, the passing of an electrical current in a conductor is an event that encompasses the manifestation of an aspect inhering in a copper wire (the wire&apos;s  electrical conductivity).</rdfs:comment>
        <rdfs:label xml:lang="en">manifestedIn</rdfs:label>
    </owl:ObjectProperty>
    


    <!-- http://purl.org/nemo/gufo#mediates -->

    <owl:ObjectProperty rdf:about="http://purl.org/nemo/gufo#mediates">
        <rdf:type rdf:resource="http://www.w3.org/2002/07/owl#AsymmetricProperty"/>
        <rdf:type rdf:resource="http://www.w3.org/2002/07/owl#IrreflexiveProperty"/>
        <rdfs:domain rdf:resource="http://purl.org/nemo/gufo#Relator"/>
        <rdfs:range rdf:resource="http://purl.org/nemo/gufo#Endurant"/>
        <rdfs:comment xml:lang="en">Identifies the endurants mediated by a gufo:Relator.

For example, John and Mary&apos;s marriage mediates John and Mary.</rdfs:comment>
        <rdfs:label xml:lang="en">mediates</rdfs:label>
    </owl:ObjectProperty>
    


    <!-- http://purl.org/nemo/gufo#participatedIn -->

    <owl:ObjectProperty rdf:about="http://purl.org/nemo/gufo#participatedIn">
        <rdfs:domain rdf:resource="http://purl.org/nemo/gufo#Object"/>
        <rdfs:range rdf:resource="http://purl.org/nemo/gufo#Event"/>
        <rdfs:comment xml:lang="en">Identifies a gufo:Event in which the gufo:Object participated.

Examples include the participation of Freddy Mercury in Queen&apos;s Live Aid Concert and the participation of an airplane in a flight.</rdfs:comment>
        <rdfs:label xml:lang="en">participatedIn</rdfs:label>
    </owl:ObjectProperty>
    


    <!-- http://purl.org/nemo/gufo#partitions -->

    <owl:ObjectProperty rdf:about="http://purl.org/nemo/gufo#partitions">
        <rdfs:subPropertyOf rdf:resource="http://purl.org/nemo/gufo#categorizes"/>
        <rdfs:domain>
            <owl:Class>
                <owl:intersectionOf rdf:parseType="Collection">
                    <rdf:Description rdf:about="http://purl.org/nemo/gufo#Type"/>
                    <owl:Class>
                        <owl:complementOf rdf:resource="http://purl.org/nemo/gufo#AbstractEntityType"/>
                    </owl:Class>
                    <owl:Class>
                        <owl:complementOf rdf:resource="http://purl.org/nemo/gufo#ConcreteEntityType"/>
                    </owl:Class>
                </owl:intersectionOf>
            </owl:Class>
        </rdfs:domain>
        <rdfs:comment xml:lang="en">Identifies a gufo:Type whose instances are classified by exactly one instance of the partitioning higher-order type.

For example, &quot;AnimalSpecies&quot; gufo:partitions &quot;Animal&quot;. Instances of &quot;AnimalSpecies&quot; such as &quot;Lion&quot;, &quot;Hiena&quot; must be disjoint subclasses of &quot;Animal&quot;. OWL 2 punning should be used to capture the two facets of &quot;Lion&quot; and &quot;Hiena&quot; in this example: (i) as instances of &quot;AnimalSpecies&quot;, and (ii) as  subclasses of &quot;Animal&quot;.

Note that the partitioned type (in the example &quot;Animal&quot;) may or may not be declared to be a disjoint union of the explicitly enumerated subclasses (such as &quot;Lion&quot;, &quot;Hiena&quot;). This is because other instances of the higher-order type (&quot;AnimalSpecies&quot;) may exist that are not explicitly enumerated in the ontology.

The partitioned type is termed the &quot;base type&quot; in the &quot;powertype pattern&quot; see Carvalho et al (2017), the higher-order type is often called the &quot;powertype&quot;.  

For further details and formalization of &quot;partitioning&quot;, see Carvalho et al (2017) which combines UFO with MLT (a multi-level modeling theory).  

V. A. Carvalho, J. P. A. Almeida, C. M. Fonseca, and G. Guizzardi, “Multi-level ontology-based conceptual modeling,” Data &amp; Knowledge Engineering, vol. 109, p. 3–24, 2017. &lt;http://dx.doi.org/10.1016/j.datak.2017.03.002&gt;</rdfs:comment>
        <rdfs:label xml:lang="en">partitions</rdfs:label>
    </owl:ObjectProperty>
    


    <!-- http://purl.org/nemo/gufo#standsIn -->

    <owl:ObjectProperty rdf:about="http://purl.org/nemo/gufo#standsIn">
        <rdfs:domain rdf:resource="http://www.w3.org/2002/07/owl#Thing"/>
        <rdfs:range rdf:resource="http://purl.org/nemo/gufo#Situation"/>
        <rdfs:comment xml:lang="en">Identifies a gufo:Situation in which the entity stands. 

This implementation includes sub-properties of gufo:standsIn to identify situations concerning the attribution of (mutable) values to qualities, variable relationships, the instantiation of non-contingent types, temporary parthood and temporary constitution.</rdfs:comment>
        <rdfs:label xml:lang="en">standsIn</rdfs:label>
    </owl:ObjectProperty>
    


    <!-- http://purl.org/nemo/gufo#standsInQualifiedAttribution -->

    <owl:ObjectProperty rdf:about="http://purl.org/nemo/gufo#standsInQualifiedAttribution">
        <rdfs:subPropertyOf rdf:resource="http://purl.org/nemo/gufo#standsIn"/>
        <rdfs:domain rdf:resource="http://purl.org/nemo/gufo#Endurant"/>
        <rdfs:range rdf:resource="http://purl.org/nemo/gufo#QualityValueAttributionSituation"/>
        <rdfs:comment xml:lang="en">Identifies a gufo:QualityValueAttributionSituation in which the endurant stands. The identified gufo:QualityValueAttributionSituation is then used with the gufo:concernsQualityValue data property or the gufo:concernsReifiedQualityValue object property to indicate a quality value attributed to the gufo:Endurant standing in the situation. This forms a pattern to represent that quality values may differ in different situations.</rdfs:comment>
        <rdfs:label xml:lang="en">standsInQualifiedAttribution</rdfs:label>
        <rdfs:seeAlso rdf:resource="http://purl.org/nemo/gufo#QualityValueAttributionSituation"/>
    </owl:ObjectProperty>
    


    <!-- http://purl.org/nemo/gufo#standsInQualifiedConstitution -->

    <owl:ObjectProperty rdf:about="http://purl.org/nemo/gufo#standsInQualifiedConstitution">
        <rdfs:subPropertyOf rdf:resource="http://purl.org/nemo/gufo#standsIn"/>
        <rdfs:domain rdf:resource="http://purl.org/nemo/gufo#Endurant"/>
        <rdfs:range rdf:resource="http://purl.org/nemo/gufo#TemporaryConstitutionSituation"/>
        <rdfs:comment xml:lang="en">Identifies a gufo:TemporaryConstitutionSituation in which an endurant stands temporarily (as a constituent). The identified gufo:TemporaryConstitutionSituation is further related with an endurant (the whole) through the gufo:concernsConstitutedEndurant object property. This forms a pattern to represent temporary constitution, in which the relationships between constituents and constituted endurant vary in different situations.

Consider, for example, a group of people (understood as a gufo:FixedCollection) constituting a band (understood as a gufo:FunctionalComplex). In this case, any change in the membership of the group (e.g., the replacement of one person) creates a different group of people. Therefore, the band&apos;s constitution can change in time, and the pattern using gufo:TemporaryConstitutionSituation is applicable.</rdfs:comment>
        <rdfs:label xml:lang="en">standsInQualifiedConstitution</rdfs:label>
        <rdfs:seeAlso rdf:resource="http://purl.org/nemo/gufo#TemporaryConstitutionSituation"/>
    </owl:ObjectProperty>
    


    <!-- http://purl.org/nemo/gufo#standsInQualifiedInstantiation -->

    <owl:ObjectProperty rdf:about="http://purl.org/nemo/gufo#standsInQualifiedInstantiation">
        <rdfs:subPropertyOf rdf:resource="http://purl.org/nemo/gufo#standsIn"/>
        <rdfs:domain rdf:resource="http://purl.org/nemo/gufo#Endurant"/>
        <rdfs:range rdf:resource="http://purl.org/nemo/gufo#TemporaryInstantiationSituation"/>
        <rdfs:comment xml:lang="en">Identifies a gufo:TemporaryInstantiationSituation in which the endurant stands. The identified gufo:TemporaryInstantiationSituation is further related with a gufo:NonRigidType through the gufo:concernsNonRigidType object property. This forms a pattern to represent the contigent instantiation of a non-rigid type by the endurant, in which case instantiation may vary in different situations.</rdfs:comment>
        <rdfs:label xml:lang="en">standsInQualifiedInstantiation</rdfs:label>
        <rdfs:seeAlso rdf:resource="http://purl.org/nemo/gufo#TemporaryInstantiationSituation"/>
    </owl:ObjectProperty>
    


    <!-- http://purl.org/nemo/gufo#standsInQualifiedParthood -->

    <owl:ObjectProperty rdf:about="http://purl.org/nemo/gufo#standsInQualifiedParthood">
        <rdfs:subPropertyOf rdf:resource="http://purl.org/nemo/gufo#standsIn"/>
        <rdfs:domain rdf:resource="http://purl.org/nemo/gufo#Endurant"/>
        <rdfs:range rdf:resource="http://purl.org/nemo/gufo#TemporaryParthoodSituation"/>
        <rdfs:comment xml:lang="en">Identifies a gufo:TemporaryParthoodSituation in which the endurant stands (as a temporary part). The identified gufo:TemporaryParthoodSituation is further related with an endurant (the whole) through the gufo:concernsTemporaryWhole object property. This forms a pattern to represent temporary parthood, in which the relationships between parts and wholes vary in different situations. In particular, this pattern is useful in case parts may be separated from their wholes, attached to other wholes, replaced.</rdfs:comment>
        <rdfs:label xml:lang="en">standsInQualifiedParthood</rdfs:label>
        <rdfs:seeAlso rdf:resource="http://purl.org/nemo/gufo#TemporaryParthoodSituation"/>
    </owl:ObjectProperty>
    


    <!-- http://purl.org/nemo/gufo#standsInQualifiedRelationship -->

    <owl:ObjectProperty rdf:about="http://purl.org/nemo/gufo#standsInQualifiedRelationship">
        <rdfs:subPropertyOf rdf:resource="http://purl.org/nemo/gufo#standsIn"/>
        <rdfs:domain rdf:resource="http://purl.org/nemo/gufo#Endurant"/>
        <rdfs:range rdf:resource="http://purl.org/nemo/gufo#TemporaryRelationshipSituation"/>
        <rdfs:comment xml:lang="en">Identifies a gufo:TemporaryRelationshipSituation in which the endurant stands. The identified gufo:TemporaryRelationshipSituation is then used with the gufo:concernsRelatedEndurant and the gufo:concernsRelationshipType object properties to indicate the related element and the type of relationship that applies. This forms a pattern to represent that relationships that may change in different situations. For example, &quot;heavierThan&quot; may change when the objects involved gain or lose weight.

For material relations, prefer the use of gufo:Relator.</rdfs:comment>
        <rdfs:label xml:lang="en">standsInQualifiedRelationship</rdfs:label>
        <rdfs:seeAlso rdf:resource="http://purl.org/nemo/gufo#Relator"/>
        <rdfs:seeAlso rdf:resource="http://purl.org/nemo/gufo#TemporaryRelationshipSituation"/>
    </owl:ObjectProperty>
    


    <!-- http://purl.org/nemo/gufo#wasCreatedIn -->

    <owl:ObjectProperty rdf:about="http://purl.org/nemo/gufo#wasCreatedIn">
        <rdfs:domain rdf:resource="http://purl.org/nemo/gufo#Endurant"/>
        <rdfs:range rdf:resource="http://purl.org/nemo/gufo#Event"/>
        <rdfs:comment xml:lang="en">Identifies the gufo:Event which brought the gufo:Endurant into existence. 

For example, a musical piece is created in an act of composition (or in an event that is part of it), a piece of legislation is created in a complex legislative process.

Benevides et al. (2019) only discussed creation of objects; gufo:wasCreatedIn is extended to endurants in general. Further, in that work &quot;createdBy&quot; required the event to &quot;bring about&quot; a situation in which the created object is present. We relax this requirement here, such that the object may be created and terminated in the scope of the identified gufo:Event.

A. B. Benevides, J. R. Bourguet, G. Guizzardi, R. Penãloza, and J. P. A. Almeida, “Representing a reference foundational ontology of events in SROIQ,” Applied ontology, vol. 14, iss. 3, p. 293–334, 2019. &lt;http://dx.doi.org/10.3233/AO-190214&gt;</rdfs:comment>
        <rdfs:label xml:lang="en">wasCreatedIn</rdfs:label>
    </owl:ObjectProperty>
    


    <!-- http://purl.org/nemo/gufo#wasTerminatedIn -->

    <owl:ObjectProperty rdf:about="http://purl.org/nemo/gufo#wasTerminatedIn">
        <rdfs:domain rdf:resource="http://purl.org/nemo/gufo#Endurant"/>
        <rdfs:range rdf:resource="http://purl.org/nemo/gufo#Event"/>
        <rdfs:comment xml:lang="en">Identifies the gufo:Event in which the gufo:Endurant was brought to an end. 

For example, the Space Shuttle Challenger (OV-099) (a gufo:FunctionalComplex) was destroyed during the launch of its tenth flight (a gufo:Event). 

Benevides et al. (2019) only discussed termination of objects; gufo:wasCreatedIn is extended to endurants in general. This means that a gufo:Relator (such as a marriage) can be declared terminated. Further, in that work &quot;terminatedBy&quot; required the event to be &quot;triggered&quot; by a situation in which the terminated object is present. We relax this requirement here, such that the object may be created and terminated in the scope of the identified gufo:Event.

A. B. Benevides, J. R. Bourguet, G. Guizzardi, R. Penãloza, and J. P. A. Almeida, “Representing a reference foundational ontology of events in SROIQ,” Applied ontology, vol. 14, iss. 3, p. 293–334, 2019. &lt;http://dx.doi.org/10.3233/AO-190214&gt;</rdfs:comment>
        <rdfs:label xml:lang="en">wasTerminatedIn</rdfs:label>
    </owl:ObjectProperty>
    


    <!-- http://www.opengis.net/ont/geosparql#defaultGeometry -->

    <owl:ObjectProperty rdf:about="http://www.opengis.net/ont/geosparql#defaultGeometry">
        <rdfs:subPropertyOf rdf:resource="http://www.opengis.net/ont/geosparql#hasGeometry"/>
        <rdfs:domain rdf:resource="http://www.opengis.net/ont/geosparql#Feature"/>
        <rdfs:range rdf:resource="http://www.opengis.net/ont/geosparql#Geometry"/>
        <dc:contributor>Matthew Perry</dc:contributor>
        <dc:creator>OGC GeoSPARQL 1.0 Standard Working Group</dc:creator>
        <dc:date rdf:datatype="http://www.w3.org/2001/XMLSchema#date">2011-06-16</dc:date>
        <dc:description xml:lang="en">
      The default geometry to be used in spatial calculations.
      It is Usually the most detailed geometry.
    </dc:description>
        <rdfs:comment xml:lang="en">
      The default geometry to be used in spatial calculations.
      It is Usually the most detailed geometry.
    </rdfs:comment>
        <rdfs:isDefinedBy rdf:resource="http://www.opengis.net/ont/geosparql"/>
        <rdfs:isDefinedBy rdf:resource="http://www.opengis.net/spec/geosparql/1.0"/>
        <rdfs:label xml:lang="en">defaultGeometry</rdfs:label>
        <skos:definition xml:lang="en">
      The default geometry to be used in spatial calculations.
      It is Usually the most detailed geometry.
    </skos:definition>
        <skos:prefLabel xml:lang="en">defaultGeometry</skos:prefLabel>
    </owl:ObjectProperty>
    


    <!-- http://www.opengis.net/ont/geosparql#ehContains -->

    <owl:ObjectProperty rdf:about="http://www.opengis.net/ont/geosparql#ehContains">
        <rdfs:domain rdf:resource="http://www.opengis.net/ont/geosparql#SpatialObject"/>
        <rdfs:range rdf:resource="http://www.opengis.net/ont/geosparql#SpatialObject"/>
        <dc:contributor>Matthew Perry</dc:contributor>
        <dc:creator>OGC GeoSPARQL 1.0 Standard Working Group</dc:creator>
        <dc:date rdf:datatype="http://www.w3.org/2001/XMLSchema#date">2011-06-16</dc:date>
        <dc:description xml:lang="en">
      Exists if the subject SpatialObject spatially contains the 
      object SpatialObject. DE-9IM: T*TFF*FF*
    </dc:description>
        <rdfs:comment xml:lang="en">
      Exists if the subject SpatialObject spatially contains the 
      object SpatialObject. DE-9IM: T*TFF*FF*
    </rdfs:comment>
        <rdfs:isDefinedBy rdf:resource="http://www.opengis.net/ont/geosparql"/>
        <rdfs:isDefinedBy rdf:resource="http://www.opengis.net/spec/geosparql/1.0"/>
        <rdfs:label xml:lang="en">contains</rdfs:label>
        <skos:definition xml:lang="en">
      Exists if the subject SpatialObject spatially contains the 
      object SpatialObject. DE-9IM: T*TFF*FF*
    </skos:definition>
        <skos:prefLabel xml:lang="en">contains</skos:prefLabel>
    </owl:ObjectProperty>
    


    <!-- http://www.opengis.net/ont/geosparql#ehCoveredBy -->

    <owl:ObjectProperty rdf:about="http://www.opengis.net/ont/geosparql#ehCoveredBy">
        <rdfs:domain rdf:resource="http://www.opengis.net/ont/geosparql#SpatialObject"/>
        <rdfs:range rdf:resource="http://www.opengis.net/ont/geosparql#SpatialObject"/>
        <dc:contributor>Matthew Perry</dc:contributor>
        <dc:creator>OGC GeoSPARQL 1.0 Standard Working Group</dc:creator>
        <dc:date rdf:datatype="http://www.w3.org/2001/XMLSchema#date">2011-06-16</dc:date>
        <dc:description xml:lang="en">
      Exists if the subject SpatialObject is spatially covered 
      by the object SpatialObject. DE-9IM: TFF*TFT**
    </dc:description>
        <rdfs:comment xml:lang="en">
      Exists if the subject SpatialObject is spatially covered 
      by the object SpatialObject. DE-9IM: TFF*TFT**
    </rdfs:comment>
        <rdfs:isDefinedBy rdf:resource="http://www.opengis.net/ont/geosparql"/>
        <rdfs:isDefinedBy rdf:resource="http://www.opengis.net/spec/geosparql/1.0"/>
        <rdfs:label xml:lang="en">coveredBy</rdfs:label>
        <skos:definition xml:lang="en">
      Exists if the subject SpatialObject is spatially covered 
      by the object SpatialObject. DE-9IM: TFF*TFT**
    </skos:definition>
        <skos:prefLabel xml:lang="en">coveredBy</skos:prefLabel>
    </owl:ObjectProperty>
    


    <!-- http://www.opengis.net/ont/geosparql#ehCovers -->

    <owl:ObjectProperty rdf:about="http://www.opengis.net/ont/geosparql#ehCovers">
        <rdfs:domain rdf:resource="http://www.opengis.net/ont/geosparql#SpatialObject"/>
        <rdfs:range rdf:resource="http://www.opengis.net/ont/geosparql#SpatialObject"/>
        <dc:contributor>Matthew Perry</dc:contributor>
        <dc:creator>OGC GeoSPARQL 1.0 Standard Working Group</dc:creator>
        <dc:date rdf:datatype="http://www.w3.org/2001/XMLSchema#date">2011-06-16</dc:date>
        <dc:description xml:lang="en">
      Exists if the subject SpatialObject spatially covers the 
      object SpatialObject. DE-9IM: T*TFT*FF*
    </dc:description>
        <rdfs:comment xml:lang="en">
      Exists if the subject SpatialObject spatially covers the 
      object SpatialObject. DE-9IM: T*TFT*FF*
    </rdfs:comment>
        <rdfs:isDefinedBy rdf:resource="http://www.opengis.net/ont/geosparql"/>
        <rdfs:isDefinedBy rdf:resource="http://www.opengis.net/spec/geosparql/1.0"/>
        <rdfs:label xml:lang="en">covers</rdfs:label>
        <skos:definition xml:lang="en">
      Exists if the subject SpatialObject spatially covers the 
      object SpatialObject. DE-9IM: T*TFT*FF*
    </skos:definition>
        <skos:prefLabel xml:lang="en">covers</skos:prefLabel>
    </owl:ObjectProperty>
    


    <!-- http://www.opengis.net/ont/geosparql#ehDisjoint -->

    <owl:ObjectProperty rdf:about="http://www.opengis.net/ont/geosparql#ehDisjoint">
        <rdfs:domain rdf:resource="http://www.opengis.net/ont/geosparql#SpatialObject"/>
        <rdfs:range rdf:resource="http://www.opengis.net/ont/geosparql#SpatialObject"/>
        <dc:contributor>Matthew Perry</dc:contributor>
        <dc:creator>OGC GeoSPARQL 1.0 Standard Working Group</dc:creator>
        <dc:date rdf:datatype="http://www.w3.org/2001/XMLSchema#date">2011-06-16</dc:date>
        <dc:description xml:lang="en">
      Exists if the subject SpatialObject is spatially disjoint
      from the object SpatialObject. DE-9IM: FF*FF****
    </dc:description>
        <rdfs:comment xml:lang="en">
      Exists if the subject SpatialObject is spatially disjoint
      from the object SpatialObject. DE-9IM: FF*FF****
    </rdfs:comment>
        <rdfs:isDefinedBy rdf:resource="http://www.opengis.net/ont/geosparql"/>
        <rdfs:isDefinedBy rdf:resource="http://www.opengis.net/spec/geosparql/1.0"/>
        <rdfs:label xml:lang="en">disjoint</rdfs:label>
        <skos:definition xml:lang="en">
      Exists if the subject SpatialObject is spatially disjoint
      from the object SpatialObject. DE-9IM: FF*FF****
    </skos:definition>
        <skos:prefLabel xml:lang="en">disjoint</skos:prefLabel>
    </owl:ObjectProperty>
    


    <!-- http://www.opengis.net/ont/geosparql#ehEquals -->

    <owl:ObjectProperty rdf:about="http://www.opengis.net/ont/geosparql#ehEquals">
        <rdfs:domain rdf:resource="http://www.opengis.net/ont/geosparql#SpatialObject"/>
        <rdfs:range rdf:resource="http://www.opengis.net/ont/geosparql#SpatialObject"/>
        <dc:contributor>Matthew Perry</dc:contributor>
        <dc:creator>OGC GeoSPARQL 1.0 Standard Working Group</dc:creator>
        <dc:date rdf:datatype="http://www.w3.org/2001/XMLSchema#date">2011-06-16</dc:date>
        <dc:description xml:lang="en">
      Exists if the subject SpatialObject spatially equals the 
      object SpatialObject. DE-9IM: TFFFTFFFT
    </dc:description>
        <rdfs:comment xml:lang="en">
      Exists if the subject SpatialObject spatially equals the 
      object SpatialObject. DE-9IM: TFFFTFFFT
    </rdfs:comment>
        <rdfs:isDefinedBy rdf:resource="http://www.opengis.net/ont/geosparql"/>
        <rdfs:isDefinedBy rdf:resource="http://www.opengis.net/spec/geosparql/1.0"/>
        <rdfs:label xml:lang="en">equals</rdfs:label>
        <skos:definition xml:lang="en">
      Exists if the subject SpatialObject spatially equals the 
      object SpatialObject. DE-9IM: TFFFTFFFT
    </skos:definition>
        <skos:prefLabel xml:lang="en">equals</skos:prefLabel>
    </owl:ObjectProperty>
    


    <!-- http://www.opengis.net/ont/geosparql#ehInside -->

    <owl:ObjectProperty rdf:about="http://www.opengis.net/ont/geosparql#ehInside">
        <rdfs:domain rdf:resource="http://www.opengis.net/ont/geosparql#SpatialObject"/>
        <rdfs:range rdf:resource="http://www.opengis.net/ont/geosparql#SpatialObject"/>
        <dc:contributor>Matthew Perry</dc:contributor>
        <dc:creator>OGC GeoSPARQL 1.0 Standard Working Group</dc:creator>
        <dc:date rdf:datatype="http://www.w3.org/2001/XMLSchema#date">2011-06-16</dc:date>
        <dc:description xml:lang="en">
      Exists if the subject SpatialObject is spatially inside 
      the object SpatialObject. DE-9IM: TFF*FFT**
    </dc:description>
        <rdfs:comment xml:lang="en">
      Exists if the subject SpatialObject is spatially inside 
      the object SpatialObject. DE-9IM: TFF*FFT**
    </rdfs:comment>
        <rdfs:isDefinedBy rdf:resource="http://www.opengis.net/ont/geosparql"/>
        <rdfs:isDefinedBy rdf:resource="http://www.opengis.net/spec/geosparql/1.0"/>
        <rdfs:label xml:lang="en">inside</rdfs:label>
        <skos:definition xml:lang="en">
      Exists if the subject SpatialObject is spatially inside 
      the object SpatialObject. DE-9IM: TFF*FFT**
    </skos:definition>
        <skos:prefLabel xml:lang="en">inside</skos:prefLabel>
    </owl:ObjectProperty>
    


    <!-- http://www.opengis.net/ont/geosparql#ehMeet -->

    <owl:ObjectProperty rdf:about="http://www.opengis.net/ont/geosparql#ehMeet">
        <rdfs:domain rdf:resource="http://www.opengis.net/ont/geosparql#SpatialObject"/>
        <rdfs:range rdf:resource="http://www.opengis.net/ont/geosparql#SpatialObject"/>
        <dc:contributor>Matthew Perry</dc:contributor>
        <dc:creator>OGC GeoSPARQL 1.0 Standard Working Group</dc:creator>
        <dc:date rdf:datatype="http://www.w3.org/2001/XMLSchema#date">2011-06-16</dc:date>
        <dc:description xml:lang="en">
      Exists if the subject SpatialObject spatially meets the 
      object SpatialObject. 
      DE-9IM: FT******* ^ F**T***** ^ F***T****
    </dc:description>
        <rdfs:comment xml:lang="en">
      Exists if the subject SpatialObject spatially meets the 
      object SpatialObject. 
      DE-9IM: FT******* ^ F**T***** ^ F***T****
    </rdfs:comment>
        <rdfs:isDefinedBy rdf:resource="http://www.opengis.net/ont/geosparql"/>
        <rdfs:isDefinedBy rdf:resource="http://www.opengis.net/spec/geosparql/1.0"/>
        <rdfs:label xml:lang="en">meet</rdfs:label>
        <skos:definition xml:lang="en">
      Exists if the subject SpatialObject spatially meets the 
      object SpatialObject. 
      DE-9IM: FT******* ^ F**T***** ^ F***T****
    </skos:definition>
        <skos:prefLabel xml:lang="en">meet</skos:prefLabel>
    </owl:ObjectProperty>
    


    <!-- http://www.opengis.net/ont/geosparql#ehOverlap -->

    <owl:ObjectProperty rdf:about="http://www.opengis.net/ont/geosparql#ehOverlap">
        <rdfs:domain rdf:resource="http://www.opengis.net/ont/geosparql#SpatialObject"/>
        <rdfs:range rdf:resource="http://www.opengis.net/ont/geosparql#SpatialObject"/>
        <dc:contributor>Matthew Perry</dc:contributor>
        <dc:creator>OGC GeoSPARQL 1.0 Standard Working Group</dc:creator>
        <dc:date rdf:datatype="http://www.w3.org/2001/XMLSchema#date">2011-06-16</dc:date>
        <dc:description xml:lang="en">
      Exists if the subject SpatialObject spatially overlaps the 
      object SpatialObject. DE-9IM: T*T***T**
    </dc:description>
        <rdfs:comment xml:lang="en">
      Exists if the subject SpatialObject spatially overlaps the 
      object SpatialObject. DE-9IM: T*T***T**
    </rdfs:comment>
        <rdfs:isDefinedBy rdf:resource="http://www.opengis.net/ont/geosparql"/>
        <rdfs:isDefinedBy rdf:resource="http://www.opengis.net/spec/geosparql/1.0"/>
        <rdfs:label xml:lang="en">overlap</rdfs:label>
        <skos:definition xml:lang="en">
      Exists if the subject SpatialObject spatially overlaps the 
      object SpatialObject. DE-9IM: T*T***T**
    </skos:definition>
        <skos:prefLabel xml:lang="en">overlap</skos:prefLabel>
    </owl:ObjectProperty>
    


    <!-- http://www.opengis.net/ont/geosparql#hasGeometry -->

    <owl:ObjectProperty rdf:about="http://www.opengis.net/ont/geosparql#hasGeometry">
        <rdfs:domain rdf:resource="http://www.opengis.net/ont/geosparql#Feature"/>
        <rdfs:range rdf:resource="http://www.opengis.net/ont/geosparql#Geometry"/>
        <dc:contributor>Matthew Perry</dc:contributor>
        <dc:creator>OGC GeoSPARQL 1.0 Standard Working Group</dc:creator>
        <dc:date rdf:datatype="http://www.w3.org/2001/XMLSchema#date">2011-06-16</dc:date>
        <dc:description xml:lang="en">
      A spatial representation for a given feature.
    </dc:description>
        <rdfs:comment xml:lang="en">
      A spatial representation for a given feature.
    </rdfs:comment>
        <rdfs:isDefinedBy rdf:resource="http://www.opengis.net/ont/geosparql"/>
        <rdfs:isDefinedBy rdf:resource="http://www.opengis.net/spec/geosparql/1.0"/>
        <rdfs:label xml:lang="en">hasGeometry</rdfs:label>
        <skos:definition xml:lang="en">
      A spatial representation for a given feature.
    </skos:definition>
        <skos:prefLabel xml:lang="en">hasGeometry</skos:prefLabel>
    </owl:ObjectProperty>
    


    <!-- http://www.opengis.net/ont/geosparql#rcc8dc -->

    <owl:ObjectProperty rdf:about="http://www.opengis.net/ont/geosparql#rcc8dc">
        <rdf:type rdf:resource="http://www.w3.org/2002/07/owl#SymmetricProperty"/>
        <rdfs:domain rdf:resource="http://www.opengis.net/ont/geosparql#SpatialObject"/>
        <rdfs:range rdf:resource="http://www.opengis.net/ont/geosparql#SpatialObject"/>
        <dc:contributor>Matthew Perry</dc:contributor>
        <dc:creator>OGC GeoSPARQL 1.0 Standard Working Group</dc:creator>
        <dc:date rdf:datatype="http://www.w3.org/2001/XMLSchema#date">2011-06-16</dc:date>
        <dc:description xml:lang="en">
      Exists if the subject SpatialObject is spatially disjoint
      from the object SpatialObject. DE-9IM: FFTFFTTTT
    </dc:description>
        <rdfs:comment xml:lang="en">
      Exists if the subject SpatialObject is spatially disjoint
      from the object SpatialObject. DE-9IM: FFTFFTTTT
    </rdfs:comment>
        <rdfs:isDefinedBy rdf:resource="http://www.opengis.net/ont/geosparql"/>
        <rdfs:isDefinedBy rdf:resource="http://www.opengis.net/spec/geosparql/1.0"/>
        <rdfs:label xml:lang="en">disconnected</rdfs:label>
        <skos:definition xml:lang="en">
      Exists if the subject SpatialObject is spatially disjoint
      from the object SpatialObject. DE-9IM: FFTFFTTTT
    </skos:definition>
        <skos:prefLabel xml:lang="en">disconnected</skos:prefLabel>
    </owl:ObjectProperty>
    


    <!-- http://www.opengis.net/ont/geosparql#rcc8ec -->

    <owl:ObjectProperty rdf:about="http://www.opengis.net/ont/geosparql#rcc8ec">
        <rdf:type rdf:resource="http://www.w3.org/2002/07/owl#SymmetricProperty"/>
        <rdfs:domain rdf:resource="http://www.opengis.net/ont/geosparql#SpatialObject"/>
        <rdfs:range rdf:resource="http://www.opengis.net/ont/geosparql#SpatialObject"/>
        <dc:contributor>Matthew Perry</dc:contributor>
        <dc:creator>OGC GeoSPARQL 1.0 Standard Working Group</dc:creator>
        <dc:date rdf:datatype="http://www.w3.org/2001/XMLSchema#date">2011-06-16</dc:date>
        <dc:description xml:lang="en">
      Exists if the subject SpatialObject spatially meets the 
      object SpatialObject. DE-9IM: FFTFTTTTT
    </dc:description>
        <rdfs:comment xml:lang="en">
      Exists if the subject SpatialObject spatially meets the 
      object SpatialObject. DE-9IM: FFTFTTTTT
    </rdfs:comment>
        <rdfs:isDefinedBy rdf:resource="http://www.opengis.net/ont/geosparql"/>
        <rdfs:isDefinedBy rdf:resource="http://www.opengis.net/spec/geosparql/1.0"/>
        <rdfs:label xml:lang="en">externally connected</rdfs:label>
        <skos:definition xml:lang="en">
      Exists if the subject SpatialObject spatially meets the 
      object SpatialObject. DE-9IM: FFTFTTTTT
    </skos:definition>
        <skos:prefLabel xml:lang="en">externally connected</skos:prefLabel>
    </owl:ObjectProperty>
    


    <!-- http://www.opengis.net/ont/geosparql#rcc8eq -->

    <owl:ObjectProperty rdf:about="http://www.opengis.net/ont/geosparql#rcc8eq">
        <rdf:type rdf:resource="http://www.w3.org/2002/07/owl#SymmetricProperty"/>
        <rdf:type rdf:resource="http://www.w3.org/2002/07/owl#TransitiveProperty"/>
        <rdfs:domain rdf:resource="http://www.opengis.net/ont/geosparql#SpatialObject"/>
        <rdfs:range rdf:resource="http://www.opengis.net/ont/geosparql#SpatialObject"/>
        <dc:contributor>Matthew Perry</dc:contributor>
        <dc:creator>OGC GeoSPARQL 1.0 Standard Working Group</dc:creator>
        <dc:date rdf:datatype="http://www.w3.org/2001/XMLSchema#date">2011-06-16</dc:date>
        <dc:description xml:lang="en">
      Exists if the subject SpatialObject spatially equals the 
      object SpatialObject. DE-9IM: TFFFTFFFT
    </dc:description>
        <rdfs:comment xml:lang="en">
      Exists if the subject SpatialObject spatially equals the 
      object SpatialObject. DE-9IM: TFFFTFFFT
    </rdfs:comment>
        <rdfs:isDefinedBy rdf:resource="http://www.opengis.net/ont/geosparql"/>
        <rdfs:isDefinedBy rdf:resource="http://www.opengis.net/spec/geosparql/1.0"/>
        <rdfs:label xml:lang="en">equals</rdfs:label>
        <skos:definition xml:lang="en">
      Exists if the subject SpatialObject spatially equals the 
      object SpatialObject. DE-9IM: TFFFTFFFT
    </skos:definition>
        <skos:prefLabel xml:lang="en">equals</skos:prefLabel>
    </owl:ObjectProperty>
    


    <!-- http://www.opengis.net/ont/geosparql#rcc8ntpp -->

    <owl:ObjectProperty rdf:about="http://www.opengis.net/ont/geosparql#rcc8ntpp">
        <owl:inverseOf rdf:resource="http://www.opengis.net/ont/geosparql#rcc8ntppi"/>
        <rdf:type rdf:resource="http://www.w3.org/2002/07/owl#TransitiveProperty"/>
        <rdfs:domain rdf:resource="http://www.opengis.net/ont/geosparql#SpatialObject"/>
        <rdfs:range rdf:resource="http://www.opengis.net/ont/geosparql#SpatialObject"/>
        <dc:contributor>Matthew Perry</dc:contributor>
        <dc:creator>OGC GeoSPARQL 1.0 Standard Working Group</dc:creator>
        <dc:date rdf:datatype="http://www.w3.org/2001/XMLSchema#date">2011-06-16</dc:date>
        <dc:description xml:lang="en">
      Exists if the subject SpatialObject is spatially inside 
      the object SpatialObject. DE-9IM: TFFTFFTTT
    </dc:description>
        <rdfs:comment xml:lang="en">
      Exists if the subject SpatialObject is spatially inside 
      the object SpatialObject. DE-9IM: TFFTFFTTT
    </rdfs:comment>
        <rdfs:isDefinedBy rdf:resource="http://www.opengis.net/ont/geosparql"/>
        <rdfs:isDefinedBy rdf:resource="http://www.opengis.net/spec/geosparql/1.0"/>
        <rdfs:label xml:lang="en">non-tangential proper part</rdfs:label>
        <skos:definition xml:lang="en">
      Exists if the subject SpatialObject is spatially inside 
      the object SpatialObject. DE-9IM: TFFTFFTTT
    </skos:definition>
        <skos:prefLabel xml:lang="en">non-tangential proper part</skos:prefLabel>
    </owl:ObjectProperty>
    


    <!-- http://www.opengis.net/ont/geosparql#rcc8ntppi -->

    <owl:ObjectProperty rdf:about="http://www.opengis.net/ont/geosparql#rcc8ntppi">
        <rdf:type rdf:resource="http://www.w3.org/2002/07/owl#TransitiveProperty"/>
        <rdfs:domain rdf:resource="http://www.opengis.net/ont/geosparql#SpatialObject"/>
        <rdfs:range rdf:resource="http://www.opengis.net/ont/geosparql#SpatialObject"/>
        <dc:contributor>Matthew Perry</dc:contributor>
        <dc:creator>OGC GeoSPARQL 1.0 Standard Working Group</dc:creator>
        <dc:date rdf:datatype="http://www.w3.org/2001/XMLSchema#date">2011-06-16</dc:date>
        <dc:description xml:lang="en">
      Exists if the subject SpatialObject spatially contains the 
      object SpatialObject. DE-9IM: TTTFFTFFT
    </dc:description>
        <rdfs:comment xml:lang="en">
      Exists if the subject SpatialObject spatially contains the 
      object SpatialObject. DE-9IM: TTTFFTFFT
    </rdfs:comment>
        <rdfs:isDefinedBy rdf:resource="http://www.opengis.net/ont/geosparql"/>
        <rdfs:isDefinedBy rdf:resource="http://www.opengis.net/spec/geosparql/1.0"/>
        <rdfs:label xml:lang="en">non-tangential proper part inverse</rdfs:label>
        <skos:definition xml:lang="en">
      Exists if the subject SpatialObject spatially contains the 
      object SpatialObject. DE-9IM: TTTFFTFFT
    </skos:definition>
        <skos:prefLabel xml:lang="en">non-tangential proper part inverse</skos:prefLabel>
    </owl:ObjectProperty>
    


    <!-- http://www.opengis.net/ont/geosparql#rcc8po -->

    <owl:ObjectProperty rdf:about="http://www.opengis.net/ont/geosparql#rcc8po">
        <rdf:type rdf:resource="http://www.w3.org/2002/07/owl#SymmetricProperty"/>
        <rdfs:domain rdf:resource="http://www.opengis.net/ont/geosparql#SpatialObject"/>
        <rdfs:range rdf:resource="http://www.opengis.net/ont/geosparql#SpatialObject"/>
        <dc:contributor>Matthew Perry</dc:contributor>
        <dc:creator>OGC GeoSPARQL 1.0 Standard Working Group</dc:creator>
        <dc:date rdf:datatype="http://www.w3.org/2001/XMLSchema#date">2011-06-16</dc:date>
        <dc:description xml:lang="en">
      Exists if the subject SpatialObject spatially overlaps the 
      object SpatialObject. DE-9IM: TTTTTTTTT
    </dc:description>
        <rdfs:comment xml:lang="en">
      Exists if the subject SpatialObject spatially overlaps the 
      object SpatialObject. DE-9IM: TTTTTTTTT
    </rdfs:comment>
        <rdfs:isDefinedBy rdf:resource="http://www.opengis.net/ont/geosparql"/>
        <rdfs:isDefinedBy rdf:resource="http://www.opengis.net/spec/geosparql/1.0"/>
        <rdfs:label xml:lang="en">partially overlapping</rdfs:label>
        <skos:definition xml:lang="en">
      Exists if the subject SpatialObject spatially overlaps the 
      object SpatialObject. DE-9IM: TTTTTTTTT
    </skos:definition>
        <skos:prefLabel xml:lang="en">partially overlapping</skos:prefLabel>
    </owl:ObjectProperty>
    


    <!-- http://www.opengis.net/ont/geosparql#rcc8tpp -->

    <owl:ObjectProperty rdf:about="http://www.opengis.net/ont/geosparql#rcc8tpp">
        <owl:inverseOf rdf:resource="http://www.opengis.net/ont/geosparql#rcc8tppi"/>
        <rdf:type rdf:resource="http://www.w3.org/2002/07/owl#TransitiveProperty"/>
        <rdfs:domain rdf:resource="http://www.opengis.net/ont/geosparql#SpatialObject"/>
        <rdfs:range rdf:resource="http://www.opengis.net/ont/geosparql#SpatialObject"/>
        <dc:contributor>Matthew Perry</dc:contributor>
        <dc:creator>OGC GeoSPARQL 1.0 Standard Working Group</dc:creator>
        <dc:date rdf:datatype="http://www.w3.org/2001/XMLSchema#date">2011-06-16</dc:date>
        <dc:description xml:lang="en">
      Exists if the subject SpatialObject is spatially covered 
      by the object SpatialObject. DE-9IM: TFFTTFTTT
    </dc:description>
        <rdfs:comment xml:lang="en">
      Exists if the subject SpatialObject is spatially covered 
      by the object SpatialObject. DE-9IM: TFFTTFTTT
    </rdfs:comment>
        <rdfs:isDefinedBy rdf:resource="http://www.opengis.net/ont/geosparql"/>
        <rdfs:isDefinedBy rdf:resource="http://www.opengis.net/spec/geosparql/1.0"/>
        <rdfs:label xml:lang="en">tangential proper part</rdfs:label>
        <skos:definition xml:lang="en">
      Exists if the subject SpatialObject is spatially covered 
      by the object SpatialObject. DE-9IM: TFFTTFTTT
    </skos:definition>
        <skos:prefLabel xml:lang="en">tangential proper part</skos:prefLabel>
    </owl:ObjectProperty>
    


    <!-- http://www.opengis.net/ont/geosparql#rcc8tppi -->

    <owl:ObjectProperty rdf:about="http://www.opengis.net/ont/geosparql#rcc8tppi">
        <rdf:type rdf:resource="http://www.w3.org/2002/07/owl#TransitiveProperty"/>
        <rdfs:domain rdf:resource="http://www.opengis.net/ont/geosparql#SpatialObject"/>
        <rdfs:range rdf:resource="http://www.opengis.net/ont/geosparql#SpatialObject"/>
        <dc:contributor>Matthew Perry</dc:contributor>
        <dc:creator>OGC GeoSPARQL 1.0 Standard Working Group</dc:creator>
        <dc:date rdf:datatype="http://www.w3.org/2001/XMLSchema#date">2011-06-16</dc:date>
        <dc:description xml:lang="en">
      Exists if the subject SpatialObject spatially covers the 
      object SpatialObject. DE-9IM: TTTFTTFFT
    </dc:description>
        <rdfs:comment xml:lang="en">
      Exists if the subject SpatialObject spatially covers the 
      object SpatialObject. DE-9IM: TTTFTTFFT
    </rdfs:comment>
        <rdfs:isDefinedBy rdf:resource="http://www.opengis.net/ont/geosparql"/>
        <rdfs:isDefinedBy rdf:resource="http://www.opengis.net/spec/geosparql/1.0"/>
        <rdfs:label xml:lang="en">tangential proper part inverse</rdfs:label>
        <skos:definition xml:lang="en">
      Exists if the subject SpatialObject spatially covers the 
      object SpatialObject. DE-9IM: TTTFTTFFT
    </skos:definition>
        <skos:prefLabel xml:lang="en">tangential proper part inverse</skos:prefLabel>
    </owl:ObjectProperty>
    


    <!-- http://www.opengis.net/ont/geosparql#sfContains -->

    <owl:ObjectProperty rdf:about="http://www.opengis.net/ont/geosparql#sfContains">
        <rdfs:domain rdf:resource="http://www.opengis.net/ont/geosparql#SpatialObject"/>
        <rdfs:range rdf:resource="http://www.opengis.net/ont/geosparql#SpatialObject"/>
        <dc:contributor>Matthew Perry</dc:contributor>
        <dc:creator>OGC GeoSPARQL 1.0 Standard Working Group</dc:creator>
        <dc:date rdf:datatype="http://www.w3.org/2001/XMLSchema#date">2011-06-16</dc:date>
        <dc:description xml:lang="en">
      Exists if the subject SpatialObject spatially contains the 
      object SpatialObject. DE-9IM: T*****FF*
    </dc:description>
        <rdfs:comment xml:lang="en">
      Exists if the subject SpatialObject spatially contains the 
      object SpatialObject. DE-9IM: T*****FF*
    </rdfs:comment>
        <rdfs:isDefinedBy rdf:resource="http://www.opengis.net/ont/geosparql"/>
        <rdfs:isDefinedBy rdf:resource="http://www.opengis.net/spec/geosparql/1.0"/>
        <rdfs:label xml:lang="en">contains</rdfs:label>
        <skos:definition xml:lang="en">
      Exists if the subject SpatialObject spatially contains the 
      object SpatialObject. DE-9IM: T*****FF*
    </skos:definition>
        <skos:prefLabel xml:lang="en">contains</skos:prefLabel>
    </owl:ObjectProperty>
    


    <!-- http://www.opengis.net/ont/geosparql#sfCrosses -->

    <owl:ObjectProperty rdf:about="http://www.opengis.net/ont/geosparql#sfCrosses">
        <rdfs:domain rdf:resource="http://www.opengis.net/ont/geosparql#SpatialObject"/>
        <rdfs:range rdf:resource="http://www.opengis.net/ont/geosparql#SpatialObject"/>
        <dc:contributor>Matthew Perry</dc:contributor>
        <dc:creator>OGC GeoSPARQL 1.0 Standard Working Group</dc:creator>
        <dc:date rdf:datatype="http://www.w3.org/2001/XMLSchema#date">2011-06-16</dc:date>
        <dc:description xml:lang="en">
      Exists if the subject SpatialObject spatially crosses the 
      object SpatialObject. DE-9IM: T*T******
    </dc:description>
        <rdfs:comment xml:lang="en">
      Exists if the subject SpatialObject spatially crosses the 
      object SpatialObject. DE-9IM: T*T******
    </rdfs:comment>
        <rdfs:isDefinedBy rdf:resource="http://www.opengis.net/ont/geosparql"/>
        <rdfs:isDefinedBy rdf:resource="http://www.opengis.net/spec/geosparql/1.0"/>
        <rdfs:label xml:lang="en">crosses</rdfs:label>
        <skos:definition xml:lang="en">
      Exists if the subject SpatialObject spatially crosses the 
      object SpatialObject. DE-9IM: T*T******
    </skos:definition>
        <skos:prefLabel xml:lang="en">crosses</skos:prefLabel>
    </owl:ObjectProperty>
    


    <!-- http://www.opengis.net/ont/geosparql#sfDisjoint -->

    <owl:ObjectProperty rdf:about="http://www.opengis.net/ont/geosparql#sfDisjoint">
        <rdfs:domain rdf:resource="http://www.opengis.net/ont/geosparql#SpatialObject"/>
        <rdfs:range rdf:resource="http://www.opengis.net/ont/geosparql#SpatialObject"/>
        <dc:contributor>Matthew Perry</dc:contributor>
        <dc:creator>OGC GeoSPARQL 1.0 Standard Working Group</dc:creator>
        <dc:date rdf:datatype="http://www.w3.org/2001/XMLSchema#date">2011-06-16</dc:date>
        <dc:description xml:lang="en">
      Exists if the subject SpatialObject is spatially disjoint 
      from the object SpatialObject. DE-9IM: FF*FF****
    </dc:description>
        <rdfs:comment xml:lang="en">
      Exists if the subject SpatialObject is spatially disjoint 
      from the object SpatialObject. DE-9IM: FF*FF****
    </rdfs:comment>
        <rdfs:isDefinedBy rdf:resource="http://www.opengis.net/ont/geosparql"/>
        <rdfs:isDefinedBy rdf:resource="http://www.opengis.net/spec/geosparql/1.0"/>
        <rdfs:label xml:lang="en">disjoint</rdfs:label>
        <skos:definition xml:lang="en">
      Exists if the subject SpatialObject is spatially disjoint 
      from the object SpatialObject. DE-9IM: FF*FF****
    </skos:definition>
        <skos:prefLabel xml:lang="en">disjoint</skos:prefLabel>
    </owl:ObjectProperty>
    


    <!-- http://www.opengis.net/ont/geosparql#sfEquals -->

    <owl:ObjectProperty rdf:about="http://www.opengis.net/ont/geosparql#sfEquals">
        <rdfs:domain rdf:resource="http://www.opengis.net/ont/geosparql#SpatialObject"/>
        <rdfs:range rdf:resource="http://www.opengis.net/ont/geosparql#SpatialObject"/>
        <dc:contributor>Matthew Perry</dc:contributor>
        <dc:creator>OGC GeoSPARQL 1.0 Standard Working Group</dc:creator>
        <dc:date rdf:datatype="http://www.w3.org/2001/XMLSchema#date">2011-06-16</dc:date>
        <dc:description xml:lang="en">
      Exists if the subject SpatialObject spatially equals the 
      object SpatialObject. DE-9IM: TFFFTFFFT
    </dc:description>
        <rdfs:comment xml:lang="en">
      Exists if the subject SpatialObject spatially equals the 
      object SpatialObject. DE-9IM: TFFFTFFFT
    </rdfs:comment>
        <rdfs:isDefinedBy rdf:resource="http://www.opengis.net/ont/geosparql"/>
        <rdfs:isDefinedBy rdf:resource="http://www.opengis.net/spec/geosparql/1.0"/>
        <rdfs:label xml:lang="en">equals</rdfs:label>
        <skos:definition xml:lang="en">
      Exists if the subject SpatialObject spatially equals the 
      object SpatialObject. DE-9IM: TFFFTFFFT
    </skos:definition>
        <skos:prefLabel xml:lang="en">equals</skos:prefLabel>
    </owl:ObjectProperty>
    


    <!-- http://www.opengis.net/ont/geosparql#sfIntersects -->

    <owl:ObjectProperty rdf:about="http://www.opengis.net/ont/geosparql#sfIntersects">
        <rdfs:domain rdf:resource="http://www.opengis.net/ont/geosparql#SpatialObject"/>
        <rdfs:range rdf:resource="http://www.opengis.net/ont/geosparql#SpatialObject"/>
        <dc:contributor>Matthew Perry</dc:contributor>
        <dc:creator>OGC GeoSPARQL 1.0 Standard Working Group</dc:creator>
        <dc:date rdf:datatype="http://www.w3.org/2001/XMLSchema#date">2011-06-16</dc:date>
        <dc:description xml:lang="en">
      Exists if the subject SpatialObject is not spatially disjoint 
      from the object SpatialObject.
      DE-9IM: T******** ^ *T******* ^ ***T***** ^ ****T**** 
    </dc:description>
        <rdfs:comment xml:lang="en">
      Exists if the subject SpatialObject is not spatially disjoint 
      from the object SpatialObject.
      DE-9IM: T******** ^ *T******* ^ ***T***** ^ ****T**** 
    </rdfs:comment>
        <rdfs:isDefinedBy rdf:resource="http://www.opengis.net/ont/geosparql"/>
        <rdfs:isDefinedBy rdf:resource="http://www.opengis.net/spec/geosparql/1.0"/>
        <rdfs:label xml:lang="en">intersects</rdfs:label>
        <skos:definition xml:lang="en">
      Exists if the subject SpatialObject is not spatially disjoint 
      from the object SpatialObject.
      DE-9IM: T******** ^ *T******* ^ ***T***** ^ ****T**** 
    </skos:definition>
        <skos:prefLabel xml:lang="en">intersects</skos:prefLabel>
    </owl:ObjectProperty>
    


    <!-- http://www.opengis.net/ont/geosparql#sfOverlaps -->

    <owl:ObjectProperty rdf:about="http://www.opengis.net/ont/geosparql#sfOverlaps">
        <rdfs:domain rdf:resource="http://www.opengis.net/ont/geosparql#SpatialObject"/>
        <rdfs:range rdf:resource="http://www.opengis.net/ont/geosparql#SpatialObject"/>
        <dc:contributor>Matthew Perry</dc:contributor>
        <dc:creator>OGC GeoSPARQL 1.0 Standard Working Group</dc:creator>
        <dc:date rdf:datatype="http://www.w3.org/2001/XMLSchema#date">2011-06-16</dc:date>
        <dc:description xml:lang="en">
      Exists if the subject SpatialObject spatially overlaps the 
      object SpatialObject. DE-9IM: T*T***T** 
    </dc:description>
        <rdfs:comment xml:lang="en">
      Exists if the subject SpatialObject spatially overlaps the 
      object SpatialObject. DE-9IM: T*T***T** 
    </rdfs:comment>
        <rdfs:isDefinedBy rdf:resource="http://www.opengis.net/ont/geosparql"/>
        <rdfs:isDefinedBy rdf:resource="http://www.opengis.net/spec/geosparql/1.0"/>
        <rdfs:label xml:lang="en">overlaps</rdfs:label>
        <skos:definition xml:lang="en">
      Exists if the subject SpatialObject spatially overlaps the 
      object SpatialObject. DE-9IM: T*T***T** 
    </skos:definition>
        <skos:prefLabel xml:lang="en">overlaps</skos:prefLabel>
    </owl:ObjectProperty>
    


    <!-- http://www.opengis.net/ont/geosparql#sfTouches -->

    <owl:ObjectProperty rdf:about="http://www.opengis.net/ont/geosparql#sfTouches">
        <rdfs:domain rdf:resource="http://www.opengis.net/ont/geosparql#SpatialObject"/>
        <rdfs:range rdf:resource="http://www.opengis.net/ont/geosparql#SpatialObject"/>
        <dc:contributor>Matthew Perry</dc:contributor>
        <dc:creator>OGC GeoSPARQL 1.0 Standard Working Group</dc:creator>
        <dc:date rdf:datatype="http://www.w3.org/2001/XMLSchema#date">2011-06-16</dc:date>
        <dc:description xml:lang="en">
      Exists if the subject SpatialObject spatially touches the 
      object SpatialObject.
      DE-9IM: FT******* ^ F**T***** ^ F***T****
    </dc:description>
        <rdfs:comment xml:lang="en">
      Exists if the subject SpatialObject spatially touches the 
      object SpatialObject.
      DE-9IM: FT******* ^ F**T***** ^ F***T****
    </rdfs:comment>
        <rdfs:isDefinedBy rdf:resource="http://www.opengis.net/ont/geosparql"/>
        <rdfs:isDefinedBy rdf:resource="http://www.opengis.net/spec/geosparql/1.0"/>
        <rdfs:label xml:lang="en">touches</rdfs:label>
        <skos:definition xml:lang="en">
      Exists if the subject SpatialObject spatially touches the 
      object SpatialObject.
      DE-9IM: FT******* ^ F**T***** ^ F***T****
    </skos:definition>
        <skos:prefLabel xml:lang="en">touches</skos:prefLabel>
    </owl:ObjectProperty>
    


    <!-- http://www.opengis.net/ont/geosparql#sfWithin -->

    <owl:ObjectProperty rdf:about="http://www.opengis.net/ont/geosparql#sfWithin">
        <rdfs:domain rdf:resource="http://www.opengis.net/ont/geosparql#SpatialObject"/>
        <rdfs:range rdf:resource="http://www.opengis.net/ont/geosparql#SpatialObject"/>
        <dc:contributor>Matthew Perry</dc:contributor>
        <dc:creator>OGC GeoSPARQL 1.0 Standard Working Group</dc:creator>
        <dc:date rdf:datatype="http://www.w3.org/2001/XMLSchema#date">2011-06-16</dc:date>
        <dc:description xml:lang="en">
      Exists if the subject SpatialObject is spatially within the 
      object SpatialObject. DE-9IM: T*F**F***
    </dc:description>
        <rdfs:comment xml:lang="en">
      Exists if the subject SpatialObject is spatially within the 
      object SpatialObject. DE-9IM: T*F**F***
    </rdfs:comment>
        <rdfs:isDefinedBy rdf:resource="http://www.opengis.net/ont/geosparql"/>
        <rdfs:isDefinedBy rdf:resource="http://www.opengis.net/spec/geosparql/1.0"/>
        <rdfs:label xml:lang="en">within</rdfs:label>
        <skos:definition xml:lang="en">
      Exists if the subject SpatialObject is spatially within the 
      object SpatialObject. DE-9IM: T*F**F***
    </skos:definition>
        <skos:prefLabel xml:lang="en">within</skos:prefLabel>
    </owl:ObjectProperty>
    


    <!-- http://www.w3.org/2004/02/skos/core#broadMatch -->

    <owl:ObjectProperty rdf:about="http://www.w3.org/2004/02/skos/core#broadMatch">
        <rdfs:subPropertyOf rdf:resource="http://www.w3.org/2004/02/skos/core#broader"/>
        <rdfs:subPropertyOf rdf:resource="http://www.w3.org/2004/02/skos/core#mappingRelation"/>
        <owl:inverseOf rdf:resource="http://www.w3.org/2004/02/skos/core#narrowMatch"/>
        <rdfs:isDefinedBy rdf:resource="http://www.w3.org/2004/02/skos/core"/>
        <rdfs:label xml:lang="en">has broader match</rdfs:label>
        <skos:definition xml:lang="en">skos:broadMatch is used to state a hierarchical mapping link between two conceptual resources in different concept schemes.</skos:definition>
    </owl:ObjectProperty>
    


    <!-- http://www.w3.org/2004/02/skos/core#broader -->

    <owl:ObjectProperty rdf:about="http://www.w3.org/2004/02/skos/core#broader">
        <rdfs:subPropertyOf rdf:resource="http://www.w3.org/2004/02/skos/core#broaderTransitive"/>
        <owl:inverseOf rdf:resource="http://www.w3.org/2004/02/skos/core#narrower"/>
        <rdfs:comment xml:lang="en">Broader concepts are typically rendered as parents in a concept hierarchy (tree).</rdfs:comment>
        <rdfs:isDefinedBy rdf:resource="http://www.w3.org/2004/02/skos/core"/>
        <rdfs:label xml:lang="en">has broader</rdfs:label>
        <skos:definition xml:lang="en">Relates a concept to a concept that is more general in meaning.</skos:definition>
        <skos:scopeNote xml:lang="en">By convention, skos:broader is only used to assert an immediate (i.e. direct) hierarchical link between two conceptual resources.</skos:scopeNote>
    </owl:ObjectProperty>
    


    <!-- http://www.w3.org/2004/02/skos/core#broaderTransitive -->

    <owl:ObjectProperty rdf:about="http://www.w3.org/2004/02/skos/core#broaderTransitive">
        <rdfs:subPropertyOf rdf:resource="http://www.w3.org/2004/02/skos/core#semanticRelation"/>
        <owl:inverseOf rdf:resource="http://www.w3.org/2004/02/skos/core#narrowerTransitive"/>
        <rdf:type rdf:resource="http://www.w3.org/2002/07/owl#TransitiveProperty"/>
        <rdfs:isDefinedBy rdf:resource="http://www.w3.org/2004/02/skos/core"/>
        <rdfs:label xml:lang="en">has broader transitive</rdfs:label>
        <skos:definition>skos:broaderTransitive is a transitive superproperty of skos:broader.</skos:definition>
        <skos:scopeNote xml:lang="en">By convention, skos:broaderTransitive is not used to make assertions. Rather, the properties can be used to draw inferences about the transitive closure of the hierarchical relation, which is useful e.g. when implementing a simple query expansion algorithm in a search application.</skos:scopeNote>
    </owl:ObjectProperty>
    


    <!-- http://www.w3.org/2004/02/skos/core#closeMatch -->

    <owl:ObjectProperty rdf:about="http://www.w3.org/2004/02/skos/core#closeMatch">
        <rdfs:subPropertyOf rdf:resource="http://www.w3.org/2004/02/skos/core#mappingRelation"/>
        <rdf:type rdf:resource="http://www.w3.org/2002/07/owl#SymmetricProperty"/>
        <rdfs:isDefinedBy rdf:resource="http://www.w3.org/2004/02/skos/core"/>
        <rdfs:label xml:lang="en">has close match</rdfs:label>
        <skos:definition xml:lang="en">skos:closeMatch is used to link two concepts that are sufficiently similar that they can be used interchangeably in some information retrieval applications. In order to avoid the possibility of &quot;compound errors&quot; when combining mappings across more than two concept schemes, skos:closeMatch is not declared to be a transitive property.</skos:definition>
    </owl:ObjectProperty>
    


    <!-- http://www.w3.org/2004/02/skos/core#exactMatch -->

    <owl:ObjectProperty rdf:about="http://www.w3.org/2004/02/skos/core#exactMatch">
        <rdfs:subPropertyOf rdf:resource="http://www.w3.org/2004/02/skos/core#closeMatch"/>
        <rdf:type rdf:resource="http://www.w3.org/2002/07/owl#SymmetricProperty"/>
        <rdf:type rdf:resource="http://www.w3.org/2002/07/owl#TransitiveProperty"/>
        <rdfs:comment xml:lang="en">skos:exactMatch is disjoint with each of the properties skos:broadMatch and skos:relatedMatch.</rdfs:comment>
        <rdfs:isDefinedBy rdf:resource="http://www.w3.org/2004/02/skos/core"/>
        <rdfs:label xml:lang="en">has exact match</rdfs:label>
        <skos:definition xml:lang="en">skos:exactMatch is used to link two concepts, indicating a high degree of confidence that the concepts can be used interchangeably across a wide range of information retrieval applications. skos:exactMatch is a transitive property, and is a sub-property of skos:closeMatch.</skos:definition>
    </owl:ObjectProperty>
    


    <!-- http://www.w3.org/2004/02/skos/core#hasTopConcept -->

    <owl:ObjectProperty rdf:about="http://www.w3.org/2004/02/skos/core#hasTopConcept">
        <owl:inverseOf rdf:resource="http://www.w3.org/2004/02/skos/core#topConceptOf"/>
        <rdfs:domain rdf:resource="http://www.w3.org/2004/02/skos/core#ConceptScheme"/>
        <rdfs:range rdf:resource="http://www.w3.org/2004/02/skos/core#Concept"/>
        <rdfs:isDefinedBy rdf:resource="http://www.w3.org/2004/02/skos/core"/>
        <rdfs:label xml:lang="en">has top concept</rdfs:label>
        <skos:definition xml:lang="en">Relates, by convention, a concept scheme to a concept which is topmost in the broader/narrower concept hierarchies for that scheme, providing an entry point to these hierarchies.</skos:definition>
    </owl:ObjectProperty>
    


    <!-- http://www.w3.org/2004/02/skos/core#inScheme -->

    <owl:ObjectProperty rdf:about="http://www.w3.org/2004/02/skos/core#inScheme">
        <rdfs:range rdf:resource="http://www.w3.org/2004/02/skos/core#ConceptScheme"/>
        <rdfs:isDefinedBy rdf:resource="http://www.w3.org/2004/02/skos/core"/>
        <rdfs:label xml:lang="en">is in scheme</rdfs:label>
        <skos:definition xml:lang="en">Relates a resource (for example a concept) to a concept scheme in which it is included.</skos:definition>
        <skos:scopeNote xml:lang="en">A concept may be a member of more than one concept scheme.</skos:scopeNote>
    </owl:ObjectProperty>
    


    <!-- http://www.w3.org/2004/02/skos/core#mappingRelation -->

    <owl:ObjectProperty rdf:about="http://www.w3.org/2004/02/skos/core#mappingRelation">
        <rdfs:subPropertyOf rdf:resource="http://www.w3.org/2004/02/skos/core#semanticRelation"/>
        <rdfs:comment xml:lang="en">These concept mapping relations mirror semantic relations, and the data model defined below is similar (with the exception of skos:exactMatch) to the data model defined for semantic relations. A distinct vocabulary is provided for concept mapping relations, to provide a convenient way to differentiate links within a concept scheme from links between concept schemes. However, this pattern of usage is not a formal requirement of the SKOS data model, and relies on informal definitions of best practice.</rdfs:comment>
        <rdfs:isDefinedBy rdf:resource="http://www.w3.org/2004/02/skos/core"/>
        <rdfs:label xml:lang="en">is in mapping relation with</rdfs:label>
        <skos:definition xml:lang="en">Relates two concepts coming, by convention, from different schemes, and that have comparable meanings</skos:definition>
    </owl:ObjectProperty>
    


    <!-- http://www.w3.org/2004/02/skos/core#member -->

    <owl:ObjectProperty rdf:about="http://www.w3.org/2004/02/skos/core#member">
        <rdfs:domain rdf:resource="http://www.w3.org/2004/02/skos/core#Collection"/>
        <rdfs:range>
            <owl:Class>
                <owl:unionOf rdf:parseType="Collection">
                    <rdf:Description rdf:about="http://www.w3.org/2004/02/skos/core#Collection"/>
                    <rdf:Description rdf:about="http://www.w3.org/2004/02/skos/core#Concept"/>
                </owl:unionOf>
            </owl:Class>
        </rdfs:range>
        <rdfs:isDefinedBy rdf:resource="http://www.w3.org/2004/02/skos/core"/>
        <rdfs:label xml:lang="en">has member</rdfs:label>
        <skos:definition xml:lang="en">Relates a collection to one of its members.</skos:definition>
    </owl:ObjectProperty>
    


    <!-- http://www.w3.org/2004/02/skos/core#memberList -->

    <owl:ObjectProperty rdf:about="http://www.w3.org/2004/02/skos/core#memberList">
        <rdf:type rdf:resource="http://www.w3.org/2002/07/owl#FunctionalProperty"/>
        <rdfs:domain rdf:resource="http://www.w3.org/2004/02/skos/core#OrderedCollection"/>
        <rdfs:range rdf:resource="http://www.w3.org/1999/02/22-rdf-syntax-ns#List"/>
        <rdfs:comment xml:lang="en">For any resource, every item in the list given as the value of the
      skos:memberList property is also a value of the skos:member property.</rdfs:comment>
        <rdfs:isDefinedBy rdf:resource="http://www.w3.org/2004/02/skos/core"/>
        <rdfs:label xml:lang="en">has member list</rdfs:label>
        <skos:definition xml:lang="en">Relates an ordered collection to the RDF list containing its members.</skos:definition>
    </owl:ObjectProperty>
    


    <!-- http://www.w3.org/2004/02/skos/core#narrowMatch -->

    <owl:ObjectProperty rdf:about="http://www.w3.org/2004/02/skos/core#narrowMatch">
        <rdfs:subPropertyOf rdf:resource="http://www.w3.org/2004/02/skos/core#mappingRelation"/>
        <rdfs:subPropertyOf rdf:resource="http://www.w3.org/2004/02/skos/core#narrower"/>
        <rdfs:isDefinedBy rdf:resource="http://www.w3.org/2004/02/skos/core"/>
        <rdfs:label xml:lang="en">has narrower match</rdfs:label>
        <skos:definition xml:lang="en">skos:narrowMatch is used to state a hierarchical mapping link between two conceptual resources in different concept schemes.</skos:definition>
    </owl:ObjectProperty>
    


    <!-- http://www.w3.org/2004/02/skos/core#narrower -->

    <owl:ObjectProperty rdf:about="http://www.w3.org/2004/02/skos/core#narrower">
        <rdfs:subPropertyOf rdf:resource="http://www.w3.org/2004/02/skos/core#narrowerTransitive"/>
        <rdfs:comment xml:lang="en">Narrower concepts are typically rendered as children in a concept hierarchy (tree).</rdfs:comment>
        <rdfs:isDefinedBy rdf:resource="http://www.w3.org/2004/02/skos/core"/>
        <rdfs:label xml:lang="en">has narrower</rdfs:label>
        <skos:definition xml:lang="en">Relates a concept to a concept that is more specific in meaning.</skos:definition>
        <skos:scopeNote xml:lang="en">By convention, skos:broader is only used to assert an immediate (i.e. direct) hierarchical link between two conceptual resources.</skos:scopeNote>
    </owl:ObjectProperty>
    


    <!-- http://www.w3.org/2004/02/skos/core#narrowerTransitive -->

    <owl:ObjectProperty rdf:about="http://www.w3.org/2004/02/skos/core#narrowerTransitive">
        <rdfs:subPropertyOf rdf:resource="http://www.w3.org/2004/02/skos/core#semanticRelation"/>
        <rdf:type rdf:resource="http://www.w3.org/2002/07/owl#TransitiveProperty"/>
        <rdfs:isDefinedBy rdf:resource="http://www.w3.org/2004/02/skos/core"/>
        <rdfs:label xml:lang="en">has narrower transitive</rdfs:label>
        <skos:definition>skos:narrowerTransitive is a transitive superproperty of skos:narrower.</skos:definition>
        <skos:scopeNote xml:lang="en">By convention, skos:narrowerTransitive is not used to make assertions. Rather, the properties can be used to draw inferences about the transitive closure of the hierarchical relation, which is useful e.g. when implementing a simple query expansion algorithm in a search application.</skos:scopeNote>
    </owl:ObjectProperty>
    


    <!-- http://www.w3.org/2004/02/skos/core#related -->

    <owl:ObjectProperty rdf:about="http://www.w3.org/2004/02/skos/core#related">
        <rdfs:subPropertyOf rdf:resource="http://www.w3.org/2004/02/skos/core#semanticRelation"/>
        <rdf:type rdf:resource="http://www.w3.org/2002/07/owl#SymmetricProperty"/>
        <rdfs:comment xml:lang="en">skos:related is disjoint with skos:broaderTransitive</rdfs:comment>
        <rdfs:isDefinedBy rdf:resource="http://www.w3.org/2004/02/skos/core"/>
        <rdfs:label xml:lang="en">has related</rdfs:label>
        <skos:definition xml:lang="en">Relates a concept to a concept with which there is an associative semantic relationship.</skos:definition>
    </owl:ObjectProperty>
    


    <!-- http://www.w3.org/2004/02/skos/core#relatedMatch -->

    <owl:ObjectProperty rdf:about="http://www.w3.org/2004/02/skos/core#relatedMatch">
        <rdfs:subPropertyOf rdf:resource="http://www.w3.org/2004/02/skos/core#mappingRelation"/>
        <rdfs:subPropertyOf rdf:resource="http://www.w3.org/2004/02/skos/core#related"/>
        <rdf:type rdf:resource="http://www.w3.org/2002/07/owl#SymmetricProperty"/>
        <rdfs:isDefinedBy rdf:resource="http://www.w3.org/2004/02/skos/core"/>
        <rdfs:label xml:lang="en">has related match</rdfs:label>
        <skos:definition xml:lang="en">skos:relatedMatch is used to state an associative mapping link between two conceptual resources in different concept schemes.</skos:definition>
    </owl:ObjectProperty>
    


    <!-- http://www.w3.org/2004/02/skos/core#semanticRelation -->

    <owl:ObjectProperty rdf:about="http://www.w3.org/2004/02/skos/core#semanticRelation">
        <rdfs:domain rdf:resource="http://www.w3.org/2004/02/skos/core#Concept"/>
        <rdfs:range rdf:resource="http://www.w3.org/2004/02/skos/core#Concept"/>
        <rdfs:isDefinedBy rdf:resource="http://www.w3.org/2004/02/skos/core"/>
        <rdfs:label xml:lang="en">is in semantic relation with</rdfs:label>
        <skos:definition xml:lang="en">Links a concept to a concept related by meaning.</skos:definition>
        <skos:scopeNote xml:lang="en">This property should not be used directly, but as a super-property for all properties denoting a relationship of meaning between concepts.</skos:scopeNote>
    </owl:ObjectProperty>
    


    <!-- http://www.w3.org/2004/02/skos/core#topConceptOf -->

    <owl:ObjectProperty rdf:about="http://www.w3.org/2004/02/skos/core#topConceptOf">
        <rdfs:subPropertyOf rdf:resource="http://www.w3.org/2004/02/skos/core#inScheme"/>
        <rdfs:domain rdf:resource="http://www.w3.org/2004/02/skos/core#Concept"/>
        <rdfs:range rdf:resource="http://www.w3.org/2004/02/skos/core#ConceptScheme"/>
        <rdfs:isDefinedBy rdf:resource="http://www.w3.org/2004/02/skos/core"/>
        <rdfs:label xml:lang="en">is top concept in scheme</rdfs:label>
        <skos:definition xml:lang="en">Relates a concept to the concept scheme that it is a top level concept of.</skos:definition>
    </owl:ObjectProperty>
    


    <!-- http://www.w3.org/2006/time#after -->

    <owl:ObjectProperty rdf:about="http://www.w3.org/2006/time#after">
        <owl:inverseOf rdf:resource="http://www.w3.org/2006/time#before"/>
        <rdfs:domain rdf:resource="http://www.w3.org/2006/time#TemporalEntity"/>
        <rdfs:range rdf:resource="http://www.w3.org/2006/time#TemporalEntity"/>
        <rdfs:comment xml:lang="es">Asume una dirección en el tiempo. Si una entidad temporal T1 está después de otra entidad temporal T2, entonces el principio de T1 está después del final de T2.</rdfs:comment>
        <rdfs:comment xml:lang="en">The subject is a temporal entity that occurs after the object. If a temporal entity T1 is after another temporal entity T2, then the beginning of T1 is after the end of T2.</rdfs:comment>
        <rdfs:label xml:lang="es">después</rdfs:label>
        <rdfs:label xml:lang="en">is after</rdfs:label>
        <skos:definition xml:lang="es">Asume una dirección en el tiempo. Si una entidad temporal T1 está después de otra entidad temporal T2, entonces el principio de T1 está después del final de T2.</skos:definition>
        <skos:definition xml:lang="en">Gives directionality to time. If a temporal entity T1 is after another temporal entity T2, then the beginning of T1 is after the end of T2.</skos:definition>
    </owl:ObjectProperty>
    


    <!-- http://www.w3.org/2006/time#before -->

    <owl:ObjectProperty rdf:about="http://www.w3.org/2006/time#before">
        <rdf:type rdf:resource="http://www.w3.org/2002/07/owl#TransitiveProperty"/>
        <rdfs:domain rdf:resource="http://www.w3.org/2006/time#TemporalEntity"/>
        <rdfs:range rdf:resource="http://www.w3.org/2006/time#TemporalEntity"/>
        <rdfs:comment xml:lang="es">Asume una dirección en el tiempo. Si una entidad temporal T1 está antes que otra entidad temporal T2, entonces el final de T1 está antes que el principio de T2. Así, &quot;antes&quot; se puede considerar básica para instantes y derivada para intervalos.</rdfs:comment>
        <rdfs:comment xml:lang="en">The subject is a temporal entity that occurs before the object. If a temporal entity T1 is before another temporal entity T2, then the end of T1 is before the beginning of T2. Thus, &quot;before&quot; can be considered to be basic to instants and derived for intervals.</rdfs:comment>
        <rdfs:label xml:lang="es">antes</rdfs:label>
        <rdfs:label xml:lang="en">is before</rdfs:label>
        <skos:definition xml:lang="es">Asume una dirección en el tiempo. Si una entidad temporal T1 está antes que otra entidad temporal T2, entonces el final de T1 está antes que el principio de T2. Así, &quot;antes&quot; se puede considerar básica para instantes y derivada para intervalos.</skos:definition>
        <skos:definition xml:lang="en">Gives directionality to time. If a temporal entity T1 is before another temporal entity T2, then the end of T1 is before the beginning of T2. Thus, &quot;before&quot; can be considered to be basic to instants and derived for intervals.</skos:definition>
    </owl:ObjectProperty>
    


    <!-- http://www.w3.org/2006/time#dayOfWeek -->

    <owl:ObjectProperty rdf:about="http://www.w3.org/2006/time#dayOfWeek">
        <rdfs:domain rdf:resource="http://www.w3.org/2006/time#GeneralDateTimeDescription"/>
        <rdfs:range rdf:resource="http://www.w3.org/2006/time#DayOfWeek"/>
        <rdfs:comment>El día de la semana, cuyo valor es un miembro de la clase &apos;día de la semana&apos;.</rdfs:comment>
        <rdfs:comment xml:lang="en">The day of week, whose value is a member of the class time:DayOfWeek</rdfs:comment>
        <rdfs:label xml:lang="en">day of week</rdfs:label>
        <rdfs:label xml:lang="es">día de la semana</rdfs:label>
        <skos:definition xml:lang="es">El día de la semana, cuyo valor es un miembro de la clase &apos;día de la semana&apos;.</skos:definition>
        <skos:definition xml:lang="en">The day of week, whose value is a member of the class time:DayOfWeek</skos:definition>
    </owl:ObjectProperty>
    


    <!-- http://www.w3.org/2006/time#hasBeginning -->

    <owl:ObjectProperty rdf:about="http://www.w3.org/2006/time#hasBeginning">
        <rdfs:subPropertyOf rdf:resource="http://www.w3.org/2006/time#hasTime"/>
        <rdfs:domain rdf:resource="http://www.w3.org/2006/time#TemporalEntity"/>
        <rdfs:range rdf:resource="http://www.w3.org/2006/time#Instant"/>
        <rdfs:comment xml:lang="en">Beginning of a temporal entity</rdfs:comment>
        <rdfs:comment xml:lang="es">Comienzo de una entidad temporal.</rdfs:comment>
        <rdfs:label xml:lang="en">has beginning</rdfs:label>
        <rdfs:label xml:lang="es">tiene principio</rdfs:label>
        <skos:definition xml:lang="en">Beginning of a temporal entity.</skos:definition>
        <skos:definition xml:lang="es">Comienzo de una entidad temporal.</skos:definition>
    </owl:ObjectProperty>
    


    <!-- http://www.w3.org/2006/time#hasDateTimeDescription -->

    <owl:ObjectProperty rdf:about="http://www.w3.org/2006/time#hasDateTimeDescription">
        <rdfs:domain rdf:resource="http://www.w3.org/2006/time#DateTimeInterval"/>
        <rdfs:range rdf:resource="http://www.w3.org/2006/time#GeneralDateTimeDescription"/>
        <rdfs:comment xml:lang="es">Valor de intervalo de fecha-hora expresado como un valor estructurado. El principio y el final del intervalo coincide con los límites del elemento más corto en la descripción.</rdfs:comment>
        <rdfs:comment xml:lang="en">Value of DateTimeInterval expressed as a structured value. The beginning and end of the interval coincide with the limits of the shortest element in the description.</rdfs:comment>
        <rdfs:label xml:lang="en">has Date-Time description</rdfs:label>
        <rdfs:label xml:lang="es">tiene descripción fecha-hora</rdfs:label>
        <skos:definition xml:lang="es">Valor de intervalo de fecha-hora expresado como un valor estructurado. El principio y el final del intervalo coincide con los límites del elemento más corto en la descripción.</skos:definition>
        <skos:definition xml:lang="en">Value of DateTimeInterval expressed as a structured value. The beginning and end of the interval coincide with the limits of the shortest element in the description.</skos:definition>
    </owl:ObjectProperty>
    


    <!-- http://www.w3.org/2006/time#hasDuration -->

    <owl:ObjectProperty rdf:about="http://www.w3.org/2006/time#hasDuration">
        <rdfs:subPropertyOf rdf:resource="http://www.w3.org/2006/time#hasTemporalDuration"/>
        <rdfs:range rdf:resource="http://www.w3.org/2006/time#Duration"/>
        <rdfs:comment xml:lang="es">Duración de una entidad temporal, expresada como un valor escalado o un valor nominal.</rdfs:comment>
        <rdfs:comment xml:lang="en">Duration of a temporal entity, expressed as a scaled value or nominal value</rdfs:comment>
        <rdfs:label xml:lang="en">has duration</rdfs:label>
        <rdfs:label xml:lang="es">tiene duración</rdfs:label>
        <skos:definition xml:lang="es">Duración de una entidad temporal, evento o actividad, o cosa, expresada como un valor escalado.</skos:definition>
        <skos:definition xml:lang="en">Duration of a temporal entity, event or activity, or thing, expressed as a scaled value</skos:definition>
    </owl:ObjectProperty>
    


    <!-- http://www.w3.org/2006/time#hasDurationDescription -->

    <owl:ObjectProperty rdf:about="http://www.w3.org/2006/time#hasDurationDescription">
        <rdfs:subPropertyOf rdf:resource="http://www.w3.org/2006/time#hasTemporalDuration"/>
        <rdfs:range rdf:resource="http://www.w3.org/2006/time#GeneralDurationDescription"/>
        <rdfs:comment xml:lang="es">Duración de una entidad temporal, expresada utilizando una descripción estructurada.</rdfs:comment>
        <rdfs:comment xml:lang="en">Duration of a temporal entity, expressed using a structured description</rdfs:comment>
        <rdfs:label xml:lang="en">has duration description</rdfs:label>
        <rdfs:label xml:lang="es">tiene descripción de duración</rdfs:label>
        <skos:definition xml:lang="es">Duración de una entidad temporal, expresada utilizando una descripción estructurada.</skos:definition>
        <skos:definition xml:lang="en">Duration of a temporal entity, expressed using a structured description</skos:definition>
    </owl:ObjectProperty>
    


    <!-- http://www.w3.org/2006/time#hasEnd -->

    <owl:ObjectProperty rdf:about="http://www.w3.org/2006/time#hasEnd">
        <rdfs:subPropertyOf rdf:resource="http://www.w3.org/2006/time#hasTime"/>
        <rdfs:domain rdf:resource="http://www.w3.org/2006/time#TemporalEntity"/>
        <rdfs:range rdf:resource="http://www.w3.org/2006/time#Instant"/>
        <rdfs:comment xml:lang="en">End of a temporal entity.</rdfs:comment>
        <rdfs:comment xml:lang="es">Final de una entidad temporal.</rdfs:comment>
        <rdfs:label xml:lang="en">has end</rdfs:label>
        <rdfs:label xml:lang="es">tiene fin</rdfs:label>
        <skos:definition xml:lang="en">End of a temporal entity.</skos:definition>
        <skos:definition xml:lang="es">Final de una entidad temporal.</skos:definition>
    </owl:ObjectProperty>
    


    <!-- http://www.w3.org/2006/time#hasTRS -->

    <owl:ObjectProperty rdf:about="http://www.w3.org/2006/time#hasTRS">
        <rdf:type rdf:resource="http://www.w3.org/2002/07/owl#FunctionalProperty"/>
        <rdfs:domain>
            <owl:Class>
                <owl:unionOf rdf:parseType="Collection">
                    <rdf:Description rdf:about="http://www.w3.org/2006/time#GeneralDurationDescription"/>
                    <rdf:Description rdf:about="http://www.w3.org/2006/time#TemporalPosition"/>
                </owl:unionOf>
            </owl:Class>
        </rdfs:domain>
        <rdfs:range rdf:resource="http://www.w3.org/2006/time#TRS"/>
        <rdfs:comment xml:lang="es">El sistema de referencia temporal utilizado por una posición temporal o descripción de extensión.</rdfs:comment>
        <rdfs:comment xml:lang="en">The temporal reference system used by a temporal position or extent description. </rdfs:comment>
        <rdfs:label xml:lang="en">Temporal reference system used</rdfs:label>
        <rdfs:label xml:lang="es">sistema de referencia temporal utilizado</rdfs:label>
        <skos:definition xml:lang="es">El sistema de referencia temporal utilizado por una posición temporal o descripción de extensión.</skos:definition>
        <skos:definition xml:lang="en">The temporal reference system used by a temporal position or extent description. </skos:definition>
    </owl:ObjectProperty>
    


    <!-- http://www.w3.org/2006/time#hasTemporalDuration -->

    <owl:ObjectProperty rdf:about="http://www.w3.org/2006/time#hasTemporalDuration">
        <rdfs:domain rdf:resource="http://www.w3.org/2006/time#TemporalEntity"/>
        <rdfs:range rdf:resource="http://www.w3.org/2006/time#TemporalDuration"/>
        <rdfs:comment xml:lang="es">Duración de una entidad temporal.</rdfs:comment>
        <rdfs:comment xml:lang="en">Duration of a temporal entity.</rdfs:comment>
        <rdfs:label xml:lang="en">has temporal duration</rdfs:label>
        <rdfs:label xml:lang="es">tiene duración temporal</rdfs:label>
        <skos:definition xml:lang="es">Duración de una entidad temporal.</skos:definition>
        <skos:definition xml:lang="en">Duration of a temporal entity.</skos:definition>
    </owl:ObjectProperty>
    


    <!-- http://www.w3.org/2006/time#hasTime -->

    <owl:ObjectProperty rdf:about="http://www.w3.org/2006/time#hasTime">
        <rdfs:range rdf:resource="http://www.w3.org/2006/time#TemporalEntity"/>
        <rdfs:comment xml:lang="es">Proporciona soporte a la asociación de una entidad temporal (instante o intervalo) a cualquier cosa.</rdfs:comment>
        <rdfs:comment xml:lang="en">Supports the association of a temporal entity (instant or interval) to any thing</rdfs:comment>
        <rdfs:label xml:lang="en">has time</rdfs:label>
        <rdfs:label xml:lang="es">tiene tiempo</rdfs:label>
        <skos:definition xml:lang="es">Proporciona soporte a la asociación de una entidad temporal (instante o intervalo) a cualquier cosa.</skos:definition>
        <skos:definition xml:lang="en">Supports the association of a temporal entity (instant or interval) to any thing</skos:definition>
        <skos:editorialNote xml:lang="es">Característica arriesgada -añadida en la revisión del 2017 que no ha sido todavía utilizada de forma amplia.</skos:editorialNote>
        <skos:editorialNote xml:lang="en">Feature at risk - added in 2017 revision, and not yet widely used. </skos:editorialNote>
    </owl:ObjectProperty>
    


    <!-- http://www.w3.org/2006/time#inDateTime -->

    <owl:ObjectProperty rdf:about="http://www.w3.org/2006/time#inDateTime">
        <rdfs:subPropertyOf rdf:resource="http://www.w3.org/2006/time#inTemporalPosition"/>
        <rdfs:domain rdf:resource="http://www.w3.org/2006/time#Instant"/>
        <rdfs:range rdf:resource="http://www.w3.org/2006/time#GeneralDateTimeDescription"/>
        <rdfs:comment xml:lang="es">Posición de un instante, expresada utilizando una descripción estructurada.</rdfs:comment>
        <rdfs:comment xml:lang="en">Position of an instant, expressed using a structured description</rdfs:comment>
        <rdfs:label xml:lang="es">en descripción de fecha-hora</rdfs:label>
        <rdfs:label xml:lang="en">in date-time description</rdfs:label>
        <skos:definition xml:lang="es">Posición de un instante, expresada utilizando una descripción estructurada.</skos:definition>
        <skos:definition xml:lang="en">Position of an instant, expressed using a structured description</skos:definition>
    </owl:ObjectProperty>
    


    <!-- http://www.w3.org/2006/time#inTemporalPosition -->

    <owl:ObjectProperty rdf:about="http://www.w3.org/2006/time#inTemporalPosition">
        <rdfs:domain rdf:resource="http://www.w3.org/2006/time#Instant"/>
        <rdfs:range rdf:resource="http://www.w3.org/2006/time#TemporalPosition"/>
        <rdfs:comment xml:lang="es">Posición de un instante de tiempo.</rdfs:comment>
        <rdfs:comment xml:lang="en">Position of a time instant</rdfs:comment>
        <rdfs:label xml:lang="en">Temporal position</rdfs:label>
        <rdfs:label xml:lang="es">posición temporal</rdfs:label>
        <skos:definition xml:lang="es">Posición de un instante de tiempo.</skos:definition>
        <skos:definition xml:lang="en">Position of a time instant</skos:definition>
    </owl:ObjectProperty>
    


    <!-- http://www.w3.org/2006/time#inTimePosition -->

    <owl:ObjectProperty rdf:about="http://www.w3.org/2006/time#inTimePosition">
        <rdfs:subPropertyOf rdf:resource="http://www.w3.org/2006/time#inTemporalPosition"/>
        <rdfs:domain rdf:resource="http://www.w3.org/2006/time#Instant"/>
        <rdfs:range rdf:resource="http://www.w3.org/2006/time#TimePosition"/>
        <rdfs:comment xml:lang="es">Posición de un instante, expresada como una coordenada temporal o un valor nominal.</rdfs:comment>
        <rdfs:comment xml:lang="en">Position of an instant, expressed as a temporal coordinate or nominal value</rdfs:comment>
        <rdfs:label xml:lang="en">Time position</rdfs:label>
        <rdfs:label xml:lang="es">posición de tiempo</rdfs:label>
        <skos:definition xml:lang="es">Posición de un instante, expresada como una coordenada temporal o un valor nominal.</skos:definition>
        <skos:definition xml:lang="en">Position of a time instant expressed as a TimePosition</skos:definition>
    </owl:ObjectProperty>
    


    <!-- http://www.w3.org/2006/time#inside -->

    <owl:ObjectProperty rdf:about="http://www.w3.org/2006/time#inside">
        <rdfs:domain rdf:resource="http://www.w3.org/2006/time#Interval"/>
        <rdfs:range rdf:resource="http://www.w3.org/2006/time#Instant"/>
        <rdfs:comment xml:lang="en">An instant that falls inside the interval. It is not intended to include beginnings and ends of intervals.</rdfs:comment>
        <rdfs:comment xml:lang="es">Un instante que cae dentro del intervalo. Se asume que no es ni el principio ni el final de ningún intervalo.</rdfs:comment>
        <rdfs:label xml:lang="en">has time instant inside</rdfs:label>
        <rdfs:label xml:lang="es">tiene instante de tiempo dentro</rdfs:label>
        <skos:definition xml:lang="en">An instant that falls inside the interval. It is not intended to include beginnings and ends of intervals.</skos:definition>
        <skos:definition xml:lang="es">Un instante que cae dentro del intervalo. Se asume que no es ni el principio ni el final de ningún intervalo.</skos:definition>
    </owl:ObjectProperty>
    


    <!-- http://www.w3.org/2006/time#intervalAfter -->

    <owl:ObjectProperty rdf:about="http://www.w3.org/2006/time#intervalAfter">
        <rdfs:subPropertyOf rdf:resource="http://www.w3.org/2006/time#after"/>
        <rdfs:subPropertyOf rdf:resource="http://www.w3.org/2006/time#intervalDisjoint"/>
        <owl:inverseOf rdf:resource="http://www.w3.org/2006/time#intervalBefore"/>
        <rdfs:domain rdf:resource="http://www.w3.org/2006/time#ProperInterval"/>
        <rdfs:range rdf:resource="http://www.w3.org/2006/time#ProperInterval"/>
        <rdfs:comment xml:lang="en">If a proper interval T1 is intervalAfter another proper interval T2, then the beginning of T1 is after the end of T2.</rdfs:comment>
        <rdfs:comment>Si un intervalo propio T1 es posterior a otro intervalo propio T2, entonces el principio de T1 está después que el final de T2.</rdfs:comment>
        <rdfs:label xml:lang="en">interval after</rdfs:label>
        <rdfs:label xml:lang="es">intervalo posterior</rdfs:label>
        <skos:definition xml:lang="en">If a proper interval T1 is intervalAfter another proper interval T2, then the beginning of T1 is after the end of T2.</skos:definition>
        <skos:definition xml:lang="es">Si un intervalo propio T1 es posterior a otro intervalo propio T2, entonces el principio de T1 está después que el final de T2.</skos:definition>
    </owl:ObjectProperty>
    


    <!-- http://www.w3.org/2006/time#intervalBefore -->

    <owl:ObjectProperty rdf:about="http://www.w3.org/2006/time#intervalBefore">
        <rdfs:subPropertyOf rdf:resource="http://www.w3.org/2006/time#before"/>
        <rdfs:subPropertyOf rdf:resource="http://www.w3.org/2006/time#intervalDisjoint"/>
        <rdfs:domain rdf:resource="http://www.w3.org/2006/time#ProperInterval"/>
        <rdfs:range rdf:resource="http://www.w3.org/2006/time#ProperInterval"/>
        <rdfs:comment xml:lang="en">If a proper interval T1 is intervalBefore another proper interval T2, then the end of T1 is before the beginning of T2.</rdfs:comment>
        <rdfs:comment xml:lang="es">Si un intervalo propio T1 está antes que otro intervalo propio T2, entonces el final de T1 está antes que el principio de T2.</rdfs:comment>
        <rdfs:label xml:lang="en">interval before</rdfs:label>
        <rdfs:label xml:lang="es">intervalo anterior</rdfs:label>
        <skos:definition xml:lang="en">If a proper interval T1 is intervalBefore another proper interval T2, then the end of T1 is before the beginning of T2.</skos:definition>
        <skos:definition xml:lang="es">Si un intervalo propio T1 está antes que otro intervalo propio T2, entonces el final de T1 está antes que el principio de T2.</skos:definition>
    </owl:ObjectProperty>
    


    <!-- http://www.w3.org/2006/time#intervalContains -->

    <owl:ObjectProperty rdf:about="http://www.w3.org/2006/time#intervalContains">
        <owl:inverseOf rdf:resource="http://www.w3.org/2006/time#intervalDuring"/>
        <rdfs:domain rdf:resource="http://www.w3.org/2006/time#ProperInterval"/>
        <rdfs:range rdf:resource="http://www.w3.org/2006/time#ProperInterval"/>
        <rdfs:comment xml:lang="en">If a proper interval T1 is intervalContains another proper interval T2, then the beginning of T1 is before the beginning of T2, and the end of T1 is after the end of T2.</rdfs:comment>
        <rdfs:comment xml:lang="es">Si un intervalo propio T1 contiene otro intervalo propio T2, entonces el principio de T1 está antes que el principio de T2, y el final de T1 está después del final de T2.</rdfs:comment>
        <rdfs:label xml:lang="en">interval contains</rdfs:label>
        <rdfs:label xml:lang="es">intervalo contiene</rdfs:label>
        <skos:definition xml:lang="en">If a proper interval T1 is intervalContains another proper interval T2, then the beginning of T1 is before the beginning of T2, and the end of T1 is after the end of T2.</skos:definition>
        <skos:definition xml:lang="es">Si un intervalo propio T1 contiene otro intervalo propio T2, entonces el principio de T1 está antes que el principio de T2, y el final de T1 está después del final de T2.</skos:definition>
    </owl:ObjectProperty>
    


    <!-- http://www.w3.org/2006/time#intervalDisjoint -->

    <owl:ObjectProperty rdf:about="http://www.w3.org/2006/time#intervalDisjoint">
        <rdfs:domain rdf:resource="http://www.w3.org/2006/time#ProperInterval"/>
        <rdfs:range rdf:resource="http://www.w3.org/2006/time#ProperInterval"/>
        <rdfs:comment xml:lang="en">If a proper interval T1 is intervalDisjoint another proper interval T2, then the beginning of T1 is after the end of T2, or the end of T1 is before the beginning of T2, i.e. the intervals do not overlap in any way, but their ordering relationship is not known.</rdfs:comment>
        <rdfs:comment xml:lang="es">Si un intervalo propio T1 es disjunto con otro intervalo propio T2, entonces el principio de T1 está después del final de T2, o el final de T1 está antes que el principio de T2, es decir, los intervalos no se solapan de ninguna forma, aunque su relación de orden no se conozca.</rdfs:comment>
        <rdfs:label xml:lang="en">interval disjoint</rdfs:label>
        <rdfs:label xml:lang="es">intervalo disjunto</rdfs:label>
        <skos:definition xml:lang="en">If a proper interval T1 is intervalDisjoint another proper interval T2, then the beginning of T1 is after the end of T2, or the end of T1 is before the beginning of T2, i.e. the intervals do not overlap in any way, but their ordering relationship is not known.</skos:definition>
        <skos:definition xml:lang="es">Si un intervalo propio T1 es disjunto con otro intervalo propio T2, entonces el principio de T1 está después del final de T2, o el final de T1 está antes que el principio de T2, es decir, los intervalos no se solapan de ninguna forma, aunque su relación de orden no se conozca.</skos:definition>
        <skos:note xml:lang="es">Esta relación entre intervalos no estaba incluida en las 13 relaciones básicas definidas por Allen (1984), pero está definida en T.3 como la unión de &apos;intervalo anterior&apos; con &apos;intervalo posterior&apos;. Sin embargo, esto está fuera de la expresividad de OWL2, por tanto, está implementado como una propiedad explícita, con &apos;intervalo anterior&apos; e &apos;intervalo posterior&apos; como sub-propiedades.</skos:note>
        <skos:note xml:lang="en">This interval relation is not included in the 13 basic relationships defined in Allen (1984), but is defined in (T.3) as the union of :intervalBefore v :intervalAfter . However, that is outside OWL2 expressivity, so is implemented as an explicit property, with :intervalBefore , :intervalAfter as sub-properties</skos:note>
    </owl:ObjectProperty>
    


    <!-- http://www.w3.org/2006/time#intervalDuring -->

    <owl:ObjectProperty rdf:about="http://www.w3.org/2006/time#intervalDuring">
        <rdfs:subPropertyOf rdf:resource="http://www.w3.org/2006/time#intervalIn"/>
        <rdfs:domain rdf:resource="http://www.w3.org/2006/time#ProperInterval"/>
        <rdfs:range rdf:resource="http://www.w3.org/2006/time#ProperInterval"/>
        <rdfs:comment xml:lang="en">If a proper interval T1 is intervalDuring another proper interval T2, then the beginning of T1 is after the beginning of T2, and the end of T1 is before the end of T2.</rdfs:comment>
        <rdfs:comment xml:lang="es">Si un intervalo propio T1 está durante otro intervalo propio T2, entonces del principio de T1 está después del principio de T2, y el final de T1 está antes que el final de T2.</rdfs:comment>
        <rdfs:label xml:lang="en">interval during</rdfs:label>
        <rdfs:label xml:lang="es">intervalo durante</rdfs:label>
        <skos:definition xml:lang="en">If a proper interval T1 is intervalDuring another proper interval T2, then the beginning of T1 is after the beginning of T2, and the end of T1 is before the end of T2.</skos:definition>
        <skos:definition xml:lang="es">Si un intervalo propio T1 está durante otro intervalo propio T2, entonces del principio de T1 está después del principio de T2, y el final de T1 está antes que el final de T2.</skos:definition>
    </owl:ObjectProperty>
    


    <!-- http://www.w3.org/2006/time#intervalEquals -->

    <owl:ObjectProperty rdf:about="http://www.w3.org/2006/time#intervalEquals">
        <rdf:type rdf:resource="http://www.w3.org/2002/07/owl#SymmetricProperty"/>
        <rdfs:domain rdf:resource="http://www.w3.org/2006/time#ProperInterval"/>
        <rdfs:range rdf:resource="http://www.w3.org/2006/time#ProperInterval"/>
        <owl:propertyDisjointWith rdf:resource="http://www.w3.org/2006/time#intervalIn"/>
        <rdfs:comment xml:lang="en">If a proper interval T1 is intervalEquals another proper interval T2, then the beginning of T1 is coincident with the beginning of T2, and the end of T1 is coincident with the end of T2.</rdfs:comment>
        <rdfs:comment xml:lang="es">Si un intervalo propio T1 es igual a otro intervalo propio T2, entonces el principio de T1 coincide con el principio de T2, y el final de T1 coincide con el final de T2.</rdfs:comment>
        <rdfs:label xml:lang="en">interval equals</rdfs:label>
        <rdfs:label xml:lang="es">intervalo igual</rdfs:label>
        <skos:definition xml:lang="en">If a proper interval T1 is intervalEquals another proper interval T2, then the beginning of T1 is coincident with the beginning of T2, and the end of T1 is coincident with the end of T2.</skos:definition>
        <skos:definition xml:lang="es">Si un intervalo propio T1 es igual a otro intervalo propio T2, entonces el principio de T1 coincide con el principio de T2, y el final de T1 coincide con el final de T2.</skos:definition>
    </owl:ObjectProperty>
    


    <!-- http://www.w3.org/2006/time#intervalFinishedBy -->

    <owl:ObjectProperty rdf:about="http://www.w3.org/2006/time#intervalFinishedBy">
        <owl:inverseOf rdf:resource="http://www.w3.org/2006/time#intervalFinishes"/>
        <rdfs:domain rdf:resource="http://www.w3.org/2006/time#ProperInterval"/>
        <rdfs:range rdf:resource="http://www.w3.org/2006/time#ProperInterval"/>
        <rdfs:comment xml:lang="en">If a proper interval T1 is intervalFinishedBy another proper interval T2, then the beginning of T1 is before the beginning of T2, and the end of T1 is coincident with the end of T2.</rdfs:comment>
        <rdfs:comment xml:lang="es">Si un intervalo propio T1 está terminado por otro intervalo propio T2, entonces el principio de T1 está antes que el principio de T2, y el final de T1 coincide con el final de T2.</rdfs:comment>
        <rdfs:label xml:lang="en">interval finished by</rdfs:label>
        <rdfs:label xml:lang="es">intervalo terminado por</rdfs:label>
        <skos:definition xml:lang="en">If a proper interval T1 is intervalFinishedBy another proper interval T2, then the beginning of T1 is before the beginning of T2, and the end of T1 is coincident with the end of T2.</skos:definition>
        <skos:definition xml:lang="es">Si un intervalo propio T1 está terminado por otro intervalo propio T2, entonces el principio de T1 está antes que el principio de T2, y el final de T1 coincide con el final de T2.</skos:definition>
    </owl:ObjectProperty>
    


    <!-- http://www.w3.org/2006/time#intervalFinishes -->

    <owl:ObjectProperty rdf:about="http://www.w3.org/2006/time#intervalFinishes">
        <rdfs:subPropertyOf rdf:resource="http://www.w3.org/2006/time#intervalIn"/>
        <rdfs:domain rdf:resource="http://www.w3.org/2006/time#ProperInterval"/>
        <rdfs:range rdf:resource="http://www.w3.org/2006/time#ProperInterval"/>
        <rdfs:comment xml:lang="en">If a proper interval T1 is intervalFinishes another proper interval T2, then the beginning of T1 is after the beginning of T2, and the end of T1 is coincident with the end of T2.</rdfs:comment>
        <rdfs:comment xml:lang="es">Si un intervalo propio T1 termina otro intervalo propio T2, entonces del principio de T1 está después del principio de T2, y el final de T1 coincide con el final de T2.</rdfs:comment>
        <rdfs:label xml:lang="en">interval finishes</rdfs:label>
        <rdfs:label xml:lang="es">intervalo termina</rdfs:label>
        <skos:definition xml:lang="en">If a proper interval T1 is intervalFinishes another proper interval T2, then the beginning of T1 is after the beginning of T2, and the end of T1 is coincident with the end of T2.</skos:definition>
        <skos:definition xml:lang="es">Si un intervalo propio T1 termina otro intervalo propio T2, entonces del principio de T1 está después del principio de T2, y el final de T1 coincide con el final de T2.</skos:definition>
    </owl:ObjectProperty>
    


    <!-- http://www.w3.org/2006/time#intervalIn -->

    <owl:ObjectProperty rdf:about="http://www.w3.org/2006/time#intervalIn">
        <rdfs:domain rdf:resource="http://www.w3.org/2006/time#ProperInterval"/>
        <rdfs:range rdf:resource="http://www.w3.org/2006/time#ProperInterval"/>
        <rdfs:comment xml:lang="en">If a proper interval T1 is intervalIn another proper interval T2, then the beginning of T1 is after the beginning of T2 or is coincident with the beginning of T2, and the end of T1 is before the end of T2, or is coincident with the end of T2, except that end of T1 may not be coincident with the end of T2 if the beginning of T1 is coincident with the beginning of T2.</rdfs:comment>
        <rdfs:comment xml:lang="es">Si un intervalo propio T1 es un intervalo interior a otro intervalo propio T2, entonces el principio de T1 está después del principio de T2 o coincide con el principio de T2, y el final de T1 está antes que el final de T2, o coincide con el final de T2, excepto que el final de T1 puede no coincidir con el final de T2 si el principio de T1 coincide con el principio de T2.</rdfs:comment>
        <rdfs:label xml:lang="en">interval in</rdfs:label>
        <rdfs:label xml:lang="es">intervalo interior</rdfs:label>
        <skos:definition xml:lang="en">If a proper interval T1 is intervalIn another proper interval T2, then the beginning of T1 is after the beginning of T2 or is coincident with the beginning of T2, and the end of T1 is before the end of T2, or is coincident with the end of T2, except that end of T1 may not be coincident with the end of T2 if the beginning of T1 is coincident with the beginning of T2.</skos:definition>
        <skos:definition xml:lang="es">Si un intervalo propio T1 es un intervalo interior a otro intervalo propio T2, entonces el principio de T1 está después del principio de T2 o coincide con el principio de T2, y el final de T1 está antes que el final de T2, o coincide con el final de T2, excepto que el final de T1 puede no coincidir con el final de T2 si el principio de T1 coincide con el principio de T2.</skos:definition>
        <skos:note xml:lang="es">Esta relación entre intervalos no estaba incluida en las 13 relaciones básicas definidas por Allen (1984), pero se hace referencia a ella como &quot;una relación importante&quot; en Allen y Ferguson (1997). Es la unión disjunta de &apos;intervalo empieza&apos;, &apos;intervalo durante&apos; y con &apos;intervalo termina&apos;. Sin embargo, esto está fuera de la expresividad de OWL2, por tanto, se implementa como una propiedad explícita, con &apos;intervalo empieza&apos;, &apos;intervalo durante&apos; e &apos;intervalo termina&apos; como sub-propiedades.</skos:note>
        <skos:note xml:lang="en">This interval relation is not included in the 13 basic relationships defined in Allen (1984), but is referred to as &apos;an important relationship&apos; in Allen and Ferguson (1997). It is the disjoint union of :intervalStarts v :intervalDuring v :intervalFinishes . However, that is outside OWL2 expressivity, so is implemented as an explicit property, with :intervalStarts , :intervalDuring , :intervalFinishes as sub-properties</skos:note>
    </owl:ObjectProperty>
    


    <!-- http://www.w3.org/2006/time#intervalMeets -->

    <owl:ObjectProperty rdf:about="http://www.w3.org/2006/time#intervalMeets">
        <owl:inverseOf rdf:resource="http://www.w3.org/2006/time#intervalMetBy"/>
        <rdfs:domain rdf:resource="http://www.w3.org/2006/time#ProperInterval"/>
        <rdfs:range rdf:resource="http://www.w3.org/2006/time#ProperInterval"/>
        <rdfs:comment xml:lang="en">If a proper interval T1 is intervalMeets another proper interval T2, then the end of T1 is coincident with the beginning of T2.</rdfs:comment>
        <rdfs:comment xml:lang="es">Si un intervalo propio T1 se encuentra con otro intervalo propio T2, entonces el final de T1 coincide con el principio de T2.</rdfs:comment>
        <rdfs:label xml:lang="en">interval meets</rdfs:label>
        <rdfs:label xml:lang="es">intervalo se encuentra</rdfs:label>
        <skos:definition xml:lang="en">If a proper interval T1 is intervalMeets another proper interval T2, then the end of T1 is coincident with the beginning of T2.</skos:definition>
        <skos:definition xml:lang="es">Si un intervalo propio T1 se encuentra con otro intervalo propio T2, entonces el final de T1 coincide con el principio de T2.</skos:definition>
    </owl:ObjectProperty>
    


    <!-- http://www.w3.org/2006/time#intervalMetBy -->

    <owl:ObjectProperty rdf:about="http://www.w3.org/2006/time#intervalMetBy">
        <rdfs:domain rdf:resource="http://www.w3.org/2006/time#ProperInterval"/>
        <rdfs:range rdf:resource="http://www.w3.org/2006/time#ProperInterval"/>
        <rdfs:comment xml:lang="en">If a proper interval T1 is intervalMetBy another proper interval T2, then the beginning of T1 is coincident with the end of T2.</rdfs:comment>
        <rdfs:comment xml:lang="es">Si un intervalo propio T1 es &apos;intervalo encontrado por&apos; otro intervalo propio T2, entonces el principio de T1 coincide con el final de T2.</rdfs:comment>
        <rdfs:label xml:lang="en">interval met by</rdfs:label>
        <rdfs:label xml:lang="es">intervalo encontrado por</rdfs:label>
        <skos:definition xml:lang="en">If a proper interval T1 is intervalMetBy another proper interval T2, then the beginning of T1 is coincident with the end of T2.</skos:definition>
        <skos:definition xml:lang="es">Si un intervalo propio T1 es &apos;intervalo encontrado por&apos; otro intervalo propio T2, entonces el principio de T1 coincide con el final de T2.</skos:definition>
    </owl:ObjectProperty>
    


    <!-- http://www.w3.org/2006/time#intervalOverlappedBy -->

    <owl:ObjectProperty rdf:about="http://www.w3.org/2006/time#intervalOverlappedBy">
        <owl:inverseOf rdf:resource="http://www.w3.org/2006/time#intervalOverlaps"/>
        <rdfs:domain rdf:resource="http://www.w3.org/2006/time#ProperInterval"/>
        <rdfs:range rdf:resource="http://www.w3.org/2006/time#ProperInterval"/>
        <rdfs:comment xml:lang="en">If a proper interval T1 is intervalOverlappedBy another proper interval T2, then the beginning of T1 is after the beginning of T2, the beginning of T1 is before the end of T2, and the end of T1 is after the end of T2.</rdfs:comment>
        <rdfs:comment xml:lang="es">Si un intervalo propio T1 es &apos;intervalo solapado por&apos; otro intervalo propio T2, entonces el principio de T1 es posterior al principio de T2, y el principio de T1 es anterior al final de T2, y el final de T1 es posterior al final de T2.</rdfs:comment>
        <rdfs:label xml:lang="en">interval overlapped by</rdfs:label>
        <rdfs:label xml:lang="es">intervalo solapado por</rdfs:label>
        <skos:definition xml:lang="en">If a proper interval T1 is intervalOverlappedBy another proper interval T2, then the beginning of T1 is after the beginning of T2, the beginning of T1 is before the end of T2, and the end of T1 is after the end of T2.</skos:definition>
        <skos:definition xml:lang="es">Si un intervalo propio T1 es &apos;intervalo solapado por&apos; otro intervalo propio T2, entonces el principio de T1 es posterior al principio de T2, y el principio de T1 es anterior al final de T2, y el final de T1 es posterior al final de T2.</skos:definition>
    </owl:ObjectProperty>
    


    <!-- http://www.w3.org/2006/time#intervalOverlaps -->

    <owl:ObjectProperty rdf:about="http://www.w3.org/2006/time#intervalOverlaps">
        <rdfs:domain rdf:resource="http://www.w3.org/2006/time#ProperInterval"/>
        <rdfs:range rdf:resource="http://www.w3.org/2006/time#ProperInterval"/>
        <rdfs:comment xml:lang="es">Asume una dirección en el tiempo. Si una entidad temporal T1 está después de otra entidad temporal T2, entonces el principio de T1 está después del final de T2.</rdfs:comment>
        <rdfs:comment xml:lang="en">If a proper interval T1 is intervalOverlaps another proper interval T2, then the beginning of T1 is before the beginning of T2, the end of T1 is after the beginning of T2, and the end of T1 is before the end of T2.</rdfs:comment>
        <rdfs:comment xml:lang="es">Si un intervalo propio T1 se solapa con otro intervalo propio T2, entonces el principio de T1 es anterior al principio de T2, el final de T1 es posterior al principio de T2, y el final de T1 es anterior al final de T2.</rdfs:comment>
        <rdfs:label xml:lang="en">interval overlaps</rdfs:label>
        <rdfs:label xml:lang="es">intervalo se solapa</rdfs:label>
        <skos:definition xml:lang="en">If a proper interval T1 is intervalOverlaps another proper interval T2, then the beginning of T1 is before the beginning of T2, the end of T1 is after the beginning of T2, and the end of T1 is before the end of T2.</skos:definition>
        <skos:definition xml:lang="es">Si un intervalo propio T1 se solapa con otro intervalo propio T2, entonces el principio de T1 es anterior al principio de T2, el final de T1 es posterior al principio de T2, y el final de T1 es anterior al final de T2.</skos:definition>
    </owl:ObjectProperty>
    


    <!-- http://www.w3.org/2006/time#intervalStartedBy -->

    <owl:ObjectProperty rdf:about="http://www.w3.org/2006/time#intervalStartedBy">
        <owl:inverseOf rdf:resource="http://www.w3.org/2006/time#intervalStarts"/>
        <rdfs:domain rdf:resource="http://www.w3.org/2006/time#ProperInterval"/>
        <rdfs:range rdf:resource="http://www.w3.org/2006/time#ProperInterval"/>
        <rdfs:comment xml:lang="en">If a proper interval T1 is intervalStarted another proper interval T2, then the beginning of T1 is coincident with the beginning of T2, and the end of T1 is after the end of T2.</rdfs:comment>
        <rdfs:comment xml:lang="es">Si un intervalo propio T1 es empezado por otro intervalo propio T2, entonces el principio de T1 coincide con el principio de T2, y el final de T1 es posterior al final de T2.</rdfs:comment>
        <rdfs:label xml:lang="en">interval started by</rdfs:label>
        <skos:definition xml:lang="en">If a proper interval T1 is intervalStarted another proper interval T2, then the beginning of T1 is coincident with the beginning of T2, and the end of T1 is after the end of T2.</skos:definition>
        <skos:definition xml:lang="es">Si un intervalo propio T1 es empezado por otro intervalo propio T2, entonces el principio de T1 coincide con el principio de T2, y el final de T1 es posterior al final de T2.</skos:definition>
    </owl:ObjectProperty>
    


    <!-- http://www.w3.org/2006/time#intervalStarts -->

    <owl:ObjectProperty rdf:about="http://www.w3.org/2006/time#intervalStarts">
        <rdfs:subPropertyOf rdf:resource="http://www.w3.org/2006/time#intervalIn"/>
        <rdfs:domain rdf:resource="http://www.w3.org/2006/time#ProperInterval"/>
        <rdfs:range rdf:resource="http://www.w3.org/2006/time#ProperInterval"/>
        <rdfs:comment xml:lang="en">If a proper interval T1 is intervalStarts another proper interval T2, then the beginning of T1 is coincident with the beginning of T2, and the end of T1 is before the end of T2.</rdfs:comment>
        <rdfs:comment xml:lang="es">Si un intervalo propio T1 empieza otro intervalo propio T2, entonces del principio de T1 con el principio de T2, y el final de T1 es anterior al final de T2.</rdfs:comment>
        <rdfs:label xml:lang="en">interval starts</rdfs:label>
        <rdfs:label xml:lang="es">intervalo empieza</rdfs:label>
        <skos:definition xml:lang="en">If a proper interval T1 is intervalStarts another proper interval T2, then the beginning of T1 is coincident with the beginning of T2, and the end of T1 is before the end of T2.</skos:definition>
        <skos:definition xml:lang="es">Si un intervalo propio T1 empieza otro intervalo propio T2, entonces del principio de T1 con el final de T2, y el final de T1 es anterior al final de T2.</skos:definition>
    </owl:ObjectProperty>
    


    <!-- http://www.w3.org/2006/time#monthOfYear -->

    <owl:ObjectProperty rdf:about="http://www.w3.org/2006/time#monthOfYear">
        <rdfs:domain rdf:resource="http://www.w3.org/2006/time#GeneralDateTimeDescription"/>
        <rdfs:range rdf:resource="http://www.w3.org/2006/time#MonthOfYear"/>
        <rdfs:comment xml:lang="es">El mes del año, cuyo valor es un miembro de la clase &apos;mes del año&apos;.</rdfs:comment>
        <rdfs:comment xml:lang="en">The month of the year, whose value is a member of the class time:MonthOfYear</rdfs:comment>
        <rdfs:label xml:lang="es">mes del año</rdfs:label>
        <rdfs:label xml:lang="en">month of year</rdfs:label>
        <skos:definition xml:lang="es">El mes del año, cuyo valor es un miembro de la clase &apos;mes del año&apos;.</skos:definition>
        <skos:definition xml:lang="en">The month of the year, whose value is a member of the class time:MonthOfYear</skos:definition>
        <skos:editorialNote xml:lang="es">Característica arriesgada - añadida en la revisión de 2017, y todavía no ampliamente utilizada.</skos:editorialNote>
        <skos:editorialNote xml:lang="en">Feature at risk - added in 2017 revision, and not yet widely used. </skos:editorialNote>
    </owl:ObjectProperty>
    


    <!-- http://www.w3.org/2006/time#timeZone -->

    <owl:ObjectProperty rdf:about="http://www.w3.org/2006/time#timeZone">
        <rdfs:domain rdf:resource="http://www.w3.org/2006/time#GeneralDateTimeDescription"/>
        <rdfs:range rdf:resource="http://www.w3.org/2006/time#TimeZone"/>
        <rdfs:comment xml:lang="en">The time zone for clock elements in the temporal position</rdfs:comment>
        <rdfs:label xml:lang="es">en huso horario</rdfs:label>
        <rdfs:label xml:lang="en">in time zone</rdfs:label>
        <skos:historyNote xml:lang="es">En la versión original de OWL-Time de 2006, el rango de &apos;en huso horario&apos; se definió en un espacio de nombres diferente &quot;http://www.w3.org/2006/timezone#&quot;.
            Un axioma de alineación permite que los datos codificados de acuerdo con la versión anterior sean consistentes con la ontología actualizada.</skos:historyNote>
        <skos:historyNote>In the original 2006 version of OWL-Time, the range of time:timeZone was a TimeZone class in a separate namespace &quot;http://www.w3.org/2006/timezone#&quot;. 
An alignment axiom 
	tzont:TimeZone rdfs:subClassOf time:TimeZone . 
allows data encoded according to the previous version to be consistent with the updated ontology. </skos:historyNote>
        <skos:note>IANA maintains a database of timezones. These are well maintained and generally considered authoritative, but individual items are not available at individual URIs, so cannot be used directly in data expressed using OWL-Time.

DBPedia provides a set of resources corresponding to the IANA timezones, with a URI for each (e.g. http://dbpedia.org/resource/Australia/Eucla). The World Clock service also provides a list of time zones with the description of each available as an individual webpage with a convenient individual URI (e.g. https://www.timeanddate.com/time/zones/acwst). These or other, similar, resources might be used as a value of the time:timeZone property.</skos:note>
        <skos:note xml:lang="es">IANA mantiene una base de datos de husos horarios. Éstas están bien mantenidas y generalmente se consideran autorizadas, pero los ítems individuales no están disponibles en URIs individuales, por tanto, no se pueden utilizar directamente en datos expresados utilizando OWL-Time.
            La BDPedia proporciona un conjunto de recursos correspondientes a los husos horarios de IANA, con una URI para cada uno (por ejemplo, http://dbpedia.org/resource/Australia/Eucla). El Servicio de Reloj Mundial también proporciona una lista de husos horarios con la descripción de cada uno de los disponibles como una página Web individual con una URI adecuada individual (por ejemplo, https://www.timeanddate.com/time/zones/acwst). Éstos, y otros recursos similares, se puden usar como un valor de la propiedad &apos;huso horario&apos;.</skos:note>
    </owl:ObjectProperty>
    


    <!-- http://www.w3.org/2006/time#unitType -->

    <owl:ObjectProperty rdf:about="http://www.w3.org/2006/time#unitType">
        <rdfs:domain>
            <owl:Class>
                <owl:unionOf rdf:parseType="Collection">
                    <rdf:Description rdf:about="http://www.w3.org/2006/time#Duration"/>
                    <rdf:Description rdf:about="http://www.w3.org/2006/time#GeneralDateTimeDescription"/>
                </owl:unionOf>
            </owl:Class>
        </rdfs:domain>
        <rdfs:range rdf:resource="http://www.w3.org/2006/time#TemporalUnit"/>
        <rdfs:comment xml:lang="es">La unidad de tiempo que proporciona la precisión de un valor fecha-hora o la escala de una extensión temporal.</rdfs:comment>
        <rdfs:comment xml:lang="en">The temporal unit which provides the precision of a date-time value or scale of a temporal extent</rdfs:comment>
        <rdfs:label xml:lang="en">temporal unit type</rdfs:label>
        <rdfs:label xml:lang="es">tipo de unidad temporal</rdfs:label>
    </owl:ObjectProperty>
    


    <!-- https://w3id.org/def/propaphen#characterizes -->

    <owl:ObjectProperty rdf:about="https://w3id.org/def/propaphen#characterizes">
        <rdfs:domain rdf:resource="http://purl.org/nemo/gufo#Entity"/>
        <rdfs:range rdf:resource="https://w3id.org/def/propaphen#Phenomenon"/>
        <rdfs:comment>&quot;Identify gufo:Individuals/entities that characterize (are crucial to the existence) of a given phen:Phenomenon.&quot;</rdfs:comment>
        <rdfs:label>Characterizes</rdfs:label>
    </owl:ObjectProperty>
    


    <!-- https://w3id.org/def/propaphen#fromPhenomenon -->

    <owl:ObjectProperty rdf:about="https://w3id.org/def/propaphen#fromPhenomenon">
        <rdf:type rdf:resource="http://www.w3.org/2002/07/owl#FunctionalProperty"/>
        <rdfs:domain rdf:resource="https://w3id.org/def/propaphen#PhenomenonOccurrence"/>
        <rdfs:range rdf:resource="https://w3id.org/def/propaphen#Phenomenon"/>
        <rdfs:comment>Identifies the phen:Phenomenon that gives the occurrence phen:PhenomenonOccurrence.


I.e. A phen:PhenomenonOccurence &quot;Occurence of a Hurricane in Paris&quot; is an occurrence of the phen:Phenomenon &quot;Hurricane&quot;.</rdfs:comment>
        <rdfs:label>fromPhenomenon</rdfs:label>
    </owl:ObjectProperty>
    


    <!-- https://w3id.org/def/propaphen#happensIn -->

    <owl:ObjectProperty rdf:about="https://w3id.org/def/propaphen#happensIn">
        <rdfs:domain rdf:resource="https://w3id.org/def/propaphen#Observation"/>
        <rdfs:range rdf:resource="https://w3id.org/seas/System"/>
        <rdfs:comment>Identifies the seas:System where the phen:Observation happens.</rdfs:comment>
        <rdfs:label>Happens In</rdfs:label>
    </owl:ObjectProperty>
    


    <!-- https://w3id.org/def/propaphen#hasPresence -->

    <owl:ObjectProperty rdf:about="https://w3id.org/def/propaphen#hasPresence">
        <owl:inverseOf rdf:resource="https://w3id.org/def/propaphen#presenceOf"/>
        <rdfs:domain rdf:resource="http://purl.org/nemo/gufo#Entity"/>
        <rdfs:range rdf:resource="https://w3id.org/def/propaphen#Presence"/>
        <rdfs:comment>Relates an instance of gufo:Individual/entity to its spatiotemporal presence.</rdfs:comment>
        <rdfs:label>Has Presence</rdfs:label>
    </owl:ObjectProperty>
    


    <!-- https://w3id.org/def/propaphen#hasSTValidPath -->

    <owl:ObjectProperty rdf:about="https://w3id.org/def/propaphen#hasSTValidPath">
        <rdf:type rdf:resource="http://www.w3.org/2002/07/owl#AsymmetricProperty"/>
        <rdfs:domain rdf:resource="https://w3id.org/def/propaphen#Observation"/>
        <rdfs:range rdf:resource="https://w3id.org/def/propaphen#Observation"/>
        <rdfs:comment>Represents a valid spatial-temporal path between two observations.


I.e. From the same phen:PhenomenonOccurrence &quot;Hurricane in France on 2019&quot;, we may have different phen:Observations like &quot;Hurricane observed in Rouen on November,2019&quot; and &quot;Hurricane observed in Paris on December,2019&quot;. We may say that there is a possibility that the Hurricane went from Rouen to Paris, so there is a valid spatial-temporal path between the first and the second observation.</rdfs:comment>
        <rdfs:label>Has Spatial-Temporal Valid Path</rdfs:label>
    </owl:ObjectProperty>
    


    <!-- https://w3id.org/def/propaphen#hasSpatialObject -->

    <owl:ObjectProperty rdf:about="https://w3id.org/def/propaphen#hasSpatialObject">
        <rdfs:domain rdf:resource="http://purl.org/nemo/gufo#Object"/>
        <rdfs:range rdf:resource="http://www.opengis.net/ont/geosparql#SpatialObject"/>
        <rdfs:comment>Relies a gufo:Object to parts of it&apos;s geo:SpatialObject.

I.e. A gufo:Object &quot;Country&quot; could be related to one geo:SpatialObject that delimits its entire zone, or it could be related to many geo:SpatialObjects for each gufo:Object &quot;City&quot; that forms the &quot;Country&quot;.</rdfs:comment>
        <rdfs:label>Has Spatial Object</rdfs:label>
    </owl:ObjectProperty>
    


    <!-- https://w3id.org/def/propaphen#hasTimeInterval -->

    <owl:ObjectProperty rdf:about="https://w3id.org/def/propaphen#hasTimeInterval">
        <rdfs:domain rdf:resource="http://purl.org/nemo/gufo#ConcreteEntity"/>
        <rdfs:range rdf:resource="http://www.w3.org/2006/time#ProperInterval"/>
        <rdfs:comment>is an additional property to facilitate the application of Allen&apos;s interval algebra of the proper time interval between the start and end point of the gufo:ConcreteEntity</rdfs:comment>
        <rdfs:label>Entity&apos;s Proper Time Interaval</rdfs:label>
    </owl:ObjectProperty>
    


    <!-- https://w3id.org/def/propaphen#observationOf -->

    <owl:ObjectProperty rdf:about="https://w3id.org/def/propaphen#observationOf">
        <rdf:type rdf:resource="http://www.w3.org/2002/07/owl#FunctionalProperty"/>
        <rdfs:domain rdf:resource="https://w3id.org/def/propaphen#Observation"/>
        <rdfs:range rdf:resource="https://w3id.org/def/propaphen#PhenomenonOccurrence"/>
        <rdfs:comment>Identifies the phen:PhenomenonOccurence observed in the phen:Observation.

I.e. From the same phen:PhenomenonOccurrence &quot;Hurricane in France on 2019&quot;, we may have different phen:Observations like &quot;Hurricane observed in Rouen on November,2019&quot; and &quot;Hurricane observed in Paris on December,2019&quot;</rdfs:comment>
        <rdfs:label>Observation</rdfs:label>
    </owl:ObjectProperty>
    


    <!-- https://w3id.org/def/propaphen#observationalPresenceIn -->

    <owl:ObjectProperty rdf:about="https://w3id.org/def/propaphen#observationalPresenceIn">
        <rdfs:domain rdf:resource="https://w3id.org/def/propaphen#Presence"/>
        <rdfs:range rdf:resource="https://w3id.org/def/propaphen#Observation"/>
        <rdfs:comment>Relates the phen:Presence of multiple gufo:Individuals in a phen:Observation.

I.e. &quot;Vacines&quot;, &quot;Pantients of COVID-19&quot; and &quot;Pneumonia&quot; gufo:Indifiduals were present (phen:Presence) on december of 2020 in the phen:Observation &quot;Spread of COVID-19 in Paris on december of 2020&quot;.</rdfs:comment>
        <rdfs:label>Observational Presence In</rdfs:label>
    </owl:ObjectProperty>
    


    <!-- https://w3id.org/def/propaphen#presenceOf -->

    <owl:ObjectProperty rdf:about="https://w3id.org/def/propaphen#presenceOf">
        <rdfs:domain rdf:resource="https://w3id.org/def/propaphen#Presence"/>
        <rdfs:range rdf:resource="http://purl.org/nemo/gufo#Entity"/>
        <rdfs:comment>Presence Of</rdfs:comment>
        <rdfs:comment>Relates an instance of propaphe:Presence with the Individual/entity spatiotemporally present.</rdfs:comment>
    </owl:ObjectProperty>
    


    <!-- https://w3id.org/def/propaphen#spatialPresenceIn -->

    <owl:ObjectProperty rdf:about="https://w3id.org/def/propaphen#spatialPresenceIn">
        <rdfs:domain rdf:resource="https://w3id.org/def/propaphen#Presence"/>
        <rdfs:range rdf:resource="http://www.opengis.net/ont/geosparql#SpatialObject"/>
        <rdfs:comment>Indicates the presence phen:Presence in a spatial region geo:SpatialObject.</rdfs:comment>
        <rdfs:label>Spatial Presence In</rdfs:label>
    </owl:ObjectProperty>
    


    <!-- https://w3id.org/seas/connectedThrough -->

    <owl:ObjectProperty rdf:about="https://w3id.org/seas/connectedThrough">
        <owl:inverseOf rdf:resource="https://w3id.org/seas/connectsSystem"/>
        <rdfs:domain rdf:resource="https://w3id.org/seas/System"/>
        <rdfs:range rdf:resource="https://w3id.org/seas/Connection"/>
        <owl:propertyChainAxiom rdf:parseType="Collection">
            <rdf:Description rdf:about="https://w3id.org/seas/connectsAt"/>
            <rdf:Description rdf:about="https://w3id.org/seas/connectsSystemThrough"/>
        </owl:propertyChainAxiom>
        <rdfs:comment xml:lang="en">Links a system to one of its connections to other systems.</rdfs:comment>
        <rdfs:isDefinedBy rdf:resource="https://w3id.org/seas/SystemOntology"/>
        <rdfs:label xml:lang="en">connected through</rdfs:label>
        <ns1:term_status>stable</ns1:term_status>
    </owl:ObjectProperty>
    


    <!-- https://w3id.org/seas/connectedTo -->

    <owl:ObjectProperty rdf:about="https://w3id.org/seas/connectedTo">
        <rdf:type rdf:resource="http://www.w3.org/2002/07/owl#SymmetricProperty"/>
        <rdfs:domain rdf:resource="https://w3id.org/seas/System"/>
        <rdfs:range rdf:resource="https://w3id.org/seas/System"/>
        <rdfs:comment xml:lang="en">Links a system to a system it is connected to.

Connected systems interact in some way. The exact meaning of _interact_ is defined by sub properties of `seas:connectedTo`.

For example, for the electricity to directly flow between an electric vehicle service equipment and an electric vehicle, then they must be linked by property `seas:exchangesElectricityWith`: 

```
seas:exchangesElectricityWith rdfs:subPropertyOf seas:connectedTo .

&lt;electric_vehicle&gt; seas:exchangesElectricityWith &lt;electric_vehicle_service_equipment&gt; .
```

Property `seas:connectedTo` is symmetric:

```
if x seas:connectedTo y, then it is true that y seas:connectedTo x.
```

This property can be qualified using class `seas:Connection`, which connects the two systems.

If there is a connection between several systems, then one may infer these systems are pairwise connected.</rdfs:comment>
        <rdfs:isDefinedBy rdf:resource="https://w3id.org/seas/SystemOntology"/>
        <rdfs:label xml:lang="en">connected to</rdfs:label>
        <ns1:term_status>stable</ns1:term_status>
    </owl:ObjectProperty>
    


    <!-- https://w3id.org/seas/connectionPointOf -->

    <owl:ObjectProperty rdf:about="https://w3id.org/seas/connectionPointOf">
        <owl:inverseOf rdf:resource="https://w3id.org/seas/connectsAt"/>
        <rdf:type rdf:resource="http://www.w3.org/2002/07/owl#FunctionalProperty"/>
        <rdfs:domain rdf:resource="https://w3id.org/seas/ConnectionPoint"/>
        <rdfs:range rdf:resource="https://w3id.org/seas/System"/>
        <rdfs:comment xml:lang="en">Links a connection point to the one and only one system it belongs to.</rdfs:comment>
        <rdfs:isDefinedBy rdf:resource="https://w3id.org/seas/SystemOntology"/>
        <rdfs:label xml:lang="en">connection point to</rdfs:label>
        <ns1:term_status>stable</ns1:term_status>
    </owl:ObjectProperty>
    


    <!-- https://w3id.org/seas/connectsAt -->

    <owl:ObjectProperty rdf:about="https://w3id.org/seas/connectsAt">
        <rdf:type rdf:resource="http://www.w3.org/2002/07/owl#InverseFunctionalProperty"/>
        <rdfs:domain rdf:resource="https://w3id.org/seas/System"/>
        <rdfs:range rdf:resource="https://w3id.org/seas/ConnectionPoint"/>
        <rdfs:comment xml:lang="en">Links a system to one of the connection points at which it connects.</rdfs:comment>
        <rdfs:isDefinedBy rdf:resource="https://w3id.org/seas/SystemOntology"/>
        <rdfs:label xml:lang="en">connects at</rdfs:label>
        <ns1:term_status>stable</ns1:term_status>
    </owl:ObjectProperty>
    


    <!-- https://w3id.org/seas/connectsSystem -->

    <owl:ObjectProperty rdf:about="https://w3id.org/seas/connectsSystem">
        <rdfs:domain rdf:resource="https://w3id.org/seas/Connection"/>
        <rdfs:range rdf:resource="https://w3id.org/seas/System"/>
        <owl:propertyChainAxiom rdf:parseType="Collection">
            <rdf:Description rdf:about="https://w3id.org/seas/connectsSystemAt"/>
            <rdf:Description rdf:about="https://w3id.org/seas/connectionPointOf"/>
        </owl:propertyChainAxiom>
        <rdfs:comment xml:lang="en">Links a connection to one of the systems it connects.</rdfs:comment>
        <rdfs:isDefinedBy rdf:resource="https://w3id.org/seas/SystemOntology"/>
        <rdfs:label xml:lang="en">connects system</rdfs:label>
        <ns1:term_status>stable</ns1:term_status>
    </owl:ObjectProperty>
    


    <!-- https://w3id.org/seas/connectsSystemAt -->

    <owl:ObjectProperty rdf:about="https://w3id.org/seas/connectsSystemAt">
        <owl:inverseOf rdf:resource="https://w3id.org/seas/connectsSystemThrough"/>
        <rdfs:domain rdf:resource="https://w3id.org/seas/Connection"/>
        <rdfs:range rdf:resource="https://w3id.org/seas/ConnectionPoint"/>
        <rdfs:comment xml:lang="en">Links a connection to one of the connection points at which it connects a system.</rdfs:comment>
        <rdfs:isDefinedBy rdf:resource="https://w3id.org/seas/SystemOntology"/>
        <rdfs:label xml:lang="en">connects system at</rdfs:label>
        <ns1:term_status>stable</ns1:term_status>
    </owl:ObjectProperty>
    


    <!-- https://w3id.org/seas/connectsSystemThrough -->

    <owl:ObjectProperty rdf:about="https://w3id.org/seas/connectsSystemThrough">
        <rdfs:domain rdf:resource="https://w3id.org/seas/ConnectionPoint"/>
        <rdfs:range rdf:resource="https://w3id.org/seas/Connection"/>
        <rdfs:comment xml:lang="en">Links a connection point to one of the connections through which it connects its system.</rdfs:comment>
        <rdfs:isDefinedBy rdf:resource="https://w3id.org/seas/SystemOntology"/>
        <rdfs:label xml:lang="en">connects system through</rdfs:label>
        <ns1:term_status>stable</ns1:term_status>
    </owl:ObjectProperty>
    


    <!-- https://w3id.org/seas/hasSubSystem -->

    <owl:ObjectProperty rdf:about="https://w3id.org/seas/hasSubSystem">
        <owl:inverseOf rdf:resource="https://w3id.org/seas/subSystemOf"/>
        <rdf:type rdf:resource="http://www.w3.org/2002/07/owl#InverseFunctionalProperty"/>
        <rdfs:domain rdf:resource="https://w3id.org/seas/System"/>
        <rdfs:range rdf:resource="https://w3id.org/seas/System"/>
        <rdfs:comment xml:lang="en">Links a system to one of its sub systems.</rdfs:comment>
        <rdfs:isDefinedBy rdf:resource="https://w3id.org/seas/SystemOntology"/>
        <rdfs:label xml:lang="en">has sub system</rdfs:label>
        <ns1:term_status>stable</ns1:term_status>
    </owl:ObjectProperty>
    


    <!-- https://w3id.org/seas/subSystemOf -->

    <owl:ObjectProperty rdf:about="https://w3id.org/seas/subSystemOf">
        <rdf:type rdf:resource="http://www.w3.org/2002/07/owl#FunctionalProperty"/>
        <rdfs:domain rdf:resource="https://w3id.org/seas/System"/>
        <rdfs:range rdf:resource="https://w3id.org/seas/System"/>
        <rdfs:comment xml:lang="en">Links a system to its super system.

Properties of subsystems somehow contribute to the properties of the super system. The exact meaning of _contribute_ is defined by sub properties of `seas:subSystemOf`.

For example, if a fridge is a subsystem of a kitchen, then its consumption power contributes to the consumption power of the kitchen. 

Property `seas:subSystemOf` is functional, and should be asymmetric:

```
if x seas:subSystemOf y1 and x seas:subSystemOf y2, then y1 and y2 refer to the same resource.
if x seas:subSystemOf y, then it can&apos;t be the case that y seas:subSystemOf x.
```

The asymmetric aspect of property `seas:subSystemOf` would prevents a system from being its own sub-system. Unfortunately, OWL 2 DL disallow a non-simple property (e.g., a functional property) from being asymmetric, see OWL 2 Syntax section 11.

If it was possible that both the fridge and the kitchen be sub systems of a common super system, say, the house, then the consumption power of the fridge would contribute twice to the consumption power of the house. The functional aspect of property `seas:subSystemOf` prevents this undesired effect. 

Due to the open world assumption of RDF, it is not possible to model the closed set of sub systems of a system using property `seas:subSystemOf`.
</rdfs:comment>
        <rdfs:isDefinedBy rdf:resource="https://w3id.org/seas/SystemOntology"/>
        <rdfs:label xml:lang="en">sub system of</rdfs:label>
        <ns1:term_status>stable</ns1:term_status>
    </owl:ObjectProperty>
    


    <!-- 
    ///////////////////////////////////////////////////////////////////////////////////////
    //
    // Data properties
    //
    ///////////////////////////////////////////////////////////////////////////////////////
     -->

    


    <!-- http://purl.org/nemo/gufo#concernsQualityValue -->

    <owl:DatatypeProperty rdf:about="http://purl.org/nemo/gufo#concernsQualityValue">
        <rdfs:domain rdf:resource="http://purl.org/nemo/gufo#QualityValueAttributionSituation"/>
        <rdfs:comment xml:lang="en">Determines a quality value associated with the gufo:ConcreteIndividual that stands in the gufo:QualityValueAttributionSituation.

Use gufo:concernsReifiedQualityValue instead when quality values are refied.

It is recommended that subproperties of gufo:concernsQualityValue are created, possibly identifying the datatype to be used. For example, &quot;concernsTemperatureValue&quot; could be defined as a sub-property of gufo:concernsQualityValue with range xsd:double.</rdfs:comment>
        <rdfs:label xml:lang="en">concernsQualityValue</rdfs:label>
        <rdfs:seeAlso rdf:resource="http://purl.org/nemo/gufo#concernsReifiedQualityValue"/>
    </owl:DatatypeProperty>
    


    <!-- http://purl.org/nemo/gufo#hasBeginPointInXSDDate -->

    <owl:DatatypeProperty rdf:about="http://purl.org/nemo/gufo#hasBeginPointInXSDDate">
        <rdf:type rdf:resource="http://www.w3.org/2002/07/owl#FunctionalProperty"/>
        <rdfs:domain rdf:resource="http://purl.org/nemo/gufo#ConcreteEntity"/>
        <rdfs:range rdf:resource="http://www.w3.org/2001/XMLSchema#date"/>
        <rdfs:comment xml:lang="en">Determines the begin point for a gufo:ConcreteIndividual, using a xsd:date literal.

In the case of endurants, gufo:asBeginPointInXSDDate determines the time point when the endurant comes into existence. In the case of events, this data property determines the time point when the event starts to take place. In the case of situation, it determines the time point when the situation begins to hold.

Use gufo:hasBeginPoint instead when temporal entities are reified.</rdfs:comment>
        <rdfs:label xml:lang="en">hasBeginPointInXSDDate</rdfs:label>
        <rdfs:seeAlso rdf:resource="http://purl.org/nemo/gufo#hasBeginPoint"/>
        <rdfs:seeAlso rdf:resource="http://purl.org/nemo/gufo#hasBeginPointInXSDDateTimeStamp"/>
    </owl:DatatypeProperty>
    


    <!-- http://purl.org/nemo/gufo#hasBeginPointInXSDDateTimeStamp -->

    <owl:DatatypeProperty rdf:about="http://purl.org/nemo/gufo#hasBeginPointInXSDDateTimeStamp">
        <rdf:type rdf:resource="http://www.w3.org/2002/07/owl#FunctionalProperty"/>
        <rdfs:domain rdf:resource="http://purl.org/nemo/gufo#ConcreteEntity"/>
        <rdfs:range rdf:resource="http://www.w3.org/2001/XMLSchema#dateTimeStamp"/>
        <rdfs:comment xml:lang="en">Determines the begin point for a gufo:ConcreteIndividual, using a xsd:dateTimeStamp literal.

In the case of endurants, gufo:hasBeginPointInXSDDateTimeStamp determines the time point when the endurant comes into existence. In the case of events, this data property determines the time point when the event starts to take place. In the case of situation, it determines the time point when the situation begins to hold.

Use gufo:hasBeginPoint instead when temporal entities are reified.</rdfs:comment>
        <rdfs:label xml:lang="en">hasBeginPointInXSDDateTimeStamp</rdfs:label>
        <rdfs:seeAlso rdf:resource="http://purl.org/nemo/gufo#hasBeginPoint"/>
        <rdfs:seeAlso rdf:resource="http://purl.org/nemo/gufo#hasBeginPointInXSDDate"/>
    </owl:DatatypeProperty>
    


    <!-- http://purl.org/nemo/gufo#hasEndPointInXSDDate -->

    <owl:DatatypeProperty rdf:about="http://purl.org/nemo/gufo#hasEndPointInXSDDate">
        <rdf:type rdf:resource="http://www.w3.org/2002/07/owl#FunctionalProperty"/>
        <rdfs:domain rdf:resource="http://purl.org/nemo/gufo#ConcreteEntity"/>
        <rdfs:range rdf:resource="http://www.w3.org/2001/XMLSchema#date"/>
        <rdfs:comment xml:lang="en">Determines the end point for a gufo:ConcreteIndividual using a xsd:date literal.
 
In the case of endurants, gufo:hasEndPointInXSDDate determines the time point when the endurant ceases to exist. In the case of events, this data property determines the time point when the event ends. In the case of situation, it determines the time point when the situation ceases to hold.

Use gufo:hasEndPoint instead when temporal entities are reified.</rdfs:comment>
        <rdfs:label xml:lang="en">hasEndPointInXSDDate</rdfs:label>
        <rdfs:seeAlso rdf:resource="http://purl.org/nemo/gufo#hasEndPoint"/>
        <rdfs:seeAlso rdf:resource="http://purl.org/nemo/gufo#hasEndPointInXSDDateTimeStamp"/>
    </owl:DatatypeProperty>
    


    <!-- http://purl.org/nemo/gufo#hasEndPointInXSDDateTimeStamp -->

    <owl:DatatypeProperty rdf:about="http://purl.org/nemo/gufo#hasEndPointInXSDDateTimeStamp">
        <rdf:type rdf:resource="http://www.w3.org/2002/07/owl#FunctionalProperty"/>
        <rdfs:domain rdf:resource="http://purl.org/nemo/gufo#ConcreteEntity"/>
        <rdfs:range rdf:resource="http://www.w3.org/2001/XMLSchema#dateTimeStamp"/>
        <rdfs:comment xml:lang="en">Determines the end point for a gufo:ConcreteIndividual using a xsd:dateTimeStamp literal.
 
In the case of endurants, gufo:hasEndPointInXSDDateTimeStamp determines the time point when the endurant ceases to exist. In the case of events, this data property determines the time point when the event ends. In the case of situation, it determines the time point when the situation ceases to hold.

Use gufo:hasEndPoint instead when temporal entities are reified.</rdfs:comment>
        <rdfs:label xml:lang="en">hasEndPointInXSDDateTimeStamp</rdfs:label>
        <rdfs:seeAlso rdf:resource="http://purl.org/nemo/gufo#hasEndPoint"/>
        <rdfs:seeAlso rdf:resource="http://purl.org/nemo/gufo#hasEndPointInXSDDate"/>
    </owl:DatatypeProperty>
    


    <!-- http://purl.org/nemo/gufo#hasQualityValue -->

    <owl:DatatypeProperty rdf:about="http://purl.org/nemo/gufo#hasQualityValue">
        <rdfs:domain rdf:resource="http://purl.org/nemo/gufo#ConcreteEntity"/>
        <rdfs:comment xml:lang="en">Determines a quality value associated with the concrete individual.

Use gufo:hasReifiedQualityValue instead when quality values are reified.

It is recommended that subproperties of gufo:hasQualityValue are created, possibly identifying the datatype to be used. For example, &quot;hasTemperatureValue&quot; could be defined as a sub-property of gufo:hasQualityValue whose domain is &quot;Temperature&quot; (specializing gufo:Quality) and whose range is xsd:double.</rdfs:comment>
        <rdfs:label xml:lang="en">hasQualityValue</rdfs:label>
        <rdfs:seeAlso rdf:resource="http://purl.org/nemo/gufo#hasReifiedQualityValue"/>
    </owl:DatatypeProperty>
    


    <!-- http://purl.org/nemo/gufo#hasValueComponent -->

    <owl:DatatypeProperty rdf:about="http://purl.org/nemo/gufo#hasValueComponent">
        <rdfs:domain rdf:resource="http://purl.org/nemo/gufo#QualityValue"/>
        <rdfs:comment xml:lang="en">This property is used for quality values that are defined in terms of a multidimensional quality structure (such as color conceived in terms of hue, saturation and brightness). Each value component of a quality value (a particular value for hue, a particular value for saturation, a particular value for brightness) is determined with this property. 

It is recommended that subproperties of gufo:hasValueComponent are created to indicate values for particular dimensions, possibly identifying the datatype to be used. For example &quot;hasHueComponent&quot;, &quot;hasSaturationComponent&quot; and &quot;hasBrightnessComponent&quot; could be used as data properties specializing gufo:hasValueComponent with the xsd:double datatype.</rdfs:comment>
        <rdfs:label xml:lang="en">hasValueComponent</rdfs:label>
    </owl:DatatypeProperty>
    


    <!-- http://www.opengis.net/ont/geosparql#asGML -->

    <owl:DatatypeProperty rdf:about="http://www.opengis.net/ont/geosparql#asGML">
        <rdfs:subPropertyOf rdf:resource="http://www.opengis.net/ont/geosparql#hasSerialization"/>
        <rdfs:domain rdf:resource="http://www.opengis.net/ont/geosparql#Geometry"/>
        <rdfs:range rdf:resource="http://www.opengis.net/ont/geosparql#gmlLiteral"/>
        <dc:contributor>Matthew Perry</dc:contributor>
        <dc:creator>OGC GeoSPARQL 1.0 Standard Working Group</dc:creator>
        <dc:date rdf:datatype="http://www.w3.org/2001/XMLSchema#date">2011-06-16</dc:date>
        <dc:description xml:lang="en">
      The GML serialization of a geometry
    </dc:description>
        <rdfs:comment xml:lang="en">
      The GML serialization of a geometry
    </rdfs:comment>
        <rdfs:isDefinedBy rdf:resource="http://www.opengis.net/ont/geosparql"/>
        <rdfs:isDefinedBy rdf:resource="http://www.opengis.net/spec/geosparql/1.0"/>
        <rdfs:label xml:lang="en">asGML</rdfs:label>
        <skos:definition xml:lang="en">
      The GML serialization of a geometry
    </skos:definition>
        <skos:prefLabel xml:lang="en">asGML</skos:prefLabel>
    </owl:DatatypeProperty>
    


    <!-- http://www.opengis.net/ont/geosparql#asWKT -->

    <owl:DatatypeProperty rdf:about="http://www.opengis.net/ont/geosparql#asWKT">
        <rdfs:subPropertyOf rdf:resource="http://www.opengis.net/ont/geosparql#hasSerialization"/>
        <rdfs:domain rdf:resource="http://www.opengis.net/ont/geosparql#Geometry"/>
        <rdfs:range rdf:resource="http://www.opengis.net/ont/geosparql#wktLiteral"/>
        <dc:contributor>Matthew Perry</dc:contributor>
        <dc:creator>OGC GeoSPARQL 1.0 Standard Working Group</dc:creator>
        <dc:date rdf:datatype="http://www.w3.org/2001/XMLSchema#date">2011-06-16</dc:date>
        <dc:description xml:lang="en">
      The WKT serialization of a geometry
    </dc:description>
        <rdfs:comment xml:lang="en">
      The WKT serialization of a geometry
    </rdfs:comment>
        <rdfs:isDefinedBy rdf:resource="http://www.opengis.net/ont/geosparql"/>
        <rdfs:isDefinedBy rdf:resource="http://www.opengis.net/spec/geosparql/1.0"/>
        <rdfs:label xml:lang="en">asWKT</rdfs:label>
        <skos:definition xml:lang="en">
      The WKT serialization of a geometry
    </skos:definition>
        <skos:prefLabel xml:lang="en">asWKT</skos:prefLabel>
    </owl:DatatypeProperty>
    


    <!-- http://www.opengis.net/ont/geosparql#coordinateDimension -->

    <owl:DatatypeProperty rdf:about="http://www.opengis.net/ont/geosparql#coordinateDimension">
        <rdfs:domain rdf:resource="http://www.opengis.net/ont/geosparql#Geometry"/>
        <rdfs:range rdf:resource="http://www.w3.org/2001/XMLSchema#integer"/>
        <dc:contributor>Matthew Perry</dc:contributor>
        <dc:creator>OGC GeoSPARQL 1.0 Standard Working Group</dc:creator>
        <dc:date rdf:datatype="http://www.w3.org/2001/XMLSchema#date">2011-06-16</dc:date>
        <dc:description xml:lang="en">
      The number of measurements or axes needed to describe the position of this
      geometry in a coordinate system.
    </dc:description>
        <rdfs:comment xml:lang="en">
      The number of measurements or axes needed to describe the position of this
      geometry in a coordinate system.
    </rdfs:comment>
        <rdfs:isDefinedBy rdf:resource="http://www.opengis.net/ont/geosparql"/>
        <rdfs:isDefinedBy rdf:resource="http://www.opengis.net/spec/geosparql/1.0"/>
        <rdfs:label xml:lang="en">coordinateDimension</rdfs:label>
        <skos:definition xml:lang="en">
      The number of measurements or axes needed to describe the position of this
      geometry in a coordinate system.
    </skos:definition>
        <skos:prefLabel xml:lang="en">coordinateDimension</skos:prefLabel>
    </owl:DatatypeProperty>
    


    <!-- http://www.opengis.net/ont/geosparql#dimension -->

    <owl:DatatypeProperty rdf:about="http://www.opengis.net/ont/geosparql#dimension">
        <rdfs:domain rdf:resource="http://www.opengis.net/ont/geosparql#Geometry"/>
        <rdfs:range rdf:resource="http://www.w3.org/2001/XMLSchema#integer"/>
        <dc:contributor>Matthew Perry</dc:contributor>
        <dc:creator>OGC GeoSPARQL 1.0 Standard Working Group</dc:creator>
        <dc:date rdf:datatype="http://www.w3.org/2001/XMLSchema#date">2011-06-16</dc:date>
        <dc:description xml:lang="en">
      The topological dimension of this geometric object, which 
      must be less than or equal to the coordinate dimension. 
      In non-homogeneous collections, this will return the largest 
      topological dimension of the contained objects.
    </dc:description>
        <rdfs:comment xml:lang="en">
      The topological dimension of this geometric object, which 
      must be less than or equal to the coordinate dimension. 
      In non-homogeneous collections, this will return the largest 
      topological dimension of the contained objects.
    </rdfs:comment>
        <rdfs:isDefinedBy rdf:resource="http://www.opengis.net/ont/geosparql"/>
        <rdfs:isDefinedBy rdf:resource="http://www.opengis.net/spec/geosparql/1.0"/>
        <rdfs:label xml:lang="en">dimension</rdfs:label>
        <skos:definition xml:lang="en">
      The topological dimension of this geometric object, which 
      must be less than or equal to the coordinate dimension. 
      In non-homogeneous collections, this will return the largest 
      topological dimension of the contained objects.
    </skos:definition>
        <skos:prefLabel xml:lang="en">dimension</skos:prefLabel>
    </owl:DatatypeProperty>
    


    <!-- http://www.opengis.net/ont/geosparql#hasSerialization -->

    <owl:DatatypeProperty rdf:about="http://www.opengis.net/ont/geosparql#hasSerialization">
        <rdfs:domain rdf:resource="http://www.opengis.net/ont/geosparql#Geometry"/>
        <rdfs:range rdf:resource="http://www.w3.org/2000/01/rdf-schema#Literal"/>
        <dc:contributor>Matthew Perry</dc:contributor>
        <dc:creator>OGC GeoSPARQL 1.0 Standard Working Group</dc:creator>
        <dc:date rdf:datatype="http://www.w3.org/2001/XMLSchema#date">2011-06-16</dc:date>
        <dc:description xml:lang="en">
      Connects a geometry object with its text-based serialization.
    </dc:description>
        <rdfs:comment xml:lang="en">
      Connects a geometry object with its text-based serialization.
    </rdfs:comment>
        <rdfs:isDefinedBy rdf:resource="http://www.opengis.net/ont/geosparql"/>
        <rdfs:isDefinedBy rdf:resource="http://www.opengis.net/spec/geosparql/1.0"/>
        <rdfs:label xml:lang="en">has serialization</rdfs:label>
        <skos:definition xml:lang="en">
      Connects a geometry object with its text-based serialization.
    </skos:definition>
        <skos:prefLabel xml:lang="en">has serialization</skos:prefLabel>
    </owl:DatatypeProperty>
    


    <!-- http://www.opengis.net/ont/geosparql#isEmpty -->

    <owl:DatatypeProperty rdf:about="http://www.opengis.net/ont/geosparql#isEmpty">
        <rdfs:domain rdf:resource="http://www.opengis.net/ont/geosparql#Geometry"/>
        <rdfs:range rdf:resource="http://www.w3.org/2001/XMLSchema#boolean"/>
        <dc:contributor>Matthew Perry</dc:contributor>
        <dc:creator>OGC GeoSPARQL 1.0 Standard Working Group</dc:creator>
        <dc:date rdf:datatype="http://www.w3.org/2001/XMLSchema#date">2011-06-16</dc:date>
        <dc:description xml:lang="en">
      (true) if this geometric object is the empty Geometry. If 
      true, then this geometric object represents the empty point 
      set for the coordinate space.
    </dc:description>
        <rdfs:comment xml:lang="en">
      (true) if this geometric object is the empty Geometry. If 
      true, then this geometric object represents the empty point 
      set for the coordinate space.
    </rdfs:comment>
        <rdfs:isDefinedBy rdf:resource="http://www.opengis.net/ont/geosparql"/>
        <rdfs:isDefinedBy rdf:resource="http://www.opengis.net/spec/geosparql/1.0"/>
        <rdfs:label xml:lang="en">isEmpty</rdfs:label>
        <skos:definition xml:lang="en">
      (true) if this geometric object is the empty Geometry. If 
      true, then this geometric object represents the empty point 
      set for the coordinate space.
    </skos:definition>
        <skos:prefLabel xml:lang="en">isEmpty</skos:prefLabel>
    </owl:DatatypeProperty>
    


    <!-- http://www.opengis.net/ont/geosparql#isSimple -->

    <owl:DatatypeProperty rdf:about="http://www.opengis.net/ont/geosparql#isSimple">
        <rdfs:domain rdf:resource="http://www.opengis.net/ont/geosparql#Geometry"/>
        <rdfs:range rdf:resource="http://www.w3.org/2001/XMLSchema#boolean"/>
        <dc:contributor>Matthew Perry</dc:contributor>
        <dc:creator>OGC GeoSPARQL 1.0 Standard Working Group</dc:creator>
        <dc:date rdf:datatype="http://www.w3.org/2001/XMLSchema#date">2011-06-16</dc:date>
        <dc:description xml:lang="en">
      (true) if this geometric object has no anomalous geometric 
      points, such as self intersection or self tangency.
    </dc:description>
        <rdfs:comment xml:lang="en">
      (true) if this geometric object has no anomalous geometric 
      points, such as self intersection or self tangency.
    </rdfs:comment>
        <rdfs:isDefinedBy rdf:resource="http://www.opengis.net/ont/geosparql"/>
        <rdfs:isDefinedBy rdf:resource="http://www.opengis.net/spec/geosparql/1.0"/>
        <rdfs:label xml:lang="en">isSimple</rdfs:label>
        <skos:definition xml:lang="en">
      (true) if this geometric object has no anomalous geometric 
      points, such as self intersection or self tangency.
    </skos:definition>
        <skos:prefLabel xml:lang="en">isSimple</skos:prefLabel>
    </owl:DatatypeProperty>
    


    <!-- http://www.opengis.net/ont/geosparql#spatialDimension -->

    <owl:DatatypeProperty rdf:about="http://www.opengis.net/ont/geosparql#spatialDimension">
        <rdfs:domain rdf:resource="http://www.opengis.net/ont/geosparql#Geometry"/>
        <rdfs:range rdf:resource="http://www.w3.org/2001/XMLSchema#integer"/>
        <dc:contributor>Matthew Perry</dc:contributor>
        <dc:creator>OGC GeoSPARQL 1.0 Standard Working Group</dc:creator>
        <dc:date rdf:datatype="http://www.w3.org/2001/XMLSchema#date">2011-06-16</dc:date>
        <dc:description xml:lang="en">
      The number of measurements or axes needed to describe the spatial position of 
      this geometry in a coordinate system.
    </dc:description>
        <rdfs:comment xml:lang="en">
      The number of measurements or axes needed to describe the spatial position of 
      this geometry in a coordinate system.
    </rdfs:comment>
        <rdfs:isDefinedBy rdf:resource="http://www.opengis.net/ont/geosparql"/>
        <rdfs:isDefinedBy rdf:resource="http://www.opengis.net/spec/geosparql/1.0"/>
        <rdfs:label xml:lang="en">spatialDimension</rdfs:label>
        <skos:definition xml:lang="en">
      The number of measurements or axes needed to describe the spatial position of 
      this geometry in a coordinate system.
    </skos:definition>
        <skos:prefLabel xml:lang="en">spatialDimension</skos:prefLabel>
    </owl:DatatypeProperty>
    


    <!-- http://www.w3.org/2004/02/skos/core#notation -->

    <owl:DatatypeProperty rdf:about="http://www.w3.org/2004/02/skos/core#notation">
        <rdfs:isDefinedBy rdf:resource="http://www.w3.org/2004/02/skos/core"/>
        <rdfs:label xml:lang="en">notation</rdfs:label>
        <skos:definition xml:lang="en">A notation, also known as classification code, is a string of characters such as &quot;T58.5&quot; or &quot;303.4833&quot; used to uniquely identify a concept within the scope of a given concept scheme.</skos:definition>
        <skos:scopeNote xml:lang="en">By convention, skos:notation is used with a typed literal in the object position of the triple.</skos:scopeNote>
    </owl:DatatypeProperty>
    


    <!-- http://www.w3.org/2006/time#day -->

    <owl:DatatypeProperty rdf:about="http://www.w3.org/2006/time#day">
        <rdfs:domain rdf:resource="http://www.w3.org/2006/time#GeneralDateTimeDescription"/>
        <rdfs:comment xml:lang="en">Day position in a calendar-clock system.

The range of this property is not specified, so can be replaced by any specific representation of a calendar day from any calendar. </rdfs:comment>
        <rdfs:comment xml:lang="es">Posición de día en un sistema calendario-reloj.</rdfs:comment>
        <rdfs:label xml:lang="en">day</rdfs:label>
        <rdfs:label xml:lang="es">día</rdfs:label>
        <skos:definition xml:lang="en">Day position in a calendar-clock system.

The range of this property is not specified, so can be replaced by any specific representation of a calendar day from any calendar. </skos:definition>
        <skos:definition xml:lang="es">Posición de día en un sistema calendario-reloj.

El rango de esta propiedad no está especificado, por tanto, se puede reemplazar por una representación específica de un día de calendario de cualquier calendario.</skos:definition>
    </owl:DatatypeProperty>
    


    <!-- http://www.w3.org/2006/time#dayOfYear -->

    <owl:DatatypeProperty rdf:about="http://www.w3.org/2006/time#dayOfYear">
        <rdfs:domain rdf:resource="http://www.w3.org/2006/time#GeneralDateTimeDescription"/>
        <rdfs:range rdf:resource="http://www.w3.org/2001/XMLSchema#nonNegativeInteger"/>
        <rdfs:comment xml:lang="es">El número de día en el año.</rdfs:comment>
        <rdfs:comment xml:lang="en">The number of the day within the year</rdfs:comment>
        <rdfs:label xml:lang="en">day of year</rdfs:label>
        <rdfs:label xml:lang="es">día del año</rdfs:label>
        <skos:definition xml:lang="es">El número de día en el año.</skos:definition>
        <skos:definition xml:lang="en">The number of the day within the year</skos:definition>
    </owl:DatatypeProperty>
    


    <!-- http://www.w3.org/2006/time#days -->

    <owl:DatatypeProperty rdf:about="http://www.w3.org/2006/time#days">
        <rdfs:domain rdf:resource="http://www.w3.org/2006/time#GeneralDurationDescription"/>
        <rdfs:range rdf:resource="http://www.w3.org/2001/XMLSchema#decimal"/>
        <rdfs:comment xml:lang="es">Longitud de, o elemento de la longitud de, una extensión temporal expresada en días.</rdfs:comment>
        <rdfs:comment xml:lang="en">length of, or element of the length of, a temporal extent expressed in days</rdfs:comment>
        <rdfs:label xml:lang="en">days duration</rdfs:label>
        <rdfs:label xml:lang="es">duración en días</rdfs:label>
        <skos:definition xml:lang="es">Longitud de, o elemento de la longitud de, una extensión temporal expresada en días.</skos:definition>
        <skos:definition xml:lang="en">length of, or element of the length of, a temporal extent expressed in days</skos:definition>
    </owl:DatatypeProperty>
    


    <!-- http://www.w3.org/2006/time#hasXSDDuration -->

    <owl:DatatypeProperty rdf:about="http://www.w3.org/2006/time#hasXSDDuration">
        <rdfs:domain rdf:resource="http://www.w3.org/2006/time#TemporalEntity"/>
        <rdfs:range rdf:resource="http://www.w3.org/2001/XMLSchema#duration"/>
        <rdfs:comment xml:lang="es">Extensión de una entidad temporal, expresada utilizando xsd:duration.</rdfs:comment>
        <rdfs:comment xml:lang="en">Extent of a temporal entity, expressed using xsd:duration</rdfs:comment>
        <rdfs:label xml:lang="en">has XSD duration</rdfs:label>
        <rdfs:label xml:lang="es">tiene duración XSD</rdfs:label>
        <skos:definition xml:lang="es">Extensión de una entidad temporal, expresada utilizando xsd:duration.</skos:definition>
        <skos:definition xml:lang="en">Extent of a temporal entity, expressed using xsd:duration</skos:definition>
        <skos:editorialNote xml:lang="es">Característica arriesgada - añadida en la revisión de 2017, y todavía no ampliamente utilizada.</skos:editorialNote>
        <skos:editorialNote xml:lang="en">Feature at risk - added in 2017 revision, and not yet widely used. </skos:editorialNote>
    </owl:DatatypeProperty>
    


    <!-- http://www.w3.org/2006/time#hour -->

    <owl:DatatypeProperty rdf:about="http://www.w3.org/2006/time#hour">
        <rdfs:domain rdf:resource="http://www.w3.org/2006/time#GeneralDateTimeDescription"/>
        <rdfs:range rdf:resource="http://www.w3.org/2001/XMLSchema#nonNegativeInteger"/>
        <rdfs:comment xml:lang="en">Hour position in a calendar-clock system.</rdfs:comment>
        <rdfs:comment xml:lang="es">Posición de hora en un sistema calendario-reloj.</rdfs:comment>
        <rdfs:label xml:lang="es">hora</rdfs:label>
        <rdfs:label xml:lang="en">hour</rdfs:label>
        <skos:definition xml:lang="en">Hour position in a calendar-clock system.</skos:definition>
        <skos:definition xml:lang="es">Posición de hora en un sistema calendario-reloj.</skos:definition>
    </owl:DatatypeProperty>
    


    <!-- http://www.w3.org/2006/time#hours -->

    <owl:DatatypeProperty rdf:about="http://www.w3.org/2006/time#hours">
        <rdfs:domain rdf:resource="http://www.w3.org/2006/time#GeneralDurationDescription"/>
        <rdfs:range rdf:resource="http://www.w3.org/2001/XMLSchema#decimal"/>
        <rdfs:comment xml:lang="es">Longitud de, o elemento de la longitud de, una extensión temporal expresada en horas.</rdfs:comment>
        <rdfs:comment xml:lang="en">length of, or element of the length of, a temporal extent expressed in hours</rdfs:comment>
        <rdfs:label xml:lang="es">duración en horas</rdfs:label>
        <rdfs:label xml:lang="en">hours duration</rdfs:label>
        <skos:definition xml:lang="es">Longitud de, o elemento de la longitud de, una extensión temporal expresada en horas.</skos:definition>
        <skos:definition xml:lang="en">length of, or element of the length of, a temporal extent expressed in hours</skos:definition>
    </owl:DatatypeProperty>
    


    <!-- http://www.w3.org/2006/time#inXSDDate -->

    <owl:DatatypeProperty rdf:about="http://www.w3.org/2006/time#inXSDDate">
        <rdfs:domain rdf:resource="http://www.w3.org/2006/time#Instant"/>
        <rdfs:range rdf:resource="http://www.w3.org/2001/XMLSchema#date"/>
        <rdfs:comment xml:lang="es">Posición de un instante, expresado utilizando xsd:date.</rdfs:comment>
        <rdfs:comment xml:lang="en">Position of an instant, expressed using xsd:date</rdfs:comment>
        <rdfs:label xml:lang="es">en fecha XSD</rdfs:label>
        <rdfs:label xml:lang="en">in XSD date</rdfs:label>
        <skos:definition xml:lang="es">Posición de un instante, expresado utilizando xsd:date.</skos:definition>
        <skos:definition xml:lang="en">Position of an instant, expressed using xsd:date</skos:definition>
    </owl:DatatypeProperty>
    


    <!-- http://www.w3.org/2006/time#inXSDDateTime -->

    <owl:DatatypeProperty rdf:about="http://www.w3.org/2006/time#inXSDDateTime">
        <rdfs:domain rdf:resource="http://www.w3.org/2006/time#Instant"/>
        <rdfs:range rdf:resource="http://www.w3.org/2001/XMLSchema#dateTime"/>
        <rdfs:comment xml:lang="es">Posición de un instante, expresado utilizando xsd:dateTime.</rdfs:comment>
        <rdfs:comment xml:lang="en">Position of an instant, expressed using xsd:dateTime</rdfs:comment>
        <rdfs:label xml:lang="es">en fecha-tiempo XSD</rdfs:label>
        <rdfs:label xml:lang="en">in XSD Date-Time</rdfs:label>
        <owl:deprecated rdf:datatype="http://www.w3.org/2001/XMLSchema#boolean">true</owl:deprecated>
        <skos:definition xml:lang="es">Posición de un instante, expresado utilizando xsd:dateTime.</skos:definition>
        <skos:definition xml:lang="en">Position of an instant, expressed using xsd:dateTime</skos:definition>
        <skos:note xml:lang="es">La propiedad &apos;en fecha-hora XSD&apos; ha sido reemplazada por &apos;en fecha-sello de tiempo XSD&apos; que hace obligatorio el campo &apos;huso horario&apos;.</skos:note>
        <skos:note xml:lang="en">The property :inXSDDateTime is replaced by :inXSDDateTimeStamp which makes the time-zone field mandatory.</skos:note>
    </owl:DatatypeProperty>
    


    <!-- http://www.w3.org/2006/time#inXSDDateTimeStamp -->

    <owl:DatatypeProperty rdf:about="http://www.w3.org/2006/time#inXSDDateTimeStamp">
        <rdfs:domain rdf:resource="http://www.w3.org/2006/time#Instant"/>
        <rdfs:range rdf:resource="http://www.w3.org/2001/XMLSchema#dateTimeStamp"/>
        <rdfs:comment xml:lang="es">Posición de un instante, expresado utilizando xsd:dateTimeStamp.</rdfs:comment>
        <rdfs:comment xml:lang="en">Position of an instant, expressed using xsd:dateTimeStamp</rdfs:comment>
        <rdfs:label xml:lang="es">en fecha-sello de tiempo XSD</rdfs:label>
        <rdfs:label xml:lang="en">in XSD Date-Time-Stamp</rdfs:label>
        <skos:definition xml:lang="es">Posición de un instante, expresado utilizando xsd:dateTimeStamp.</skos:definition>
        <skos:definition xml:lang="en">Position of an instant, expressed using xsd:dateTimeStamp</skos:definition>
    </owl:DatatypeProperty>
    


    <!-- http://www.w3.org/2006/time#inXSDgYear -->

    <owl:DatatypeProperty rdf:about="http://www.w3.org/2006/time#inXSDgYear">
        <rdfs:domain rdf:resource="http://www.w3.org/2006/time#Instant"/>
        <rdfs:range rdf:resource="http://www.w3.org/2001/XMLSchema#gYear"/>
        <rdfs:comment xml:lang="es">Posición de un instante, expresado utilizando xsd:gYear.</rdfs:comment>
        <rdfs:comment xml:lang="en">Position of an instant, expressed using xsd:gYear</rdfs:comment>
        <rdfs:label xml:lang="es">en año gregoriano XSD</rdfs:label>
        <rdfs:label xml:lang="en">in XSD g-Year</rdfs:label>
        <skos:definition xml:lang="es">Posición de un instante, expresado utilizando xsd:gYear.</skos:definition>
        <skos:definition xml:lang="en">Position of an instant, expressed using xsd:gYear</skos:definition>
    </owl:DatatypeProperty>
    


    <!-- http://www.w3.org/2006/time#inXSDgYearMonth -->

    <owl:DatatypeProperty rdf:about="http://www.w3.org/2006/time#inXSDgYearMonth">
        <rdfs:domain rdf:resource="http://www.w3.org/2006/time#Instant"/>
        <rdfs:range rdf:resource="http://www.w3.org/2001/XMLSchema#gYearMonth"/>
        <rdfs:comment xml:lang="es">Posición de un instante, expresado utilizando xsd:gYearMonth.</rdfs:comment>
        <rdfs:comment xml:lang="en">Position of an instant, expressed using xsd:gYearMonth</rdfs:comment>
        <rdfs:label xml:lang="es">en año-mes gregoriano XSD</rdfs:label>
        <rdfs:label xml:lang="en">in XSD g-YearMonth</rdfs:label>
        <skos:definition xml:lang="es">Posición de un instante, expresado utilizando xsd:gYearMonth.</skos:definition>
        <skos:definition xml:lang="en">Position of an instant, expressed using xsd:gYearMonth</skos:definition>
    </owl:DatatypeProperty>
    


    <!-- http://www.w3.org/2006/time#minute -->

    <owl:DatatypeProperty rdf:about="http://www.w3.org/2006/time#minute">
        <rdfs:domain rdf:resource="http://www.w3.org/2006/time#GeneralDateTimeDescription"/>
        <rdfs:range rdf:resource="http://www.w3.org/2001/XMLSchema#nonNegativeInteger"/>
        <rdfs:comment xml:lang="en">Minute position in a calendar-clock system.</rdfs:comment>
        <rdfs:comment xml:lang="es">Posición de minuto en un sistema calendario-reloj.</rdfs:comment>
        <rdfs:label xml:lang="en">minute</rdfs:label>
        <rdfs:label xml:lang="es">minuto</rdfs:label>
        <skos:definition xml:lang="en">Minute position in a calendar-clock system.</skos:definition>
        <skos:definition xml:lang="es">Posición de minuto en un sistema calendario-reloj.</skos:definition>
    </owl:DatatypeProperty>
    


    <!-- http://www.w3.org/2006/time#minutes -->

    <owl:DatatypeProperty rdf:about="http://www.w3.org/2006/time#minutes">
        <rdfs:domain rdf:resource="http://www.w3.org/2006/time#GeneralDurationDescription"/>
        <rdfs:range rdf:resource="http://www.w3.org/2001/XMLSchema#decimal"/>
        <rdfs:comment xml:lang="es">Longitud de, o elemento de la longitud de, una extensión temporal expresada en minutos.</rdfs:comment>
        <rdfs:comment xml:lang="en">length, or element of, a temporal extent expressed in minutes</rdfs:comment>
        <rdfs:label xml:lang="en">minutes</rdfs:label>
        <rdfs:label xml:lang="es">minutos</rdfs:label>
        <skos:definition xml:lang="es">Longitud de, o elemento de la longitud de, una extensión temporal expresada en minutos.</skos:definition>
        <skos:definition xml:lang="en">length, or element of, a temporal extent expressed in minutes</skos:definition>
    </owl:DatatypeProperty>
    


    <!-- http://www.w3.org/2006/time#month -->

    <owl:DatatypeProperty rdf:about="http://www.w3.org/2006/time#month">
        <rdfs:domain rdf:resource="http://www.w3.org/2006/time#GeneralDateTimeDescription"/>
        <rdfs:comment xml:lang="en">Month position in a calendar-clock system.

The range of this property is not specified, so can be replaced by any specific representation of a calendar month from any calendar. </rdfs:comment>
        <rdfs:comment xml:lang="es">Posición de mes en un sistema calendario-reloj.
    El rango de esta propiedad no está especificado, por tanto, se puede reemplazar por cualquier representación específica de un mes de calendario de un calendario cualquiera.</rdfs:comment>
        <rdfs:label xml:lang="es">mes</rdfs:label>
        <rdfs:label xml:lang="en">month</rdfs:label>
        <skos:definition xml:lang="en">Month position in a calendar-clock system.

The range of this property is not specified, so can be replaced by any specific representation of a calendar month from any calendar. </skos:definition>
        <skos:definition xml:lang="es">Posición de mes en un sistema calendario-reloj.
            El rango de esta propiedad no está especificado, por tanto, se puede reemplazar por cualquier representación específica de un mes de calendario de un calendario cualquiera.</skos:definition>
    </owl:DatatypeProperty>
    


    <!-- http://www.w3.org/2006/time#months -->

    <owl:DatatypeProperty rdf:about="http://www.w3.org/2006/time#months">
        <rdfs:domain rdf:resource="http://www.w3.org/2006/time#GeneralDurationDescription"/>
        <rdfs:range rdf:resource="http://www.w3.org/2001/XMLSchema#decimal"/>
        <rdfs:comment xml:lang="es">Longitud de, o elemento de la longitud de, una extensión temporal expresada en meses.</rdfs:comment>
        <rdfs:comment xml:lang="en">length of, or element of the length of, a temporal extent expressed in months</rdfs:comment>
        <rdfs:label xml:lang="es">duración en meses</rdfs:label>
        <rdfs:label xml:lang="en">months duration</rdfs:label>
        <skos:definition xml:lang="es">Longitud de, o elemento de la longitud de, una extensión temporal expresada en meses.</skos:definition>
        <skos:definition xml:lang="en">length of, or element of the length of, a temporal extent expressed in months</skos:definition>
    </owl:DatatypeProperty>
    


    <!-- http://www.w3.org/2006/time#nominalPosition -->

    <owl:DatatypeProperty rdf:about="http://www.w3.org/2006/time#nominalPosition">
        <rdfs:domain rdf:resource="http://www.w3.org/2006/time#TimePosition"/>
        <rdfs:range rdf:resource="http://www.w3.org/2001/XMLSchema#string"/>
        <rdfs:comment xml:lang="es">El valor (nominal) que indica posición temporal en un sistema de referencia ordinal.</rdfs:comment>
        <rdfs:comment xml:lang="en">The (nominal) value indicating temporal position in an ordinal reference system </rdfs:comment>
        <rdfs:label xml:lang="en">Name of temporal position</rdfs:label>
        <rdfs:label xml:lang="es">nombre de posición temporal</rdfs:label>
        <skos:definition xml:lang="es">El valor (nominal) que indica posición temporal en un sistema de referencia ordinal.</skos:definition>
        <skos:definition xml:lang="en">The (nominal) value indicating temporal position in an ordinal reference system </skos:definition>
    </owl:DatatypeProperty>
    


    <!-- http://www.w3.org/2006/time#numericDuration -->

    <owl:DatatypeProperty rdf:about="http://www.w3.org/2006/time#numericDuration">
        <rdfs:domain rdf:resource="http://www.w3.org/2006/time#Duration"/>
        <rdfs:range rdf:resource="http://www.w3.org/2001/XMLSchema#decimal"/>
        <rdfs:comment xml:lang="es">Valor de una extensión temporal expresada como un número decimal escalado por una unidad de tiempo.</rdfs:comment>
        <rdfs:comment xml:lang="en">Value of a temporal extent expressed as a decimal number scaled by a temporal unit</rdfs:comment>
        <rdfs:label xml:lang="en">Numeric value of temporal duration</rdfs:label>
        <rdfs:label xml:lang="es">valor numérico de duración temporal</rdfs:label>
        <skos:definition xml:lang="es">Valor de una extensión temporal expresada como un número decimal escalado por una unidad de tiempo.</skos:definition>
        <skos:definition xml:lang="en">Value of a temporal extent expressed as a decimal number scaled by a temporal unit</skos:definition>
    </owl:DatatypeProperty>
    


    <!-- http://www.w3.org/2006/time#numericPosition -->

    <owl:DatatypeProperty rdf:about="http://www.w3.org/2006/time#numericPosition">
        <rdfs:domain rdf:resource="http://www.w3.org/2006/time#TimePosition"/>
        <rdfs:range rdf:resource="http://www.w3.org/2001/XMLSchema#decimal"/>
        <rdfs:comment xml:lang="es">El valor (numérico) que indica posición temporal en un sistema de referencia ordinal.</rdfs:comment>
        <rdfs:comment xml:lang="en">The (numeric) value indicating position within a temporal coordinate system </rdfs:comment>
        <rdfs:label xml:lang="en">Numeric value of temporal position</rdfs:label>
        <rdfs:label xml:lang="es">valor numérico de posición temporal</rdfs:label>
        <skos:definition xml:lang="es">El valor (numérico) que indica posición temporal en un sistema de referencia ordinal.</skos:definition>
        <skos:definition xml:lang="en">The (numeric) value indicating position within a temporal coordinate system </skos:definition>
    </owl:DatatypeProperty>
    


    <!-- http://www.w3.org/2006/time#second -->

    <owl:DatatypeProperty rdf:about="http://www.w3.org/2006/time#second">
        <rdfs:domain rdf:resource="http://www.w3.org/2006/time#GeneralDateTimeDescription"/>
        <rdfs:range rdf:resource="http://www.w3.org/2001/XMLSchema#decimal"/>
        <rdfs:comment xml:lang="es">Posición de segundo en un sistema calendario-reloj.</rdfs:comment>
        <rdfs:comment xml:lang="en">Second position in a calendar-clock system.</rdfs:comment>
        <rdfs:label xml:lang="en">second</rdfs:label>
        <rdfs:label xml:lang="es">segundo</rdfs:label>
    </owl:DatatypeProperty>
    


    <!-- http://www.w3.org/2006/time#seconds -->

    <owl:DatatypeProperty rdf:about="http://www.w3.org/2006/time#seconds">
        <rdfs:domain rdf:resource="http://www.w3.org/2006/time#GeneralDurationDescription"/>
        <rdfs:range rdf:resource="http://www.w3.org/2001/XMLSchema#decimal"/>
        <rdfs:comment xml:lang="es">Longitud de, o elemento de la longitud de, una extensión temporal expresada en segundos.</rdfs:comment>
        <rdfs:comment xml:lang="en">length of, or element of the length of, a temporal extent expressed in seconds</rdfs:comment>
        <rdfs:label xml:lang="es">duración en segundos</rdfs:label>
        <rdfs:label xml:lang="en">seconds duration</rdfs:label>
        <rdfs:seeAlso rdf:resource="http://www.bipm.org/en/publications/si-brochure/second.html"/>
    </owl:DatatypeProperty>
    


    <!-- http://www.w3.org/2006/time#week -->

    <owl:DatatypeProperty rdf:about="http://www.w3.org/2006/time#week">
        <rdfs:domain rdf:resource="http://www.w3.org/2006/time#GeneralDateTimeDescription"/>
        <rdfs:range rdf:resource="http://www.w3.org/2001/XMLSchema#nonNegativeInteger"/>
        <rdfs:comment xml:lang="es">Número de semana en el año.</rdfs:comment>
        <rdfs:comment xml:lang="en">Week number within the year.</rdfs:comment>
        <rdfs:label xml:lang="es">semana</rdfs:label>
        <rdfs:label xml:lang="en">week</rdfs:label>
        <skos:note xml:lang="en">Weeks are numbered differently depending on the calendar in use and the local language or cultural conventions (locale). ISO-8601 specifies that the first week of the year includes at least four days, and that Monday is the first day of the week. In that system, week 1 is the week that contains the first Thursday in the year.</skos:note>
        <skos:scopeNote xml:lang="es">Las semanas están numeradas de forma diferente dependiendo del calendario en uso y de las convenciones lingüísticas y culturales locales (locale en inglés). El ISO-8601 especifica que la primera semana del año incluye al menos cuatro días, y que el lunes es el primer día de la semana. En ese sistema, la semana 1 es la semana que contiene el primer jueves del año.</skos:scopeNote>
    </owl:DatatypeProperty>
    


    <!-- http://www.w3.org/2006/time#weeks -->

    <owl:DatatypeProperty rdf:about="http://www.w3.org/2006/time#weeks">
        <rdfs:domain rdf:resource="http://www.w3.org/2006/time#GeneralDurationDescription"/>
        <rdfs:range rdf:resource="http://www.w3.org/2001/XMLSchema#decimal"/>
        <rdfs:comment xml:lang="es">Longitud de, o elemento de la longitud de, una extensión temporal expresada en semanas.</rdfs:comment>
        <rdfs:comment xml:lang="en">length of, or element of the length of, a temporal extent expressed in weeks</rdfs:comment>
        <rdfs:label xml:lang="es">duración en semanas</rdfs:label>
        <rdfs:label xml:lang="en">weeks duration</rdfs:label>
    </owl:DatatypeProperty>
    


    <!-- http://www.w3.org/2006/time#xsdDateTime -->

    <owl:DatatypeProperty rdf:about="http://www.w3.org/2006/time#xsdDateTime">
        <rdfs:domain rdf:resource="http://www.w3.org/2006/time#DateTimeInterval"/>
        <rdfs:range rdf:resource="http://www.w3.org/2001/XMLSchema#dateTime"/>
        <rdfs:comment xml:lang="es">Valor de &apos;intervalo de fecha-hora&apos; expresado como un valor compacto.</rdfs:comment>
        <rdfs:comment xml:lang="en">Value of DateTimeInterval expressed as a compact value.</rdfs:comment>
        <rdfs:label xml:lang="en">has XSD date-time</rdfs:label>
        <rdfs:label xml:lang="es">tiene fecha-hora XSD</rdfs:label>
        <owl:deprecated rdf:datatype="http://www.w3.org/2001/XMLSchema#boolean">true</owl:deprecated>
        <skos:note xml:lang="en">Using xsd:dateTime in this place means that the duration of the interval is implicit: it corresponds to the length of the smallest non-zero element of the date-time literal. However, this rule cannot be used for intervals whose duration is more than one rank smaller than the starting time - e.g. the first minute or second of a day, the first hour of a month, or the first day of a year. In these cases the desired interval cannot be distinguished from the interval corresponding to the next rank up. Because of this essential ambiguity, use of this property is not recommended and it is deprecated.</skos:note>
        <skos:note>Utilizando xsd:dateTime en este lugar significa que la duración del intervalo está implícita: se corresponde con la longitud del elemento más pequeño distinto de cero del literal fecha-hora. Sin embargo, esta regla no se puede utilizar para intervalos cuya duración es mayor que un rango más pequeño que el tiempo de comienzo - p.ej. el primer minuto o segundo del día, la primera hora del mes, o el primer día del año. En estos casos el intervalo deseado no se puede distinguir del intervalo correspondiente al próximo rango más alto. Debido a esta ambigüedad esencial, no se recomienda el uso de esta propiedad y está desaprobada.</skos:note>
    </owl:DatatypeProperty>
    


    <!-- http://www.w3.org/2006/time#year -->

    <owl:DatatypeProperty rdf:about="http://www.w3.org/2006/time#year">
        <rdfs:domain rdf:resource="http://www.w3.org/2006/time#GeneralDateTimeDescription"/>
        <rdfs:comment xml:lang="es">Posición de año en un sistema calendario-reloj.

l rango de esta propiedad no está especificado, por tanto, se puede reemplazar por cualquier representación específica de un año de calendario de un calendario cualquiera.</rdfs:comment>
        <rdfs:comment xml:lang="en">Year position in a calendar-clock system.

The range of this property is not specified, so can be replaced by any specific representation of a calendar year from any calendar. </rdfs:comment>
        <rdfs:label xml:lang="en">year</rdfs:label>
    </owl:DatatypeProperty>
    


    <!-- http://www.w3.org/2006/time#years -->

    <owl:DatatypeProperty rdf:about="http://www.w3.org/2006/time#years">
        <rdfs:domain rdf:resource="http://www.w3.org/2006/time#GeneralDurationDescription"/>
        <rdfs:range rdf:resource="http://www.w3.org/2001/XMLSchema#decimal"/>
        <rdfs:comment xml:lang="es">Longitud de, o elemento de la longitud de, una extensión temporal expresada en años.</rdfs:comment>
        <rdfs:comment xml:lang="en">length of, or element of the length of, a temporal extent expressed in years</rdfs:comment>
        <rdfs:label xml:lang="es">duración en años</rdfs:label>
        <rdfs:label xml:lang="en">years duration</rdfs:label>
    </owl:DatatypeProperty>
    


    <!-- 
    ///////////////////////////////////////////////////////////////////////////////////////
    //
    // Classes
    //
    ///////////////////////////////////////////////////////////////////////////////////////
     -->

    


    <!-- http://purl.org/nemo/gufo#AbstractEntity -->

    <owl:Class rdf:about="http://purl.org/nemo/gufo#AbstractEntity">
        <rdfs:subClassOf rdf:resource="http://purl.org/nemo/gufo#Entity"/>
        <owl:disjointWith rdf:resource="http://purl.org/nemo/gufo#ConcreteEntity"/>
        <rdfs:comment xml:lang="en">A gufo:Individual that does not exist in space-time in the same way as a gufo:ConcreteIndividual does. A gufo:AbstractIndividual has no spatiotemporal qualities in its own right. Hence, it does not make sense to ask how much space it now occupies (Gideon, 2018) and when it was created or destroyed.

Examples include the number ten, the null set, and the proposition that &apos;Obama was the president of the United States&apos;.

Rosen, Gideon, &quot;Abstract Objects&quot;, The Stanford Encyclopedia of Philosophy (Winter 2018 Edition), Edward N. Zalta (ed.), &lt;https://plato.stanford.edu/archives/win2018/entries/abstract-objects/&gt;</rdfs:comment>
        <rdfs:label xml:lang="en">AbstractIndividual</rdfs:label>
    </owl:Class>
    


    <!-- http://purl.org/nemo/gufo#AbstractEntityType -->

    <owl:Class rdf:about="http://purl.org/nemo/gufo#AbstractEntityType">
        <rdfs:subClassOf rdf:resource="http://purl.org/nemo/gufo#Type"/>
        <owl:disjointWith rdf:resource="http://purl.org/nemo/gufo#ConcreteEntityType"/>
        <owl:disjointWith rdf:resource="http://purl.org/nemo/gufo#RelationshipType"/>
        <rdfs:comment xml:lang="en">A gufo:Type whose instances are abstract individuals.

Instances of gufo:AbstractIndividualType are subclasses of gufo:AbstractIndividual.

Examples include the types &quot;NaturalNumber&quot;, &quot;Set&quot;, &quot;Proposition&quot;.</rdfs:comment>
        <rdfs:label xml:lang="en">AbstractIndividualType</rdfs:label>
    </owl:Class>
    


    <!-- http://purl.org/nemo/gufo#AntiRigidType -->

    <owl:Class rdf:about="http://purl.org/nemo/gufo#AntiRigidType">
        <rdfs:subClassOf rdf:resource="http://purl.org/nemo/gufo#NonRigidType"/>
        <owl:disjointWith rdf:resource="http://purl.org/nemo/gufo#SemiRigidType"/>
        <rdfs:comment xml:lang="en">A gufo:NonRigidType that applies contingently to all its instances (see Guizzardi, 2005, chapter 4).

Examples include the gufo:Phase &quot;Child&quot;, the gufo:PhaseMixin &quot;InfantAnimal&quot;, the gufo:Role &quot;Student&quot;, and the gufo:RoleMixin &quot;Customer&quot;.</rdfs:comment>
        <rdfs:label xml:lang="en">AntiRigidType</rdfs:label>
    </owl:Class>
    


    <!-- http://purl.org/nemo/gufo#Aspect -->

    <owl:Class rdf:about="http://purl.org/nemo/gufo#Aspect">
        <rdfs:subClassOf rdf:resource="http://purl.org/nemo/gufo#Endurant"/>
        <owl:disjointWith rdf:resource="http://purl.org/nemo/gufo#Object"/>
        <owl:disjointUnionOf rdf:parseType="Collection">
            <rdf:Description rdf:about="http://purl.org/nemo/gufo#ExtrinsicAspect"/>
            <rdf:Description rdf:about="http://purl.org/nemo/gufo#IntrinsicAspect"/>
        </owl:disjointUnionOf>
        <rdfs:comment xml:lang="en">A gufo:Endurant that depends on at least one other concrete individual for its existence. A gufo:Aspect is a characteristic or trait of a concrete individual that is itself conceived as an individual. 

Examples include: intrinsic physical aspects, such as the Moon&apos;s mass, Lassie&apos;s fur color; mental dispositions, such as Bob&apos;s math skills, his belief that the number one is odd; as well as relational aspects, such as John&apos;s love for Mary and the marriage between John and Mary. 

The specific sort of existential dependence connecting aspects to their bearers is called inherence.

Corresponds to &quot;Moment&quot; in Guizzardi (2005). 

Also termed &quot;property instance&quot;, &quot;particularized property&quot;, &quot;individual accident&quot;, or &quot;(variable) trope&quot; in the philosophical literature.</rdfs:comment>
        <rdfs:label xml:lang="en">Aspect</rdfs:label>
    </owl:Class>
    


    <!-- http://purl.org/nemo/gufo#AtomicEvent -->

    <owl:Class rdf:about="http://purl.org/nemo/gufo#AtomicEvent">
        <rdfs:subClassOf rdf:resource="http://purl.org/nemo/gufo#Event"/>
    </owl:Class>
    


    <!-- http://purl.org/nemo/gufo#Category -->

    <owl:Class rdf:about="http://purl.org/nemo/gufo#Category">
        <rdfs:subClassOf rdf:resource="http://purl.org/nemo/gufo#NonSortal"/>
        <rdfs:subClassOf rdf:resource="http://purl.org/nemo/gufo#RigidType"/>
        <rdfs:comment xml:lang="en">A gufo:EndurantType that is both non-sortal and rigid. It captures essential properties that apply to instances of different kinds.

For example, &quot;PhysicalObject&quot; may be considered a gufo:Category, encompassing objects such as cars, planets, trees. &quot;Agent&quot; may be a gufo:Category that classifies both people and organizations.</rdfs:comment>
        <rdfs:label xml:lang="en">Category</rdfs:label>
    </owl:Class>
    


    <!-- http://purl.org/nemo/gufo#Collection -->

    <owl:Class rdf:about="http://purl.org/nemo/gufo#Collection">
        <rdfs:subClassOf rdf:resource="http://purl.org/nemo/gufo#Object"/>
        <owl:disjointUnionOf rdf:parseType="Collection">
            <rdf:Description rdf:about="http://purl.org/nemo/gufo#FixedCollection"/>
            <rdf:Description rdf:about="http://purl.org/nemo/gufo#VariableCollection"/>
        </owl:disjointUnionOf>
        <rdfs:comment xml:lang="en">A complex gufo:Object whose parts (the members of the collection) have a uniform structure (i.e., members are conceived as playing the same role in the collection). Collections may have a fixed or variable membership, which can be asserted using gufo:FixedCollection and gufo:VariableCollection respectively.

Examples include a deck of cards, a pile of bricks, a forest (conceived as a collection of trees), and a group of people.

Collections in many cases constitute a functional complex. For example, a pile of bricks may constitute a wall, a group of people may constitute a football team.

A gufo:Collection may be decomposed into &quot;smaller&quot; collections. For instance, a group of people may be decomposed into a group of English speakers and a group of Italian speakers. Sub collections may or may not share members among them.</rdfs:comment>
        <rdfs:label xml:lang="en">Collection</rdfs:label>
    </owl:Class>
    


    <!-- http://purl.org/nemo/gufo#ComparativeRelationshipType -->

    <owl:Class rdf:about="http://purl.org/nemo/gufo#ComparativeRelationshipType">
        <rdfs:subClassOf rdf:resource="http://purl.org/nemo/gufo#RelationshipType"/>
        <owl:disjointWith rdf:resource="http://purl.org/nemo/gufo#MaterialRelationshipType"/>
        <rdfs:comment xml:lang="en">A gufo:RelationshipType derived from intrinsic aspects of the related entities.

For example, &quot;heavierThan&quot;, &quot;olderThan&quot;. 

For a gufo:ComparativeRelationshipType it is recommended to identify the types of intrinsic aspects from which it is derived (see gufo:isDerivedFrom). For example &quot;heavierThan&quot; is derived from the &quot;Weight&quot; quality type.

Note that, in the case of relationships that may change in different circumstances or times, the use of a qualified relation pattern enables indicating the period of time in which the relationship holds. See gufo:TemporaryRelationshipSituation.

Corresponds to &quot;comparative formal relation&quot; in Guizzardi (2005) and &quot;Comparative Relation&quot; in Fonseca et al. (2019).</rdfs:comment>
        <rdfs:label xml:lang="en">ComparativeRelationshipType</rdfs:label>
        <rdfs:seeAlso rdf:resource="http://purl.org/nemo/gufo#isDerivedFrom"/>
    </owl:Class>
    


    <!-- http://purl.org/nemo/gufo#ComplexEvent -->

    <owl:Class rdf:about="http://purl.org/nemo/gufo#ComplexEvent">
        <rdfs:subClassOf rdf:resource="http://purl.org/nemo/gufo#Event"/>
    </owl:Class>
    


    <!-- http://purl.org/nemo/gufo#ConcreteEntity -->

    <owl:Class rdf:about="http://purl.org/nemo/gufo#ConcreteEntity">
        <rdfs:subClassOf rdf:resource="http://purl.org/nemo/gufo#Entity"/>
        <owl:disjointUnionOf rdf:parseType="Collection">
            <rdf:Description rdf:about="http://purl.org/nemo/gufo#Endurant"/>
            <rdf:Description rdf:about="http://purl.org/nemo/gufo#Event"/>
            <rdf:Description rdf:about="http://purl.org/nemo/gufo#Situation"/>
        </owl:disjointUnionOf>
        <rdfs:comment xml:lang="en">A gufo:Individual that exists in space-time. 

Concrete individuals comprise not only object-like entities (a car, a mountain, a person, a marriage, a belief), but also events (a business meeting, a soccer match) and situations (the situation in which a person weighs 80 kilograms, the situation in which a bank account is overdrawn).</rdfs:comment>
        <rdfs:label xml:lang="en">ConcreteIndividual</rdfs:label>
    </owl:Class>
    


    <!-- http://purl.org/nemo/gufo#ConcreteEntityType -->

    <owl:Class rdf:about="http://purl.org/nemo/gufo#ConcreteEntityType">
        <rdfs:subClassOf rdf:resource="http://purl.org/nemo/gufo#Type"/>
        <owl:disjointWith rdf:resource="http://purl.org/nemo/gufo#RelationshipType"/>
        <rdfs:comment xml:lang="en">A gufo:Type whose instances are concrete individuals.

Instances of gufo:ConcreteIndividualType are subclasses of gufo:ConcreteIndividual.

Examples include the gufo:Kind &quot;Person&quot;, the gufo:Category &quot;Physical Object&quot;, the gufo:EventType &quot;Business Meeting&quot;.</rdfs:comment>
        <rdfs:label xml:lang="en">ConcreteIndividualType</rdfs:label>
    </owl:Class>
    


    <!-- http://purl.org/nemo/gufo#Endurant -->

    <owl:Class rdf:about="http://purl.org/nemo/gufo#Endurant">
        <rdfs:subClassOf rdf:resource="http://purl.org/nemo/gufo#ConcreteEntity"/>
        <owl:disjointUnionOf rdf:parseType="Collection">
            <rdf:Description rdf:about="http://purl.org/nemo/gufo#Aspect"/>
            <rdf:Description rdf:about="http://purl.org/nemo/gufo#Object"/>
        </owl:disjointUnionOf>
        <rdfs:comment xml:lang="en">A gufo:ConcreteIndividual that endures in time and may change qualitatively while keeping its identity. 

Examples include: ordinary objects of everyday experience, such as a person, a house, and a car; reified relationships, such as a marriage, a rental contract, and a person&apos;s love for another; and existentially-dependent aspects of objects, such as a car&apos;s weight, a person&apos;s language skills, and a house&apos;s color. 

Also termed &quot;continuant&quot; in the philosophical literature.</rdfs:comment>
        <rdfs:label xml:lang="en">Endurant</rdfs:label>
    </owl:Class>
    


    <!-- http://purl.org/nemo/gufo#EndurantType -->

    <owl:Class rdf:about="http://purl.org/nemo/gufo#EndurantType">
        <rdfs:subClassOf rdf:resource="http://purl.org/nemo/gufo#ConcreteEntityType"/>
        <owl:disjointWith rdf:resource="http://purl.org/nemo/gufo#EventType"/>
        <owl:disjointWith rdf:resource="http://purl.org/nemo/gufo#SituationType"/>
        <owl:disjointUnionOf rdf:parseType="Collection">
            <rdf:Description rdf:about="http://purl.org/nemo/gufo#NonRigidType"/>
            <rdf:Description rdf:about="http://purl.org/nemo/gufo#RigidType"/>
        </owl:disjointUnionOf>
        <owl:disjointUnionOf rdf:parseType="Collection">
            <rdf:Description rdf:about="http://purl.org/nemo/gufo#NonSortal"/>
            <rdf:Description rdf:about="http://purl.org/nemo/gufo#Sortal"/>
        </owl:disjointUnionOf>
        <rdfs:comment xml:lang="en">A gufo:Type whose instances are endurants. 

Instances of gufo:EndurantType are subclasses of gufo:Endurant.

Examples include the object kind &quot;Person&quot;, the phase &quot;Child&quot;, the relator kind &quot;Marriage&quot;.

See Guizzardi et al. (2018) for details concerning the taxonomy of endurant types included here.</rdfs:comment>
        <rdfs:label xml:lang="en">EndurantType</rdfs:label>
    </owl:Class>
    


    <!-- http://purl.org/nemo/gufo#Entity -->

    <owl:Class rdf:about="http://purl.org/nemo/gufo#Entity">
        <owl:disjointWith rdf:resource="http://purl.org/nemo/gufo#Type"/>
        <owl:disjointUnionOf rdf:parseType="Collection">
            <rdf:Description rdf:about="http://purl.org/nemo/gufo#AbstractEntity"/>
            <rdf:Description rdf:about="http://purl.org/nemo/gufo#ConcreteEntity"/>
        </owl:disjointUnionOf>
        <rdfs:comment xml:lang="en">An entity that (unlike a gufo:Type) cannot be instantiated.

Individuals may be either concrete (e.g., the Earth, Mick Jagger, Brazil, the 1985 Mexico City Earthquake) or abstract (e.g., the number two, the proposition that &apos;three is a prime number&apos;).

Also known as &quot;particular&quot; in the philosophical literature.</rdfs:comment>
        <rdfs:label xml:lang="en">Individual</rdfs:label>
    </owl:Class>
    


    <!-- http://purl.org/nemo/gufo#Event -->

    <owl:Class rdf:about="http://purl.org/nemo/gufo#Event">
        <rdfs:subClassOf rdf:resource="http://purl.org/nemo/gufo#Perdurants"/>
        <rdfs:comment xml:lang="en">A gufo:ConcreteIndividual that &apos;occurs&apos; or &apos;happens&apos; in time. They may be instantaneous or long-running. Events are those &quot;things that happen to or are performed by&quot; (Casati and Varzi, 2015) endurants. 

Examples include actions and processes, such as a business meeting, a communicative act, a soccer match, a goal kick, the clicking of a mouse button; as well as natural occurrences such as an earthquake, the fall of the meteor that caused the extinction of the dinosaurs.

Also termed &quot;happening&quot;, &quot;occurrence&quot;, &quot;perdurant&quot; or &quot;occurrent&quot; in the philosophical literature.

Casati, R. &amp; Varzi, A. (2015). Events. In E.N. Zalta (Ed.), The Stanford Encyclopedia of Philosophy (Winter 2015 ed.). 19 Metaphysics Research Lab, Stanford University. https://plato.stanford.edu/archives/win2015/entries/events/</rdfs:comment>
        <rdfs:label xml:lang="en">Event</rdfs:label>
        <rdfs:seeAlso rdf:resource="http://purl.org/nemo/gufo#participatedIn"/>
    </owl:Class>
    


    <!-- http://purl.org/nemo/gufo#EventType -->

    <owl:Class rdf:about="http://purl.org/nemo/gufo#EventType">
        <rdfs:subClassOf rdf:resource="http://purl.org/nemo/gufo#PerdurantType"/>
        <owl:disjointWith rdf:resource="http://purl.org/nemo/gufo#SituationType"/>
        <rdfs:comment xml:lang="en">A gufo:Type whose instances are events.

Instances of gufo:EventType are subclasses of gufo:Event.

Examples include &quot;Business Meeting&quot;, &quot;Birth&quot;, &quot;Musical Performance&quot;.</rdfs:comment>
        <rdfs:label xml:lang="en">EventType</rdfs:label>
    </owl:Class>
    


    <!-- http://purl.org/nemo/gufo#ExtrinsicAspect -->

    <owl:Class rdf:about="http://purl.org/nemo/gufo#ExtrinsicAspect">
        <rdfs:subClassOf rdf:resource="http://purl.org/nemo/gufo#Aspect"/>
        <owl:disjointWith rdf:resource="http://purl.org/nemo/gufo#IntrinsicAspect"/>
        <owl:disjointUnionOf rdf:parseType="Collection">
            <rdf:Description rdf:about="http://purl.org/nemo/gufo#ExtrinsicMode"/>
            <rdf:Description rdf:about="http://purl.org/nemo/gufo#Relator"/>
        </owl:disjointUnionOf>
        <rdfs:comment xml:lang="en">A gufo:Aspect that depends on one or more concrete individuals.

Extrinsic (or &quot;relational&quot;) aspects are reified relationships, e.g., John and Mary&apos;s marriage, Mary&apos;s employment contract at Nasa, or parts of those relationships, e.g., John&apos;s obligations towards Mary in the scope of the marriage, Mary&apos;s reciprocal claims, Mary&apos;s obligations towards John, John&apos;s reciprocal claims. Extrinsic aspects can also be reified one-sided relationships, e.g., John&apos;s admiration for Obama (which depends on Obama but does not characterize him).

Corresponds to &quot;Extrinsic Moment&quot; in Fonseca et al (2019). Encompasses &quot;Externally Depedent Mode&quot;, &quot;Qua Individual&quot; and &quot;Relator&quot; in Guizzardi (2005).</rdfs:comment>
        <rdfs:label xml:lang="en">ExtrinsicAspect</rdfs:label>
    </owl:Class>
    


    <!-- http://purl.org/nemo/gufo#ExtrinsicMode -->

    <owl:Class rdf:about="http://purl.org/nemo/gufo#ExtrinsicMode">
        <rdfs:subClassOf rdf:resource="http://purl.org/nemo/gufo#ExtrinsicAspect"/>
        <rdfs:subClassOf>
            <owl:Restriction>
                <owl:onProperty rdf:resource="http://purl.org/nemo/gufo#externallyDependsOn"/>
                <owl:someValuesFrom rdf:resource="http://purl.org/nemo/gufo#ConcreteEntity"/>
            </owl:Restriction>
        </rdfs:subClassOf>
        <rdfs:subClassOf>
            <owl:Restriction>
                <owl:onProperty rdf:resource="http://purl.org/nemo/gufo#inheresIn"/>
                <owl:qualifiedCardinality rdf:datatype="http://www.w3.org/2001/XMLSchema#nonNegativeInteger">1</owl:qualifiedCardinality>
                <owl:onClass rdf:resource="http://purl.org/nemo/gufo#ConcreteEntity"/>
            </owl:Restriction>
        </rdfs:subClassOf>
        <owl:disjointWith rdf:resource="http://purl.org/nemo/gufo#Relator"/>
        <rdfs:comment xml:lang="en">A gufo:ExtrinsicAspect that inheres in a concrete individual and depends on others for its existence.

A gufo:ExtrinsicMode can be understood as a reified one-sided relationship, such as John&apos;s admiration for Mary.

Corresponds to &quot;Extrinsic Moment&quot; in Fonseca et al (2019). Encompasses what &quot;Externally Dependent Mode&quot;, &quot;Qua Individual&quot; and &quot;Relator&quot; in Guizzardi (2005).</rdfs:comment>
        <rdfs:label xml:lang="en">ExtrinsicMode</rdfs:label>
        <rdfs:seeAlso rdf:resource="http://purl.org/nemo/gufo#externallyDependsOn"/>
        <rdfs:seeAlso rdf:resource="http://purl.org/nemo/gufo#inheresIn"/>
    </owl:Class>
    


    <!-- http://purl.org/nemo/gufo#FixedCollection -->

    <owl:Class rdf:about="http://purl.org/nemo/gufo#FixedCollection">
        <rdfs:subClassOf rdf:resource="http://purl.org/nemo/gufo#Collection"/>
        <owl:disjointWith rdf:resource="http://purl.org/nemo/gufo#VariableCollection"/>
        <rdfs:comment xml:lang="en">A gufo:Collection for which no change in membership is possible.

Such a collection obeys an extensional principle of identity, i.e., two fixed collections are the same if, and only if, they have the same members.

Consider, for example, a group of people understood as a gufo:FixedCollection. In this case, any change in the membership of the group (e.g., the addition of one person) would in fact create a different group of people. In this case, the gufo:FixedCollection may be contrasted with the complexes they constitute. For instance, The Beatles (the band conceived as a gufo:FunctionalComplex) was in a certain circumstance constituted by the collection {John, Paul, George, Pete} and in another one constituted by the collection {John, Paul, George, Ringo}. The replacement of Pete Best by Ringo Star does not alter the identity of the band, but creates a  different group of people.</rdfs:comment>
        <rdfs:label xml:lang="en">FixedCollection</rdfs:label>
        <rdfs:seeAlso rdf:resource="http://purl.org/nemo/gufo#isCollectionMemberOf"/>
        <rdfs:seeAlso rdf:resource="http://purl.org/nemo/gufo#isSubCollectionOf"/>
    </owl:Class>
    


    <!-- http://purl.org/nemo/gufo#FunctionalComplex -->

    <owl:Class rdf:about="http://purl.org/nemo/gufo#FunctionalComplex">
        <rdfs:subClassOf rdf:resource="http://purl.org/nemo/gufo#Object"/>
        <rdfs:comment rdf:resource="http://purl.org/nemo/gufo#isComponentOf"/>
        <rdfs:comment xml:lang="en">A complex gufo:Object whose parts (components) play different roles in its composition. 

For example, a person could be considered a gufo:FunctionalComplex with the various organs (heart, brain, lungs, etc.) playing different roles. Another example is a scrum team, which is composed by people playing the roles of scrum master, product owner, developer, etc.

To explicitly capture temporary components, use gufo:TemporaryParthoodSituation.</rdfs:comment>
        <rdfs:label xml:lang="en">FunctionalComplex</rdfs:label>
        <rdfs:seeAlso rdf:resource="http://purl.org/nemo/gufo#TemporaryParthoodSituation"/>
    </owl:Class>
    


    <!-- http://purl.org/nemo/gufo#History -->

    <owl:Class rdf:about="http://purl.org/nemo/gufo#History">
        <rdfs:subClassOf rdf:resource="http://purl.org/nemo/gufo#Perdurants"/>
    </owl:Class>
    


    <!-- http://purl.org/nemo/gufo#IntrinsicAspect -->

    <owl:Class rdf:about="http://purl.org/nemo/gufo#IntrinsicAspect">
        <rdfs:subClassOf rdf:resource="http://purl.org/nemo/gufo#Aspect"/>
        <rdfs:subClassOf>
            <owl:Restriction>
                <owl:onProperty rdf:resource="http://purl.org/nemo/gufo#inheresIn"/>
                <owl:qualifiedCardinality rdf:datatype="http://www.w3.org/2001/XMLSchema#nonNegativeInteger">1</owl:qualifiedCardinality>
                <owl:onClass rdf:resource="http://purl.org/nemo/gufo#ConcreteEntity"/>
            </owl:Restriction>
        </rdfs:subClassOf>
        <owl:disjointUnionOf rdf:parseType="Collection">
            <rdf:Description rdf:about="http://purl.org/nemo/gufo#IntrinsicMode"/>
            <rdf:Description rdf:about="http://purl.org/nemo/gufo#Quality"/>
        </owl:disjointUnionOf>
        <rdfs:comment xml:lang="en">A gufo:Aspect that depends on a single concrete individual in which it inheres. 

Examples include intrinsic physical aspects, such as the Moon&apos;s mass, Lassie&apos;s fur color; the fragility of John Lennon&apos;s glasses; mental dispositions, such as Bob&apos;s math skills, his belief that the number one is odd.

A gufo:IntrinsicAspect is classified as a gufo:Quality (e.g., an apple&apos;s weight, the height of the Statue of Liberty) if it is measurable by a certain value space, or as a gufo:IntrinsicMode (e.g. Bob&apos;s belief that the Eiffel Tower is in Paris) otherwise.

Corresponds to &quot;Instrinsic Moment&quot; in Guizzardi (2005). Different from Guizzardi (2005), here we consider that aspects can inhere in concrete individuals in general, and not only in endurants.</rdfs:comment>
        <rdfs:label xml:lang="en">IntrinsicAspect</rdfs:label>
        <rdfs:seeAlso rdf:resource="http://purl.org/nemo/gufo#inheresIn"/>
    </owl:Class>
    


    <!-- http://purl.org/nemo/gufo#IntrinsicMode -->

    <owl:Class rdf:about="http://purl.org/nemo/gufo#IntrinsicMode">
        <rdfs:subClassOf rdf:resource="http://purl.org/nemo/gufo#IntrinsicAspect"/>
        <owl:disjointWith rdf:resource="http://purl.org/nemo/gufo#Quality"/>
        <rdfs:comment xml:lang="en">A gufo:IntrinsicAspect that is not measurable.

For example, Bob&apos;s belief that the Eiffel Tower is in Paris, his math skills, his headache.

Corresponds to &quot;Mode&quot; in Guizzardi (2005).</rdfs:comment>
        <rdfs:label xml:lang="en">IntrinsicMode</rdfs:label>
    </owl:Class>
    


    <!-- http://purl.org/nemo/gufo#Kind -->

    <owl:Class rdf:about="http://purl.org/nemo/gufo#Kind">
        <rdfs:subClassOf rdf:resource="http://purl.org/nemo/gufo#RigidType"/>
        <rdfs:subClassOf rdf:resource="http://purl.org/nemo/gufo#Sortal"/>
        <owl:disjointWith rdf:resource="http://purl.org/nemo/gufo#SubKind"/>
        <rdfs:comment xml:lang="en">A gufo:EndurantType that is both sortal and rigid. It provides a uniform principle of identity for its instances. Every gufo:Endurant instantiates one and only one gufo:Kind. 

Examples include kinds of ordinary objects of everyday experience, such as: &quot;Person&quot;, &quot;House&quot;, &quot;Car&quot;; kinds of relators, such as &quot;Marriage&quot;, &quot;RentalContract&quot;; kinds of existentially-dependent aspects of objects, such as &quot;Weight&quot;, &quot;Belief&quot;, &quot;Vulnerability&quot;.</rdfs:comment>
        <rdfs:label xml:lang="en">Kind</rdfs:label>
    </owl:Class>
    


    <!-- http://purl.org/nemo/gufo#MaterialRelationshipType -->

    <owl:Class rdf:about="http://purl.org/nemo/gufo#MaterialRelationshipType">
        <rdfs:subClassOf rdf:resource="http://purl.org/nemo/gufo#RelationshipType"/>
        <rdfs:comment xml:lang="en">A gufo:RelationshipType derived from extrinsic aspects of the related entities.

For example, &quot;marriedWith&quot;, &quot;employedBy&quot;, &quot;enrolledIn&quot;, &quot;admires&quot;. 

For a gufo:MaterialRelationshipType it is recommended to identify the type of extrinsic aspect from which the material relationship type is derived (see gufo:isDerivedFrom). For example &quot;marriedWith&quot; can be derived from the &quot;Marriage&quot; relator type, &quot;employedBy&quot; can be derived from the &quot;Employment&quot; relator type.

Encompasses &quot;Material Relation&quot; in Guizzardi (2005) and corresponds to &quot;Material Relation&quot; in Fonseca et al. (2019).</rdfs:comment>
        <rdfs:label xml:lang="en">MaterialRelationshipType</rdfs:label>
        <rdfs:seeAlso rdf:resource="http://purl.org/nemo/gufo#isDerivedFrom"/>
    </owl:Class>
    


    <!-- http://purl.org/nemo/gufo#Mixin -->

    <owl:Class rdf:about="http://purl.org/nemo/gufo#Mixin">
        <rdfs:subClassOf rdf:resource="http://purl.org/nemo/gufo#NonSortal"/>
        <rdfs:subClassOf rdf:resource="http://purl.org/nemo/gufo#SemiRigidType"/>
        <rdfs:comment xml:lang="en">A gufo:EndurantType that is both non-sortal and semi-rigid. As a semi-rigid type, it applies necessarily to some of its instances and contingently to some others. As a non-sortal, it captures properties shared by instances of different kinds.

For example, the type &quot;FemaleAnimal&quot; may be considered a gufo:Mixin as it applies necessarily to animals of certain species, e.g., lions and sharks, while it applies contingently to animals of other species such as clownfish and mushroom corals (which may change sex given certain conditions).</rdfs:comment>
        <rdfs:label xml:lang="en">Mixin</rdfs:label>
    </owl:Class>
    


    <!-- http://purl.org/nemo/gufo#NonRigidType -->

    <owl:Class rdf:about="http://purl.org/nemo/gufo#NonRigidType">
        <rdfs:subClassOf rdf:resource="http://purl.org/nemo/gufo#EndurantType"/>
        <owl:disjointWith rdf:resource="http://purl.org/nemo/gufo#RigidType"/>
        <owl:disjointUnionOf rdf:parseType="Collection">
            <rdf:Description rdf:about="http://purl.org/nemo/gufo#AntiRigidType"/>
            <rdf:Description rdf:about="http://purl.org/nemo/gufo#SemiRigidType"/>
        </owl:disjointUnionOf>
        <rdfs:comment xml:lang="en">A gufo:EndurantType that does not apply necessarily to at least one of its instances (see Guizzardi, 2005, chapter 4).

Examples include anti-rigid types, such as the role &quot;Student&quot; and the phase &quot;Child&quot;, and semi-rigid types, such as the mixin &quot;MusicalArtist&quot; (which necessarily characterizes bands, but contingently characterizes people) and the mixin &quot;FemaleAnimal&quot; (which is necessarily characterizes female dogs, but contigently characterizes clownfish).</rdfs:comment>
        <rdfs:label xml:lang="en">NonRigidType</rdfs:label>
    </owl:Class>
    


    <!-- http://purl.org/nemo/gufo#NonSortal -->

    <owl:Class rdf:about="http://purl.org/nemo/gufo#NonSortal">
        <rdfs:subClassOf rdf:resource="http://purl.org/nemo/gufo#EndurantType"/>
        <owl:disjointWith rdf:resource="http://purl.org/nemo/gufo#Sortal"/>
        <rdfs:comment xml:lang="en">A gufo:EndurantType that applies to individuals of different kinds (see Guizzardi, 2005, chapter 4).

Non-sortals do not provide a uniform principle of identity for their instances; instead, they just classify things that share common properties but which obey different principles of identity.

Also termed &quot;dispersive&quot; types in the philosophical literature.</rdfs:comment>
        <rdfs:label xml:lang="en">NonSortal</rdfs:label>
    </owl:Class>
    


    <!-- http://purl.org/nemo/gufo#Object -->

    <owl:Class rdf:about="http://purl.org/nemo/gufo#Object">
        <rdfs:subClassOf rdf:resource="http://purl.org/nemo/gufo#Endurant"/>
        <rdfs:comment xml:lang="en">A gufo:Endurant that does not depend on another endurant for its existence (excluding its essential parts and aspects). 

Examples of objects include ordinary physical entities, such as a dog, a house, a tomato, a car, Alan Turing, but also socially-defined entities such as The Rolling Stones, the European Union, the Brazilian 1988 Constitution.

Guizzardi (2005) also included the more abstract notion of &quot;Substantial&quot;, which generalizes both objects and amounts of matter. That notion was left out from this implementation, together with the notion of amount of matter. Support for the representation of maximally-self-connected amounts of matter is given by gufo:Quantity.</rdfs:comment>
        <rdfs:label xml:lang="en">Object</rdfs:label>
    </owl:Class>
    


    <!-- http://purl.org/nemo/gufo#Participation -->

    <owl:Class rdf:about="http://purl.org/nemo/gufo#Participation">
        <rdfs:subClassOf rdf:resource="http://purl.org/nemo/gufo#Event"/>
        <rdfs:subClassOf>
            <owl:Restriction>
                <owl:onProperty>
                    <rdf:Description>
                        <owl:inverseOf rdf:resource="http://purl.org/nemo/gufo#participatedIn"/>
                    </rdf:Description>
                </owl:onProperty>
                <owl:qualifiedCardinality rdf:datatype="http://www.w3.org/2001/XMLSchema#nonNegativeInteger">1</owl:qualifiedCardinality>
                <owl:onClass rdf:resource="http://purl.org/nemo/gufo#Object"/>
            </owl:Restriction>
        </rdfs:subClassOf>
        <rdfs:comment xml:lang="en">A gufo:Event that depends on a single object. 

Participations can be used to partition an event into portions, each of which depend exclusively on a single object. Consider a business meeting with multiple participants, including John and Mary. John&apos;s participation in the meeting encompasses all events that are part of the meeting and that depend solely on him. Likewise, Mary&apos;s participation encompasses all events that are part of the meeting and that depend solely on her. Similarly, in Brutus’ stabbing of Caesar, we may identify the participations of Brutus, of Caesar, and of the dagger.</rdfs:comment>
        <rdfs:label xml:lang="en">Participation</rdfs:label>
        <rdfs:seeAlso rdf:resource="http://purl.org/nemo/gufo#participatedIn"/>
    </owl:Class>
    


    <!-- http://purl.org/nemo/gufo#PerdurantType -->

    <owl:Class rdf:about="http://purl.org/nemo/gufo#PerdurantType">
        <rdfs:subClassOf rdf:resource="http://purl.org/nemo/gufo#ConcreteEntityType"/>
    </owl:Class>
    


    <!-- http://purl.org/nemo/gufo#Perdurants -->

    <owl:Class rdf:about="http://purl.org/nemo/gufo#Perdurants">
        <rdfs:subClassOf rdf:resource="http://purl.org/nemo/gufo#ConcreteEntity"/>
    </owl:Class>
    


    <!-- http://purl.org/nemo/gufo#Phase -->

    <owl:Class rdf:about="http://purl.org/nemo/gufo#Phase">
        <rdfs:subClassOf rdf:resource="http://purl.org/nemo/gufo#AntiRigidType"/>
        <rdfs:subClassOf rdf:resource="http://purl.org/nemo/gufo#Sortal"/>
        <owl:disjointWith rdf:resource="http://purl.org/nemo/gufo#Role"/>
        <rdfs:comment xml:lang="en">A gufo:EndurantType that is both sortal and anti-rigid. It is defined by instrinsic but contingent instantiation conditions. Phases are relationally independent types that capturec instrinsic properties shared by instances of a given kind.

For example, &quot;Child&quot; may be considered a gufo:Phase as a subclass of the gufo:Kind &quot;Person&quot;, instantiated by persons younger than 12. Another example is the type &quot;IllPerson&quot;, which may be considered a gufo:Phase that is instantiated whenever an instance of &quot;Disease&quot; (a gufo:IntrinsicMode) inheres in a person.</rdfs:comment>
        <rdfs:label xml:lang="en">Phase</rdfs:label>
    </owl:Class>
    


    <!-- http://purl.org/nemo/gufo#PhaseMixin -->

    <owl:Class rdf:about="http://purl.org/nemo/gufo#PhaseMixin">
        <rdfs:subClassOf rdf:resource="http://purl.org/nemo/gufo#AntiRigidType"/>
        <rdfs:subClassOf rdf:resource="http://purl.org/nemo/gufo#NonSortal"/>
        <owl:disjointWith rdf:resource="http://purl.org/nemo/gufo#RoleMixin"/>
        <rdfs:comment xml:lang="en">A gufo:EndurantType that is both non-sortal and anti-rigid. It is defined by instrinsic but contingent instantiation conditions. Phase mixins are relationally independent types that capture instrinsic properties shared by instances of different kinds.

For example, &quot;LivingAnimal&quot; may be considered a gufo:PhaseMixin as a superclass of the phases &quot;LivingPerson&quot; (specializing the gufo:Kind &quot;Person&quot;) and &quot;LivingDog&quot; (specializing the gufo:Kind &quot;Dog&quot;).</rdfs:comment>
        <rdfs:label xml:lang="en">PhaseMixin</rdfs:label>
    </owl:Class>
    


    <!-- http://purl.org/nemo/gufo#Quality -->

    <owl:Class rdf:about="http://purl.org/nemo/gufo#Quality">
        <rdfs:subClassOf rdf:resource="http://purl.org/nemo/gufo#IntrinsicAspect"/>
        <rdfs:comment xml:lang="en">A gufo:IntrinsicAspect that is measurable by some value spaces. A quality may be used to compare individuals, on the basis of the value it takes in a certain quality space (for instance, a position within the RGB spectrum).

Examples include the weight of a person, the name of organization, the color of a car, and the duration of a concert.</rdfs:comment>
        <rdfs:label xml:lang="en">Quality</rdfs:label>
    </owl:Class>
    


    <!-- http://purl.org/nemo/gufo#QualityValue -->

    <owl:Class rdf:about="http://purl.org/nemo/gufo#QualityValue">
        <rdfs:subClassOf rdf:resource="http://purl.org/nemo/gufo#AbstractEntity"/>
        <rdfs:comment xml:lang="en">A gufo:AbstractIndividual that can be associated with a gufo:Quality reflecting the perception or conception of the quality in a certain value space. 

Instances of gufo:QualityValue include the rational number 2.5 when used to conceive of the acidity of a portion of wine (in a pH scale), the tuple &lt;38.8897,-77.0089&gt; when used to conceive of the location of a building (in a space formed by latitude and longitude), or the triplet &lt;0,0,0&gt; when used to conceive of the color of a physical object (in a trimensional space formed by red, green and blue color components).  

Corresponds to &quot;Quale&quot; in Guizzardi (2005). 

Use this class only for quality values (qualia) that are to be reified in the A-box and associated with a gufo:ConcreteIndividual through the object property gufo:hasReifiedQualityValue. Otherwise, use the gufo:hasQualityValue data property and a literal to determine the quality value.</rdfs:comment>
        <rdfs:label xml:lang="en">QualityValue</rdfs:label>
        <rdfs:seeAlso rdf:resource="http://purl.org/nemo/gufo#hasReifiedQualityValue"/>
    </owl:Class>
    


    <!-- http://purl.org/nemo/gufo#QualityValueAttributionSituation -->

    <owl:Class rdf:about="http://purl.org/nemo/gufo#QualityValueAttributionSituation">
        <rdfs:subClassOf rdf:resource="http://purl.org/nemo/gufo#Situation"/>
        <rdfs:subClassOf>
            <owl:Class>
                <owl:unionOf rdf:parseType="Collection">
                    <owl:Restriction>
                        <owl:onProperty rdf:resource="http://purl.org/nemo/gufo#concernsReifiedQualityValue"/>
                        <owl:qualifiedCardinality rdf:datatype="http://www.w3.org/2001/XMLSchema#nonNegativeInteger">1</owl:qualifiedCardinality>
                        <owl:onClass rdf:resource="http://purl.org/nemo/gufo#QualityValue"/>
                    </owl:Restriction>
                    <owl:Restriction>
                        <owl:onProperty rdf:resource="http://purl.org/nemo/gufo#concernsQualityValue"/>
                        <owl:cardinality rdf:datatype="http://www.w3.org/2001/XMLSchema#nonNegativeInteger">1</owl:cardinality>
                    </owl:Restriction>
                </owl:unionOf>
            </owl:Class>
        </rdfs:subClassOf>
        <rdfs:subClassOf>
            <owl:Restriction>
                <owl:onProperty rdf:resource="http://purl.org/nemo/gufo#concernsQualityType"/>
                <owl:qualifiedCardinality rdf:datatype="http://www.w3.org/2001/XMLSchema#nonNegativeInteger">1</owl:qualifiedCardinality>
                <owl:onClass rdf:resource="http://purl.org/nemo/gufo#EndurantType"/>
            </owl:Restriction>
        </rdfs:subClassOf>
        <rdfs:subClassOf>
            <owl:Restriction>
                <owl:onProperty>
                    <rdf:Description>
                        <owl:inverseOf rdf:resource="http://purl.org/nemo/gufo#standsInQualifiedAttribution"/>
                    </rdf:Description>
                </owl:onProperty>
                <owl:qualifiedCardinality rdf:datatype="http://www.w3.org/2001/XMLSchema#nonNegativeInteger">1</owl:qualifiedCardinality>
                <owl:onClass rdf:resource="http://purl.org/nemo/gufo#Endurant"/>
            </owl:Restriction>
        </rdfs:subClassOf>
        <owl:disjointWith rdf:resource="http://purl.org/nemo/gufo#TemporaryConstitutionSituation"/>
        <owl:disjointWith rdf:resource="http://purl.org/nemo/gufo#TemporaryInstantiationSituation"/>
        <owl:disjointWith rdf:resource="http://purl.org/nemo/gufo#TemporaryParthoodSituation"/>
        <owl:disjointWith rdf:resource="http://purl.org/nemo/gufo#TemporaryRelationshipSituation"/>
        <rdfs:comment xml:lang="en">A gufo:Situation in which a quality value is temporarily attributed to a gufo:Endurant.

A gufo:QualityValueAttributionSituation should be used only for mutable qualities, i.e. those whose value can vary in time.

Examples include: the situation in which the value of a bitcoin in Euros is 6.526,12, which lasted from 10/12/2019 to 11/12/2019; the situation in which the weight of Mike Tyson was 100 kg; and the situation in which the color of Einstein&apos; hair was grey.

This is a reification of the quality value attribution (in a solution that is similar to the qualified relation pattern  http://patterns.dataincubator.org/book/qualified-relation.html )</rdfs:comment>
        <rdfs:label xml:lang="en">QualityValueAttributionSituation</rdfs:label>
        <rdfs:seeAlso rdf:resource="http://purl.org/nemo/gufo#concernsQualityValue"/>
        <rdfs:seeAlso rdf:resource="http://purl.org/nemo/gufo#concernsReifiedQualityValue"/>
    </owl:Class>
    


    <!-- http://purl.org/nemo/gufo#Quantity -->

    <owl:Class rdf:about="http://purl.org/nemo/gufo#Quantity">
        <rdfs:subClassOf rdf:resource="http://purl.org/nemo/gufo#Object"/>
        <rdfs:comment xml:lang="en">A complex gufo:Object that is a maximally-connected portion of stuff. A gufo:Quantity has a fixed constitution, and thus, removing or adding a sub-quantity would result in a different quantity.

Examples include the portion of wine in a wine tank, a lump of clay, the gold that constitutes a wedding ring.

Also termed &quot;quantity of matter&quot;, &quot;objectified portion of matter&quot;, &quot;piece&quot; in the philosophical literature.</rdfs:comment>
        <rdfs:label xml:lang="en">Quantity</rdfs:label>
        <rdfs:seeAlso rdf:resource="http://purl.org/nemo/gufo#isSubQuantityOf"/>
    </owl:Class>
    


    <!-- http://purl.org/nemo/gufo#RelationshipType -->

    <owl:Class rdf:about="http://purl.org/nemo/gufo#RelationshipType">
        <rdfs:subClassOf rdf:resource="http://purl.org/nemo/gufo#Type"/>
        <rdfs:comment xml:lang="en">A gufo:Type whose instances are ordered pairs of related entities. Instances of gufo:RelationshipType are object properties in UFO-based ontologies.

The object properties &quot;marriedWith&quot; and &quot;enrolledIn&quot; are examples of material relationship types. The object properties &quot;heavierThan&quot;, &quot;olderThan&quot; are examples of comparative relationship types.

The use of gufo:RelationshipType and its subclasses requires OWL 2 punning.

Corresponds to &quot;Relation&quot; in Guizzardi (2005) and Fonseca et al. (2019).</rdfs:comment>
        <rdfs:label xml:lang="en">RelationshipType</rdfs:label>
    </owl:Class>
    


    <!-- http://purl.org/nemo/gufo#Relator -->

    <owl:Class rdf:about="http://purl.org/nemo/gufo#Relator">
        <rdfs:subClassOf rdf:resource="http://purl.org/nemo/gufo#ExtrinsicAspect"/>
        <rdfs:subClassOf>
            <owl:Restriction>
                <owl:onProperty rdf:resource="http://purl.org/nemo/gufo#mediates"/>
                <owl:minQualifiedCardinality rdf:datatype="http://www.w3.org/2001/XMLSchema#nonNegativeInteger">2</owl:minQualifiedCardinality>
                <owl:onClass rdf:resource="http://purl.org/nemo/gufo#Endurant"/>
            </owl:Restriction>
        </rdfs:subClassOf>
        <rdfs:comment xml:lang="en">A gufo:ExtrinsicAspect that connects (involves, mediates) two or more concrete individuals. Relators are reified relationships composed of reciprocal extrinsic modes.

Examples of relators include John and Mary&apos;s marriage (composed of John&apos;s obligations towards Mary in the scope of the marriage, Mary&apos;s reciprocal claims, Mary&apos;s obligations towards John, John&apos;s reciprocal claims), Mary&apos;s employment contract at Nasa, a covalent bond between two atoms.</rdfs:comment>
        <rdfs:label xml:lang="en">Relator</rdfs:label>
        <rdfs:seeAlso rdf:resource="http://purl.org/nemo/gufo#mediates"/>
    </owl:Class>
    


    <!-- http://purl.org/nemo/gufo#RigidType -->

    <owl:Class rdf:about="http://purl.org/nemo/gufo#RigidType">
        <rdfs:subClassOf rdf:resource="http://purl.org/nemo/gufo#EndurantType"/>
        <rdfs:comment xml:lang="en">A gufo:EndurantType which applies necessarily to its instances (see Guizzardi, 2005, chapter 4).

Examples include the types &quot;Agent&quot;, &quot;Person&quot;, &quot;Animal&quot;, &quot;PhysicalObject&quot;, &quot;Car&quot;, and &quot;Tree&quot;.</rdfs:comment>
        <rdfs:label xml:lang="en">RigidType</rdfs:label>
    </owl:Class>
    


    <!-- http://purl.org/nemo/gufo#Role -->

    <owl:Class rdf:about="http://purl.org/nemo/gufo#Role">
        <rdfs:subClassOf rdf:resource="http://purl.org/nemo/gufo#AntiRigidType"/>
        <rdfs:subClassOf rdf:resource="http://purl.org/nemo/gufo#Sortal"/>
        <rdfs:comment xml:lang="en">A gufo:EndurantType that both sortal and anti-rigid. It is defined by relational instantiation conditions. Roles are relationally dependent types, capturing relational properties shared by instances of a given kind.

For example, &quot;Student&quot; may be considered a gufo:Role as a subclass of the gufo:Kind &quot;Person&quot;, instantiated by all persons enrolled in a school. &quot;</rdfs:comment>
        <rdfs:label xml:lang="en">Role</rdfs:label>
    </owl:Class>
    


    <!-- http://purl.org/nemo/gufo#RoleMixin -->

    <owl:Class rdf:about="http://purl.org/nemo/gufo#RoleMixin">
        <rdfs:subClassOf rdf:resource="http://purl.org/nemo/gufo#AntiRigidType"/>
        <rdfs:subClassOf rdf:resource="http://purl.org/nemo/gufo#NonSortal"/>
        <rdfs:comment xml:lang="en">A gufo:EndurantType that is both non-sortal and anti-rigid. It is defined by relational instantiation conditions. Role mixins are relationally dependent types, capturing relational properties shared by instances of different kinds.

For example, &quot;Customer&quot; may be considered a gufo:RoleMixin as a superclass of the roles &quot;CorporateCustomer&quot; (specializing the gufo:Kind &quot;BusinessOrganization&quot;) and &quot;PersonalCustomer&quot; (specializing the gufo:Kind &quot;Person&quot;).</rdfs:comment>
        <rdfs:label xml:lang="en">RoleMixin</rdfs:label>
    </owl:Class>
    


    <!-- http://purl.org/nemo/gufo#Scene -->

    <owl:Class rdf:about="http://purl.org/nemo/gufo#Scene">
        <rdfs:subClassOf rdf:resource="http://purl.org/nemo/gufo#Perdurants"/>
    </owl:Class>
    


    <!-- http://purl.org/nemo/gufo#SemiRigidType -->

    <owl:Class rdf:about="http://purl.org/nemo/gufo#SemiRigidType">
        <rdfs:subClassOf rdf:resource="http://purl.org/nemo/gufo#NonRigidType"/>
        <rdfs:comment xml:lang="en">A gufo:NonRigidType that applies necessarily to some of its instances and contingently to some others (see Guizzardi, 2005, chapter 4).</rdfs:comment>
        <rdfs:label xml:lang="en">SemiRigidType</rdfs:label>
    </owl:Class>
    


    <!-- http://purl.org/nemo/gufo#Situation -->

    <owl:Class rdf:about="http://purl.org/nemo/gufo#Situation">
        <rdfs:subClassOf rdf:resource="http://purl.org/nemo/gufo#Perdurants"/>
        <rdfs:comment xml:lang="en">A gufo:ConcreteIndividual that is a particular configuration of a part of reality which can be understood as a whole and in which entities stand in relations. A situation may be counterfactual or actual. An actual situation (or in other words, a &quot;fact&quot;) &quot;obtains&quot; in a certain time instant or during a time interval.

Note that, in Guizzardi et al. (2013), situations were considered to obtain at a specific point in time. Here, instead, they obtain in a time interval when begin and end points differ.

The various subclasses of Situation in this implementation are used to capture &quot;mutable&quot; facts which obtain during some time and fail to obtain at other times. This includes the contingent instantiation of non-rigid types (e.g., as someone is a child at one point in time and a teenager later), the attribution of value to mutable qualities (such as a person&apos;s weight) and temporary participation in part-whole relations for replaceable parts (such as a car&apos;s tires). Other subclasses may be created to capture domain-specific notions such as &quot;HazardousSituation&quot;, &quot;PersonHasFever&quot;.</rdfs:comment>
        <rdfs:label xml:lang="en">Situation</rdfs:label>
    </owl:Class>
    


    <!-- http://purl.org/nemo/gufo#SituationType -->

    <owl:Class rdf:about="http://purl.org/nemo/gufo#SituationType">
        <rdfs:subClassOf rdf:resource="http://purl.org/nemo/gufo#PerdurantType"/>
        <rdfs:comment xml:lang="en">A gufo:Type whose instances are situations.

Instances of gufo:SituationType are subclasses of gufo:Situation.

Examples include &quot;HazardousSituation&quot;, &quot;PersonHasFever&quot;,  &quot;PersonIsStudent&quot;.</rdfs:comment>
        <rdfs:label xml:lang="en">SituationType</rdfs:label>
    </owl:Class>
    


    <!-- http://purl.org/nemo/gufo#Sortal -->

    <owl:Class rdf:about="http://purl.org/nemo/gufo#Sortal">
        <rdfs:subClassOf rdf:resource="http://purl.org/nemo/gufo#EndurantType"/>
        <rdfs:comment xml:lang="en">A gufo:EndurantType which carries (or supplies) a principle of identity for its instances  (see Guizzardi, 2005, chapter 4).</rdfs:comment>
        <rdfs:label xml:lang="en">Sortal</rdfs:label>
    </owl:Class>
    


    <!-- http://purl.org/nemo/gufo#SubKind -->

    <owl:Class rdf:about="http://purl.org/nemo/gufo#SubKind">
        <rdfs:subClassOf rdf:resource="http://purl.org/nemo/gufo#RigidType"/>
        <rdfs:subClassOf rdf:resource="http://purl.org/nemo/gufo#Sortal"/>
        <rdfs:comment xml:lang="en">A gufo:EndurantType that is both sortal and rigid. It specializes a gufo:Kind carrying the principle of identity supplied by that kind. Every gufo:SubKind should directly or indirectly specialize a gufo:Kind.

For example, the gufo:Kind &quot;Lion&quot; may be specialized into the &quot;Lionness&quot; and &quot;Male Lion&quot; subkinds, while the gufo:Kind &quot;Computer&quot; may be specialized into the &quot;Laptop&quot; and &quot;Desktop&quot; subkinds.</rdfs:comment>
        <rdfs:label xml:lang="en">SubKind</rdfs:label>
    </owl:Class>
    


    <!-- http://purl.org/nemo/gufo#TemporaryConstitutionSituation -->

    <owl:Class rdf:about="http://purl.org/nemo/gufo#TemporaryConstitutionSituation">
        <rdfs:subClassOf rdf:resource="http://purl.org/nemo/gufo#Situation"/>
        <rdfs:subClassOf>
            <owl:Restriction>
                <owl:onProperty rdf:resource="http://purl.org/nemo/gufo#concernsConstitutedEndurant"/>
                <owl:qualifiedCardinality rdf:datatype="http://www.w3.org/2001/XMLSchema#nonNegativeInteger">1</owl:qualifiedCardinality>
                <owl:onClass rdf:resource="http://purl.org/nemo/gufo#Object"/>
            </owl:Restriction>
        </rdfs:subClassOf>
        <rdfs:subClassOf>
            <owl:Restriction>
                <owl:onProperty>
                    <rdf:Description>
                        <owl:inverseOf rdf:resource="http://purl.org/nemo/gufo#standsInQualifiedConstitution"/>
                    </rdf:Description>
                </owl:onProperty>
                <owl:qualifiedCardinality rdf:datatype="http://www.w3.org/2001/XMLSchema#nonNegativeInteger">1</owl:qualifiedCardinality>
                <owl:onClass rdf:resource="http://purl.org/nemo/gufo#Object"/>
            </owl:Restriction>
        </rdfs:subClassOf>
        <owl:disjointWith rdf:resource="http://purl.org/nemo/gufo#TemporaryInstantiationSituation"/>
        <owl:disjointWith rdf:resource="http://purl.org/nemo/gufo#TemporaryRelationshipSituation"/>
        <rdfs:comment xml:lang="en">A gufo:Situation in which a gufo:Endurant temporarly constitutes another gufo:Endurant.

When constitution of an object may change in time, it may be qualified by the period in time in which the relation applies. 

Examples include: the situation in which the Beatles is constituted by the group composed of {John,Paul,Ringo,George}; and the situation in which the statue of Venus de Milo was constituted by its original quantity of marble (including its arms).

This is a reification of constitution (in a solution that is similar to the qualified relation pattern  http://patterns.dataincubator.org/book/qualified-relation.html)</rdfs:comment>
        <rdfs:label xml:lang="en">TemporaryConstitutionSituation</rdfs:label>
    </owl:Class>
    


    <!-- http://purl.org/nemo/gufo#TemporaryInstantiationSituation -->

    <owl:Class rdf:about="http://purl.org/nemo/gufo#TemporaryInstantiationSituation">
        <rdfs:subClassOf rdf:resource="http://purl.org/nemo/gufo#Situation"/>
        <rdfs:subClassOf>
            <owl:Restriction>
                <owl:onProperty rdf:resource="http://purl.org/nemo/gufo#concernsNonRigidType"/>
                <owl:qualifiedCardinality rdf:datatype="http://www.w3.org/2001/XMLSchema#nonNegativeInteger">1</owl:qualifiedCardinality>
                <owl:onClass rdf:resource="http://purl.org/nemo/gufo#NonRigidType"/>
            </owl:Restriction>
        </rdfs:subClassOf>
        <rdfs:subClassOf>
            <owl:Restriction>
                <owl:onProperty>
                    <rdf:Description>
                        <owl:inverseOf rdf:resource="http://purl.org/nemo/gufo#standsInQualifiedInstantiation"/>
                    </rdf:Description>
                </owl:onProperty>
                <owl:qualifiedCardinality rdf:datatype="http://www.w3.org/2001/XMLSchema#nonNegativeInteger">1</owl:qualifiedCardinality>
                <owl:onClass rdf:resource="http://purl.org/nemo/gufo#Endurant"/>
            </owl:Restriction>
        </rdfs:subClassOf>
        <owl:disjointWith rdf:resource="http://purl.org/nemo/gufo#TemporaryParthoodSituation"/>
        <owl:disjointWith rdf:resource="http://purl.org/nemo/gufo#TemporaryRelationshipSituation"/>
        <rdfs:comment xml:lang="en">A gufo:Situation in which a gufo:Endurant temporarily instantiates a gufo:NonRigidType.

A gufo:TemporaryInstantiationSituation can account for the time period in which a particular instantiation holds.

Examples include: the situation in which Obama instantiates the role of president, which began in 20/01/2009 and lasted until 20/01/2017; the situation in which Coatria instantiates the role of EU Member, which began in 01/07/2013 (and is still on-going); and the situation in which Steve Jobs instantiates the child phase, which began in 24/02/1955 and lasted until 24/02/1965.

This solution is inspired in the qualified relation pattern (http://patterns.dataincubator.org/book/qualified-relation.html).</rdfs:comment>
        <rdfs:label xml:lang="en">TemporaryInstantiationSituation</rdfs:label>
    </owl:Class>
    


    <!-- http://purl.org/nemo/gufo#TemporaryParthoodSituation -->

    <owl:Class rdf:about="http://purl.org/nemo/gufo#TemporaryParthoodSituation">
        <rdfs:subClassOf rdf:resource="http://purl.org/nemo/gufo#Situation"/>
        <rdfs:subClassOf>
            <owl:Restriction>
                <owl:onProperty rdf:resource="http://purl.org/nemo/gufo#concernsTemporaryWhole"/>
                <owl:qualifiedCardinality rdf:datatype="http://www.w3.org/2001/XMLSchema#nonNegativeInteger">1</owl:qualifiedCardinality>
                <owl:onClass rdf:resource="http://purl.org/nemo/gufo#Endurant"/>
            </owl:Restriction>
        </rdfs:subClassOf>
        <rdfs:subClassOf>
            <owl:Restriction>
                <owl:onProperty>
                    <rdf:Description>
                        <owl:inverseOf rdf:resource="http://purl.org/nemo/gufo#standsInQualifiedParthood"/>
                    </rdf:Description>
                </owl:onProperty>
                <owl:qualifiedCardinality rdf:datatype="http://www.w3.org/2001/XMLSchema#nonNegativeInteger">1</owl:qualifiedCardinality>
                <owl:onClass rdf:resource="http://purl.org/nemo/gufo#Endurant"/>
            </owl:Restriction>
        </rdfs:subClassOf>
        <owl:disjointWith rdf:resource="http://purl.org/nemo/gufo#TemporaryRelationshipSituation"/>
        <rdfs:comment>A gufo:Situation in which a gufo:Endurant is temporarily a part of another gufo:Endurant.

A gufo:TemporaryParthoodSituation should only be used for mutable parts. It may be qualified by the period in time in which the relation applies. 

Examples include: the situation in which the United Kingdom is a member of the European Union; the situation in which Messi is a a member of the Barcelona FC squad; the situation in which an engine is part of a car; and the situation in which a transplanted heart is part of a person.

Note that, since every instance of gufo:Quantity or gufo:FixedCollection only has essential parts, the gufo:TemporaryParthoodSituation should not be used to represent these parthood relations.
 
This solution is inspired in the qualified relation pattern (http://patterns.dataincubator.org/book/qualified-relation.html).</rdfs:comment>
        <rdfs:label xml:lang="en">TemporaryParthoodSituation</rdfs:label>
    </owl:Class>
    


    <!-- http://purl.org/nemo/gufo#TemporaryRelationshipSituation -->

    <owl:Class rdf:about="http://purl.org/nemo/gufo#TemporaryRelationshipSituation">
        <rdfs:subClassOf rdf:resource="http://purl.org/nemo/gufo#Situation"/>
        <rdfs:subClassOf>
            <owl:Restriction>
                <owl:onProperty rdf:resource="http://purl.org/nemo/gufo#concernsRelatedEndurant"/>
                <owl:someValuesFrom rdf:resource="http://purl.org/nemo/gufo#Endurant"/>
            </owl:Restriction>
        </rdfs:subClassOf>
        <rdfs:subClassOf>
            <owl:Restriction>
                <owl:onProperty rdf:resource="http://purl.org/nemo/gufo#concernsRelationshipType"/>
                <owl:qualifiedCardinality rdf:datatype="http://www.w3.org/2001/XMLSchema#nonNegativeInteger">1</owl:qualifiedCardinality>
                <owl:onClass rdf:resource="http://purl.org/nemo/gufo#RelationshipType"/>
            </owl:Restriction>
        </rdfs:subClassOf>
        <rdfs:subClassOf>
            <owl:Restriction>
                <owl:onProperty>
                    <rdf:Description>
                        <owl:inverseOf rdf:resource="http://purl.org/nemo/gufo#standsInQualifiedRelationship"/>
                    </rdf:Description>
                </owl:onProperty>
                <owl:qualifiedCardinality rdf:datatype="http://www.w3.org/2001/XMLSchema#nonNegativeInteger">1</owl:qualifiedCardinality>
                <owl:onClass rdf:resource="http://purl.org/nemo/gufo#Endurant"/>
            </owl:Restriction>
        </rdfs:subClassOf>
        <rdfs:comment xml:lang="en">A gufo:Situation in which a gufo:Endurant temporarily stands in a relation with another gufo:Endurant (or other endurants in the case of n-ary relationships). 

Reification of a gufo:TemporaryRelationshipSituation allows qualification of the relationship with the period in time in which it applies. 

Examples include: the situation in which Einstein works at the Swiss Patent Office in Bern; the situation in which Elon Musk studies at the University of Pennsylvania; the situation in which John Lennon is married to Yoko Ono; and the situation in which Facebook has a lower market value than Amazon.

For material relationships, prefer the use of gufo:Relator.

This is a reification of the relationship (in a solution that is similar to the qualified relation pattern  http://patterns.dataincubator.org/book/qualified-relation.html).</rdfs:comment>
        <rdfs:label xml:lang="en">TemporaryRelationshipSituation</rdfs:label>
    </owl:Class>
    


    <!-- http://purl.org/nemo/gufo#Type -->

    <owl:Class rdf:about="http://purl.org/nemo/gufo#Type">
        <rdfs:comment xml:lang="en">An entity that may be instantiated by (or predicated over) other entities. Types encompass what we often call &quot;sorts&quot;, &quot;kinds&quot;, &quot;categories&quot;, etc. 

Examples include the kind &quot;Person&quot;, the event type &quot;Earthquake&quot;, and the abstract individual type &quot;NaturalNumber&quot;. Relations, such as &quot;marriedTo&quot; and &quot;olderThan&quot;, are also considered as types.

Instances of gufo:Type are classes, and should specialize the taxonomy of individuals of gUFO. For example, &quot;Person&quot; is a gufo:Type (more specifically a gufo:Kind), specializing gufo:Object. The mechanism that allows for this is called punning in OWL 2.

Encompasses the notion of &quot;Universal&quot; in Guizzardi (2005).</rdfs:comment>
        <rdfs:label xml:lang="en">Type</rdfs:label>
    </owl:Class>
    


    <!-- http://purl.org/nemo/gufo#VariableCollection -->

    <owl:Class rdf:about="http://purl.org/nemo/gufo#VariableCollection">
        <rdfs:subClassOf rdf:resource="http://purl.org/nemo/gufo#Collection"/>
        <rdfs:comment rdf:resource="http://purl.org/nemo/gufo#TemporaryParthoodSituation"/>
        <rdfs:comment xml:lang="en">A gufo:Collection for which change in membership is possible.

Such a collection obeys an intensional principle of identity, i.e., change in membership does not necessarily create a different collection.

For example, KLM&apos;s fleet of airplanes could be understood as a gufo:VariableCollection. In this case, when the company acquires (or retires) an airplane, the fleet changes. Note that, in this case, the airplanes are conceptualized as playing the role of &quot;member of a fleet&quot;. If various roles for the parts of a fleet were envisioned (such as &quot;cargo airplane&quot;, &quot;passenger airplane&quot;), then a fleet would be best understood as a gufo:FunctionalComplex.

See gufo:TemporaryParthoodSituation for the pattern to represent the relation of a variable collection to its temporary parts.</rdfs:comment>
        <rdfs:label xml:lang="en">VariableCollection</rdfs:label>
    </owl:Class>
    


    <!-- http://www.opengis.net/ont/geosparql#Feature -->

    <owl:Class rdf:about="http://www.opengis.net/ont/geosparql#Feature">
        <rdfs:subClassOf rdf:resource="http://www.opengis.net/ont/geosparql#SpatialObject"/>
        <owl:disjointWith rdf:resource="http://www.opengis.net/ont/geosparql#Geometry"/>
        <dc:contributor>Matthew Perry</dc:contributor>
        <dc:creator>OGC GeoSPARQL 1.0 Standard Working Group</dc:creator>
        <dc:date rdf:datatype="http://www.w3.org/2001/XMLSchema#date">2011-06-16</dc:date>
        <dc:description xml:lang="en">
      This class represents the top-level feature type. This class is 
      equivalent to GFI_Feature defined in ISO 19156:2011, and it is 
      superclass of all feature types.
    </dc:description>
        <rdfs:comment xml:lang="en">
      This class represents the top-level feature type. This class is 
      equivalent to GFI_Feature defined in ISO 19156:2011, and it is 
      superclass of all feature types.
    </rdfs:comment>
        <rdfs:isDefinedBy rdf:resource="http://www.opengis.net/ont/geosparql"/>
        <rdfs:isDefinedBy rdf:resource="http://www.opengis.net/ont/gml"/>
        <rdfs:isDefinedBy rdf:resource="http://www.opengis.net/spec/geosparql/1.0"/>
        <rdfs:label xml:lang="en">Feature</rdfs:label>
        <skos:definition xml:lang="en">
      This class represents the top-level feature type. This class is 
      equivalent to GFI_Feature defined in ISO 19156:2011, and it is 
      superclass of all feature types.
    </skos:definition>
        <skos:definition>A discrete spatial phenomenon in a universe of discourse.

Spatial phenomena can generally be thought of as either discrete objects with clear boundaries or as a continuous phenomenon that can be observed everywhere, but does not have natural boundaries. 

Discrete spatial objects may refer to a river, road, country, town, or a research site.

Examples of continuous phenomena, or “spatial fields”, include elevation and qualities.</skos:definition>
        <skos:prefLabel xml:lang="en">Feature</skos:prefLabel>
    </owl:Class>
    


    <!-- http://www.opengis.net/ont/geosparql#Geometry -->

    <owl:Class rdf:about="http://www.opengis.net/ont/geosparql#Geometry">
        <rdfs:subClassOf rdf:resource="http://www.opengis.net/ont/geosparql#SpatialObject"/>
        <dc:contributor>Matthew Perry</dc:contributor>
        <dc:creator>OGC GeoSPARQL 1.0 Standard Working Group</dc:creator>
        <dc:date rdf:datatype="http://www.w3.org/2001/XMLSchema#date">2011-06-16</dc:date>
        <dc:description xml:lang="en">
      The class represents the top-level geometry type. This class is 
      equivalent to the UML class GM_Object defined in ISO 19107, and 
      it is superclass of all geometry types.
    </dc:description>
        <rdfs:comment xml:lang="en">
      The class represents the top-level geometry type. This class is 
      equivalent to the UML class GM_Object defined in ISO 19107, and 
      it is superclass of all geometry types.
    </rdfs:comment>
        <rdfs:isDefinedBy rdf:resource="http://www.opengis.net/ont/geosparql"/>
        <rdfs:isDefinedBy rdf:resource="http://www.opengis.net/ont/gml"/>
        <rdfs:isDefinedBy rdf:resource="http://www.opengis.net/spec/geosparql/1.0"/>
        <rdfs:label xml:lang="en">Geometry</rdfs:label>
        <skos:definition xml:lang="en">
      The class represents the top-level geometry type. This class is 
      equivalent to the UML class GM_Object defined in ISO 19107, and 
      it is superclass of all geometry types.
    </skos:definition>
        <skos:prefLabel xml:lang="en">Geometry</skos:prefLabel>
    </owl:Class>
    


    <!-- http://www.opengis.net/ont/geosparql#SpatialObject -->

    <owl:Class rdf:about="http://www.opengis.net/ont/geosparql#SpatialObject">
        <rdfs:subClassOf rdf:resource="http://purl.org/nemo/gufo#Object"/>
        <dc:contributor>Matthew Perry</dc:contributor>
        <dc:creator>OGC GeoSPARQL 1.0 Standard Working Group</dc:creator>
        <dc:date rdf:datatype="http://www.w3.org/2001/XMLSchema#date">2011-06-16</dc:date>
        <dc:description xml:lang="en">
      The class spatial-object represents everything that can have 
      a spatial representation. It is superclass of feature and geometry.
    </dc:description>
        <rdfs:comment xml:lang="en">
      The class spatial-object represents everything that can have 
      a spatial representation. It is superclass of feature and geometry.
    </rdfs:comment>
        <rdfs:isDefinedBy rdf:resource="http://www.opengis.net/ont/geosparql"/>
        <rdfs:isDefinedBy rdf:resource="http://www.opengis.net/ont/gml"/>
        <rdfs:isDefinedBy rdf:resource="http://www.opengis.net/spec/geosparql/1.0"/>
        <rdfs:label xml:lang="en">SpatialObject</rdfs:label>
        <skos:definition xml:lang="en">
      The class spatial-object represents everything that can have 
      a spatial representation. It is superclass of feature and geometry.
    </skos:definition>
        <skos:prefLabel xml:lang="en">SpatialObject</skos:prefLabel>
    </owl:Class>
    


    <!-- http://www.opengis.net/ont/gml#AbstractCurveSegment -->

    <owl:Class rdf:about="http://www.opengis.net/ont/gml#AbstractCurveSegment">
        <rdfs:subClassOf rdf:resource="http://www.opengis.net/ont/geosparql#Geometry"/>
        <rdfs:isDefinedBy rdf:resource="http://www.opengis.net/ont/gml"/>
        <rdfs:label xml:lang="en">Abstract Curve Segment</rdfs:label>
    </owl:Class>
    


    <!-- http://www.opengis.net/ont/gml#AbstractGeometricPrimitive -->

    <owl:Class rdf:about="http://www.opengis.net/ont/gml#AbstractGeometricPrimitive">
        <rdfs:subClassOf rdf:resource="http://www.opengis.net/ont/gml#AbstractGeometry"/>
        <rdfs:isDefinedBy rdf:resource="http://www.opengis.net/ont/gml"/>
        <rdfs:label xml:lang="en">Abstract Geometric Primitive</rdfs:label>
    </owl:Class>
    


    <!-- http://www.opengis.net/ont/gml#AbstractGeometry -->

    <owl:Class rdf:about="http://www.opengis.net/ont/gml#AbstractGeometry">
        <rdfs:subClassOf rdf:resource="http://www.opengis.net/ont/geosparql#Geometry"/>
        <rdfs:isDefinedBy rdf:resource="http://www.opengis.net/ont/gml"/>
        <rdfs:label xml:lang="en">Abstract Geometry</rdfs:label>
    </owl:Class>
    


    <!-- http://www.opengis.net/ont/gml#AbstractGriddedSurface -->

    <owl:Class rdf:about="http://www.opengis.net/ont/gml#AbstractGriddedSurface">
        <rdfs:subClassOf rdf:resource="http://www.opengis.net/ont/gml#AbstractParametricCurveSurface"/>
        <rdfs:isDefinedBy rdf:resource="http://www.opengis.net/ont/gml"/>
        <rdfs:label xml:lang="en">Abstract Gridded Surface</rdfs:label>
    </owl:Class>
    


    <!-- http://www.opengis.net/ont/gml#AbstractParametricCurveSurface -->

    <owl:Class rdf:about="http://www.opengis.net/ont/gml#AbstractParametricCurveSurface">
        <rdfs:subClassOf rdf:resource="http://www.opengis.net/ont/gml#AbstractSurfacePatch"/>
        <rdfs:isDefinedBy rdf:resource="http://www.opengis.net/ont/gml"/>
        <rdfs:label xml:lang="en">Abstract Parametric Curve Surface</rdfs:label>
    </owl:Class>
    


    <!-- http://www.opengis.net/ont/gml#AbstractSurfacePatch -->

    <owl:Class rdf:about="http://www.opengis.net/ont/gml#AbstractSurfacePatch">
        <rdfs:subClassOf rdf:resource="http://www.opengis.net/ont/geosparql#Geometry"/>
        <rdfs:isDefinedBy rdf:resource="http://www.opengis.net/ont/gml"/>
        <rdfs:label xml:lang="en">Abstract Surface Patch</rdfs:label>
    </owl:Class>
    


    <!-- http://www.opengis.net/ont/gml#Arc -->

    <owl:Class rdf:about="http://www.opengis.net/ont/gml#Arc">
        <rdfs:subClassOf rdf:resource="http://www.opengis.net/ont/gml#ArcString"/>
        <rdfs:isDefinedBy rdf:resource="http://www.opengis.net/ont/gml"/>
        <rdfs:label xml:lang="en">Arc</rdfs:label>
    </owl:Class>
    


    <!-- http://www.opengis.net/ont/gml#ArcByBulge -->

    <owl:Class rdf:about="http://www.opengis.net/ont/gml#ArcByBulge">
        <rdfs:subClassOf rdf:resource="http://www.opengis.net/ont/gml#ArcStringByBulge"/>
        <rdfs:isDefinedBy rdf:resource="http://www.opengis.net/ont/gml"/>
        <rdfs:label xml:lang="en">Arc by Bulge</rdfs:label>
    </owl:Class>
    


    <!-- http://www.opengis.net/ont/gml#ArcByCenterPoint -->

    <owl:Class rdf:about="http://www.opengis.net/ont/gml#ArcByCenterPoint">
        <rdfs:subClassOf rdf:resource="http://www.opengis.net/ont/gml#AbstractCurveSegment"/>
        <rdfs:isDefinedBy rdf:resource="http://www.opengis.net/ont/gml"/>
        <rdfs:label xml:lang="en">Arc by Center Point</rdfs:label>
    </owl:Class>
    


    <!-- http://www.opengis.net/ont/gml#ArcString -->

    <owl:Class rdf:about="http://www.opengis.net/ont/gml#ArcString">
        <rdfs:subClassOf rdf:resource="http://www.opengis.net/ont/gml#AbstractCurveSegment"/>
        <rdfs:isDefinedBy rdf:resource="http://www.opengis.net/ont/gml"/>
        <rdfs:label xml:lang="en">Arc String</rdfs:label>
    </owl:Class>
    


    <!-- http://www.opengis.net/ont/gml#ArcStringByBulge -->

    <owl:Class rdf:about="http://www.opengis.net/ont/gml#ArcStringByBulge">
        <rdfs:subClassOf rdf:resource="http://www.opengis.net/ont/gml#AbstractCurveSegment"/>
        <rdfs:isDefinedBy rdf:resource="http://www.opengis.net/ont/gml"/>
        <rdfs:label xml:lang="en">Arc String by Bulge</rdfs:label>
    </owl:Class>
    


    <!-- http://www.opengis.net/ont/gml#BSpline -->

    <owl:Class rdf:about="http://www.opengis.net/ont/gml#BSpline">
        <rdfs:subClassOf rdf:resource="http://www.opengis.net/ont/gml#SplineCurve"/>
        <rdfs:isDefinedBy rdf:resource="http://www.opengis.net/ont/gml"/>
        <rdfs:label xml:lang="en">BSpline</rdfs:label>
    </owl:Class>
    


    <!-- http://www.opengis.net/ont/gml#Bezier -->

    <owl:Class rdf:about="http://www.opengis.net/ont/gml#Bezier">
        <rdfs:subClassOf rdf:resource="http://www.opengis.net/ont/gml#BSpline"/>
        <rdfs:isDefinedBy rdf:resource="http://www.opengis.net/ont/gml"/>
        <rdfs:label xml:lang="en">Bezier</rdfs:label>
    </owl:Class>
    


    <!-- http://www.opengis.net/ont/gml#Circle -->

    <owl:Class rdf:about="http://www.opengis.net/ont/gml#Circle">
        <rdfs:subClassOf rdf:resource="http://www.opengis.net/ont/gml#Arc"/>
        <rdfs:isDefinedBy rdf:resource="http://www.opengis.net/ont/gml"/>
        <rdfs:label xml:lang="en">Circle</rdfs:label>
    </owl:Class>
    


    <!-- http://www.opengis.net/ont/gml#CircleByCenterPoint -->

    <owl:Class rdf:about="http://www.opengis.net/ont/gml#CircleByCenterPoint">
        <rdfs:subClassOf rdf:resource="http://www.opengis.net/ont/gml#ArcByCenterPoint"/>
        <rdfs:isDefinedBy rdf:resource="http://www.opengis.net/ont/gml"/>
        <rdfs:label xml:lang="en">CircleByCenterPoint</rdfs:label>
    </owl:Class>
    


    <!-- http://www.opengis.net/ont/gml#Clothoid -->

    <owl:Class rdf:about="http://www.opengis.net/ont/gml#Clothoid">
        <rdfs:subClassOf rdf:resource="http://www.opengis.net/ont/gml#AbstractCurveSegment"/>
        <rdfs:isDefinedBy rdf:resource="http://www.opengis.net/ont/gml"/>
        <rdfs:label xml:lang="en">Clothoid</rdfs:label>
    </owl:Class>
    


    <!-- http://www.opengis.net/ont/gml#Composite -->

    <owl:Class rdf:about="http://www.opengis.net/ont/gml#Composite">
        <rdfs:subClassOf rdf:resource="http://www.opengis.net/ont/gml#GeometricComplex"/>
        <rdfs:isDefinedBy rdf:resource="http://www.opengis.net/ont/gml"/>
        <rdfs:label xml:lang="en">Composite</rdfs:label>
    </owl:Class>
    


    <!-- http://www.opengis.net/ont/gml#CompositeCurve -->

    <owl:Class rdf:about="http://www.opengis.net/ont/gml#CompositeCurve">
        <rdfs:subClassOf rdf:resource="http://www.opengis.net/ont/gml#Composite"/>
        <rdfs:subClassOf rdf:resource="http://www.opengis.net/ont/gml#OrientableCurve"/>
        <rdfs:isDefinedBy rdf:resource="http://www.opengis.net/ont/gml"/>
        <rdfs:label xml:lang="en">Composite Curve</rdfs:label>
    </owl:Class>
    


    <!-- http://www.opengis.net/ont/gml#CompositeSolid -->

    <owl:Class rdf:about="http://www.opengis.net/ont/gml#CompositeSolid">
        <rdfs:subClassOf rdf:resource="http://www.opengis.net/ont/gml#Composite"/>
        <rdfs:subClassOf rdf:resource="http://www.opengis.net/ont/gml#Solid"/>
        <rdfs:isDefinedBy rdf:resource="http://www.opengis.net/ont/gml"/>
        <rdfs:label xml:lang="en">Composite Solid</rdfs:label>
    </owl:Class>
    


    <!-- http://www.opengis.net/ont/gml#CompositeSurface -->

    <owl:Class rdf:about="http://www.opengis.net/ont/gml#CompositeSurface">
        <rdfs:subClassOf rdf:resource="http://www.opengis.net/ont/gml#Composite"/>
        <rdfs:subClassOf rdf:resource="http://www.opengis.net/ont/gml#OrientableSurface"/>
        <rdfs:isDefinedBy rdf:resource="http://www.opengis.net/ont/gml"/>
        <rdfs:label xml:lang="en">Composite Surface</rdfs:label>
    </owl:Class>
    


    <!-- http://www.opengis.net/ont/gml#Cone -->

    <owl:Class rdf:about="http://www.opengis.net/ont/gml#Cone">
        <rdfs:subClassOf rdf:resource="http://www.opengis.net/ont/gml#AbstractGriddedSurface"/>
        <rdfs:isDefinedBy rdf:resource="http://www.opengis.net/ont/gml"/>
        <rdfs:label xml:lang="en">Cone</rdfs:label>
    </owl:Class>
    


    <!-- http://www.opengis.net/ont/gml#CubicSpline -->

    <owl:Class rdf:about="http://www.opengis.net/ont/gml#CubicSpline">
        <rdfs:subClassOf rdf:resource="http://www.opengis.net/ont/gml#PolynomialSpline"/>
        <rdfs:isDefinedBy rdf:resource="http://www.opengis.net/ont/gml"/>
        <rdfs:label xml:lang="en">Cubic Spline</rdfs:label>
    </owl:Class>
    


    <!-- http://www.opengis.net/ont/gml#Curve -->

    <owl:Class rdf:about="http://www.opengis.net/ont/gml#Curve">
        <rdfs:subClassOf rdf:resource="http://www.opengis.net/ont/gml#AbstractGeometricPrimitive"/>
        <rdfs:subClassOf rdf:resource="http://www.opengis.net/ont/gml#OrientableCurve"/>
        <rdfs:isDefinedBy rdf:resource="http://www.opengis.net/ont/gml"/>
        <rdfs:label xml:lang="en">Curve</rdfs:label>
    </owl:Class>
    


    <!-- http://www.opengis.net/ont/gml#Cylinder -->

    <owl:Class rdf:about="http://www.opengis.net/ont/gml#Cylinder">
        <rdfs:subClassOf rdf:resource="http://www.opengis.net/ont/gml#AbstractGriddedSurface"/>
        <rdfs:isDefinedBy rdf:resource="http://www.opengis.net/ont/gml"/>
        <rdfs:label xml:lang="en">Cylinder</rdfs:label>
    </owl:Class>
    


    <!-- http://www.opengis.net/ont/gml#Geodesic -->

    <owl:Class rdf:about="http://www.opengis.net/ont/gml#Geodesic">
        <rdfs:subClassOf rdf:resource="http://www.opengis.net/ont/gml#GeodesicString"/>
        <rdfs:isDefinedBy rdf:resource="http://www.opengis.net/ont/gml"/>
        <rdfs:label xml:lang="en">Geodesic</rdfs:label>
    </owl:Class>
    


    <!-- http://www.opengis.net/ont/gml#GeodesicString -->

    <owl:Class rdf:about="http://www.opengis.net/ont/gml#GeodesicString">
        <rdfs:subClassOf rdf:resource="http://www.opengis.net/ont/gml#AbstractCurveSegment"/>
        <rdfs:isDefinedBy rdf:resource="http://www.opengis.net/ont/gml"/>
        <rdfs:label xml:lang="en">Geodesic String</rdfs:label>
    </owl:Class>
    


    <!-- http://www.opengis.net/ont/gml#GeometricComplex -->

    <owl:Class rdf:about="http://www.opengis.net/ont/gml#GeometricComplex">
        <rdfs:subClassOf rdf:resource="http://www.opengis.net/ont/gml#AbstractGeometry"/>
        <rdfs:isDefinedBy rdf:resource="http://www.opengis.net/ont/gml"/>
        <rdfs:label xml:lang="en">Geometric Complex</rdfs:label>
    </owl:Class>
    


    <!-- http://www.opengis.net/ont/gml#LineString -->

    <owl:Class rdf:about="http://www.opengis.net/ont/gml#LineString">
        <rdfs:subClassOf rdf:resource="http://www.opengis.net/ont/gml#LineStringSegment"/>
        <rdfs:isDefinedBy rdf:resource="http://www.opengis.net/ont/gml"/>
        <rdfs:label xml:lang="en">Line String</rdfs:label>
    </owl:Class>
    


    <!-- http://www.opengis.net/ont/gml#LineStringSegment -->

    <owl:Class rdf:about="http://www.opengis.net/ont/gml#LineStringSegment">
        <rdfs:subClassOf rdf:resource="http://www.opengis.net/ont/gml#AbstractCurveSegment"/>
        <rdfs:isDefinedBy rdf:resource="http://www.opengis.net/ont/gml"/>
        <rdfs:label xml:lang="en">Line String Segment</rdfs:label>
    </owl:Class>
    


    <!-- http://www.opengis.net/ont/gml#LinearRing -->

    <owl:Class rdf:about="http://www.opengis.net/ont/gml#LinearRing">
        <rdfs:subClassOf rdf:resource="http://www.opengis.net/ont/gml#Ring"/>
        <rdfs:isDefinedBy rdf:resource="http://www.opengis.net/ont/gml"/>
        <rdfs:label xml:lang="en">Linear Ring</rdfs:label>
    </owl:Class>
    


    <!-- http://www.opengis.net/ont/gml#MultiCurve -->

    <owl:Class rdf:about="http://www.opengis.net/ont/gml#MultiCurve">
        <rdfs:subClassOf rdf:resource="http://www.opengis.net/ont/gml#MultiGeometry"/>
        <rdfs:isDefinedBy rdf:resource="http://www.opengis.net/ont/gml"/>
        <rdfs:label xml:lang="en">Multi-Curve</rdfs:label>
    </owl:Class>
    


    <!-- http://www.opengis.net/ont/gml#MultiGeometry -->

    <owl:Class rdf:about="http://www.opengis.net/ont/gml#MultiGeometry">
        <rdfs:subClassOf rdf:resource="http://www.opengis.net/ont/gml#AbstractGeometry"/>
        <rdfs:isDefinedBy rdf:resource="http://www.opengis.net/ont/gml"/>
        <rdfs:label xml:lang="en">Multi-Geometry</rdfs:label>
    </owl:Class>
    


    <!-- http://www.opengis.net/ont/gml#MultiPoint -->

    <owl:Class rdf:about="http://www.opengis.net/ont/gml#MultiPoint">
        <rdfs:subClassOf rdf:resource="http://www.opengis.net/ont/gml#MultiGeometry"/>
        <rdfs:isDefinedBy rdf:resource="http://www.opengis.net/ont/gml"/>
        <rdfs:label xml:lang="en">Multi-Point</rdfs:label>
    </owl:Class>
    


    <!-- http://www.opengis.net/ont/gml#MultiSolid -->

    <owl:Class rdf:about="http://www.opengis.net/ont/gml#MultiSolid">
        <rdfs:subClassOf rdf:resource="http://www.opengis.net/ont/gml#MultiGeometry"/>
        <rdfs:isDefinedBy rdf:resource="http://www.opengis.net/ont/gml"/>
        <rdfs:label xml:lang="en">Multi-Solid</rdfs:label>
    </owl:Class>
    


    <!-- http://www.opengis.net/ont/gml#MultiSurface -->

    <owl:Class rdf:about="http://www.opengis.net/ont/gml#MultiSurface">
        <rdfs:subClassOf rdf:resource="http://www.opengis.net/ont/gml#MultiGeometry"/>
        <rdfs:isDefinedBy rdf:resource="http://www.opengis.net/ont/gml"/>
        <rdfs:label xml:lang="en">Multi-Surface</rdfs:label>
    </owl:Class>
    


    <!-- http://www.opengis.net/ont/gml#OffsetCurve -->

    <owl:Class rdf:about="http://www.opengis.net/ont/gml#OffsetCurve">
        <rdfs:subClassOf rdf:resource="http://www.opengis.net/ont/gml#AbstractCurveSegment"/>
        <rdfs:isDefinedBy rdf:resource="http://www.opengis.net/ont/gml"/>
        <rdfs:label xml:lang="en">Offset Curve</rdfs:label>
    </owl:Class>
    


    <!-- http://www.opengis.net/ont/gml#OrientableCurve -->

    <owl:Class rdf:about="http://www.opengis.net/ont/gml#OrientableCurve">
        <rdfs:subClassOf rdf:resource="http://www.opengis.net/ont/gml#AbstractGeometricPrimitive"/>
        <rdfs:isDefinedBy rdf:resource="http://www.opengis.net/ont/gml"/>
        <rdfs:label xml:lang="en">Orientable Curve</rdfs:label>
    </owl:Class>
    


    <!-- http://www.opengis.net/ont/gml#OrientableSurface -->

    <owl:Class rdf:about="http://www.opengis.net/ont/gml#OrientableSurface">
        <rdfs:subClassOf rdf:resource="http://www.opengis.net/ont/gml#AbstractGeometricPrimitive"/>
        <rdfs:isDefinedBy rdf:resource="http://www.opengis.net/ont/gml"/>
        <rdfs:label xml:lang="en">Orientable Surface</rdfs:label>
    </owl:Class>
    


    <!-- http://www.opengis.net/ont/gml#Point -->

    <owl:Class rdf:about="http://www.opengis.net/ont/gml#Point">
        <rdfs:subClassOf rdf:resource="http://www.opengis.net/ont/gml#AbstractGeometricPrimitive"/>
        <rdfs:isDefinedBy rdf:resource="http://www.opengis.net/ont/gml"/>
        <rdfs:label xml:lang="en">Point</rdfs:label>
    </owl:Class>
    


    <!-- http://www.opengis.net/ont/gml#Polygon -->

    <owl:Class rdf:about="http://www.opengis.net/ont/gml#Polygon">
        <rdfs:subClassOf rdf:resource="http://www.opengis.net/ont/gml#Surface"/>
        <rdfs:isDefinedBy rdf:resource="http://www.opengis.net/ont/gml"/>
        <rdfs:label xml:lang="en">Polygon</rdfs:label>
    </owl:Class>
    


    <!-- http://www.opengis.net/ont/gml#PolygonPatch -->

    <owl:Class rdf:about="http://www.opengis.net/ont/gml#PolygonPatch">
        <rdfs:subClassOf rdf:resource="http://www.opengis.net/ont/gml#AbstractSurfacePatch"/>
        <rdfs:isDefinedBy rdf:resource="http://www.opengis.net/ont/gml"/>
        <rdfs:label xml:lang="en">Polygon Patch</rdfs:label>
    </owl:Class>
    


    <!-- http://www.opengis.net/ont/gml#PolyhedralSurface -->

    <owl:Class rdf:about="http://www.opengis.net/ont/gml#PolyhedralSurface">
        <rdfs:subClassOf rdf:resource="http://www.opengis.net/ont/gml#Surface"/>
        <rdfs:isDefinedBy rdf:resource="http://www.opengis.net/ont/gml"/>
        <rdfs:label xml:lang="en">Polyhedral Surface</rdfs:label>
    </owl:Class>
    


    <!-- http://www.opengis.net/ont/gml#PolynomialSpline -->

    <owl:Class rdf:about="http://www.opengis.net/ont/gml#PolynomialSpline">
        <rdfs:subClassOf rdf:resource="http://www.opengis.net/ont/gml#SplineCurve"/>
        <rdfs:isDefinedBy rdf:resource="http://www.opengis.net/ont/gml"/>
        <rdfs:label xml:lang="en">Polynomial Spline</rdfs:label>
    </owl:Class>
    


    <!-- http://www.opengis.net/ont/gml#Rectangle -->

    <owl:Class rdf:about="http://www.opengis.net/ont/gml#Rectangle">
        <rdfs:subClassOf rdf:resource="http://www.opengis.net/ont/gml#PolygonPatch"/>
        <rdfs:isDefinedBy rdf:resource="http://www.opengis.net/ont/gml"/>
        <rdfs:label xml:lang="en">Rectangle</rdfs:label>
    </owl:Class>
    


    <!-- http://www.opengis.net/ont/gml#Ring -->

    <owl:Class rdf:about="http://www.opengis.net/ont/gml#Ring">
        <rdfs:subClassOf rdf:resource="http://www.opengis.net/ont/gml#CompositeCurve"/>
        <rdfs:isDefinedBy rdf:resource="http://www.opengis.net/ont/gml"/>
        <rdfs:label xml:lang="en">Ring</rdfs:label>
    </owl:Class>
    


    <!-- http://www.opengis.net/ont/gml#Shell -->

    <owl:Class rdf:about="http://www.opengis.net/ont/gml#Shell">
        <rdfs:subClassOf rdf:resource="http://www.opengis.net/ont/gml#CompositeSurface"/>
        <rdfs:isDefinedBy rdf:resource="http://www.opengis.net/ont/gml"/>
        <rdfs:label xml:lang="en">Shell</rdfs:label>
    </owl:Class>
    


    <!-- http://www.opengis.net/ont/gml#Solid -->

    <owl:Class rdf:about="http://www.opengis.net/ont/gml#Solid">
        <rdfs:subClassOf rdf:resource="http://www.opengis.net/ont/gml#AbstractGeometricPrimitive"/>
        <rdfs:isDefinedBy rdf:resource="http://www.opengis.net/ont/gml"/>
        <rdfs:label xml:lang="en">Solid</rdfs:label>
    </owl:Class>
    


    <!-- http://www.opengis.net/ont/gml#Sphere -->

    <owl:Class rdf:about="http://www.opengis.net/ont/gml#Sphere">
        <rdfs:subClassOf rdf:resource="http://www.opengis.net/ont/gml#AbstractGriddedSurface"/>
        <rdfs:isDefinedBy rdf:resource="http://www.opengis.net/ont/gml"/>
        <rdfs:label xml:lang="en">Sphere</rdfs:label>
    </owl:Class>
    


    <!-- http://www.opengis.net/ont/gml#SplineCurve -->

    <owl:Class rdf:about="http://www.opengis.net/ont/gml#SplineCurve">
        <rdfs:subClassOf rdf:resource="http://www.opengis.net/ont/gml#AbstractCurveSegment"/>
        <rdfs:isDefinedBy rdf:resource="http://www.opengis.net/ont/gml"/>
        <rdfs:label xml:lang="en">Spline Curve</rdfs:label>
    </owl:Class>
    


    <!-- http://www.opengis.net/ont/gml#Surface -->

    <owl:Class rdf:about="http://www.opengis.net/ont/gml#Surface">
        <rdfs:subClassOf rdf:resource="http://www.opengis.net/ont/gml#AbstractGeometricPrimitive"/>
        <rdfs:subClassOf rdf:resource="http://www.opengis.net/ont/gml#OrientableSurface"/>
        <rdfs:isDefinedBy rdf:resource="http://www.opengis.net/ont/gml"/>
        <rdfs:label xml:lang="en">Surface</rdfs:label>
    </owl:Class>
    


    <!-- http://www.opengis.net/ont/gml#Tin -->

    <owl:Class rdf:about="http://www.opengis.net/ont/gml#Tin">
        <rdfs:subClassOf rdf:resource="http://www.opengis.net/ont/gml#TriangulatedSurface"/>
        <rdfs:isDefinedBy rdf:resource="http://www.opengis.net/ont/gml"/>
        <rdfs:label xml:lang="en">Triangulated Irregular Network</rdfs:label>
    </owl:Class>
    


    <!-- http://www.opengis.net/ont/gml#Triangle -->

    <owl:Class rdf:about="http://www.opengis.net/ont/gml#Triangle">
        <rdfs:subClassOf rdf:resource="http://www.opengis.net/ont/gml#PolygonPatch"/>
        <rdfs:isDefinedBy rdf:resource="http://www.opengis.net/ont/gml"/>
        <rdfs:label xml:lang="en">Triangle</rdfs:label>
    </owl:Class>
    


    <!-- http://www.opengis.net/ont/gml#TriangulatedSurface -->

    <owl:Class rdf:about="http://www.opengis.net/ont/gml#TriangulatedSurface">
        <rdfs:subClassOf rdf:resource="http://www.opengis.net/ont/gml#PolyhedralSurface"/>
        <rdfs:isDefinedBy rdf:resource="http://www.opengis.net/ont/gml"/>
        <rdfs:label xml:lang="en">Triangulated Surface</rdfs:label>
    </owl:Class>
    


    <!-- http://www.w3.org/2004/02/skos/core#Collection -->

    <owl:Class rdf:about="http://www.w3.org/2004/02/skos/core#Collection">
        <owl:disjointWith rdf:resource="http://www.w3.org/2004/02/skos/core#Concept"/>
        <owl:disjointWith rdf:resource="http://www.w3.org/2004/02/skos/core#ConceptScheme"/>
        <rdfs:isDefinedBy rdf:resource="http://www.w3.org/2004/02/skos/core"/>
        <rdfs:label xml:lang="en">Collection</rdfs:label>
        <skos:definition xml:lang="en">A meaningful collection of concepts.</skos:definition>
        <skos:scopeNote xml:lang="en">Labelled collections can be used where you would like a set of concepts to be displayed under a &apos;node label&apos; in the hierarchy.</skos:scopeNote>
    </owl:Class>
    


    <!-- http://www.w3.org/2004/02/skos/core#Concept -->

    <owl:Class rdf:about="http://www.w3.org/2004/02/skos/core#Concept">
        <owl:disjointWith rdf:resource="http://www.w3.org/2004/02/skos/core#ConceptScheme"/>
        <rdfs:isDefinedBy rdf:resource="http://www.w3.org/2004/02/skos/core"/>
        <rdfs:label xml:lang="en">Concept</rdfs:label>
        <skos:definition xml:lang="en">An idea or notion; a unit of thought.</skos:definition>
    </owl:Class>
    


    <!-- http://www.w3.org/2004/02/skos/core#ConceptScheme -->

    <owl:Class rdf:about="http://www.w3.org/2004/02/skos/core#ConceptScheme">
        <rdfs:isDefinedBy rdf:resource="http://www.w3.org/2004/02/skos/core"/>
        <rdfs:label xml:lang="en">Concept Scheme</rdfs:label>
        <skos:definition xml:lang="en">A set of concepts, optionally including statements about semantic relationships between those concepts.</skos:definition>
        <skos:example xml:lang="en">Thesauri, classification schemes, subject heading lists, taxonomies, &apos;folksonomies&apos;, and other types of controlled vocabulary are all examples of concept schemes. Concept schemes are also embedded in glossaries and terminologies.</skos:example>
        <skos:scopeNote xml:lang="en">A concept scheme may be defined to include concepts from different sources.</skos:scopeNote>
    </owl:Class>
    


    <!-- http://www.w3.org/2004/02/skos/core#OrderedCollection -->

    <owl:Class rdf:about="http://www.w3.org/2004/02/skos/core#OrderedCollection">
        <rdfs:subClassOf rdf:resource="http://www.w3.org/2004/02/skos/core#Collection"/>
        <rdfs:isDefinedBy rdf:resource="http://www.w3.org/2004/02/skos/core"/>
        <rdfs:label xml:lang="en">Ordered Collection</rdfs:label>
        <skos:definition xml:lang="en">An ordered collection of concepts, where both the grouping and the ordering are meaningful.</skos:definition>
        <skos:scopeNote xml:lang="en">Ordered collections can be used where you would like a set of concepts to be displayed in a specific order, and optionally under a &apos;node label&apos;.</skos:scopeNote>
    </owl:Class>
    


    <!-- http://www.w3.org/2006/time#DateTimeDescription -->

    <owl:Class rdf:about="http://www.w3.org/2006/time#DateTimeDescription">
        <rdfs:subClassOf rdf:resource="http://www.w3.org/2006/time#GeneralDateTimeDescription"/>
        <rdfs:subClassOf>
            <owl:Restriction>
                <owl:onProperty rdf:resource="http://www.w3.org/2006/time#day"/>
                <owl:allValuesFrom rdf:resource="http://www.w3.org/2001/XMLSchema#gDay"/>
            </owl:Restriction>
        </rdfs:subClassOf>
        <rdfs:subClassOf>
            <owl:Restriction>
                <owl:onProperty rdf:resource="http://www.w3.org/2006/time#month"/>
                <owl:allValuesFrom rdf:resource="http://www.w3.org/2001/XMLSchema#gMonth"/>
            </owl:Restriction>
        </rdfs:subClassOf>
        <rdfs:subClassOf>
            <owl:Restriction>
                <owl:onProperty rdf:resource="http://www.w3.org/2006/time#year"/>
                <owl:allValuesFrom rdf:resource="http://www.w3.org/2001/XMLSchema#gYear"/>
            </owl:Restriction>
        </rdfs:subClassOf>
        <rdfs:comment xml:lang="es">Descripción de fecha y tiempo estructurada con valores separados para los diferentes elementos de un sistema calendario-reloj. El sistema de referencia temporal está fijado al calendario gregoriano, y el rango de las propiedades año, mes, día restringidas a los correspondientes tipos del XML Schema xsd:gYear, xsd:gMonth y xsd:gDay respectivamente.</rdfs:comment>
        <rdfs:comment xml:lang="en">Description of date and time structured with separate values for the various elements of a calendar-clock system. The temporal reference system is fixed to Gregorian Calendar, and the range of year, month, day properties restricted to corresponding XML Schema types xsd:gYear, xsd:gMonth and xsd:gDay, respectively.</rdfs:comment>
        <rdfs:label xml:lang="en">Date-Time description</rdfs:label>
        <rdfs:label xml:lang="es">descripción de fecha-tiempo</rdfs:label>
        <skos:definition xml:lang="es">Descripción de fecha y tiempo estructurada con valores separados para los diferentes elementos de un sistema calendario-reloj. El sistema de referencia temporal está fijado al calendario gregoriano, y el rango de las propiedades año, mes, día restringidas a los correspondientes tipos del XML Schema xsd:gYear, xsd:gMonth y xsd:gDay respectivamente.</skos:definition>
        <skos:definition xml:lang="en">Description of date and time structured with separate values for the various elements of a calendar-clock system. The temporal reference system is fixed to Gregorian Calendar, and the range of year, month, day properties restricted to corresponding XML Schema types xsd:gYear, xsd:gMonth and xsd:gDay, respectively.</skos:definition>
    </owl:Class>
    


    <!-- http://www.w3.org/2006/time#DateTimeInterval -->

    <owl:Class rdf:about="http://www.w3.org/2006/time#DateTimeInterval">
        <rdfs:subClassOf rdf:resource="http://www.w3.org/2006/time#ProperInterval"/>
        <rdfs:comment xml:lang="es">&apos;intervalo de fecha-hora&apos; es una subclase de &apos;intervalo propio&apos;, definida utilizando el multi-elemento &apos;descripción de fecha-hora&apos;.</rdfs:comment>
        <rdfs:comment xml:lang="en">DateTimeInterval is a subclass of ProperInterval, defined using the multi-element DateTimeDescription.</rdfs:comment>
        <rdfs:label xml:lang="en">Date-time interval</rdfs:label>
        <rdfs:label xml:lang="es">intervalo de fecha-hora</rdfs:label>
        <skos:definition xml:lang="es">&apos;intervalo de fecha-hora&apos; es una subclase de &apos;intervalo propio&apos;, definida utilizando el multi-elemento &apos;descripción de fecha-hora&apos;.</skos:definition>
        <skos:definition xml:lang="en">DateTimeInterval is a subclass of ProperInterval, defined using the multi-element DateTimeDescription.</skos:definition>
        <skos:note xml:lang="es">&apos;intervalo de fecha-hora&apos; se puede utilizar sólo para un intervalo cuyos límites coinciden con un elemento de fecha-hora alineados con el calendario y la zona horaria indicados. Por ejemplo, aunque ambos tienen una duración de un día, el intervalo de 24 horas que empieza en la media noche del comienzo del 8 mayo en Europa Central se puede expresar como un &apos;intervalo de fecha-hora&apos;, el intervalo de 24 horas que empieza a las 1:30pm no.</skos:note>
        <skos:note xml:lang="en">:DateTimeInterval can only be used for an interval whose limits coincide with a date-time element aligned to the calendar and timezone indicated. For example, while both have a duration of one day, the 24-hour interval beginning at midnight at the beginning of 8 May in Central Europe can be expressed as a :DateTimeInterval, but the 24-hour interval starting at 1:30pm cannot.</skos:note>
    </owl:Class>
    


    <!-- http://www.w3.org/2006/time#DayOfWeek -->

    <owl:Class rdf:about="http://www.w3.org/2006/time#DayOfWeek">
        <rdfs:subClassOf rdf:resource="http://www.w3.org/2002/07/owl#Thing"/>
        <rdfs:comment xml:lang="es">El día de la semana</rdfs:comment>
        <rdfs:comment xml:lang="en">The day of week</rdfs:comment>
        <rdfs:label xml:lang="en">Day of week</rdfs:label>
        <rdfs:label xml:lang="es">día de la semana</rdfs:label>
        <skos:changeNote xml:lang="en">Remove enumeration from definition, in order to allow other days to be used when required in other calendars. 
NOTE: existing days are still present as members of the class, but the class membership is now open. 

In the original OWL-Time the following constraint appeared: 
  owl:oneOf (
      time:Monday
      time:Tuesday
      time:Wednesday
      time:Thursday
      time:Friday
      time:Saturday
      time:Sunday
    ) ;</skos:changeNote>
        <skos:definition xml:lang="es">El día de la semana</skos:definition>
        <skos:definition xml:lang="en">The day of week</skos:definition>
        <skos:note xml:lang="es">La pertenencia a la clase &apos;día de la semana&apos; está abierta, para permitir longitudes de semana alternativas y diferentes nombres de días.</skos:note>
        <skos:note xml:lang="en">Membership of the class :DayOfWeek is open, to allow for alternative week lengths and different day names.</skos:note>
    </owl:Class>
    


    <!-- http://www.w3.org/2006/time#Duration -->

    <owl:Class rdf:about="http://www.w3.org/2006/time#Duration">
        <rdfs:subClassOf rdf:resource="http://www.w3.org/2006/time#TemporalDuration"/>
        <rdfs:subClassOf>
            <owl:Restriction>
                <owl:onProperty rdf:resource="http://www.w3.org/2006/time#unitType"/>
                <owl:cardinality rdf:datatype="http://www.w3.org/2001/XMLSchema#nonNegativeInteger">1</owl:cardinality>
            </owl:Restriction>
        </rdfs:subClassOf>
        <rdfs:subClassOf>
            <owl:Restriction>
                <owl:onProperty rdf:resource="http://www.w3.org/2006/time#numericDuration"/>
                <owl:cardinality rdf:datatype="http://www.w3.org/2001/XMLSchema#nonNegativeInteger">1</owl:cardinality>
            </owl:Restriction>
        </rdfs:subClassOf>
        <rdfs:comment xml:lang="es">Duración de una extensión temporal expresada como un número escalado por una unidad temporal.</rdfs:comment>
        <rdfs:comment xml:lang="en">Duration of a temporal extent expressed as a number scaled by a temporal unit</rdfs:comment>
        <rdfs:label xml:lang="en">Time duration</rdfs:label>
        <rdfs:label>duración de tiempo</rdfs:label>
        <skos:definition xml:lang="es">Duración de una extensión temporal expresada como un número escalado por una unidad temporal.</skos:definition>
        <skos:definition xml:lang="en">Duration of a temporal extent expressed as a number scaled by a temporal unit</skos:definition>
        <skos:note xml:lang="es">Alternativa a &apos;descripción de tiempo&apos; para proporcionar descripción soporte a una duración temporal diferente a utilizar un sistema de calendario/reloj.</skos:note>
        <skos:note xml:lang="en">Alternative to time:DurationDescription to support description of a temporal duration other than using a calendar/clock system.</skos:note>
    </owl:Class>
    


    <!-- http://www.w3.org/2006/time#DurationDescription -->

    <owl:Class rdf:about="http://www.w3.org/2006/time#DurationDescription">
        <rdfs:subClassOf rdf:resource="http://www.w3.org/2006/time#GeneralDurationDescription"/>
        <rdfs:subClassOf>
            <owl:Restriction>
                <owl:onProperty rdf:resource="http://www.w3.org/2006/time#days"/>
                <owl:allValuesFrom rdf:resource="http://www.w3.org/2001/XMLSchema#decimal"/>
            </owl:Restriction>
        </rdfs:subClassOf>
        <rdfs:subClassOf>
            <owl:Restriction>
                <owl:onProperty rdf:resource="http://www.w3.org/2006/time#hours"/>
                <owl:allValuesFrom rdf:resource="http://www.w3.org/2001/XMLSchema#decimal"/>
            </owl:Restriction>
        </rdfs:subClassOf>
        <rdfs:subClassOf>
            <owl:Restriction>
                <owl:onProperty rdf:resource="http://www.w3.org/2006/time#minutes"/>
                <owl:allValuesFrom rdf:resource="http://www.w3.org/2001/XMLSchema#decimal"/>
            </owl:Restriction>
        </rdfs:subClassOf>
        <rdfs:subClassOf>
            <owl:Restriction>
                <owl:onProperty rdf:resource="http://www.w3.org/2006/time#months"/>
                <owl:allValuesFrom rdf:resource="http://www.w3.org/2001/XMLSchema#decimal"/>
            </owl:Restriction>
        </rdfs:subClassOf>
        <rdfs:subClassOf>
            <owl:Restriction>
                <owl:onProperty rdf:resource="http://www.w3.org/2006/time#seconds"/>
                <owl:allValuesFrom rdf:resource="http://www.w3.org/2001/XMLSchema#decimal"/>
            </owl:Restriction>
        </rdfs:subClassOf>
        <rdfs:subClassOf>
            <owl:Restriction>
                <owl:onProperty rdf:resource="http://www.w3.org/2006/time#weeks"/>
                <owl:allValuesFrom rdf:resource="http://www.w3.org/2001/XMLSchema#decimal"/>
            </owl:Restriction>
        </rdfs:subClassOf>
        <rdfs:subClassOf>
            <owl:Restriction>
                <owl:onProperty rdf:resource="http://www.w3.org/2006/time#years"/>
                <owl:allValuesFrom rdf:resource="http://www.w3.org/2001/XMLSchema#decimal"/>
            </owl:Restriction>
        </rdfs:subClassOf>
        <rdfs:comment xml:lang="es">Descripción de extensión temporal estructurada con valores separados para los distintos elementos de un sistema de horario-calendario. El sistema de referencia temporal se fija al calendario gregoriano, y el intervalo de cada una de las propiedades numéricas se restringe a xsd:decimal.</rdfs:comment>
        <rdfs:comment xml:lang="en">Description of temporal extent structured with separate values for the various elements of a calendar-clock system. The temporal reference system is fixed to Gregorian Calendar, and the range of each of the numeric properties is restricted to xsd:decimal</rdfs:comment>
        <rdfs:label xml:lang="en">Duration description</rdfs:label>
        <rdfs:label xml:lang="es">descripción de duración</rdfs:label>
        <skos:definition xml:lang="es">Descripción de extensión temporal estructurada con valores separados para los distintos elementos de un sistema de horario-calendario. El sistema de referencia temporal se fija al calendario gregoriano, y el intervalo de cada una de las propiedades numéricas se restringe a xsd:decimal.</skos:definition>
        <skos:definition xml:lang="en">Description of temporal extent structured with separate values for the various elements of a calendar-clock system. The temporal reference system is fixed to Gregorian Calendar, and the range of each of the numeric properties is restricted to xsd:decimal</skos:definition>
        <skos:note xml:lang="es">En el calendario gregoriano la longitud de los meses no es fija. Por lo tanto, un valor como &quot;2,5 meses&quot; no se puede comparar exactamente con una duración similar expresada en términos de semanas o días.</skos:note>
        <skos:note xml:lang="en">In the Gregorian calendar the length of the month is not fixed. Therefore, a value like &quot;2.5 months&quot; cannot be exactly compared with a similar duration expressed in terms of weeks or days.</skos:note>
    </owl:Class>
    


    <!-- http://www.w3.org/2006/time#GeneralDateTimeDescription -->

    <owl:Class rdf:about="http://www.w3.org/2006/time#GeneralDateTimeDescription">
        <rdfs:subClassOf rdf:resource="http://www.w3.org/2006/time#TemporalPosition"/>
        <rdfs:subClassOf>
            <owl:Restriction>
                <owl:onProperty rdf:resource="http://www.w3.org/2006/time#unitType"/>
                <owl:cardinality rdf:datatype="http://www.w3.org/2001/XMLSchema#nonNegativeInteger">1</owl:cardinality>
            </owl:Restriction>
        </rdfs:subClassOf>
        <rdfs:subClassOf>
            <owl:Restriction>
                <owl:onProperty rdf:resource="http://www.w3.org/2006/time#dayOfWeek"/>
                <owl:maxCardinality rdf:datatype="http://www.w3.org/2001/XMLSchema#nonNegativeInteger">1</owl:maxCardinality>
            </owl:Restriction>
        </rdfs:subClassOf>
        <rdfs:subClassOf>
            <owl:Restriction>
                <owl:onProperty rdf:resource="http://www.w3.org/2006/time#monthOfYear"/>
                <owl:maxCardinality rdf:datatype="http://www.w3.org/2001/XMLSchema#nonNegativeInteger">1</owl:maxCardinality>
            </owl:Restriction>
        </rdfs:subClassOf>
        <rdfs:subClassOf>
            <owl:Restriction>
                <owl:onProperty rdf:resource="http://www.w3.org/2006/time#timeZone"/>
                <owl:maxCardinality rdf:datatype="http://www.w3.org/2001/XMLSchema#nonNegativeInteger">1</owl:maxCardinality>
            </owl:Restriction>
        </rdfs:subClassOf>
        <rdfs:subClassOf>
            <owl:Restriction>
                <owl:onProperty rdf:resource="http://www.w3.org/2006/time#day"/>
                <owl:maxCardinality rdf:datatype="http://www.w3.org/2001/XMLSchema#nonNegativeInteger">1</owl:maxCardinality>
            </owl:Restriction>
        </rdfs:subClassOf>
        <rdfs:subClassOf>
            <owl:Restriction>
                <owl:onProperty rdf:resource="http://www.w3.org/2006/time#dayOfYear"/>
                <owl:maxCardinality rdf:datatype="http://www.w3.org/2001/XMLSchema#nonNegativeInteger">1</owl:maxCardinality>
            </owl:Restriction>
        </rdfs:subClassOf>
        <rdfs:subClassOf>
            <owl:Restriction>
                <owl:onProperty rdf:resource="http://www.w3.org/2006/time#hour"/>
                <owl:maxCardinality rdf:datatype="http://www.w3.org/2001/XMLSchema#nonNegativeInteger">1</owl:maxCardinality>
            </owl:Restriction>
        </rdfs:subClassOf>
        <rdfs:subClassOf>
            <owl:Restriction>
                <owl:onProperty rdf:resource="http://www.w3.org/2006/time#minute"/>
                <owl:maxCardinality rdf:datatype="http://www.w3.org/2001/XMLSchema#nonNegativeInteger">1</owl:maxCardinality>
            </owl:Restriction>
        </rdfs:subClassOf>
        <rdfs:subClassOf>
            <owl:Restriction>
                <owl:onProperty rdf:resource="http://www.w3.org/2006/time#month"/>
                <owl:maxCardinality rdf:datatype="http://www.w3.org/2001/XMLSchema#nonNegativeInteger">1</owl:maxCardinality>
            </owl:Restriction>
        </rdfs:subClassOf>
        <rdfs:subClassOf>
            <owl:Restriction>
                <owl:onProperty rdf:resource="http://www.w3.org/2006/time#second"/>
                <owl:maxCardinality rdf:datatype="http://www.w3.org/2001/XMLSchema#nonNegativeInteger">1</owl:maxCardinality>
            </owl:Restriction>
        </rdfs:subClassOf>
        <rdfs:subClassOf>
            <owl:Restriction>
                <owl:onProperty rdf:resource="http://www.w3.org/2006/time#week"/>
                <owl:maxCardinality rdf:datatype="http://www.w3.org/2001/XMLSchema#nonNegativeInteger">1</owl:maxCardinality>
            </owl:Restriction>
        </rdfs:subClassOf>
        <rdfs:subClassOf>
            <owl:Restriction>
                <owl:onProperty rdf:resource="http://www.w3.org/2006/time#year"/>
                <owl:maxCardinality rdf:datatype="http://www.w3.org/2001/XMLSchema#nonNegativeInteger">1</owl:maxCardinality>
            </owl:Restriction>
        </rdfs:subClassOf>
        <rdfs:comment xml:lang="es">Descripción de fecha y hora estructurada con valores separados para los distintos elementos de un sistema calendario-reloj.</rdfs:comment>
        <rdfs:comment xml:lang="en">Description of date and time structured with separate values for the various elements of a calendar-clock system</rdfs:comment>
        <rdfs:label xml:lang="en">Generalized date-time description</rdfs:label>
        <rdfs:label xml:lang="es">descripción de fecha-hora generalizada</rdfs:label>
        <skos:definition>Descripción de fecha y hora estructurada con valores separados para los distintos elementos de un sistema calendario-reloj.</skos:definition>
        <skos:definition xml:lang="en">Description of date and time structured with separate values for the various elements of a calendar-clock system</skos:definition>
        <skos:note xml:lang="es">Algunas combinaciones de propiedades son redundantes - por ejemplo, dentro de un &apos;año&apos; especificado si se proporciona &apos;día del año&apos; entonces &apos;día&apos; y &apos;mes&apos; se pueden computar, y viceversa. Los valores individuales deberían ser consistentes entre ellos y con el calendario, indicado a través del valor de la propiedad &apos;tiene TRS&apos;.</skos:note>
        <skos:note>Some combinations of properties are redundant - for example, within a specified :year if :dayOfYear is provided then :day and :month can be computed, and vice versa. Individual values should be consistent with each other and the calendar, indicated through the value of the :hasTRS property.</skos:note>
    </owl:Class>
    


    <!-- http://www.w3.org/2006/time#GeneralDurationDescription -->

    <owl:Class rdf:about="http://www.w3.org/2006/time#GeneralDurationDescription">
        <rdfs:subClassOf rdf:resource="http://www.w3.org/2006/time#TemporalDuration"/>
        <rdfs:subClassOf>
            <owl:Restriction>
                <owl:onProperty rdf:resource="http://www.w3.org/2006/time#hasTRS"/>
                <owl:cardinality rdf:datatype="http://www.w3.org/2001/XMLSchema#nonNegativeInteger">1</owl:cardinality>
            </owl:Restriction>
        </rdfs:subClassOf>
        <rdfs:subClassOf>
            <owl:Restriction>
                <owl:onProperty rdf:resource="http://www.w3.org/2006/time#days"/>
                <owl:maxCardinality rdf:datatype="http://www.w3.org/2001/XMLSchema#nonNegativeInteger">1</owl:maxCardinality>
            </owl:Restriction>
        </rdfs:subClassOf>
        <rdfs:subClassOf>
            <owl:Restriction>
                <owl:onProperty rdf:resource="http://www.w3.org/2006/time#hours"/>
                <owl:maxCardinality rdf:datatype="http://www.w3.org/2001/XMLSchema#nonNegativeInteger">1</owl:maxCardinality>
            </owl:Restriction>
        </rdfs:subClassOf>
        <rdfs:subClassOf>
            <owl:Restriction>
                <owl:onProperty rdf:resource="http://www.w3.org/2006/time#minutes"/>
                <owl:maxCardinality rdf:datatype="http://www.w3.org/2001/XMLSchema#nonNegativeInteger">1</owl:maxCardinality>
            </owl:Restriction>
        </rdfs:subClassOf>
        <rdfs:subClassOf>
            <owl:Restriction>
                <owl:onProperty rdf:resource="http://www.w3.org/2006/time#months"/>
                <owl:maxCardinality rdf:datatype="http://www.w3.org/2001/XMLSchema#nonNegativeInteger">1</owl:maxCardinality>
            </owl:Restriction>
        </rdfs:subClassOf>
        <rdfs:subClassOf>
            <owl:Restriction>
                <owl:onProperty rdf:resource="http://www.w3.org/2006/time#seconds"/>
                <owl:maxCardinality rdf:datatype="http://www.w3.org/2001/XMLSchema#nonNegativeInteger">1</owl:maxCardinality>
            </owl:Restriction>
        </rdfs:subClassOf>
        <rdfs:subClassOf>
            <owl:Restriction>
                <owl:onProperty rdf:resource="http://www.w3.org/2006/time#weeks"/>
                <owl:maxCardinality rdf:datatype="http://www.w3.org/2001/XMLSchema#nonNegativeInteger">1</owl:maxCardinality>
            </owl:Restriction>
        </rdfs:subClassOf>
        <rdfs:subClassOf>
            <owl:Restriction>
                <owl:onProperty rdf:resource="http://www.w3.org/2006/time#years"/>
                <owl:maxCardinality rdf:datatype="http://www.w3.org/2001/XMLSchema#nonNegativeInteger">1</owl:maxCardinality>
            </owl:Restriction>
        </rdfs:subClassOf>
        <rdfs:comment xml:lang="es">Descripción de extensión temporal estructurada con valores separados para los distintos elementos de un sistema de horario-calendario.</rdfs:comment>
        <rdfs:comment xml:lang="en">Description of temporal extent structured with separate values for the various elements of a calendar-clock system.</rdfs:comment>
        <rdfs:label xml:lang="en">Generalized duration description</rdfs:label>
        <rdfs:label xml:lang="es">descripción de duración generalizada</rdfs:label>
        <skos:definition xml:lang="es">Descripción de extensión temporal estructurada con valores separados para los distintos elementos de un sistema de horario-calendario.</skos:definition>
        <skos:definition xml:lang="en">Description of temporal extent structured with separate values for the various elements of a calendar-clock system.</skos:definition>
        <skos:note xml:lang="es">La extensión de una duración de tiempo expresada como una &apos;descripción de duración general&apos; depende del Sistema de Referencia Temporal. En algunos calendarios la longitud de la semana o del mes no es constante a lo largo del año. Por tanto, un valor como &quot;25 meses&quot; puede no ser necesariamente ser comparado con un duración similar expresada en términos de semanas o días. Cuando se consideran calendarios que no están basados en el movimiento de la Tierra, se deben tomar incluso más precauciones en la comparación de duraciones.</skos:note>
        <skos:note xml:lang="en">The extent of a time duration expressed as a GeneralDurationDescription depends on the Temporal Reference System. In some calendars the length of the week or month is not constant within the year. Therefore, a value like &quot;2.5 months&quot; may not necessarily be exactly compared with a similar duration expressed in terms of weeks or days. When non-earth-based calendars are considered even more care must be taken in comparing durations.</skos:note>
    </owl:Class>
    


    <!-- http://www.w3.org/2006/time#Instant -->

    <owl:Class rdf:about="http://www.w3.org/2006/time#Instant">
        <rdfs:subClassOf rdf:resource="http://purl.org/nemo/gufo#AbstractEntity"/>
        <rdfs:subClassOf rdf:resource="http://www.w3.org/2006/time#TemporalEntity"/>
        <owl:disjointWith rdf:resource="http://www.w3.org/2006/time#ProperInterval"/>
        <rdfs:comment xml:lang="en">A temporal entity with zero extent or duration</rdfs:comment>
        <rdfs:comment xml:lang="en">An gufo:AbstractIndividual that reifies time instants. It is used as a target of the gufo:hasBeginPoint and gufo:hasEndPoint object properties.</rdfs:comment>
        <rdfs:comment xml:lang="es">Una entidad temporal con una extensión o duración cero.</rdfs:comment>
        <rdfs:label xml:lang="en">Instant</rdfs:label>
        <rdfs:label xml:lang="en">Time instant</rdfs:label>
        <rdfs:label xml:lang="es">instante de tiempo.</rdfs:label>
        <skos:definition xml:lang="en">A temporal entity with zero extent or duration</skos:definition>
        <skos:definition xml:lang="es">Una entidad temporal con una extensión o duración cero.</skos:definition>
    </owl:Class>
    


    <!-- http://www.w3.org/2006/time#Interval -->

    <owl:Class rdf:about="http://www.w3.org/2006/time#Interval">
        <rdfs:subClassOf rdf:resource="http://www.w3.org/2006/time#TemporalEntity"/>
        <rdfs:comment xml:lang="en">A temporal entity with an extent or duration</rdfs:comment>
        <rdfs:comment xml:lang="es">Una entidad temporal con una extensión o duración.</rdfs:comment>
        <rdfs:label xml:lang="en">Time interval</rdfs:label>
        <rdfs:label xml:lang="es">intervalo de tiempo</rdfs:label>
        <skos:definition xml:lang="en">A temporal entity with an extent or duration</skos:definition>
        <skos:definition xml:lang="es">Una entidad temporal con una extensión o duración.</skos:definition>
    </owl:Class>
    


    <!-- http://www.w3.org/2006/time#MonthOfYear -->

    <owl:Class rdf:about="http://www.w3.org/2006/time#MonthOfYear">
        <rdfs:subClassOf rdf:resource="http://www.w3.org/2006/time#DateTimeDescription"/>
        <rdfs:subClassOf>
            <owl:Restriction>
                <owl:onProperty rdf:resource="http://www.w3.org/2006/time#unitType"/>
                <owl:hasValue rdf:resource="http://www.w3.org/2006/time#unitMonth"/>
            </owl:Restriction>
        </rdfs:subClassOf>
        <rdfs:subClassOf>
            <owl:Restriction>
                <owl:onProperty rdf:resource="http://www.w3.org/2006/time#day"/>
                <owl:cardinality rdf:datatype="http://www.w3.org/2001/XMLSchema#nonNegativeInteger">0</owl:cardinality>
            </owl:Restriction>
        </rdfs:subClassOf>
        <rdfs:subClassOf>
            <owl:Restriction>
                <owl:onProperty rdf:resource="http://www.w3.org/2006/time#hour"/>
                <owl:cardinality rdf:datatype="http://www.w3.org/2001/XMLSchema#nonNegativeInteger">0</owl:cardinality>
            </owl:Restriction>
        </rdfs:subClassOf>
        <rdfs:subClassOf>
            <owl:Restriction>
                <owl:onProperty rdf:resource="http://www.w3.org/2006/time#minute"/>
                <owl:cardinality rdf:datatype="http://www.w3.org/2001/XMLSchema#nonNegativeInteger">0</owl:cardinality>
            </owl:Restriction>
        </rdfs:subClassOf>
        <rdfs:subClassOf>
            <owl:Restriction>
                <owl:onProperty rdf:resource="http://www.w3.org/2006/time#month"/>
                <owl:cardinality rdf:datatype="http://www.w3.org/2001/XMLSchema#nonNegativeInteger">1</owl:cardinality>
            </owl:Restriction>
        </rdfs:subClassOf>
        <rdfs:subClassOf>
            <owl:Restriction>
                <owl:onProperty rdf:resource="http://www.w3.org/2006/time#second"/>
                <owl:cardinality rdf:datatype="http://www.w3.org/2001/XMLSchema#nonNegativeInteger">0</owl:cardinality>
            </owl:Restriction>
        </rdfs:subClassOf>
        <rdfs:subClassOf>
            <owl:Restriction>
                <owl:onProperty rdf:resource="http://www.w3.org/2006/time#week"/>
                <owl:cardinality rdf:datatype="http://www.w3.org/2001/XMLSchema#nonNegativeInteger">0</owl:cardinality>
            </owl:Restriction>
        </rdfs:subClassOf>
        <rdfs:subClassOf>
            <owl:Restriction>
                <owl:onProperty rdf:resource="http://www.w3.org/2006/time#year"/>
                <owl:cardinality rdf:datatype="http://www.w3.org/2001/XMLSchema#nonNegativeInteger">0</owl:cardinality>
            </owl:Restriction>
        </rdfs:subClassOf>
        <rdfs:comment xml:lang="es">El mes del año.</rdfs:comment>
        <rdfs:comment xml:lang="en">The month of the year</rdfs:comment>
        <rdfs:label xml:lang="en">Month of year</rdfs:label>
        <rdfs:label xml:lang="es">mes del año</rdfs:label>
        <skos:definition xml:lang="es">El mes del año.</skos:definition>
        <skos:definition xml:lang="en">The month of the year</skos:definition>
        <skos:editorialNote xml:lang="es">Característica en riesgo - añadida en la revisión de 2017, y no utilizada todavía de forma amplia.</skos:editorialNote>
        <skos:editorialNote xml:lang="en">Feature at risk - added in 2017 revision, and not yet widely used. </skos:editorialNote>
        <skos:note xml:lang="es">La pertenencia a la clase &apos;mes del año&apos; está abierta, a permitir calendarios anuales alternativos y diferentes nombres de meses.</skos:note>
        <skos:note xml:lang="en">Membership of the class :MonthOfYear is open, to allow for alternative annual calendars and different month names.</skos:note>
    </owl:Class>
    


    <!-- http://www.w3.org/2006/time#ProperInterval -->

    <owl:Class rdf:about="http://www.w3.org/2006/time#ProperInterval">
        <rdfs:subClassOf rdf:resource="http://www.w3.org/2006/time#Interval"/>
        <rdfs:comment xml:lang="en">A temporal entity with non-zero extent or duration, i.e. for which the value of the beginning and end are different</rdfs:comment>
        <rdfs:comment xml:lang="es">Una entidad temporal con extensión o duración distinta de cero, es decir, para la cual los valores de principio y fin del intervalo son diferentes.</rdfs:comment>
        <rdfs:label xml:lang="en">Proper interval</rdfs:label>
        <rdfs:label xml:lang="es">intervalo propio</rdfs:label>
        <skos:definition xml:lang="en">A temporal entity with non-zero extent or duration, i.e. for which the value of the beginning and end are different</skos:definition>
        <skos:definition xml:lang="es">Una entidad temporal con extensión o duración distinta de cero, es decir, para la cual los valores de principio y fin del intervalo son diferentes.</skos:definition>
    </owl:Class>
    


    <!-- http://www.w3.org/2006/time#TRS -->

    <owl:Class rdf:about="http://www.w3.org/2006/time#TRS">
        <rdfs:comment xml:lang="en">A temporal reference system, such as a temporal coordinate system (with an origin, direction, and scale), a calendar-clock combination, or a (possibly hierarchical) ordinal system. 

This is a stub class, representing the set of all temporal reference systems.</rdfs:comment>
        <rdfs:comment xml:lang="es">Un sistema de referencia temporal, tal como un sistema de coordenadas temporales (con un origen, una dirección y una escala), una combinación calendario-reloj, o un sistema ordinal (posiblemente jerárquico).
        Esta clase comodín representa el conjunto de todos los sistemas de referencia temporal.</rdfs:comment>
        <rdfs:label xml:lang="en">Temporal Reference System</rdfs:label>
        <rdfs:label xml:lang="es">sistema de referencia temporal</rdfs:label>
        <skos:definition xml:lang="en">A temporal reference system, such as a temporal coordinate system (with an origin, direction, and scale), a calendar-clock combination, or a (possibly hierarchical) ordinal system. 

This is a stub class, representing the set of all temporal reference systems.</skos:definition>
        <skos:definition xml:lang="es">Un sistema de referencia temporal, tal como un sistema de coordenadas temporales (con un origen, una dirección y una escala), una combinación calendario-reloj, o un sistema ordinal (posiblemente jerárquico).
    Esta clase comodín representa el conjunto de todos los sistemas de referencia temporal.</skos:definition>
        <skos:note xml:lang="en">A taxonomy of temporal reference systems is provided in ISO 19108:2002 [ISO19108], including (a) calendar + clock systems; (b) temporal coordinate systems (i.e. numeric offset from an epoch); (c) temporal ordinal reference systems (i.e. ordered sequence of named intervals, not necessarily of equal duration).</skos:note>
        <skos:note xml:lang="es">En el ISO 19108:2002 [ISO19108] se proporciona una taxonomía de sistemas de referencia temporal, incluyendo (a) sistemas de calendario + reloj; (b) sistemas de coordenadas temporales (es decir, desplazamiento numérico a partir de una época); (c) sistemas de referencia ordinales temporales (es decir, secuencia ordenada de intervalos nombrados, no necesariamente de igual duración).</skos:note>
    </owl:Class>
    


    <!-- http://www.w3.org/2006/time#TemporalDuration -->

    <owl:Class rdf:about="http://www.w3.org/2006/time#TemporalDuration">
        <rdfs:comment xml:lang="es">Extensión de tiempo; duración de un intervalo de tiempo independiente de su posición de inicio particular.</rdfs:comment>
        <rdfs:comment xml:lang="en">Time extent; duration of a time interval separate from its particular start position</rdfs:comment>
        <rdfs:label xml:lang="en">Temporal duration</rdfs:label>
        <rdfs:label xml:lang="es">duración temporal</rdfs:label>
        <skos:definition xml:lang="es">Extensión de tiempo; duración de un intervalo de tiempo independiente de su posición de inicio particular.</skos:definition>
        <skos:definition xml:lang="en">Time extent; duration of a time interval separate from its particular start position</skos:definition>
    </owl:Class>
    


    <!-- http://www.w3.org/2006/time#TemporalEntity -->

    <owl:Class rdf:about="http://www.w3.org/2006/time#TemporalEntity">
        <owl:equivalentClass>
            <owl:Class>
                <owl:unionOf rdf:parseType="Collection">
                    <rdf:Description rdf:about="http://www.w3.org/2006/time#Instant"/>
                    <rdf:Description rdf:about="http://www.w3.org/2006/time#Interval"/>
                </owl:unionOf>
            </owl:Class>
        </owl:equivalentClass>
        <rdfs:subClassOf rdf:resource="http://www.w3.org/2002/07/owl#Thing"/>
        <rdfs:comment xml:lang="en">A temporal interval or instant.</rdfs:comment>
        <rdfs:comment xml:lang="es">Un intervalo temporal o un instante.</rdfs:comment>
        <rdfs:label xml:lang="en">Temporal entity</rdfs:label>
        <rdfs:label xml:lang="es">entidad temporal</rdfs:label>
        <skos:definition xml:lang="en">A temporal interval or instant.</skos:definition>
        <skos:definition xml:lang="es">Un intervalo temporal o un instante.</skos:definition>
    </owl:Class>
    


    <!-- http://www.w3.org/2006/time#TemporalPosition -->

    <owl:Class rdf:about="http://www.w3.org/2006/time#TemporalPosition">
        <rdfs:subClassOf>
            <owl:Restriction>
                <owl:onProperty rdf:resource="http://www.w3.org/2006/time#hasTRS"/>
                <owl:cardinality rdf:datatype="http://www.w3.org/2001/XMLSchema#nonNegativeInteger">1</owl:cardinality>
            </owl:Restriction>
        </rdfs:subClassOf>
        <rdfs:comment xml:lang="en">A position on a time-line</rdfs:comment>
        <rdfs:comment xml:lang="es">Una posición sobre una línea de tiempo.</rdfs:comment>
        <rdfs:label xml:lang="en">Temporal position</rdfs:label>
        <rdfs:label xml:lang="es">posición temporal</rdfs:label>
        <skos:definition xml:lang="en">A position on a time-line</skos:definition>
        <skos:definition xml:lang="es">Una posición sobre una línea de tiempo.</skos:definition>
    </owl:Class>
    


    <!-- http://www.w3.org/2006/time#TemporalUnit -->

    <owl:Class rdf:about="http://www.w3.org/2006/time#TemporalUnit">
        <rdfs:subClassOf rdf:resource="http://www.w3.org/2006/time#TemporalDuration"/>
        <rdfs:comment xml:lang="en">A standard duration, which provides a scale factor for a time extent, or the granularity or precision for a time position.</rdfs:comment>
        <rdfs:comment xml:lang="es">Una duración estándar, que proporciona un factor de escala para una extensión de tiempo, o la granularidad o precisión para una posición de tiempo.</rdfs:comment>
        <rdfs:label xml:lang="en">Temporal unit</rdfs:label>
        <rdfs:label xml:lang="es">unidad de tiempo</rdfs:label>
        <skos:changeNote xml:lang="en">Remove enumeration from definition, in order to allow other units to be used when required in other coordinate systems. 
NOTE: existing units are still present as members of the class, but the class membership is now open. 

In the original OWL-Time the following constraint appeared: 
  owl:oneOf (
      time:unitSecond
      time:unitMinute
      time:unitHour
      time:unitDay
      time:unitWeek
      time:unitMonth
      time:unitYear
    ) ;</skos:changeNote>
        <skos:definition xml:lang="en">A standard duration, which provides a scale factor for a time extent, or the granularity or precision for a time position.</skos:definition>
        <skos:definition xml:lang="es">Una duración estándar, que proporciona un factor de escala para una extensión de tiempo, o la granularidad o precisión para una posición de tiempo.</skos:definition>
        <skos:note xml:lang="es">La pertenencia de la clase &apos;unidad de tiempo&apos; está abierta, para permitir otras unidades de tiempo utilizadas en algunas aplicaciones técnicas (por ejemplo, millones de años o el mes Baha&apos;i).</skos:note>
        <skos:note xml:lang="en">Membership of the class TemporalUnit is open, to allow for other temporal units used in some technical applications (e.g. millions of years, Baha&apos;i month).</skos:note>
    </owl:Class>
    


    <!-- http://www.w3.org/2006/time#TimePosition -->

    <owl:Class rdf:about="http://www.w3.org/2006/time#TimePosition">
        <rdfs:subClassOf rdf:resource="http://www.w3.org/2006/time#TemporalPosition"/>
        <rdfs:subClassOf>
            <owl:Class>
                <owl:unionOf rdf:parseType="Collection">
                    <owl:Restriction>
                        <owl:onProperty rdf:resource="http://www.w3.org/2006/time#nominalPosition"/>
                        <owl:cardinality rdf:datatype="http://www.w3.org/2001/XMLSchema#nonNegativeInteger">1</owl:cardinality>
                    </owl:Restriction>
                    <owl:Restriction>
                        <owl:onProperty rdf:resource="http://www.w3.org/2006/time#numericPosition"/>
                        <owl:cardinality rdf:datatype="http://www.w3.org/2001/XMLSchema#nonNegativeInteger">1</owl:cardinality>
                    </owl:Restriction>
                </owl:unionOf>
            </owl:Class>
        </rdfs:subClassOf>
        <rdfs:comment xml:lang="en">A temporal position described using either a (nominal) value from an ordinal reference system, or a (numeric) value in a temporal coordinate system. </rdfs:comment>
        <rdfs:comment xml:lang="es">Una posición temporal descrita utilizando bien un valor (nominal) de un sistema de referencia ordinal, o un valor (numérico) en un sistema de coordenadas temporales.</rdfs:comment>
        <rdfs:label xml:lang="en">Time position</rdfs:label>
        <rdfs:label xml:lang="es">posición de tiempo</rdfs:label>
        <skos:definition xml:lang="en">A temporal position described using either a (nominal) value from an ordinal reference system, or a (numeric) value in a temporal coordinate system. </skos:definition>
        <skos:definition xml:lang="es">Una posición temporal descrita utilizando bien un valor (nominal) de un sistema de referencia ordinal, o un valor (numérico) en un sistema de coordenadas temporales.</skos:definition>
    </owl:Class>
    


    <!-- http://www.w3.org/2006/time#TimeZone -->

    <owl:Class rdf:about="http://www.w3.org/2006/time#TimeZone">
        <rdfs:comment xml:lang="en">A Time Zone specifies the amount by which the local time is offset from UTC. 
	A time zone is usually denoted geographically (e.g. Australian Eastern Daylight Time), with a constant value in a given region. 
The region where it applies and the offset from UTC are specified by a locally recognised governing authority.</rdfs:comment>
        <rdfs:comment xml:lang="es">Un huso horario especifica la cantidad en que la hora local está desplazada con respecto a UTC.
        Un huso horario normalmente se denota geográficamente (p.ej. el horario de verano del este de Australia), con un valor constante en una región dada.
        La región donde aplica y el desplazamiento desde UTC las especifica una autoridad gubernamental localmente reconocida.</rdfs:comment>
        <rdfs:label xml:lang="en">Time Zone</rdfs:label>
        <rdfs:label xml:lang="es">huso horario</rdfs:label>
        <skos:definition xml:lang="en">A Time Zone specifies the amount by which the local time is offset from UTC. 
	A time zone is usually denoted geographically (e.g. Australian Eastern Daylight Time), with a constant value in a given region. 
The region where it applies and the offset from UTC are specified by a locally recognised governing authority.</skos:definition>
        <skos:definition xml:lang="es">Un huso horario especifica la cantidad en que la hora local está desplazada con respecto a UTC.
    Un huso horario normalmente se denota geográficamente (p.ej. el horario de verano del este de Australia), con un valor constante en una región dada.
    La región donde aplica y el desplazamiento desde UTC las especifica una autoridad gubernamental localmente reconocida.</skos:definition>
        <skos:historyNote xml:lang="es">En la versión original de OWL-Time de 2006, se definió, en un espacio de nombres diferente &quot;http://www.w3.org/2006/timezone#&quot;, la clase &apos;huso horario&apos;, con varias propiedades específicas correspondientes a un modelo específico de huso horario.
    En la versión actual hay una clase con el mismo nombre local en el espacio de nombres de OWL-Time, eliminando la dependencia del espacio de nombres externo.
    Un axioma de alineación permite que los datos codificados de acuerdo con la versión anterior sean consistentes con la ontología actualizada.</skos:historyNote>
        <skos:historyNote>In the original 2006 version of OWL-Time, the TimeZone class, with several properties corresponding to a specific model of time-zones, was defined in a separate namespace &quot;http://www.w3.org/2006/timezone#&quot;. 

In the current version a class with same local name is put into the main OWL-Time namespace, removing the dependency on the external namespace. 

An alignment axiom 
	tzont:TimeZone rdfs:subClassOf time:TimeZone . 
allows data encoded according to the previous version to be consistent with the updated ontology. </skos:historyNote>
        <skos:note xml:lang="en">A designated timezone is associated with a geographic region. However, for a particular region the offset from UTC often varies seasonally, and the dates of the changes may vary from year to year. The timezone designation usually changes for the different seasons (e.g. Australian Eastern Standard Time vs. Australian Eastern Daylight Time). Furthermore, the offset for a timezone may change over longer timescales, though its designation might not.  

Detailed guidance about working with time zones is given in http://www.w3.org/TR/timezone/ .</skos:note>
        <skos:note xml:lang="en">An ontology for time zone descriptions was described in [owl-time-20060927] and provided as RDF in a separate namespace tzont:. However, that ontology was incomplete in scope, and the example datasets were selective. Furthermore, since the use of a class from an external ontology as the range of an ObjectProperty in OWL-Time creates a dependency, reference to the time zone class has been replaced with the &apos;stub&apos; class in the normative part of this version of OWL-Time.</skos:note>
        <skos:note xml:lang="es">Un huso horario designado está asociado con una región geográfica. Sin embargo, para una región particular el desplazamiento desde UTC a menudo varía según las estaciones, y las fechas de los cambios pueden variar de un año a otro. La designación de huso horario  normalmente cambia de una estación a otra (por ejemplo, el horario estándar frente al horario de verano ambos del este de Australia). Además, del desplazamiento para un huso horario puede cambiar sobre escalas de tiempo mayores, aunque su designación no lo haga.
    Se puede encontrar una guía detallada sobre el funcionamiento de husos horarios en http://www.w3.org/TR/timezone/.&quot;@es , &quot;En [owl-time-20060927] se describió una ontología para descripciones de husos horarios, y se proporcionó en un espacio de nombres separado tzont:. Sin embargo, dicha ontología estaba incompleta en su alcance, y el ejemplo de conjuntos de datos (datasets) era selectivo. Además, puesto que el uso de una clase de una ontología externa como el rango de una propiedad de objeto en OWL-Time crea una dependencia, la referencia a la clase huso horario se ha reemplazado por una clase que viene a ser un &quot;cajón de sastre&quot; en la en la parte normativa de esta versión de OWL-Time.</skos:note>
        <skos:scopeNote xml:lang="es">En esta implementación &apos;huso horario&apos; no tiene definidas propiedades. Se debería pensar como una superclase &quot;abstracta&quot; de todas las implementaciones de huso horario específicas.</skos:scopeNote>
        <skos:scopeNote>In this implementation TimeZone has no properties defined. It should be thought of as an &apos;abstract&apos; superclass of all specific timezone implementations.</skos:scopeNote>
    </owl:Class>
    


    <!-- http://www.w3.org/2006/time#Year -->

    <owl:Class rdf:about="http://www.w3.org/2006/time#Year">
        <rdfs:subClassOf rdf:resource="http://www.w3.org/2006/time#DurationDescription"/>
        <rdfs:subClassOf>
            <owl:Restriction>
                <owl:onProperty rdf:resource="http://www.w3.org/2006/time#days"/>
                <owl:cardinality rdf:datatype="http://www.w3.org/2001/XMLSchema#nonNegativeInteger">0</owl:cardinality>
            </owl:Restriction>
        </rdfs:subClassOf>
        <rdfs:subClassOf>
            <owl:Restriction>
                <owl:onProperty rdf:resource="http://www.w3.org/2006/time#hours"/>
                <owl:cardinality rdf:datatype="http://www.w3.org/2001/XMLSchema#nonNegativeInteger">0</owl:cardinality>
            </owl:Restriction>
        </rdfs:subClassOf>
        <rdfs:subClassOf>
            <owl:Restriction>
                <owl:onProperty rdf:resource="http://www.w3.org/2006/time#minutes"/>
                <owl:cardinality rdf:datatype="http://www.w3.org/2001/XMLSchema#nonNegativeInteger">0</owl:cardinality>
            </owl:Restriction>
        </rdfs:subClassOf>
        <rdfs:subClassOf>
            <owl:Restriction>
                <owl:onProperty rdf:resource="http://www.w3.org/2006/time#months"/>
                <owl:cardinality rdf:datatype="http://www.w3.org/2001/XMLSchema#nonNegativeInteger">0</owl:cardinality>
            </owl:Restriction>
        </rdfs:subClassOf>
        <rdfs:subClassOf>
            <owl:Restriction>
                <owl:onProperty rdf:resource="http://www.w3.org/2006/time#seconds"/>
                <owl:cardinality rdf:datatype="http://www.w3.org/2001/XMLSchema#nonNegativeInteger">0</owl:cardinality>
            </owl:Restriction>
        </rdfs:subClassOf>
        <rdfs:subClassOf>
            <owl:Restriction>
                <owl:onProperty rdf:resource="http://www.w3.org/2006/time#weeks"/>
                <owl:cardinality rdf:datatype="http://www.w3.org/2001/XMLSchema#nonNegativeInteger">0</owl:cardinality>
            </owl:Restriction>
        </rdfs:subClassOf>
        <rdfs:subClassOf>
            <owl:Restriction>
                <owl:onProperty rdf:resource="http://www.w3.org/2006/time#years"/>
                <owl:cardinality rdf:datatype="http://www.w3.org/2001/XMLSchema#nonNegativeInteger">1</owl:cardinality>
            </owl:Restriction>
        </rdfs:subClassOf>
        <rdfs:comment>Year duration</rdfs:comment>
        <rdfs:label xml:lang="en">Year</rdfs:label>
        <owl:deprecated rdf:datatype="http://www.w3.org/2001/XMLSchema#boolean">true</owl:deprecated>
        <skos:definition>Year duration</skos:definition>
        <skos:historyNote>Year was proposed in the 2006 version of OWL-Time as an example of how DurationDescription could be specialized to allow for a duration to be restricted to a number of years. 

It is deprecated in this edition of OWL-Time. </skos:historyNote>
        <skos:prefLabel xml:lang="it">Anno</skos:prefLabel>
        <skos:prefLabel xml:lang="fr">Année (calendrier)</skos:prefLabel>
        <skos:prefLabel xml:lang="pt">Ano</skos:prefLabel>
        <skos:prefLabel xml:lang="es">Año</skos:prefLabel>
        <skos:prefLabel xml:lang="nl">Jaar</skos:prefLabel>
        <skos:prefLabel xml:lang="de">Jahr</skos:prefLabel>
        <skos:prefLabel xml:lang="pl">Rok</skos:prefLabel>
        <skos:prefLabel xml:lang="en">Year</skos:prefLabel>
        <skos:prefLabel xml:lang="ru">Год</skos:prefLabel>
        <skos:prefLabel xml:lang="ar">سنة</skos:prefLabel>
        <skos:prefLabel xml:lang="ja">年</skos:prefLabel>
        <skos:prefLabel xml:lang="zh">年</skos:prefLabel>
    </owl:Class>
    


    <!-- https://w3id.org/def/propaphen#Observation -->

    <owl:Class rdf:about="https://w3id.org/def/propaphen#Observation">
        <rdfs:subClassOf>
            <owl:Class>
                <owl:intersectionOf rdf:parseType="Collection">
                    <rdf:Description rdf:about="http://purl.org/nemo/gufo#Perdurants"/>
                    <owl:Class>
                        <owl:complementOf rdf:resource="https://w3id.org/def/propaphen#Phenomenon"/>
                    </owl:Class>
                    <owl:Class>
                        <owl:complementOf rdf:resource="https://w3id.org/def/propaphen#PhenomenonOccurrence"/>
                    </owl:Class>
                    <owl:Class>
                        <owl:complementOf rdf:resource="https://w3id.org/def/propaphen#Presence"/>
                    </owl:Class>
                    <owl:Restriction>
                        <owl:onProperty rdf:resource="https://w3id.org/def/propaphen#observationOf"/>
                        <owl:someValuesFrom rdf:resource="https://w3id.org/def/propaphen#PhenomenonOccurrence"/>
                    </owl:Restriction>
                </owl:intersectionOf>
            </owl:Class>
        </rdfs:subClassOf>
        <rdfs:comment rdf:datatype="http://www.w3.org/2001/XMLSchema#string">As a propagation phenomenon is still a general phenomenon (&quot;
            Smith, David Woodruff. « Phenomenology ». The Stanford Encyclopedia of Philosophy, édité par Edward N. Zalta, Summer 2018, Metaphysics Research Lab, Stanford University, 2018. Stanford Encyclopedia of Philosophy, https://plato.stanford.edu/archives/sum2018/entries/phenomenology/.
            &quot;), different points of view or observations may result in different experiences. A phen:Observation is a gufo:Perdurant that represents a spatial-temporal perspective of a phen:PhenomenonOccurrence (i.e., two observations from different people may differ in the number of details one can give).

            In practice, a phen:Observation may be used to identify what gufo:Individual are participating in a phen:PhenomenonOccurrence for a given node of the network for a given time interval.

            As phen:Observation designs a spatial-temporal cluster itself, it can be used to track valid spatial-temporal paths between several pairs of phen:Observation.</rdfs:comment>
        <rdfs:label rdf:datatype="http://www.w3.org/2001/XMLSchema#string">Observation of Propagation Phenomenon Occurrence</rdfs:label>
    </owl:Class>
    


    <!-- https://w3id.org/def/propaphen#Phenomenon -->

    <owl:Class rdf:about="https://w3id.org/def/propaphen#Phenomenon">
        <rdfs:subClassOf>
            <owl:Class>
                <owl:intersectionOf rdf:parseType="Collection">
                    <rdf:Description rdf:about="http://purl.org/nemo/gufo#Perdurants"/>
                    <owl:Class>
                        <owl:complementOf rdf:resource="https://w3id.org/def/propaphen#Observation"/>
                    </owl:Class>
                    <owl:Class>
                        <owl:complementOf rdf:resource="https://w3id.org/def/propaphen#PhenomenonOccurrence"/>
                    </owl:Class>
                    <owl:Class>
                        <owl:complementOf rdf:resource="https://w3id.org/def/propaphen#Presence"/>
                    </owl:Class>
                </owl:intersectionOf>
            </owl:Class>
        </rdfs:subClassOf>
        <rdfs:comment rdf:datatype="http://www.w3.org/2001/XMLSchema#string">It is based on the meaning of the Propagation Phenomenon presented by &quot;Król, Dariusz, Damien Fay, et Bogdan Gabryś, éd. Propagation Phenomena in Real World Networks. Vol. 85. Intelligent Systems Reference Library. Cham: Springer International Publishing, 2015. https://doi.org/10.1007/978-3-319-15916-4.&quot;
        A phenomenon is a gufo:Perdurant that defines a fact or event of scientific interest susceptible to scientific description and explanation (Merriam-Webster dictionary). It does not define the occurrence of a phenomenon but the study of a type of it (i.e., Epidemic phenomena such as COVID-19, Influenza, etc.). As the mentioned phenomena, the study of a phenomenon may only be valid from the first occurrence of it until the last occurrence of it.</rdfs:comment>
        <rdfs:label>Propagation Phenomenon Type</rdfs:label>
    </owl:Class>
    


    <!-- https://w3id.org/def/propaphen#PhenomenonOccurrence -->

    <owl:Class rdf:about="https://w3id.org/def/propaphen#PhenomenonOccurrence">
        <rdfs:subClassOf>
            <owl:Class>
                <owl:intersectionOf rdf:parseType="Collection">
                    <rdf:Description rdf:about="http://purl.org/nemo/gufo#Perdurants"/>
                    <owl:Class>
                        <owl:complementOf rdf:resource="https://w3id.org/def/propaphen#Observation"/>
                    </owl:Class>
                    <owl:Class>
                        <owl:complementOf rdf:resource="https://w3id.org/def/propaphen#Phenomenon"/>
                    </owl:Class>
                    <owl:Class>
                        <owl:complementOf rdf:resource="https://w3id.org/def/propaphen#Presence"/>
                    </owl:Class>
                    <owl:Restriction>
                        <owl:onProperty rdf:resource="https://w3id.org/def/propaphen#fromPhenomenon"/>
                        <owl:qualifiedCardinality rdf:datatype="http://www.w3.org/2001/XMLSchema#nonNegativeInteger">1</owl:qualifiedCardinality>
                        <owl:onClass rdf:resource="https://w3id.org/def/propaphen#Phenomenon"/>
                    </owl:Restriction>
                </owl:intersectionOf>
            </owl:Class>
        </rdfs:subClassOf>
        <rdfs:comment rdf:datatype="http://www.w3.org/2001/XMLSchema#string">A gufo:Perdurant that represents the occurrence of a phen:Phenomenon. Similar to the concept of the occurrence of information being propagated in the social information propagation phenomenon on &quot;Król, Dariusz, Damien Fay, et Bogdan Gabryś, éd. Propagation Phenomena in Real World Networks. Vol. 85. Intelligent Systems Reference Library. Cham: Springer International Publishing, 2015. https://doi.org/10.1007/978-3-319-15916-4.&quot;. Another example would be an outburst in a network from a particular virus type.

        For example, the occurrence of a hurricane in Paris is different from the occurrence of a hurricane in the United States if they are happening simultaneously. Therefore, they are two different instances of phen:PhenomenonOccurrence of the same phen:Phenomenon (Hurricane).</rdfs:comment>
        <rdfs:label rdf:datatype="http://www.w3.org/2001/XMLSchema#string">Phenomenon Occurrence</rdfs:label>
    </owl:Class>
    


    <!-- https://w3id.org/def/propaphen#Presence -->

    <owl:Class rdf:about="https://w3id.org/def/propaphen#Presence">
        <rdfs:subClassOf>
            <owl:Class>
                <owl:intersectionOf rdf:parseType="Collection">
                    <rdf:Description rdf:about="http://purl.org/nemo/gufo#Perdurants"/>
                    <owl:Class>
                        <owl:complementOf rdf:resource="https://w3id.org/def/propaphen#Observation"/>
                    </owl:Class>
                    <owl:Class>
                        <owl:complementOf rdf:resource="https://w3id.org/def/propaphen#Phenomenon"/>
                    </owl:Class>
                    <owl:Class>
                        <owl:complementOf rdf:resource="https://w3id.org/def/propaphen#PhenomenonOccurrence"/>
                    </owl:Class>
                    <owl:Restriction>
                        <owl:onProperty rdf:resource="https://w3id.org/def/propaphen#observationalPresenceIn"/>
                        <owl:someValuesFrom rdf:resource="https://w3id.org/def/propaphen#Observation"/>
                    </owl:Restriction>
                    <owl:Restriction>
                        <owl:onProperty rdf:resource="https://w3id.org/def/propaphen#presenceOf"/>
                        <owl:someValuesFrom rdf:resource="http://purl.org/nemo/gufo#Entity"/>
                    </owl:Restriction>
                </owl:intersectionOf>
            </owl:Class>
        </rdfs:subClassOf>
        <rdfs:comment rdf:datatype="http://www.w3.org/2001/XMLSchema#string">A gufo:Perdurant whose sole purpose is to identify the presence of instances of gufo:Individual in a node of the network or, consequently, in a phen:Observation for a given time interval.</rdfs:comment>
        <rdfs:label rdf:datatype="http://www.w3.org/2001/XMLSchema#string">Presence of entities in a network node</rdfs:label>
    </owl:Class>
    


    <!-- https://w3id.org/seas/Connection -->

    <owl:Class rdf:about="https://w3id.org/seas/Connection">
        <rdfs:subClassOf rdf:resource="http://purl.org/nemo/gufo#Perdurants"/>
        <rdfs:subClassOf>
            <owl:Restriction>
                <owl:onProperty rdf:resource="https://w3id.org/seas/connectsSystem"/>
                <owl:someValuesFrom rdf:resource="https://w3id.org/seas/System"/>
            </owl:Restriction>
        </rdfs:subClassOf>
        <rdfs:subClassOf>
            <owl:Restriction>
                <owl:onProperty rdf:resource="https://w3id.org/seas/connectsSystemAt"/>
                <owl:someValuesFrom rdf:resource="https://w3id.org/seas/ConnectionPoint"/>
            </owl:Restriction>
        </rdfs:subClassOf>
        <owl:disjointWith rdf:resource="https://w3id.org/seas/ConnectionPoint"/>
        <owl:disjointWith rdf:resource="https://w3id.org/seas/System"/>
        <rdfs:comment xml:lang="en">The class of connections between systems.

This class qualifies property `seas:connectedTo`. 

A connection describes potential interactions between systems. 

For example, a power connection between power systems describes the fact that these systems may exchange electricity.

```
&lt;connection&gt; seas:connectsSystem &lt;electric_vehicle&gt; , &lt;electric_vehicle_service_equipment&gt; .
&lt;electric_vehicle&gt; seas:connectedThrough &lt;connection&gt; .
&lt;electric_vehicle_service_equipment&gt; seas:connectedThrough &lt;connection&gt; .
```

Any two connected systems are connected through a connection. If:

```
&lt;system1&gt; a seas:System .
&lt;system2&gt; a seas:System .
&lt;system1&gt; seas:connectedTo &lt;system2&gt; .
```

then there exists `_:connection` such that:

```
_:connection seas:connectsSystem &lt;system1&gt; , &lt;system2&gt; .
```

A connection can connect more than two systems at the same time.


Figure below illustrates connections of systems:

[![Connections of systems](https://w3id.org/seas/system2.png)](https://w3id.org/seas/system2.png)

</rdfs:comment>
        <rdfs:isDefinedBy rdf:resource="https://w3id.org/seas/SystemOntology"/>
        <rdfs:label xml:lang="en">Connection</rdfs:label>
        <ns1:term_status>stable</ns1:term_status>
    </owl:Class>
    


    <!-- https://w3id.org/seas/ConnectionPoint -->

    <owl:Class rdf:about="https://w3id.org/seas/ConnectionPoint">
        <rdfs:subClassOf rdf:resource="http://www.opengis.net/ont/geosparql#Feature"/>
        <rdfs:subClassOf>
            <owl:Restriction>
                <owl:onProperty rdf:resource="https://w3id.org/seas/connectionPointOf"/>
                <owl:cardinality rdf:datatype="http://www.w3.org/2001/XMLSchema#nonNegativeInteger">1</owl:cardinality>
            </owl:Restriction>
        </rdfs:subClassOf>
        <owl:disjointWith rdf:resource="https://w3id.org/seas/System"/>
        <rdfs:comment xml:lang="en">The class of connection points of systems, at which they may be connected to other systems.

This class qualifies properties `seas:connectsSystem` and `seas:connectedThrough`.

A connection point belongs to exactly one system.


For example, an electric vehicle service equipment may have three power connection points: two different kinds of plugs that enable to charge electric vehicles, and a three phase power bus connection point to the grid:

```
&lt;electric_vehicle&gt; seas:connectsAt &lt;plug_high_voltage&gt; , &lt;normal_plug&gt; , &lt;three_phase_connection_point&gt; .
```


Any system connected through a connection is connected at one of its connection points to the connection:
  if:

```
&lt;system&gt; a seas:System .
&lt;system&gt; seas:connectedThrough &lt;connection&gt; .
&lt;connection&gt; a seas:Connection .
```

  then there exists `_:connectionPoint` such that:

```
&lt;system&gt; seas:connectsAt _:connectionPoint .

_:connectionPoint seas:connectsSystemAt &lt;connection&gt; .
```


The system of a connection point that is connected through a connection is itself connected through the connection:. If:

```
&lt;connection&gt; a seas:Connection .
&lt;system&gt; a seas:System .
&lt;connectionPoint&gt; a seas:ConnectionPoint ;
&lt;connectionPoint&gt; seas:connectsSystemThrough &lt;connection&gt; .
```

then it is true that:

```
&lt;connectionPoint&gt; seas:connectionPointOf &lt;system&gt; .
```

Figure below illustrates connection points of systems:

[![Connection points of systems](https://w3id.org/seas/system3.png)](https://w3id.org/seas/system3.png)

</rdfs:comment>
        <rdfs:isDefinedBy rdf:resource="https://w3id.org/seas/SystemOntology"/>
        <rdfs:label xml:lang="en">Connection Point</rdfs:label>
        <ns1:term_status>stable</ns1:term_status>
    </owl:Class>
    


    <!-- https://w3id.org/seas/System -->

    <owl:Class rdf:about="https://w3id.org/seas/System">
        <rdfs:subClassOf rdf:resource="http://www.opengis.net/ont/geosparql#Feature"/>
        <rdfs:comment xml:lang="en">The class of systems, i.e., systems virtually isolated from the environment, whose behaviour and interactions with the environment are modeled.

  Systems can be connected to other systems. Connected systems interact in some ways. For example:

```
&lt;electric_vehicle&gt; seas:connectedTo &lt;electric_vehicle_service_equipment&gt; .
```

  Systems can also have subsystems. Properties of subsystems somehow contribute to the properties of the supersystem. For example:

```
&lt;battery&gt; seas:subSystemOf &lt;electric_vehicle&gt; .
```

Figure below illustrates systems and their connections:

[![Systems and their connections](https://w3id.org/seas/system1.png)](https://w3id.org/seas/system1.png)

</rdfs:comment>
        <rdfs:isDefinedBy rdf:resource="https://w3id.org/seas/SystemOntology"/>
        <rdfs:label xml:lang="en">System</rdfs:label>
        <ns1:term_status>stable</ns1:term_status>
    </owl:Class>
    


    <!-- 
    ///////////////////////////////////////////////////////////////////////////////////////
    //
    // Individuals
    //
    ///////////////////////////////////////////////////////////////////////////////////////
     -->

    


    <!-- http://www.w3.org/2006/time#Friday -->

    <owl:NamedIndividual rdf:about="http://www.w3.org/2006/time#Friday">
        <rdf:type rdf:resource="http://www.w3.org/2006/time#DayOfWeek"/>
        <rdfs:label xml:lang="en">Friday</rdfs:label>
        <skos:prefLabel xml:lang="de">Freitag</skos:prefLabel>
        <skos:prefLabel xml:lang="en">Friday</skos:prefLabel>
        <skos:prefLabel xml:lang="pl">Piątek</skos:prefLabel>
        <skos:prefLabel xml:lang="pt">Sexta-feira</skos:prefLabel>
        <skos:prefLabel xml:lang="fr">Vendredi</skos:prefLabel>
        <skos:prefLabel xml:lang="it">Venerdì</skos:prefLabel>
        <skos:prefLabel xml:lang="es">Viernes</skos:prefLabel>
        <skos:prefLabel xml:lang="nl">Vrijdag</skos:prefLabel>
        <skos:prefLabel xml:lang="ru">Пятница</skos:prefLabel>
        <skos:prefLabel xml:lang="ar">الجمعة</skos:prefLabel>
        <skos:prefLabel xml:lang="zh">星期五</skos:prefLabel>
        <skos:prefLabel xml:lang="ja">金曜日</skos:prefLabel>
    </owl:NamedIndividual>
    


    <!-- http://www.w3.org/2006/time#Monday -->

    <owl:NamedIndividual rdf:about="http://www.w3.org/2006/time#Monday">
        <rdf:type rdf:resource="http://www.w3.org/2006/time#DayOfWeek"/>
        <rdfs:label xml:lang="en">Monday</rdfs:label>
        <skos:prefLabel xml:lang="fr">Lundi</skos:prefLabel>
        <skos:prefLabel xml:lang="it">Lunedì</skos:prefLabel>
        <skos:prefLabel xml:lang="es">Lunes</skos:prefLabel>
        <skos:prefLabel xml:lang="nl">Maandag</skos:prefLabel>
        <skos:prefLabel xml:lang="en">Monday</skos:prefLabel>
        <skos:prefLabel xml:lang="de">Montag</skos:prefLabel>
        <skos:prefLabel xml:lang="pl">Poniedziałek</skos:prefLabel>
        <skos:prefLabel xml:lang="pt">Segunda-feira</skos:prefLabel>
        <skos:prefLabel xml:lang="ru">Понедельник</skos:prefLabel>
        <skos:prefLabel xml:lang="ar">الاثنين</skos:prefLabel>
        <skos:prefLabel xml:lang="zh">星期一</skos:prefLabel>
        <skos:prefLabel xml:lang="ja">月曜日</skos:prefLabel>
    </owl:NamedIndividual>
    


    <!-- http://www.w3.org/2006/time#Saturday -->

    <owl:NamedIndividual rdf:about="http://www.w3.org/2006/time#Saturday">
        <rdf:type rdf:resource="http://www.w3.org/2006/time#DayOfWeek"/>
        <rdfs:label xml:lang="en">Saturday</rdfs:label>
        <skos:prefLabel xml:lang="it">Sabato</skos:prefLabel>
        <skos:prefLabel xml:lang="fr">Samedi</skos:prefLabel>
        <skos:prefLabel xml:lang="de">Samstag</skos:prefLabel>
        <skos:prefLabel xml:lang="en">Saturday</skos:prefLabel>
        <skos:prefLabel xml:lang="pl">Sobota</skos:prefLabel>
        <skos:prefLabel xml:lang="es">Sábado</skos:prefLabel>
        <skos:prefLabel xml:lang="pt">Sábado</skos:prefLabel>
        <skos:prefLabel xml:lang="nl">Zaterdag</skos:prefLabel>
        <skos:prefLabel xml:lang="ru">Суббота</skos:prefLabel>
        <skos:prefLabel xml:lang="ar">السبت</skos:prefLabel>
        <skos:prefLabel xml:lang="ja">土曜日</skos:prefLabel>
        <skos:prefLabel xml:lang="zh">星期六</skos:prefLabel>
    </owl:NamedIndividual>
    


    <!-- http://www.w3.org/2006/time#Sunday -->

    <owl:NamedIndividual rdf:about="http://www.w3.org/2006/time#Sunday">
        <rdf:type rdf:resource="http://www.w3.org/2006/time#DayOfWeek"/>
        <rdfs:label xml:lang="en">Sunday</rdfs:label>
        <skos:prefLabel xml:lang="fr">Dimanche</skos:prefLabel>
        <skos:prefLabel xml:lang="it">Domenica</skos:prefLabel>
        <skos:prefLabel xml:lang="es">Domingo</skos:prefLabel>
        <skos:prefLabel xml:lang="pt">Domingo</skos:prefLabel>
        <skos:prefLabel xml:lang="pl">Niedziela</skos:prefLabel>
        <skos:prefLabel xml:lang="de">Sonntag</skos:prefLabel>
        <skos:prefLabel xml:lang="en">Sunday</skos:prefLabel>
        <skos:prefLabel xml:lang="nl">Zondag</skos:prefLabel>
        <skos:prefLabel xml:lang="ru">Воскресенье</skos:prefLabel>
        <skos:prefLabel xml:lang="ar">الأحد (يوم)</skos:prefLabel>
        <skos:prefLabel xml:lang="ja">日曜日</skos:prefLabel>
        <skos:prefLabel xml:lang="zh">星期日</skos:prefLabel>
    </owl:NamedIndividual>
    


    <!-- http://www.w3.org/2006/time#Thursday -->

    <owl:NamedIndividual rdf:about="http://www.w3.org/2006/time#Thursday">
        <rdf:type rdf:resource="http://www.w3.org/2006/time#DayOfWeek"/>
        <rdfs:label xml:lang="en">Thursday</rdfs:label>
        <skos:prefLabel xml:lang="pl">Czwartek</skos:prefLabel>
        <skos:prefLabel xml:lang="nl">Donderdag</skos:prefLabel>
        <skos:prefLabel xml:lang="de">Donnerstag</skos:prefLabel>
        <skos:prefLabel xml:lang="it">Giovedì</skos:prefLabel>
        <skos:prefLabel xml:lang="fr">Jeudi</skos:prefLabel>
        <skos:prefLabel xml:lang="es">Jueves</skos:prefLabel>
        <skos:prefLabel xml:lang="pt">Quinta-feira</skos:prefLabel>
        <skos:prefLabel xml:lang="en">Thursday</skos:prefLabel>
        <skos:prefLabel xml:lang="ru">Четверг</skos:prefLabel>
        <skos:prefLabel xml:lang="ar">الخميس</skos:prefLabel>
        <skos:prefLabel xml:lang="zh">星期四</skos:prefLabel>
        <skos:prefLabel xml:lang="ja">木曜日</skos:prefLabel>
    </owl:NamedIndividual>
    


    <!-- http://www.w3.org/2006/time#Tuesday -->

    <owl:NamedIndividual rdf:about="http://www.w3.org/2006/time#Tuesday">
        <rdf:type rdf:resource="http://www.w3.org/2006/time#DayOfWeek"/>
        <rdfs:label xml:lang="en">Tuesday</rdfs:label>
        <skos:prefLabel xml:lang="de">Dienstag</skos:prefLabel>
        <skos:prefLabel xml:lang="nl">Dinsdag</skos:prefLabel>
        <skos:prefLabel xml:lang="fr">Mardi</skos:prefLabel>
        <skos:prefLabel xml:lang="it">Martedì</skos:prefLabel>
        <skos:prefLabel xml:lang="es">Martes</skos:prefLabel>
        <skos:prefLabel xml:lang="pt">Terça-feira</skos:prefLabel>
        <skos:prefLabel xml:lang="en">Tuesday</skos:prefLabel>
        <skos:prefLabel xml:lang="pl">Wtorek</skos:prefLabel>
        <skos:prefLabel xml:lang="ru">Вторник</skos:prefLabel>
        <skos:prefLabel xml:lang="ar">الثلاثاء</skos:prefLabel>
        <skos:prefLabel xml:lang="zh">星期二</skos:prefLabel>
        <skos:prefLabel xml:lang="ja">火曜日</skos:prefLabel>
    </owl:NamedIndividual>
    


    <!-- http://www.w3.org/2006/time#Wednesday -->

    <owl:NamedIndividual rdf:about="http://www.w3.org/2006/time#Wednesday">
        <rdf:type rdf:resource="http://www.w3.org/2006/time#DayOfWeek"/>
        <rdfs:label xml:lang="en">Wednesday</rdfs:label>
        <skos:prefLabel xml:lang="it">Mercoledì</skos:prefLabel>
        <skos:prefLabel xml:lang="fr">Mercredi</skos:prefLabel>
        <skos:prefLabel xml:lang="de">Mittwoch</skos:prefLabel>
        <skos:prefLabel xml:lang="es">Miércoles</skos:prefLabel>
        <skos:prefLabel xml:lang="pt">Quarta-feira</skos:prefLabel>
        <skos:prefLabel xml:lang="en">Wednesday</skos:prefLabel>
        <skos:prefLabel xml:lang="nl">Woensdag</skos:prefLabel>
        <skos:prefLabel xml:lang="pl">Środa</skos:prefLabel>
        <skos:prefLabel xml:lang="ru">Среда</skos:prefLabel>
        <skos:prefLabel xml:lang="ar">الأربعاء</skos:prefLabel>
        <skos:prefLabel xml:lang="zh">星期三</skos:prefLabel>
        <skos:prefLabel xml:lang="ja">水曜日</skos:prefLabel>
    </owl:NamedIndividual>
    


    <!-- http://www.w3.org/2006/time#unitCentury -->

    <owl:NamedIndividual rdf:about="http://www.w3.org/2006/time#unitCentury">
        <rdf:type rdf:resource="http://www.w3.org/2006/time#TemporalUnit"/>
        <time:days rdf:datatype="http://www.w3.org/2001/XMLSchema#integer">0</time:days>
        <time:hours rdf:datatype="http://www.w3.org/2001/XMLSchema#integer">0</time:hours>
        <time:minutes rdf:datatype="http://www.w3.org/2001/XMLSchema#integer">0</time:minutes>
        <time:months rdf:datatype="http://www.w3.org/2001/XMLSchema#integer">0</time:months>
        <time:seconds rdf:datatype="http://www.w3.org/2001/XMLSchema#integer">0</time:seconds>
        <time:weeks rdf:datatype="http://www.w3.org/2001/XMLSchema#integer">0</time:weeks>
        <time:years rdf:datatype="http://www.w3.org/2001/XMLSchema#integer">100</time:years>
        <rdfs:label xml:lang="en">Century (unit of temporal duration)</rdfs:label>
        <skos:prefLabel xml:lang="de">Jahrhundert</skos:prefLabel>
        <skos:prefLabel xml:lang="en">century</skos:prefLabel>
        <skos:prefLabel xml:lang="nl">eeuw</skos:prefLabel>
        <skos:prefLabel xml:lang="it">secolo</skos:prefLabel>
        <skos:prefLabel xml:lang="es">siglo</skos:prefLabel>
        <skos:prefLabel xml:lang="fr">siècle</skos:prefLabel>
        <skos:prefLabel xml:lang="pl">stulecie</skos:prefLabel>
        <skos:prefLabel xml:lang="pt">século</skos:prefLabel>
        <skos:prefLabel xml:lang="ru">век</skos:prefLabel>
        <skos:prefLabel xml:lang="ar">قرن واحد</skos:prefLabel>
        <skos:prefLabel xml:lang="ja">一世紀</skos:prefLabel>
        <skos:prefLabel xml:lang="zh">一个世纪</skos:prefLabel>
        <skos:prefLabel xml:lang="kr">한 세기</skos:prefLabel>
    </owl:NamedIndividual>
    


    <!-- http://www.w3.org/2006/time#unitDay -->

    <owl:NamedIndividual rdf:about="http://www.w3.org/2006/time#unitDay">
        <rdf:type rdf:resource="http://www.w3.org/2006/time#TemporalUnit"/>
        <time:days rdf:datatype="http://www.w3.org/2001/XMLSchema#integer">1</time:days>
        <time:hours rdf:datatype="http://www.w3.org/2001/XMLSchema#integer">0</time:hours>
        <time:minutes rdf:datatype="http://www.w3.org/2001/XMLSchema#integer">0</time:minutes>
        <time:months rdf:datatype="http://www.w3.org/2001/XMLSchema#integer">0</time:months>
        <time:seconds rdf:datatype="http://www.w3.org/2001/XMLSchema#integer">0</time:seconds>
        <time:weeks rdf:datatype="http://www.w3.org/2001/XMLSchema#integer">0</time:weeks>
        <time:years rdf:datatype="http://www.w3.org/2001/XMLSchema#integer">0</time:years>
        <rdfs:label xml:lang="en">Day (unit of temporal duration)</rdfs:label>
        <skos:prefLabel xml:lang="de">Tag</skos:prefLabel>
        <skos:prefLabel xml:lang="nl">dag</skos:prefLabel>
        <skos:prefLabel xml:lang="en">day</skos:prefLabel>
        <skos:prefLabel xml:lang="pt">dia</skos:prefLabel>
        <skos:prefLabel xml:lang="pl">doba</skos:prefLabel>
        <skos:prefLabel xml:lang="es">día</skos:prefLabel>
        <skos:prefLabel xml:lang="it">giorno</skos:prefLabel>
        <skos:prefLabel xml:lang="fr">jour</skos:prefLabel>
        <skos:prefLabel xml:lang="ar">يوماً ما</skos:prefLabel>
        <skos:prefLabel xml:lang="ja">ある日</skos:prefLabel>
        <skos:prefLabel xml:lang="zh">一天</skos:prefLabel>
        <skos:prefLabel xml:lang="kr">언젠가</skos:prefLabel>
    </owl:NamedIndividual>
    


    <!-- http://www.w3.org/2006/time#unitDecade -->

    <owl:NamedIndividual rdf:about="http://www.w3.org/2006/time#unitDecade">
        <rdf:type rdf:resource="http://www.w3.org/2006/time#TemporalUnit"/>
        <time:days rdf:datatype="http://www.w3.org/2001/XMLSchema#integer">0</time:days>
        <time:hours rdf:datatype="http://www.w3.org/2001/XMLSchema#integer">0</time:hours>
        <time:minutes rdf:datatype="http://www.w3.org/2001/XMLSchema#integer">0</time:minutes>
        <time:months rdf:datatype="http://www.w3.org/2001/XMLSchema#integer">0</time:months>
        <time:seconds rdf:datatype="http://www.w3.org/2001/XMLSchema#integer">0</time:seconds>
        <time:weeks rdf:datatype="http://www.w3.org/2001/XMLSchema#integer">0</time:weeks>
        <time:years rdf:datatype="http://www.w3.org/2001/XMLSchema#integer">10</time:years>
        <rdfs:label xml:lang="en">Decade (unit of temporal duration)</rdfs:label>
        <skos:prefLabel xml:lang="kr">1 열개의</skos:prefLabel>
        <skos:prefLabel xml:lang="ja">10年</skos:prefLabel>
        <skos:prefLabel xml:lang="de">Dekade</skos:prefLabel>
        <skos:prefLabel xml:lang="en">decade</skos:prefLabel>
        <skos:prefLabel xml:lang="it">decennio</skos:prefLabel>
        <skos:prefLabel xml:lang="nl">decennium</skos:prefLabel>
        <skos:prefLabel xml:lang="pl">dekada</skos:prefLabel>
        <skos:prefLabel xml:lang="pt">década</skos:prefLabel>
        <skos:prefLabel xml:lang="fr">décennie</skos:prefLabel>
        <skos:prefLabel xml:lang="es">una década</skos:prefLabel>
        <skos:prefLabel xml:lang="ru">одно десятилетие</skos:prefLabel>
        <skos:prefLabel xml:lang="ar">عقد واحد</skos:prefLabel>
        <skos:prefLabel xml:lang="zh">十年</skos:prefLabel>
    </owl:NamedIndividual>
    


    <!-- http://www.w3.org/2006/time#unitHour -->

    <owl:NamedIndividual rdf:about="http://www.w3.org/2006/time#unitHour">
        <rdf:type rdf:resource="http://www.w3.org/2006/time#TemporalUnit"/>
        <time:days rdf:datatype="http://www.w3.org/2001/XMLSchema#integer">0</time:days>
        <time:hours rdf:datatype="http://www.w3.org/2001/XMLSchema#integer">1</time:hours>
        <time:minutes rdf:datatype="http://www.w3.org/2001/XMLSchema#integer">0</time:minutes>
        <time:months rdf:datatype="http://www.w3.org/2001/XMLSchema#integer">0</time:months>
        <time:seconds rdf:datatype="http://www.w3.org/2001/XMLSchema#integer">0</time:seconds>
        <time:weeks rdf:datatype="http://www.w3.org/2001/XMLSchema#integer">0</time:weeks>
        <time:years rdf:datatype="http://www.w3.org/2001/XMLSchema#integer">0</time:years>
        <rdfs:label xml:lang="en">Hour (unit of temporal duration)</rdfs:label>
        <skos:prefLabel xml:lang="de">Stunde</skos:prefLabel>
        <skos:prefLabel xml:lang="pl">godzina</skos:prefLabel>
        <skos:prefLabel xml:lang="fr">heure</skos:prefLabel>
        <skos:prefLabel xml:lang="es">hora</skos:prefLabel>
        <skos:prefLabel xml:lang="pt">hora</skos:prefLabel>
        <skos:prefLabel xml:lang="en">hour</skos:prefLabel>
        <skos:prefLabel xml:lang="it">ora</skos:prefLabel>
        <skos:prefLabel xml:lang="nl">uur</skos:prefLabel>
        <skos:prefLabel>один час&quot;@ru</skos:prefLabel>
        <skos:prefLabel xml:lang="ar">ساعة واحدة</skos:prefLabel>
        <skos:prefLabel xml:lang="zh">一小時</skos:prefLabel>
        <skos:prefLabel xml:lang="ja">一時間</skos:prefLabel>
        <skos:prefLabel xml:lang="kr">한 시간</skos:prefLabel>
    </owl:NamedIndividual>
    


    <!-- http://www.w3.org/2006/time#unitMillenium -->

    <owl:NamedIndividual rdf:about="http://www.w3.org/2006/time#unitMillenium">
        <rdf:type rdf:resource="http://www.w3.org/2006/time#TemporalUnit"/>
        <time:days rdf:datatype="http://www.w3.org/2001/XMLSchema#integer">0</time:days>
        <time:hours rdf:datatype="http://www.w3.org/2001/XMLSchema#integer">0</time:hours>
        <time:minutes rdf:datatype="http://www.w3.org/2001/XMLSchema#integer">0</time:minutes>
        <time:months rdf:datatype="http://www.w3.org/2001/XMLSchema#integer">0</time:months>
        <time:seconds rdf:datatype="http://www.w3.org/2001/XMLSchema#integer">0</time:seconds>
        <time:weeks rdf:datatype="http://www.w3.org/2001/XMLSchema#integer">0</time:weeks>
        <time:years rdf:datatype="http://www.w3.org/2001/XMLSchema#integer">1000</time:years>
        <rdfs:label xml:lang="en">Century (unit of temporal duration)</rdfs:label>
        <skos:prefLabel xml:lang="de">Jahrtausend</skos:prefLabel>
        <skos:prefLabel xml:lang="es">milenio</skos:prefLabel>
        <skos:prefLabel xml:lang="en">millenium</skos:prefLabel>
        <skos:prefLabel xml:lang="it">millennio</skos:prefLabel>
        <skos:prefLabel xml:lang="nl">millennium</skos:prefLabel>
        <skos:prefLabel xml:lang="fr">millénaire</skos:prefLabel>
        <skos:prefLabel xml:lang="pt">milênio</skos:prefLabel>
        <skos:prefLabel xml:lang="pl">tysiąclecie</skos:prefLabel>
        <skos:prefLabel xml:lang="ru">тысячелетие</skos:prefLabel>
        <skos:prefLabel xml:lang="ar">الألفية</skos:prefLabel>
        <skos:prefLabel xml:lang="ja">ミレニアム</skos:prefLabel>
        <skos:prefLabel xml:lang="zh">千年</skos:prefLabel>
        <skos:prefLabel xml:lang="kr">밀레니엄</skos:prefLabel>
    </owl:NamedIndividual>
    


    <!-- http://www.w3.org/2006/time#unitMinute -->

    <owl:NamedIndividual rdf:about="http://www.w3.org/2006/time#unitMinute">
        <rdf:type rdf:resource="http://www.w3.org/2006/time#TemporalUnit"/>
        <time:days rdf:datatype="http://www.w3.org/2001/XMLSchema#integer">0</time:days>
        <time:hours rdf:datatype="http://www.w3.org/2001/XMLSchema#integer">0</time:hours>
        <time:minutes rdf:datatype="http://www.w3.org/2001/XMLSchema#integer">1</time:minutes>
        <time:months rdf:datatype="http://www.w3.org/2001/XMLSchema#integer">0</time:months>
        <time:seconds rdf:datatype="http://www.w3.org/2001/XMLSchema#integer">0</time:seconds>
        <time:weeks rdf:datatype="http://www.w3.org/2001/XMLSchema#integer">0</time:weeks>
        <time:years rdf:datatype="http://www.w3.org/2001/XMLSchema#integer">0</time:years>
        <rdfs:label xml:lang="en">Minute (unit of temporal duration)</rdfs:label>
        <skos:prefLabel xml:lang="de">Minute</skos:prefLabel>
        <skos:prefLabel xml:lang="pl">minuta</skos:prefLabel>
        <skos:prefLabel xml:lang="en">minute</skos:prefLabel>
        <skos:prefLabel xml:lang="fr">minute</skos:prefLabel>
        <skos:prefLabel xml:lang="es">minuto</skos:prefLabel>
        <skos:prefLabel xml:lang="it">minuto</skos:prefLabel>
        <skos:prefLabel xml:lang="pt">minuto</skos:prefLabel>
        <skos:prefLabel xml:lang="nl">minuut</skos:prefLabel>
        <skos:prefLabel xml:lang="ru">одна минута</skos:prefLabel>
        <skos:prefLabel xml:lang="ar">دقيقة واحدة</skos:prefLabel>
        <skos:prefLabel xml:lang="ja">一分</skos:prefLabel>
        <skos:prefLabel xml:lang="zh">等一下</skos:prefLabel>
        <skos:prefLabel xml:lang="kr">분</skos:prefLabel>
    </owl:NamedIndividual>
    


    <!-- http://www.w3.org/2006/time#unitMonth -->

    <owl:NamedIndividual rdf:about="http://www.w3.org/2006/time#unitMonth">
        <rdf:type rdf:resource="http://www.w3.org/2006/time#TemporalUnit"/>
        <time:days rdf:datatype="http://www.w3.org/2001/XMLSchema#integer">0</time:days>
        <time:hours rdf:datatype="http://www.w3.org/2001/XMLSchema#integer">0</time:hours>
        <time:minutes rdf:datatype="http://www.w3.org/2001/XMLSchema#integer">0</time:minutes>
        <time:months rdf:datatype="http://www.w3.org/2001/XMLSchema#integer">1</time:months>
        <time:seconds rdf:datatype="http://www.w3.org/2001/XMLSchema#integer">0</time:seconds>
        <time:weeks rdf:datatype="http://www.w3.org/2001/XMLSchema#integer">0</time:weeks>
        <time:years rdf:datatype="http://www.w3.org/2001/XMLSchema#integer">0</time:years>
        <rdfs:label xml:lang="en">Month (unit of temporal duration)</rdfs:label>
        <skos:prefLabel xml:lang="de">Monat</skos:prefLabel>
        <skos:prefLabel xml:lang="nl">maand</skos:prefLabel>
        <skos:prefLabel xml:lang="es">mes</skos:prefLabel>
        <skos:prefLabel xml:lang="it">mese</skos:prefLabel>
        <skos:prefLabel xml:lang="pl">miesiąc</skos:prefLabel>
        <skos:prefLabel xml:lang="fr">mois</skos:prefLabel>
        <skos:prefLabel xml:lang="en">month</skos:prefLabel>
        <skos:prefLabel xml:lang="ru">один месяц</skos:prefLabel>
        <skos:prefLabel xml:lang="ar">شهر واحد</skos:prefLabel>
        <skos:prefLabel xml:lang="ja">一か月</skos:prefLabel>
        <skos:prefLabel xml:lang="zh">一個月</skos:prefLabel>
        <skos:prefLabel xml:lang="kr">한달</skos:prefLabel>
    </owl:NamedIndividual>
    


    <!-- http://www.w3.org/2006/time#unitSecond -->

    <owl:NamedIndividual rdf:about="http://www.w3.org/2006/time#unitSecond">
        <rdf:type rdf:resource="http://www.w3.org/2006/time#TemporalUnit"/>
        <time:days rdf:datatype="http://www.w3.org/2001/XMLSchema#integer">0</time:days>
        <time:hours rdf:datatype="http://www.w3.org/2001/XMLSchema#integer">0</time:hours>
        <time:minutes rdf:datatype="http://www.w3.org/2001/XMLSchema#integer">0</time:minutes>
        <time:months rdf:datatype="http://www.w3.org/2001/XMLSchema#integer">0</time:months>
        <time:seconds rdf:datatype="http://www.w3.org/2001/XMLSchema#integer">1</time:seconds>
        <time:weeks rdf:datatype="http://www.w3.org/2001/XMLSchema#integer">0</time:weeks>
        <time:years rdf:datatype="http://www.w3.org/2001/XMLSchema#integer">0</time:years>
        <rdfs:label xml:lang="en">Second (unit of temporal duration)</rdfs:label>
        <skos:prefLabel xml:lang="de">Sekunde</skos:prefLabel>
        <skos:prefLabel xml:lang="en">second</skos:prefLabel>
        <skos:prefLabel xml:lang="fr">seconde</skos:prefLabel>
        <skos:prefLabel xml:lang="nl">seconde</skos:prefLabel>
        <skos:prefLabel xml:lang="it">secondo</skos:prefLabel>
        <skos:prefLabel xml:lang="es">segundo</skos:prefLabel>
        <skos:prefLabel xml:lang="pt">segundo</skos:prefLabel>
        <skos:prefLabel xml:lang="pl">sekundę</skos:prefLabel>
        <skos:prefLabel xml:lang="ar">ثانية واحدة</skos:prefLabel>
        <skos:prefLabel xml:lang="ja">一秒</skos:prefLabel>
        <skos:prefLabel xml:lang="zh">一秒</skos:prefLabel>
        <skos:prefLabel xml:lang="kr">일초</skos:prefLabel>
    </owl:NamedIndividual>
    


    <!-- http://www.w3.org/2006/time#unitWeek -->

    <owl:NamedIndividual rdf:about="http://www.w3.org/2006/time#unitWeek">
        <rdf:type rdf:resource="http://www.w3.org/2006/time#TemporalUnit"/>
        <time:days rdf:datatype="http://www.w3.org/2001/XMLSchema#integer">0</time:days>
        <time:hours rdf:datatype="http://www.w3.org/2001/XMLSchema#integer">0</time:hours>
        <time:minutes rdf:datatype="http://www.w3.org/2001/XMLSchema#integer">0</time:minutes>
        <time:months rdf:datatype="http://www.w3.org/2001/XMLSchema#integer">0</time:months>
        <time:seconds rdf:datatype="http://www.w3.org/2001/XMLSchema#integer">0</time:seconds>
        <time:weeks rdf:datatype="http://www.w3.org/2001/XMLSchema#integer">1</time:weeks>
        <time:years rdf:datatype="http://www.w3.org/2001/XMLSchema#integer">0</time:years>
        <rdfs:label xml:lang="en">Week (unit of temporal duration)</rdfs:label>
        <skos:prefLabel xml:lang="de">Woche</skos:prefLabel>
        <skos:prefLabel xml:lang="fr">semaine</skos:prefLabel>
        <skos:prefLabel xml:lang="es">semana</skos:prefLabel>
        <skos:prefLabel xml:lang="pt">semana</skos:prefLabel>
        <skos:prefLabel xml:lang="it">settimana</skos:prefLabel>
        <skos:prefLabel xml:lang="pl">tydzień</skos:prefLabel>
        <skos:prefLabel xml:lang="en">week</skos:prefLabel>
        <skos:prefLabel xml:lang="nl">week</skos:prefLabel>
        <skos:prefLabel xml:lang="ru">одна неделя</skos:prefLabel>
        <skos:prefLabel xml:lang="ar">سبوع واحد</skos:prefLabel>
        <skos:prefLabel xml:lang="zh">一周</skos:prefLabel>
        <skos:prefLabel xml:lang="ja">一週間</skos:prefLabel>
        <skos:prefLabel xml:lang="kr">일주일</skos:prefLabel>
    </owl:NamedIndividual>
    


    <!-- http://www.w3.org/2006/time#unitYear -->

    <owl:NamedIndividual rdf:about="http://www.w3.org/2006/time#unitYear">
        <rdf:type rdf:resource="http://www.w3.org/2006/time#TemporalUnit"/>
        <time:days rdf:datatype="http://www.w3.org/2001/XMLSchema#integer">0</time:days>
        <time:hours rdf:datatype="http://www.w3.org/2001/XMLSchema#integer">0</time:hours>
        <time:minutes rdf:datatype="http://www.w3.org/2001/XMLSchema#integer">0</time:minutes>
        <time:months rdf:datatype="http://www.w3.org/2001/XMLSchema#integer">0</time:months>
        <time:seconds rdf:datatype="http://www.w3.org/2001/XMLSchema#integer">0</time:seconds>
        <time:weeks rdf:datatype="http://www.w3.org/2001/XMLSchema#integer">0</time:weeks>
        <time:years rdf:datatype="http://www.w3.org/2001/XMLSchema#integer">1</time:years>
        <rdfs:label xml:lang="en">Year (unit of temporal duration)</rdfs:label>
        <skos:prefLabel xml:lang="kr">1 년</skos:prefLabel>
        <skos:prefLabel xml:lang="de">Jahr</skos:prefLabel>
        <skos:prefLabel xml:lang="fr">an</skos:prefLabel>
        <skos:prefLabel xml:lang="it">anno</skos:prefLabel>
        <skos:prefLabel xml:lang="pt">ano</skos:prefLabel>
        <skos:prefLabel xml:lang="nl">jaar</skos:prefLabel>
        <skos:prefLabel xml:lang="pl">rok</skos:prefLabel>
        <skos:prefLabel xml:lang="es">un año</skos:prefLabel>
        <skos:prefLabel xml:lang="en">year</skos:prefLabel>
        <skos:prefLabel xml:lang="ru">один год</skos:prefLabel>
        <skos:prefLabel xml:lang="ar">سنة واحدة</skos:prefLabel>
        <skos:prefLabel xml:lang="ja">一年</skos:prefLabel>
        <skos:prefLabel xml:lang="zh">一年</skos:prefLabel>
    </owl:NamedIndividual>
    


    <!-- https://w3id.org/def/propaphen#t1 -->

    <owl:NamedIndividual rdf:about="https://w3id.org/def/propaphen#t1">
        <rdf:type rdf:resource="http://www.w3.org/2006/time#Instant"/>
    </owl:NamedIndividual>
    


    <!-- https://w3id.org/def/propaphen#t2 -->

    <owl:NamedIndividual rdf:about="https://w3id.org/def/propaphen#t2">
        <rdf:type rdf:resource="http://www.w3.org/2006/time#Instant"/>
    </owl:NamedIndividual>
    


    <!-- https://w3id.org/def/propaphen#t3 -->

    <owl:NamedIndividual rdf:about="https://w3id.org/def/propaphen#t3">
        <rdf:type rdf:resource="http://www.w3.org/2006/time#Instant"/>
        <time:after rdf:resource="https://w3id.org/def/propaphen#t1"/>
    </owl:NamedIndividual>
    


    <!-- https://w3id.org/def/propaphen#t4 -->

    <owl:NamedIndividual rdf:about="https://w3id.org/def/propaphen#t4">
        <rdf:type rdf:resource="http://www.w3.org/2006/time#Instant"/>
    </owl:NamedIndividual>
    


    <!-- https://w3id.org/def/propaphen#ti1 -->

    <owl:NamedIndividual rdf:about="https://w3id.org/def/propaphen#ti1">
        <rdf:type rdf:resource="http://www.w3.org/2006/time#Interval"/>
        <time:hasBeginning rdf:resource="https://w3id.org/def/propaphen#t1"/>
        <time:intervalContains rdf:resource="https://w3id.org/def/propaphen#ti2"/>
    </owl:NamedIndividual>
    


    <!-- https://w3id.org/def/propaphen#ti2 -->

    <owl:NamedIndividual rdf:about="https://w3id.org/def/propaphen#ti2">
        <rdf:type rdf:resource="http://www.w3.org/2006/time#Interval"/>
        <time:hasEnd rdf:resource="https://w3id.org/def/propaphen#t4"/>
    </owl:NamedIndividual>
    <rdf:Description>
        <xsd:pattern>-?([1-9][0-9]{3,}|0[0-9]{3})(Z|(\+|-)((0[0-9]|1[0-3]):[0-5][0-9]|14:00))?</xsd:pattern>
    </rdf:Description>
    <rdf:Description>
        <xsd:pattern>---(0[1-9]|[1-9][0-9])(Z|(\+|-)((0[0-9]|1[0-3]):[0-5][0-9]|14:00))?</xsd:pattern>
    </rdf:Description>
    <rdf:Description>
        <xsd:pattern>--(0[1-9]|1[0-9]|20)(Z|(\+|-)((0[0-9]|1[0-3]):[0-5][0-9]|14:00))?</xsd:pattern>
    </rdf:Description>
    


    <!-- 
    ///////////////////////////////////////////////////////////////////////////////////////
    //
    // Annotations
    //
    ///////////////////////////////////////////////////////////////////////////////////////
     -->

    <rdf:Description rdf:about="https://w3id.org/seas/BalanceEvaluation">
        <ns1:term_status>testing</ns1:term_status>
        <rdfs:label>Balance Evaluation</rdfs:label>
        <rdfs:comment xml:lang="en">Evaluation of the difference between the incoming evaluation and the outgoing evaluation.</rdfs:comment>
        <rdfs:isDefinedBy rdf:resource="https://w3id.org/seas/ZoneOntology"/>
    </rdf:Description>
    


    <!-- 
    ///////////////////////////////////////////////////////////////////////////////////////
    //
    // General axioms
    //
    ///////////////////////////////////////////////////////////////////////////////////////
     -->

    <rdf:Description>
        <rdf:type rdf:resource="http://www.w3.org/2002/07/owl#AllDisjointClasses"/>
        <owl:members rdf:parseType="Collection">
            <rdf:Description rdf:about="http://purl.org/nemo/gufo#Collection"/>
            <rdf:Description rdf:about="http://purl.org/nemo/gufo#FunctionalComplex"/>
            <rdf:Description rdf:about="http://purl.org/nemo/gufo#Quantity"/>
        </owl:members>
    </rdf:Description>
    <rdf:Description>
        <rdf:type rdf:resource="http://www.w3.org/2002/07/owl#AllDisjointClasses"/>
        <owl:members rdf:parseType="Collection">
            <rdf:Description rdf:about="http://purl.org/nemo/gufo#Endurant"/>
            <rdf:Description rdf:about="http://purl.org/nemo/gufo#Event"/>
            <rdf:Description rdf:about="http://purl.org/nemo/gufo#Situation"/>
        </owl:members>
    </rdf:Description>
    


    <!-- 
    ///////////////////////////////////////////////////////////////////////////////////////
    //
    // Rules
    //
    ///////////////////////////////////////////////////////////////////////////////////////
     -->

    <rdf:Description rdf:about="http://www.semanticweb.org/alencga1/ontologies/2023/2/PhenOWL/GCE">
        <rdf:type rdf:resource="http://www.w3.org/2003/11/swrl#Variable"/>
    </rdf:Description>
    <rdf:Description rdf:about="http://www.semanticweb.org/alencga1/ontologies/2023/2/PhenOWL/PI1">
        <rdf:type rdf:resource="http://www.w3.org/2003/11/swrl#Variable"/>
    </rdf:Description>
    <rdf:Description rdf:about="http://www.semanticweb.org/alencga1/ontologies/2023/2/PhenOWL/t1">
        <rdf:type rdf:resource="http://www.w3.org/2003/11/swrl#Variable"/>
    </rdf:Description>
    <rdf:Description rdf:about="http://www.semanticweb.org/alencga1/ontologies/2023/2/PhenOWL/SO2">
        <rdf:type rdf:resource="http://www.w3.org/2003/11/swrl#Variable"/>
    </rdf:Description>
    <rdf:Description rdf:about="http://www.semanticweb.org/alencga1/ontologies/2023/2/PhenOWL/SO1">
        <rdf:type rdf:resource="http://www.w3.org/2003/11/swrl#Variable"/>
    </rdf:Description>
    <rdf:Description rdf:about="http://www.semanticweb.org/alencga1/ontologies/2023/2/PhenOWL/PR1">
        <rdf:type rdf:resource="http://www.w3.org/2003/11/swrl#Variable"/>
    </rdf:Description>
    <rdf:Description rdf:about="http://www.semanticweb.org/alencga1/ontologies/2023/2/PhenOWL/PI2">
        <rdf:type rdf:resource="http://www.w3.org/2003/11/swrl#Variable"/>
    </rdf:Description>
    <rdf:Description rdf:about="http://www.semanticweb.org/alencga1/ontologies/2023/2/PhenOWL/O1">
        <rdf:type rdf:resource="http://www.w3.org/2003/11/swrl#Variable"/>
    </rdf:Description>
    <rdf:Description rdf:about="http://www.semanticweb.org/alencga1/ontologies/2023/2/PhenOWL/S1">
        <rdf:type rdf:resource="http://www.w3.org/2003/11/swrl#Variable"/>
    </rdf:Description>
    <rdf:Description rdf:about="http://www.semanticweb.org/alencga1/ontologies/2023/2/PhenOWL/S2">
        <rdf:type rdf:resource="http://www.w3.org/2003/11/swrl#Variable"/>
    </rdf:Description>
    <rdf:Description rdf:about="http://www.semanticweb.org/alencga1/ontologies/2023/2/PhenOWL/OP1">
        <rdf:type rdf:resource="http://www.w3.org/2003/11/swrl#Variable"/>
    </rdf:Description>
    <rdf:Description rdf:about="http://www.semanticweb.org/alencga1/ontologies/2023/2/PhenOWL/P1">
        <rdf:type rdf:resource="http://www.w3.org/2003/11/swrl#Variable"/>
    </rdf:Description>
    <rdf:Description rdf:about="http://www.semanticweb.org/alencga1/ontologies/2023/2/PhenOWL/t2">
        <rdf:type rdf:resource="http://www.w3.org/2003/11/swrl#Variable"/>
    </rdf:Description>
    <rdf:Description rdf:about="http://www.semanticweb.org/alencga1/ontologies/2023/2/PhenOWL/OP2">
        <rdf:type rdf:resource="http://www.w3.org/2003/11/swrl#Variable"/>
    </rdf:Description>
    <rdf:Description rdf:about="http://www.semanticweb.org/alencga1/ontologies/2023/2/PhenOWL/O2">
        <rdf:type rdf:resource="http://www.w3.org/2003/11/swrl#Variable"/>
    </rdf:Description>
    <rdf:Description>
        <swrla:isRuleEnabled rdf:datatype="http://www.w3.org/2001/XMLSchema#boolean">true</swrla:isRuleEnabled>
        <rdfs:comment rdf:datatype="http://www.w3.org/2001/XMLSchema#string">Associates begin point with beginning of time interval</rdfs:comment>
        <rdfs:label rdf:datatype="http://www.w3.org/2001/XMLSchema#string">s3.1 - time interval beginning</rdfs:label>
        <rdf:type rdf:resource="http://www.w3.org/2003/11/swrl#Imp"/>
        <swrl:body>
            <rdf:Description>
                <rdf:type rdf:resource="http://www.w3.org/2003/11/swrl#AtomList"/>
                <rdf:first>
                    <rdf:Description>
                        <rdf:type rdf:resource="http://www.w3.org/2003/11/swrl#IndividualPropertyAtom"/>
                        <swrl:propertyPredicate rdf:resource="https://w3id.org/def/propaphen#hasTimeInterval"/>
                        <swrl:argument1 rdf:resource="http://www.semanticweb.org/alencga1/ontologies/2023/2/PhenOWL/GCE"/>
                        <swrl:argument2 rdf:resource="http://www.semanticweb.org/alencga1/ontologies/2023/2/PhenOWL/PI1"/>
                    </rdf:Description>
                </rdf:first>
                <rdf:rest>
                    <rdf:Description>
                        <rdf:type rdf:resource="http://www.w3.org/2003/11/swrl#AtomList"/>
                        <rdf:first>
                            <rdf:Description>
                                <rdf:type rdf:resource="http://www.w3.org/2003/11/swrl#ClassAtom"/>
                                <swrl:classPredicate rdf:resource="http://www.w3.org/2006/time#Instant"/>
                                <swrl:argument1 rdf:resource="http://www.semanticweb.org/alencga1/ontologies/2023/2/PhenOWL/t1"/>
                            </rdf:Description>
                        </rdf:first>
                        <rdf:rest>
                            <rdf:Description>
                                <rdf:type rdf:resource="http://www.w3.org/2003/11/swrl#AtomList"/>
                                <rdf:first>
                                    <rdf:Description>
                                        <rdf:type rdf:resource="http://www.w3.org/2003/11/swrl#ClassAtom"/>
                                        <swrl:classPredicate rdf:resource="http://purl.org/nemo/gufo#ConcreteEntity"/>
                                        <swrl:argument1 rdf:resource="http://www.semanticweb.org/alencga1/ontologies/2023/2/PhenOWL/GCE"/>
                                    </rdf:Description>
                                </rdf:first>
                                <rdf:rest>
                                    <rdf:Description>
                                        <rdf:type rdf:resource="http://www.w3.org/2003/11/swrl#AtomList"/>
                                        <rdf:first>
                                            <rdf:Description>
                                                <rdf:type rdf:resource="http://www.w3.org/2003/11/swrl#ClassAtom"/>
                                                <swrl:classPredicate rdf:resource="http://www.w3.org/2006/time#ProperInterval"/>
                                                <swrl:argument1 rdf:resource="http://www.semanticweb.org/alencga1/ontologies/2023/2/PhenOWL/PI1"/>
                                            </rdf:Description>
                                        </rdf:first>
                                        <rdf:rest>
                                            <rdf:Description>
                                                <rdf:type rdf:resource="http://www.w3.org/2003/11/swrl#AtomList"/>
                                                <rdf:first>
                                                    <rdf:Description>
                                                        <rdf:type rdf:resource="http://www.w3.org/2003/11/swrl#IndividualPropertyAtom"/>
                                                        <swrl:propertyPredicate rdf:resource="http://purl.org/nemo/gufo#hasBeginPoint"/>
                                                        <swrl:argument1 rdf:resource="http://www.semanticweb.org/alencga1/ontologies/2023/2/PhenOWL/GCE"/>
                                                        <swrl:argument2 rdf:resource="http://www.semanticweb.org/alencga1/ontologies/2023/2/PhenOWL/t1"/>
                                                    </rdf:Description>
                                                </rdf:first>
                                                <rdf:rest rdf:resource="http://www.w3.org/1999/02/22-rdf-syntax-ns#nil"/>
                                            </rdf:Description>
                                        </rdf:rest>
                                    </rdf:Description>
                                </rdf:rest>
                            </rdf:Description>
                        </rdf:rest>
                    </rdf:Description>
                </rdf:rest>
            </rdf:Description>
        </swrl:body>
        <swrl:head>
            <rdf:Description>
                <rdf:type rdf:resource="http://www.w3.org/2003/11/swrl#AtomList"/>
                <rdf:first>
                    <rdf:Description>
                        <rdf:type rdf:resource="http://www.w3.org/2003/11/swrl#IndividualPropertyAtom"/>
                        <swrl:propertyPredicate rdf:resource="http://www.w3.org/2006/time#hasBeginning"/>
                        <swrl:argument1 rdf:resource="http://www.semanticweb.org/alencga1/ontologies/2023/2/PhenOWL/PI1"/>
                        <swrl:argument2 rdf:resource="http://www.semanticweb.org/alencga1/ontologies/2023/2/PhenOWL/t1"/>
                    </rdf:Description>
                </rdf:first>
                <rdf:rest rdf:resource="http://www.w3.org/1999/02/22-rdf-syntax-ns#nil"/>
            </rdf:Description>
        </swrl:head>
    </rdf:Description>
    <rdf:Description>
        <swrla:isRuleEnabled rdf:datatype="http://www.w3.org/2001/XMLSchema#boolean">true</swrla:isRuleEnabled>
        <rdfs:comment rdf:datatype="http://www.w3.org/2001/XMLSchema#string">Associates end point with beginning of time interval</rdfs:comment>
        <rdfs:label rdf:datatype="http://www.w3.org/2001/XMLSchema#string">s3.2 - time interval end</rdfs:label>
        <rdf:type rdf:resource="http://www.w3.org/2003/11/swrl#Imp"/>
        <swrl:body>
            <rdf:Description>
                <rdf:type rdf:resource="http://www.w3.org/2003/11/swrl#AtomList"/>
                <rdf:first>
                    <rdf:Description>
                        <rdf:type rdf:resource="http://www.w3.org/2003/11/swrl#IndividualPropertyAtom"/>
                        <swrl:propertyPredicate rdf:resource="https://w3id.org/def/propaphen#hasTimeInterval"/>
                        <swrl:argument1 rdf:resource="http://www.semanticweb.org/alencga1/ontologies/2023/2/PhenOWL/GCE"/>
                        <swrl:argument2 rdf:resource="http://www.semanticweb.org/alencga1/ontologies/2023/2/PhenOWL/PI1"/>
                    </rdf:Description>
                </rdf:first>
                <rdf:rest>
                    <rdf:Description>
                        <rdf:type rdf:resource="http://www.w3.org/2003/11/swrl#AtomList"/>
                        <rdf:first>
                            <rdf:Description>
                                <rdf:type rdf:resource="http://www.w3.org/2003/11/swrl#ClassAtom"/>
                                <swrl:classPredicate rdf:resource="http://www.w3.org/2006/time#Instant"/>
                                <swrl:argument1 rdf:resource="http://www.semanticweb.org/alencga1/ontologies/2023/2/PhenOWL/t1"/>
                            </rdf:Description>
                        </rdf:first>
                        <rdf:rest>
                            <rdf:Description>
                                <rdf:type rdf:resource="http://www.w3.org/2003/11/swrl#AtomList"/>
                                <rdf:first>
                                    <rdf:Description>
                                        <rdf:type rdf:resource="http://www.w3.org/2003/11/swrl#ClassAtom"/>
                                        <swrl:classPredicate rdf:resource="http://purl.org/nemo/gufo#ConcreteEntity"/>
                                        <swrl:argument1 rdf:resource="http://www.semanticweb.org/alencga1/ontologies/2023/2/PhenOWL/GCE"/>
                                    </rdf:Description>
                                </rdf:first>
                                <rdf:rest>
                                    <rdf:Description>
                                        <rdf:type rdf:resource="http://www.w3.org/2003/11/swrl#AtomList"/>
                                        <rdf:first>
                                            <rdf:Description>
                                                <rdf:type rdf:resource="http://www.w3.org/2003/11/swrl#ClassAtom"/>
                                                <swrl:classPredicate rdf:resource="http://www.w3.org/2006/time#ProperInterval"/>
                                                <swrl:argument1 rdf:resource="http://www.semanticweb.org/alencga1/ontologies/2023/2/PhenOWL/PI1"/>
                                            </rdf:Description>
                                        </rdf:first>
                                        <rdf:rest>
                                            <rdf:Description>
                                                <rdf:type rdf:resource="http://www.w3.org/2003/11/swrl#AtomList"/>
                                                <rdf:first>
                                                    <rdf:Description>
                                                        <rdf:type rdf:resource="http://www.w3.org/2003/11/swrl#IndividualPropertyAtom"/>
                                                        <swrl:propertyPredicate rdf:resource="http://purl.org/nemo/gufo#hasEndPoint"/>
                                                        <swrl:argument1 rdf:resource="http://www.semanticweb.org/alencga1/ontologies/2023/2/PhenOWL/GCE"/>
                                                        <swrl:argument2 rdf:resource="http://www.semanticweb.org/alencga1/ontologies/2023/2/PhenOWL/t1"/>
                                                    </rdf:Description>
                                                </rdf:first>
                                                <rdf:rest rdf:resource="http://www.w3.org/1999/02/22-rdf-syntax-ns#nil"/>
                                            </rdf:Description>
                                        </rdf:rest>
                                    </rdf:Description>
                                </rdf:rest>
                            </rdf:Description>
                        </rdf:rest>
                    </rdf:Description>
                </rdf:rest>
            </rdf:Description>
        </swrl:body>
        <swrl:head>
            <rdf:Description>
                <rdf:type rdf:resource="http://www.w3.org/2003/11/swrl#AtomList"/>
                <rdf:first>
                    <rdf:Description>
                        <rdf:type rdf:resource="http://www.w3.org/2003/11/swrl#IndividualPropertyAtom"/>
                        <swrl:propertyPredicate rdf:resource="http://www.w3.org/2006/time#hasEnd"/>
                        <swrl:argument1 rdf:resource="http://www.semanticweb.org/alencga1/ontologies/2023/2/PhenOWL/PI1"/>
                        <swrl:argument2 rdf:resource="http://www.semanticweb.org/alencga1/ontologies/2023/2/PhenOWL/t1"/>
                    </rdf:Description>
                </rdf:first>
                <rdf:rest rdf:resource="http://www.w3.org/1999/02/22-rdf-syntax-ns#nil"/>
            </rdf:Description>
        </swrl:head>
    </rdf:Description>
    <rdf:Description>
        <swrla:isRuleEnabled rdf:datatype="http://www.w3.org/2001/XMLSchema#boolean">true</swrla:isRuleEnabled>
        <rdfs:comment rdf:datatype="http://www.w3.org/2001/XMLSchema#string">Associates begin point with beginning of time interval</rdfs:comment>
        <rdfs:label rdf:datatype="http://www.w3.org/2001/XMLSchema#string">s3.3 - inverse time interval beginning</rdfs:label>
        <rdf:type rdf:resource="http://www.w3.org/2003/11/swrl#Imp"/>
        <swrl:body>
            <rdf:Description>
                <rdf:type rdf:resource="http://www.w3.org/2003/11/swrl#AtomList"/>
                <rdf:first>
                    <rdf:Description>
                        <rdf:type rdf:resource="http://www.w3.org/2003/11/swrl#IndividualPropertyAtom"/>
                        <swrl:propertyPredicate rdf:resource="https://w3id.org/def/propaphen#hasTimeInterval"/>
                        <swrl:argument1 rdf:resource="http://www.semanticweb.org/alencga1/ontologies/2023/2/PhenOWL/GCE"/>
                        <swrl:argument2 rdf:resource="http://www.semanticweb.org/alencga1/ontologies/2023/2/PhenOWL/PI1"/>
                    </rdf:Description>
                </rdf:first>
                <rdf:rest>
                    <rdf:Description>
                        <rdf:type rdf:resource="http://www.w3.org/2003/11/swrl#AtomList"/>
                        <rdf:first>
                            <rdf:Description>
                                <rdf:type rdf:resource="http://www.w3.org/2003/11/swrl#ClassAtom"/>
                                <swrl:classPredicate rdf:resource="http://www.w3.org/2006/time#Instant"/>
                                <swrl:argument1 rdf:resource="http://www.semanticweb.org/alencga1/ontologies/2023/2/PhenOWL/t1"/>
                            </rdf:Description>
                        </rdf:first>
                        <rdf:rest>
                            <rdf:Description>
                                <rdf:type rdf:resource="http://www.w3.org/2003/11/swrl#AtomList"/>
                                <rdf:first>
                                    <rdf:Description>
                                        <rdf:type rdf:resource="http://www.w3.org/2003/11/swrl#ClassAtom"/>
                                        <swrl:classPredicate rdf:resource="http://purl.org/nemo/gufo#ConcreteEntity"/>
                                        <swrl:argument1 rdf:resource="http://www.semanticweb.org/alencga1/ontologies/2023/2/PhenOWL/GCE"/>
                                    </rdf:Description>
                                </rdf:first>
                                <rdf:rest>
                                    <rdf:Description>
                                        <rdf:type rdf:resource="http://www.w3.org/2003/11/swrl#AtomList"/>
                                        <rdf:first>
                                            <rdf:Description>
                                                <rdf:type rdf:resource="http://www.w3.org/2003/11/swrl#ClassAtom"/>
                                                <swrl:classPredicate rdf:resource="http://www.w3.org/2006/time#ProperInterval"/>
                                                <swrl:argument1 rdf:resource="http://www.semanticweb.org/alencga1/ontologies/2023/2/PhenOWL/PI1"/>
                                            </rdf:Description>
                                        </rdf:first>
                                        <rdf:rest>
                                            <rdf:Description>
                                                <rdf:type rdf:resource="http://www.w3.org/2003/11/swrl#AtomList"/>
                                                <rdf:first>
                                                    <rdf:Description>
                                                        <rdf:type rdf:resource="http://www.w3.org/2003/11/swrl#IndividualPropertyAtom"/>
                                                        <swrl:propertyPredicate rdf:resource="http://www.w3.org/2006/time#hasBeginning"/>
                                                        <swrl:argument1 rdf:resource="http://www.semanticweb.org/alencga1/ontologies/2023/2/PhenOWL/PI1"/>
                                                        <swrl:argument2 rdf:resource="http://www.semanticweb.org/alencga1/ontologies/2023/2/PhenOWL/t1"/>
                                                    </rdf:Description>
                                                </rdf:first>
                                                <rdf:rest rdf:resource="http://www.w3.org/1999/02/22-rdf-syntax-ns#nil"/>
                                            </rdf:Description>
                                        </rdf:rest>
                                    </rdf:Description>
                                </rdf:rest>
                            </rdf:Description>
                        </rdf:rest>
                    </rdf:Description>
                </rdf:rest>
            </rdf:Description>
        </swrl:body>
        <swrl:head>
            <rdf:Description>
                <rdf:type rdf:resource="http://www.w3.org/2003/11/swrl#AtomList"/>
                <rdf:first>
                    <rdf:Description>
                        <rdf:type rdf:resource="http://www.w3.org/2003/11/swrl#IndividualPropertyAtom"/>
                        <swrl:propertyPredicate rdf:resource="http://purl.org/nemo/gufo#hasBeginPoint"/>
                        <swrl:argument1 rdf:resource="http://www.semanticweb.org/alencga1/ontologies/2023/2/PhenOWL/GCE"/>
                        <swrl:argument2 rdf:resource="http://www.semanticweb.org/alencga1/ontologies/2023/2/PhenOWL/t1"/>
                    </rdf:Description>
                </rdf:first>
                <rdf:rest rdf:resource="http://www.w3.org/1999/02/22-rdf-syntax-ns#nil"/>
            </rdf:Description>
        </swrl:head>
    </rdf:Description>
    <rdf:Description>
        <swrla:isRuleEnabled rdf:datatype="http://www.w3.org/2001/XMLSchema#boolean">true</swrla:isRuleEnabled>
        <rdfs:comment rdf:datatype="http://www.w3.org/2001/XMLSchema#string">Associates end point with beginning of time interval</rdfs:comment>
        <rdfs:label rdf:datatype="http://www.w3.org/2001/XMLSchema#string">s3.4 - inverse time interval end</rdfs:label>
        <rdf:type rdf:resource="http://www.w3.org/2003/11/swrl#Imp"/>
        <swrl:body>
            <rdf:Description>
                <rdf:type rdf:resource="http://www.w3.org/2003/11/swrl#AtomList"/>
                <rdf:first>
                    <rdf:Description>
                        <rdf:type rdf:resource="http://www.w3.org/2003/11/swrl#IndividualPropertyAtom"/>
                        <swrl:propertyPredicate rdf:resource="https://w3id.org/def/propaphen#hasTimeInterval"/>
                        <swrl:argument1 rdf:resource="http://www.semanticweb.org/alencga1/ontologies/2023/2/PhenOWL/GCE"/>
                        <swrl:argument2 rdf:resource="http://www.semanticweb.org/alencga1/ontologies/2023/2/PhenOWL/PI1"/>
                    </rdf:Description>
                </rdf:first>
                <rdf:rest>
                    <rdf:Description>
                        <rdf:type rdf:resource="http://www.w3.org/2003/11/swrl#AtomList"/>
                        <rdf:first>
                            <rdf:Description>
                                <rdf:type rdf:resource="http://www.w3.org/2003/11/swrl#ClassAtom"/>
                                <swrl:classPredicate rdf:resource="http://www.w3.org/2006/time#Instant"/>
                                <swrl:argument1 rdf:resource="http://www.semanticweb.org/alencga1/ontologies/2023/2/PhenOWL/t1"/>
                            </rdf:Description>
                        </rdf:first>
                        <rdf:rest>
                            <rdf:Description>
                                <rdf:type rdf:resource="http://www.w3.org/2003/11/swrl#AtomList"/>
                                <rdf:first>
                                    <rdf:Description>
                                        <rdf:type rdf:resource="http://www.w3.org/2003/11/swrl#IndividualPropertyAtom"/>
                                        <swrl:propertyPredicate rdf:resource="http://www.w3.org/2006/time#hasEnd"/>
                                        <swrl:argument1 rdf:resource="http://www.semanticweb.org/alencga1/ontologies/2023/2/PhenOWL/PI1"/>
                                        <swrl:argument2 rdf:resource="http://www.semanticweb.org/alencga1/ontologies/2023/2/PhenOWL/t1"/>
                                    </rdf:Description>
                                </rdf:first>
                                <rdf:rest>
                                    <rdf:Description>
                                        <rdf:type rdf:resource="http://www.w3.org/2003/11/swrl#AtomList"/>
                                        <rdf:first>
                                            <rdf:Description>
                                                <rdf:type rdf:resource="http://www.w3.org/2003/11/swrl#ClassAtom"/>
                                                <swrl:classPredicate rdf:resource="http://purl.org/nemo/gufo#ConcreteEntity"/>
                                                <swrl:argument1 rdf:resource="http://www.semanticweb.org/alencga1/ontologies/2023/2/PhenOWL/GCE"/>
                                            </rdf:Description>
                                        </rdf:first>
                                        <rdf:rest>
                                            <rdf:Description>
                                                <rdf:type rdf:resource="http://www.w3.org/2003/11/swrl#AtomList"/>
                                                <rdf:first>
                                                    <rdf:Description>
                                                        <rdf:type rdf:resource="http://www.w3.org/2003/11/swrl#ClassAtom"/>
                                                        <swrl:classPredicate rdf:resource="http://www.w3.org/2006/time#ProperInterval"/>
                                                        <swrl:argument1 rdf:resource="http://www.semanticweb.org/alencga1/ontologies/2023/2/PhenOWL/PI1"/>
                                                    </rdf:Description>
                                                </rdf:first>
                                                <rdf:rest rdf:resource="http://www.w3.org/1999/02/22-rdf-syntax-ns#nil"/>
                                            </rdf:Description>
                                        </rdf:rest>
                                    </rdf:Description>
                                </rdf:rest>
                            </rdf:Description>
                        </rdf:rest>
                    </rdf:Description>
                </rdf:rest>
            </rdf:Description>
        </swrl:body>
        <swrl:head>
            <rdf:Description>
                <rdf:type rdf:resource="http://www.w3.org/2003/11/swrl#AtomList"/>
                <rdf:first>
                    <rdf:Description>
                        <rdf:type rdf:resource="http://www.w3.org/2003/11/swrl#IndividualPropertyAtom"/>
                        <swrl:propertyPredicate rdf:resource="http://purl.org/nemo/gufo#hasEndPoint"/>
                        <swrl:argument1 rdf:resource="http://www.semanticweb.org/alencga1/ontologies/2023/2/PhenOWL/GCE"/>
                        <swrl:argument2 rdf:resource="http://www.semanticweb.org/alencga1/ontologies/2023/2/PhenOWL/t1"/>
                    </rdf:Description>
                </rdf:first>
                <rdf:rest rdf:resource="http://www.w3.org/1999/02/22-rdf-syntax-ns#nil"/>
            </rdf:Description>
        </swrl:head>
    </rdf:Description>
    <rdf:Description>
        <swrla:isRuleEnabled rdf:datatype="http://www.w3.org/2001/XMLSchema#boolean">true</swrla:isRuleEnabled>
        <rdfs:comment rdf:datatype="http://www.w3.org/2001/XMLSchema#string">If presence of cluster of individuals happens in one spatial region SO2, it must also happen in a region equals to it (SO1):</rdfs:comment>
        <rdfs:label rdf:datatype="http://www.w3.org/2001/XMLSchema#string">S1.2 - Presence SO eq</rdfs:label>
        <rdf:type rdf:resource="http://www.w3.org/2003/11/swrl#Imp"/>
        <swrl:body>
            <rdf:Description>
                <rdf:type rdf:resource="http://www.w3.org/2003/11/swrl#AtomList"/>
                <rdf:first>
                    <rdf:Description>
                        <rdf:type rdf:resource="http://www.w3.org/2003/11/swrl#ClassAtom"/>
                        <swrl:classPredicate rdf:resource="http://www.opengis.net/ont/geosparql#SpatialObject"/>
                        <swrl:argument1 rdf:resource="http://www.semanticweb.org/alencga1/ontologies/2023/2/PhenOWL/SO2"/>
                    </rdf:Description>
                </rdf:first>
                <rdf:rest>
                    <rdf:Description>
                        <rdf:type rdf:resource="http://www.w3.org/2003/11/swrl#AtomList"/>
                        <rdf:first>
                            <rdf:Description>
                                <rdf:type rdf:resource="http://www.w3.org/2003/11/swrl#ClassAtom"/>
                                <swrl:classPredicate rdf:resource="http://www.opengis.net/ont/geosparql#SpatialObject"/>
                                <swrl:argument1 rdf:resource="http://www.semanticweb.org/alencga1/ontologies/2023/2/PhenOWL/SO1"/>
                            </rdf:Description>
                        </rdf:first>
                        <rdf:rest>
                            <rdf:Description>
                                <rdf:type rdf:resource="http://www.w3.org/2003/11/swrl#AtomList"/>
                                <rdf:first>
                                    <rdf:Description>
                                        <rdf:type rdf:resource="http://www.w3.org/2003/11/swrl#IndividualPropertyAtom"/>
                                        <swrl:propertyPredicate rdf:resource="http://www.opengis.net/ont/geosparql#rcc8eq"/>
                                        <swrl:argument1 rdf:resource="http://www.semanticweb.org/alencga1/ontologies/2023/2/PhenOWL/SO1"/>
                                        <swrl:argument2 rdf:resource="http://www.semanticweb.org/alencga1/ontologies/2023/2/PhenOWL/SO2"/>
                                    </rdf:Description>
                                </rdf:first>
                                <rdf:rest>
                                    <rdf:Description>
                                        <rdf:type rdf:resource="http://www.w3.org/2003/11/swrl#AtomList"/>
                                        <rdf:first>
                                            <rdf:Description>
                                                <rdf:type rdf:resource="http://www.w3.org/2003/11/swrl#IndividualPropertyAtom"/>
                                                <swrl:propertyPredicate rdf:resource="https://w3id.org/def/propaphen#spatialPresenceIn"/>
                                                <swrl:argument1 rdf:resource="http://www.semanticweb.org/alencga1/ontologies/2023/2/PhenOWL/PR1"/>
                                                <swrl:argument2 rdf:resource="http://www.semanticweb.org/alencga1/ontologies/2023/2/PhenOWL/SO1"/>
                                            </rdf:Description>
                                        </rdf:first>
                                        <rdf:rest>
                                            <rdf:Description>
                                                <rdf:type rdf:resource="http://www.w3.org/2003/11/swrl#AtomList"/>
                                                <rdf:first>
                                                    <rdf:Description>
                                                        <rdf:type rdf:resource="http://www.w3.org/2003/11/swrl#ClassAtom"/>
                                                        <swrl:classPredicate rdf:resource="https://w3id.org/def/propaphen#Presence"/>
                                                        <swrl:argument1 rdf:resource="http://www.semanticweb.org/alencga1/ontologies/2023/2/PhenOWL/PR1"/>
                                                    </rdf:Description>
                                                </rdf:first>
                                                <rdf:rest rdf:resource="http://www.w3.org/1999/02/22-rdf-syntax-ns#nil"/>
                                            </rdf:Description>
                                        </rdf:rest>
                                    </rdf:Description>
                                </rdf:rest>
                            </rdf:Description>
                        </rdf:rest>
                    </rdf:Description>
                </rdf:rest>
            </rdf:Description>
        </swrl:body>
        <swrl:head>
            <rdf:Description>
                <rdf:type rdf:resource="http://www.w3.org/2003/11/swrl#AtomList"/>
                <rdf:first>
                    <rdf:Description>
                        <rdf:type rdf:resource="http://www.w3.org/2003/11/swrl#IndividualPropertyAtom"/>
                        <swrl:propertyPredicate rdf:resource="https://w3id.org/def/propaphen#spatialPresenceIn"/>
                        <swrl:argument1 rdf:resource="http://www.semanticweb.org/alencga1/ontologies/2023/2/PhenOWL/PR1"/>
                        <swrl:argument2 rdf:resource="http://www.semanticweb.org/alencga1/ontologies/2023/2/PhenOWL/SO2"/>
                    </rdf:Description>
                </rdf:first>
                <rdf:rest rdf:resource="http://www.w3.org/1999/02/22-rdf-syntax-ns#nil"/>
            </rdf:Description>
        </swrl:head>
    </rdf:Description>
    <rdf:Description>
        <swrla:isRuleEnabled rdf:datatype="http://www.w3.org/2001/XMLSchema#boolean">true</swrla:isRuleEnabled>
        <rdfs:comment rdf:datatype="http://www.w3.org/2001/XMLSchema#string">If presence of cluster of individuals happens in one spatial region SO2, it must also happen in a region containing it (SO1):</rdfs:comment>
        <rdfs:label rdf:datatype="http://www.w3.org/2001/XMLSchema#string">S1.3 - Presence SO nttp</rdfs:label>
        <rdf:type rdf:resource="http://www.w3.org/2003/11/swrl#Imp"/>
        <swrl:body>
            <rdf:Description>
                <rdf:type rdf:resource="http://www.w3.org/2003/11/swrl#AtomList"/>
                <rdf:first>
                    <rdf:Description>
                        <rdf:type rdf:resource="http://www.w3.org/2003/11/swrl#IndividualPropertyAtom"/>
                        <swrl:propertyPredicate rdf:resource="http://www.opengis.net/ont/geosparql#rcc8ntpp"/>
                        <swrl:argument1 rdf:resource="http://www.semanticweb.org/alencga1/ontologies/2023/2/PhenOWL/SO1"/>
                        <swrl:argument2 rdf:resource="http://www.semanticweb.org/alencga1/ontologies/2023/2/PhenOWL/SO2"/>
                    </rdf:Description>
                </rdf:first>
                <rdf:rest>
                    <rdf:Description>
                        <rdf:type rdf:resource="http://www.w3.org/2003/11/swrl#AtomList"/>
                        <rdf:first>
                            <rdf:Description>
                                <rdf:type rdf:resource="http://www.w3.org/2003/11/swrl#ClassAtom"/>
                                <swrl:classPredicate rdf:resource="http://www.opengis.net/ont/geosparql#SpatialObject"/>
                                <swrl:argument1 rdf:resource="http://www.semanticweb.org/alencga1/ontologies/2023/2/PhenOWL/SO2"/>
                            </rdf:Description>
                        </rdf:first>
                        <rdf:rest>
                            <rdf:Description>
                                <rdf:type rdf:resource="http://www.w3.org/2003/11/swrl#AtomList"/>
                                <rdf:first>
                                    <rdf:Description>
                                        <rdf:type rdf:resource="http://www.w3.org/2003/11/swrl#ClassAtom"/>
                                        <swrl:classPredicate rdf:resource="http://www.opengis.net/ont/geosparql#SpatialObject"/>
                                        <swrl:argument1 rdf:resource="http://www.semanticweb.org/alencga1/ontologies/2023/2/PhenOWL/SO1"/>
                                    </rdf:Description>
                                </rdf:first>
                                <rdf:rest>
                                    <rdf:Description>
                                        <rdf:type rdf:resource="http://www.w3.org/2003/11/swrl#AtomList"/>
                                        <rdf:first>
                                            <rdf:Description>
                                                <rdf:type rdf:resource="http://www.w3.org/2003/11/swrl#IndividualPropertyAtom"/>
                                                <swrl:propertyPredicate rdf:resource="https://w3id.org/def/propaphen#spatialPresenceIn"/>
                                                <swrl:argument1 rdf:resource="http://www.semanticweb.org/alencga1/ontologies/2023/2/PhenOWL/PR1"/>
                                                <swrl:argument2 rdf:resource="http://www.semanticweb.org/alencga1/ontologies/2023/2/PhenOWL/SO1"/>
                                            </rdf:Description>
                                        </rdf:first>
                                        <rdf:rest>
                                            <rdf:Description>
                                                <rdf:type rdf:resource="http://www.w3.org/2003/11/swrl#AtomList"/>
                                                <rdf:first>
                                                    <rdf:Description>
                                                        <rdf:type rdf:resource="http://www.w3.org/2003/11/swrl#ClassAtom"/>
                                                        <swrl:classPredicate rdf:resource="https://w3id.org/def/propaphen#Presence"/>
                                                        <swrl:argument1 rdf:resource="http://www.semanticweb.org/alencga1/ontologies/2023/2/PhenOWL/PR1"/>
                                                    </rdf:Description>
                                                </rdf:first>
                                                <rdf:rest rdf:resource="http://www.w3.org/1999/02/22-rdf-syntax-ns#nil"/>
                                            </rdf:Description>
                                        </rdf:rest>
                                    </rdf:Description>
                                </rdf:rest>
                            </rdf:Description>
                        </rdf:rest>
                    </rdf:Description>
                </rdf:rest>
            </rdf:Description>
        </swrl:body>
        <swrl:head>
            <rdf:Description>
                <rdf:type rdf:resource="http://www.w3.org/2003/11/swrl#AtomList"/>
                <rdf:first>
                    <rdf:Description>
                        <rdf:type rdf:resource="http://www.w3.org/2003/11/swrl#IndividualPropertyAtom"/>
                        <swrl:propertyPredicate rdf:resource="https://w3id.org/def/propaphen#spatialPresenceIn"/>
                        <swrl:argument1 rdf:resource="http://www.semanticweb.org/alencga1/ontologies/2023/2/PhenOWL/PR1"/>
                        <swrl:argument2 rdf:resource="http://www.semanticweb.org/alencga1/ontologies/2023/2/PhenOWL/SO2"/>
                    </rdf:Description>
                </rdf:first>
                <rdf:rest rdf:resource="http://www.w3.org/1999/02/22-rdf-syntax-ns#nil"/>
            </rdf:Description>
        </swrl:head>
    </rdf:Description>
    <rdf:Description>
        <swrla:isRuleEnabled rdf:datatype="http://www.w3.org/2001/XMLSchema#boolean">true</swrla:isRuleEnabled>
        <rdfs:comment rdf:datatype="http://www.w3.org/2001/XMLSchema#string">If presence of cluster of individuals happens in one spatial region SO2, it must also happen in a region containing it (SO1)</rdfs:comment>
        <rdfs:label rdf:datatype="http://www.w3.org/2001/XMLSchema#string">S1.1 - Presence SO ttp</rdfs:label>
        <rdf:type rdf:resource="http://www.w3.org/2003/11/swrl#Imp"/>
        <swrl:body>
            <rdf:Description>
                <rdf:type rdf:resource="http://www.w3.org/2003/11/swrl#AtomList"/>
                <rdf:first>
                    <rdf:Description>
                        <rdf:type rdf:resource="http://www.w3.org/2003/11/swrl#ClassAtom"/>
                        <swrl:classPredicate rdf:resource="http://www.opengis.net/ont/geosparql#SpatialObject"/>
                        <swrl:argument1 rdf:resource="http://www.semanticweb.org/alencga1/ontologies/2023/2/PhenOWL/SO2"/>
                    </rdf:Description>
                </rdf:first>
                <rdf:rest>
                    <rdf:Description>
                        <rdf:type rdf:resource="http://www.w3.org/2003/11/swrl#AtomList"/>
                        <rdf:first>
                            <rdf:Description>
                                <rdf:type rdf:resource="http://www.w3.org/2003/11/swrl#ClassAtom"/>
                                <swrl:classPredicate rdf:resource="http://www.opengis.net/ont/geosparql#SpatialObject"/>
                                <swrl:argument1 rdf:resource="http://www.semanticweb.org/alencga1/ontologies/2023/2/PhenOWL/SO1"/>
                            </rdf:Description>
                        </rdf:first>
                        <rdf:rest>
                            <rdf:Description>
                                <rdf:type rdf:resource="http://www.w3.org/2003/11/swrl#AtomList"/>
                                <rdf:first>
                                    <rdf:Description>
                                        <rdf:type rdf:resource="http://www.w3.org/2003/11/swrl#IndividualPropertyAtom"/>
                                        <swrl:propertyPredicate rdf:resource="http://www.opengis.net/ont/geosparql#rcc8tpp"/>
                                        <swrl:argument1 rdf:resource="http://www.semanticweb.org/alencga1/ontologies/2023/2/PhenOWL/SO1"/>
                                        <swrl:argument2 rdf:resource="http://www.semanticweb.org/alencga1/ontologies/2023/2/PhenOWL/SO2"/>
                                    </rdf:Description>
                                </rdf:first>
                                <rdf:rest>
                                    <rdf:Description>
                                        <rdf:type rdf:resource="http://www.w3.org/2003/11/swrl#AtomList"/>
                                        <rdf:first>
                                            <rdf:Description>
                                                <rdf:type rdf:resource="http://www.w3.org/2003/11/swrl#IndividualPropertyAtom"/>
                                                <swrl:propertyPredicate rdf:resource="https://w3id.org/def/propaphen#spatialPresenceIn"/>
                                                <swrl:argument1 rdf:resource="http://www.semanticweb.org/alencga1/ontologies/2023/2/PhenOWL/PR1"/>
                                                <swrl:argument2 rdf:resource="http://www.semanticweb.org/alencga1/ontologies/2023/2/PhenOWL/SO1"/>
                                            </rdf:Description>
                                        </rdf:first>
                                        <rdf:rest>
                                            <rdf:Description>
                                                <rdf:type rdf:resource="http://www.w3.org/2003/11/swrl#AtomList"/>
                                                <rdf:first>
                                                    <rdf:Description>
                                                        <rdf:type rdf:resource="http://www.w3.org/2003/11/swrl#ClassAtom"/>
                                                        <swrl:classPredicate rdf:resource="https://w3id.org/def/propaphen#Presence"/>
                                                        <swrl:argument1 rdf:resource="http://www.semanticweb.org/alencga1/ontologies/2023/2/PhenOWL/PR1"/>
                                                    </rdf:Description>
                                                </rdf:first>
                                                <rdf:rest rdf:resource="http://www.w3.org/1999/02/22-rdf-syntax-ns#nil"/>
                                            </rdf:Description>
                                        </rdf:rest>
                                    </rdf:Description>
                                </rdf:rest>
                            </rdf:Description>
                        </rdf:rest>
                    </rdf:Description>
                </rdf:rest>
            </rdf:Description>
        </swrl:body>
        <swrl:head>
            <rdf:Description>
                <rdf:type rdf:resource="http://www.w3.org/2003/11/swrl#AtomList"/>
                <rdf:first>
                    <rdf:Description>
                        <rdf:type rdf:resource="http://www.w3.org/2003/11/swrl#IndividualPropertyAtom"/>
                        <swrl:propertyPredicate rdf:resource="https://w3id.org/def/propaphen#spatialPresenceIn"/>
                        <swrl:argument1 rdf:resource="http://www.semanticweb.org/alencga1/ontologies/2023/2/PhenOWL/PR1"/>
                        <swrl:argument2 rdf:resource="http://www.semanticweb.org/alencga1/ontologies/2023/2/PhenOWL/SO2"/>
                    </rdf:Description>
                </rdf:first>
                <rdf:rest rdf:resource="http://www.w3.org/1999/02/22-rdf-syntax-ns#nil"/>
            </rdf:Description>
        </swrl:head>
    </rdf:Description>
    <rdf:Description>
        <swrla:isRuleEnabled rdf:datatype="http://www.w3.org/2001/XMLSchema#boolean">true</swrla:isRuleEnabled>
        <rdfs:comment rdf:datatype="http://www.w3.org/2001/XMLSchema#string">Presence of group of Individuals in both node/system and observation (eq contains)</rdfs:comment>
        <rdfs:label rdf:datatype="http://www.w3.org/2001/XMLSchema#string">S4.6 - Pr in Obs (eq contains)</rdfs:label>
        <rdf:type rdf:resource="http://www.w3.org/2003/11/swrl#Imp"/>
        <swrl:body>
            <rdf:Description>
                <rdf:type rdf:resource="http://www.w3.org/2003/11/swrl#AtomList"/>
                <rdf:first>
                    <rdf:Description>
                        <rdf:type rdf:resource="http://www.w3.org/2003/11/swrl#IndividualPropertyAtom"/>
                        <swrl:propertyPredicate rdf:resource="http://www.w3.org/2006/time#intervalContains"/>
                        <swrl:argument1 rdf:resource="http://www.semanticweb.org/alencga1/ontologies/2023/2/PhenOWL/PI1"/>
                        <swrl:argument2 rdf:resource="http://www.semanticweb.org/alencga1/ontologies/2023/2/PhenOWL/PI2"/>
                    </rdf:Description>
                </rdf:first>
                <rdf:rest>
                    <rdf:Description>
                        <rdf:type rdf:resource="http://www.w3.org/2003/11/swrl#AtomList"/>
                        <rdf:first>
                            <rdf:Description>
                                <rdf:type rdf:resource="http://www.w3.org/2003/11/swrl#ClassAtom"/>
                                <swrl:classPredicate rdf:resource="https://w3id.org/def/propaphen#Observation"/>
                                <swrl:argument1 rdf:resource="http://www.semanticweb.org/alencga1/ontologies/2023/2/PhenOWL/O1"/>
                            </rdf:Description>
                        </rdf:first>
                        <rdf:rest>
                            <rdf:Description>
                                <rdf:type rdf:resource="http://www.w3.org/2003/11/swrl#AtomList"/>
                                <rdf:first>
                                    <rdf:Description>
                                        <rdf:type rdf:resource="http://www.w3.org/2003/11/swrl#ClassAtom"/>
                                        <swrl:classPredicate rdf:resource="http://www.opengis.net/ont/geosparql#SpatialObject"/>
                                        <swrl:argument1 rdf:resource="http://www.semanticweb.org/alencga1/ontologies/2023/2/PhenOWL/SO2"/>
                                    </rdf:Description>
                                </rdf:first>
                                <rdf:rest>
                                    <rdf:Description>
                                        <rdf:type rdf:resource="http://www.w3.org/2003/11/swrl#AtomList"/>
                                        <rdf:first>
                                            <rdf:Description>
                                                <rdf:type rdf:resource="http://www.w3.org/2003/11/swrl#ClassAtom"/>
                                                <swrl:classPredicate rdf:resource="http://www.w3.org/2006/time#ProperInterval"/>
                                                <swrl:argument1 rdf:resource="http://www.semanticweb.org/alencga1/ontologies/2023/2/PhenOWL/PI1"/>
                                            </rdf:Description>
                                        </rdf:first>
                                        <rdf:rest>
                                            <rdf:Description>
                                                <rdf:type rdf:resource="http://www.w3.org/2003/11/swrl#AtomList"/>
                                                <rdf:first>
                                                    <rdf:Description>
                                                        <rdf:type rdf:resource="http://www.w3.org/2003/11/swrl#ClassAtom"/>
                                                        <swrl:classPredicate rdf:resource="https://w3id.org/seas/System"/>
                                                        <swrl:argument1 rdf:resource="http://www.semanticweb.org/alencga1/ontologies/2023/2/PhenOWL/S1"/>
                                                    </rdf:Description>
                                                </rdf:first>
                                                <rdf:rest>
                                                    <rdf:Description>
                                                        <rdf:type rdf:resource="http://www.w3.org/2003/11/swrl#AtomList"/>
                                                        <rdf:first>
                                                            <rdf:Description>
                                                                <rdf:type rdf:resource="http://www.w3.org/2003/11/swrl#ClassAtom"/>
                                                                <swrl:classPredicate rdf:resource="http://www.w3.org/2006/time#ProperInterval"/>
                                                                <swrl:argument1 rdf:resource="http://www.semanticweb.org/alencga1/ontologies/2023/2/PhenOWL/PI2"/>
                                                            </rdf:Description>
                                                        </rdf:first>
                                                        <rdf:rest>
                                                            <rdf:Description>
                                                                <rdf:type rdf:resource="http://www.w3.org/2003/11/swrl#AtomList"/>
                                                                <rdf:first>
                                                                    <rdf:Description>
                                                                        <rdf:type rdf:resource="http://www.w3.org/2003/11/swrl#IndividualPropertyAtom"/>
                                                                        <swrl:propertyPredicate rdf:resource="https://w3id.org/def/propaphen#hasTimeInterval"/>
                                                                        <swrl:argument1 rdf:resource="http://www.semanticweb.org/alencga1/ontologies/2023/2/PhenOWL/O1"/>
                                                                        <swrl:argument2 rdf:resource="http://www.semanticweb.org/alencga1/ontologies/2023/2/PhenOWL/PI1"/>
                                                                    </rdf:Description>
                                                                </rdf:first>
                                                                <rdf:rest>
                                                                    <rdf:Description>
                                                                        <rdf:type rdf:resource="http://www.w3.org/2003/11/swrl#AtomList"/>
                                                                        <rdf:first>
                                                                            <rdf:Description>
                                                                                <rdf:type rdf:resource="http://www.w3.org/2003/11/swrl#IndividualPropertyAtom"/>
                                                                                <swrl:propertyPredicate rdf:resource="https://w3id.org/def/propaphen#happensIn"/>
                                                                                <swrl:argument1 rdf:resource="http://www.semanticweb.org/alencga1/ontologies/2023/2/PhenOWL/O1"/>
                                                                                <swrl:argument2 rdf:resource="http://www.semanticweb.org/alencga1/ontologies/2023/2/PhenOWL/S1"/>
                                                                            </rdf:Description>
                                                                        </rdf:first>
                                                                        <rdf:rest>
                                                                            <rdf:Description>
                                                                                <rdf:type rdf:resource="http://www.w3.org/2003/11/swrl#AtomList"/>
                                                                                <rdf:first>
                                                                                    <rdf:Description>
                                                                                        <rdf:type rdf:resource="http://www.w3.org/2003/11/swrl#IndividualPropertyAtom"/>
                                                                                        <swrl:propertyPredicate rdf:resource="https://w3id.org/def/propaphen#spatialPresenceIn"/>
                                                                                        <swrl:argument1 rdf:resource="http://www.semanticweb.org/alencga1/ontologies/2023/2/PhenOWL/PR1"/>
                                                                                        <swrl:argument2 rdf:resource="http://www.semanticweb.org/alencga1/ontologies/2023/2/PhenOWL/SO2"/>
                                                                                    </rdf:Description>
                                                                                </rdf:first>
                                                                                <rdf:rest>
                                                                                    <rdf:Description>
                                                                                        <rdf:type rdf:resource="http://www.w3.org/2003/11/swrl#AtomList"/>
                                                                                        <rdf:first>
                                                                                            <rdf:Description>
                                                                                                <rdf:type rdf:resource="http://www.w3.org/2003/11/swrl#ClassAtom"/>
                                                                                                <swrl:classPredicate rdf:resource="https://w3id.org/def/propaphen#Presence"/>
                                                                                                <swrl:argument1 rdf:resource="http://www.semanticweb.org/alencga1/ontologies/2023/2/PhenOWL/PR1"/>
                                                                                            </rdf:Description>
                                                                                        </rdf:first>
                                                                                        <rdf:rest>
                                                                                            <rdf:Description>
                                                                                                <rdf:type rdf:resource="http://www.w3.org/2003/11/swrl#AtomList"/>
                                                                                                <rdf:first>
                                                                                                    <rdf:Description>
                                                                                                        <rdf:type rdf:resource="http://www.w3.org/2003/11/swrl#IndividualPropertyAtom"/>
                                                                                                        <swrl:propertyPredicate rdf:resource="https://w3id.org/def/propaphen#hasTimeInterval"/>
                                                                                                        <swrl:argument1 rdf:resource="http://www.semanticweb.org/alencga1/ontologies/2023/2/PhenOWL/PR1"/>
                                                                                                        <swrl:argument2 rdf:resource="http://www.semanticweb.org/alencga1/ontologies/2023/2/PhenOWL/PI2"/>
                                                                                                    </rdf:Description>
                                                                                                </rdf:first>
                                                                                                <rdf:rest>
                                                                                                    <rdf:Description>
                                                                                                        <rdf:type rdf:resource="http://www.w3.org/2003/11/swrl#AtomList"/>
                                                                                                        <rdf:first>
                                                                                                            <rdf:Description>
                                                                                                                <rdf:type rdf:resource="http://www.w3.org/2003/11/swrl#IndividualPropertyAtom"/>
                                                                                                                <swrl:propertyPredicate rdf:resource="http://www.opengis.net/ont/geosparql#rcc8eq"/>
                                                                                                                <swrl:argument1 rdf:resource="http://www.semanticweb.org/alencga1/ontologies/2023/2/PhenOWL/SO2"/>
                                                                                                                <swrl:argument2 rdf:resource="http://www.semanticweb.org/alencga1/ontologies/2023/2/PhenOWL/S1"/>
                                                                                                            </rdf:Description>
                                                                                                        </rdf:first>
                                                                                                        <rdf:rest rdf:resource="http://www.w3.org/1999/02/22-rdf-syntax-ns#nil"/>
                                                                                                    </rdf:Description>
                                                                                                </rdf:rest>
                                                                                            </rdf:Description>
                                                                                        </rdf:rest>
                                                                                    </rdf:Description>
                                                                                </rdf:rest>
                                                                            </rdf:Description>
                                                                        </rdf:rest>
                                                                    </rdf:Description>
                                                                </rdf:rest>
                                                            </rdf:Description>
                                                        </rdf:rest>
                                                    </rdf:Description>
                                                </rdf:rest>
                                            </rdf:Description>
                                        </rdf:rest>
                                    </rdf:Description>
                                </rdf:rest>
                            </rdf:Description>
                        </rdf:rest>
                    </rdf:Description>
                </rdf:rest>
            </rdf:Description>
        </swrl:body>
        <swrl:head>
            <rdf:Description>
                <rdf:type rdf:resource="http://www.w3.org/2003/11/swrl#AtomList"/>
                <rdf:first>
                    <rdf:Description>
                        <rdf:type rdf:resource="http://www.w3.org/2003/11/swrl#IndividualPropertyAtom"/>
                        <swrl:propertyPredicate rdf:resource="https://w3id.org/def/propaphen#observationalPresenceIn"/>
                        <swrl:argument1 rdf:resource="http://www.semanticweb.org/alencga1/ontologies/2023/2/PhenOWL/PR1"/>
                        <swrl:argument2 rdf:resource="http://www.semanticweb.org/alencga1/ontologies/2023/2/PhenOWL/O1"/>
                    </rdf:Description>
                </rdf:first>
                <rdf:rest rdf:resource="http://www.w3.org/1999/02/22-rdf-syntax-ns#nil"/>
            </rdf:Description>
        </swrl:head>
    </rdf:Description>
    <rdf:Description>
        <swrla:isRuleEnabled rdf:datatype="http://www.w3.org/2001/XMLSchema#boolean">true</swrla:isRuleEnabled>
        <rdfs:comment rdf:datatype="http://www.w3.org/2001/XMLSchema#string">Presence of group of Individuals in both node/system and observation (eq equals)</rdfs:comment>
        <rdfs:label rdf:datatype="http://www.w3.org/2001/XMLSchema#string">S4.3 - Pr in Obs (eq equals)</rdfs:label>
        <rdf:type rdf:resource="http://www.w3.org/2003/11/swrl#Imp"/>
        <swrl:body>
            <rdf:Description>
                <rdf:type rdf:resource="http://www.w3.org/2003/11/swrl#AtomList"/>
                <rdf:first>
                    <rdf:Description>
                        <rdf:type rdf:resource="http://www.w3.org/2003/11/swrl#IndividualPropertyAtom"/>
                        <swrl:propertyPredicate rdf:resource="http://www.w3.org/2006/time#intervalEquals"/>
                        <swrl:argument1 rdf:resource="http://www.semanticweb.org/alencga1/ontologies/2023/2/PhenOWL/PI1"/>
                        <swrl:argument2 rdf:resource="http://www.semanticweb.org/alencga1/ontologies/2023/2/PhenOWL/PI2"/>
                    </rdf:Description>
                </rdf:first>
                <rdf:rest>
                    <rdf:Description>
                        <rdf:type rdf:resource="http://www.w3.org/2003/11/swrl#AtomList"/>
                        <rdf:first>
                            <rdf:Description>
                                <rdf:type rdf:resource="http://www.w3.org/2003/11/swrl#ClassAtom"/>
                                <swrl:classPredicate rdf:resource="https://w3id.org/def/propaphen#Observation"/>
                                <swrl:argument1 rdf:resource="http://www.semanticweb.org/alencga1/ontologies/2023/2/PhenOWL/O1"/>
                            </rdf:Description>
                        </rdf:first>
                        <rdf:rest>
                            <rdf:Description>
                                <rdf:type rdf:resource="http://www.w3.org/2003/11/swrl#AtomList"/>
                                <rdf:first>
                                    <rdf:Description>
                                        <rdf:type rdf:resource="http://www.w3.org/2003/11/swrl#ClassAtom"/>
                                        <swrl:classPredicate rdf:resource="http://www.opengis.net/ont/geosparql#SpatialObject"/>
                                        <swrl:argument1 rdf:resource="http://www.semanticweb.org/alencga1/ontologies/2023/2/PhenOWL/SO2"/>
                                    </rdf:Description>
                                </rdf:first>
                                <rdf:rest>
                                    <rdf:Description>
                                        <rdf:type rdf:resource="http://www.w3.org/2003/11/swrl#AtomList"/>
                                        <rdf:first>
                                            <rdf:Description>
                                                <rdf:type rdf:resource="http://www.w3.org/2003/11/swrl#ClassAtom"/>
                                                <swrl:classPredicate rdf:resource="http://www.w3.org/2006/time#ProperInterval"/>
                                                <swrl:argument1 rdf:resource="http://www.semanticweb.org/alencga1/ontologies/2023/2/PhenOWL/PI1"/>
                                            </rdf:Description>
                                        </rdf:first>
                                        <rdf:rest>
                                            <rdf:Description>
                                                <rdf:type rdf:resource="http://www.w3.org/2003/11/swrl#AtomList"/>
                                                <rdf:first>
                                                    <rdf:Description>
                                                        <rdf:type rdf:resource="http://www.w3.org/2003/11/swrl#ClassAtom"/>
                                                        <swrl:classPredicate rdf:resource="https://w3id.org/seas/System"/>
                                                        <swrl:argument1 rdf:resource="http://www.semanticweb.org/alencga1/ontologies/2023/2/PhenOWL/S1"/>
                                                    </rdf:Description>
                                                </rdf:first>
                                                <rdf:rest>
                                                    <rdf:Description>
                                                        <rdf:type rdf:resource="http://www.w3.org/2003/11/swrl#AtomList"/>
                                                        <rdf:first>
                                                            <rdf:Description>
                                                                <rdf:type rdf:resource="http://www.w3.org/2003/11/swrl#ClassAtom"/>
                                                                <swrl:classPredicate rdf:resource="http://www.w3.org/2006/time#ProperInterval"/>
                                                                <swrl:argument1 rdf:resource="http://www.semanticweb.org/alencga1/ontologies/2023/2/PhenOWL/PI2"/>
                                                            </rdf:Description>
                                                        </rdf:first>
                                                        <rdf:rest>
                                                            <rdf:Description>
                                                                <rdf:type rdf:resource="http://www.w3.org/2003/11/swrl#AtomList"/>
                                                                <rdf:first>
                                                                    <rdf:Description>
                                                                        <rdf:type rdf:resource="http://www.w3.org/2003/11/swrl#IndividualPropertyAtom"/>
                                                                        <swrl:propertyPredicate rdf:resource="https://w3id.org/def/propaphen#hasTimeInterval"/>
                                                                        <swrl:argument1 rdf:resource="http://www.semanticweb.org/alencga1/ontologies/2023/2/PhenOWL/O1"/>
                                                                        <swrl:argument2 rdf:resource="http://www.semanticweb.org/alencga1/ontologies/2023/2/PhenOWL/PI1"/>
                                                                    </rdf:Description>
                                                                </rdf:first>
                                                                <rdf:rest>
                                                                    <rdf:Description>
                                                                        <rdf:type rdf:resource="http://www.w3.org/2003/11/swrl#AtomList"/>
                                                                        <rdf:first>
                                                                            <rdf:Description>
                                                                                <rdf:type rdf:resource="http://www.w3.org/2003/11/swrl#IndividualPropertyAtom"/>
                                                                                <swrl:propertyPredicate rdf:resource="https://w3id.org/def/propaphen#happensIn"/>
                                                                                <swrl:argument1 rdf:resource="http://www.semanticweb.org/alencga1/ontologies/2023/2/PhenOWL/O1"/>
                                                                                <swrl:argument2 rdf:resource="http://www.semanticweb.org/alencga1/ontologies/2023/2/PhenOWL/S1"/>
                                                                            </rdf:Description>
                                                                        </rdf:first>
                                                                        <rdf:rest>
                                                                            <rdf:Description>
                                                                                <rdf:type rdf:resource="http://www.w3.org/2003/11/swrl#AtomList"/>
                                                                                <rdf:first>
                                                                                    <rdf:Description>
                                                                                        <rdf:type rdf:resource="http://www.w3.org/2003/11/swrl#IndividualPropertyAtom"/>
                                                                                        <swrl:propertyPredicate rdf:resource="https://w3id.org/def/propaphen#spatialPresenceIn"/>
                                                                                        <swrl:argument1 rdf:resource="http://www.semanticweb.org/alencga1/ontologies/2023/2/PhenOWL/PR1"/>
                                                                                        <swrl:argument2 rdf:resource="http://www.semanticweb.org/alencga1/ontologies/2023/2/PhenOWL/SO2"/>
                                                                                    </rdf:Description>
                                                                                </rdf:first>
                                                                                <rdf:rest>
                                                                                    <rdf:Description>
                                                                                        <rdf:type rdf:resource="http://www.w3.org/2003/11/swrl#AtomList"/>
                                                                                        <rdf:first>
                                                                                            <rdf:Description>
                                                                                                <rdf:type rdf:resource="http://www.w3.org/2003/11/swrl#ClassAtom"/>
                                                                                                <swrl:classPredicate rdf:resource="https://w3id.org/def/propaphen#Presence"/>
                                                                                                <swrl:argument1 rdf:resource="http://www.semanticweb.org/alencga1/ontologies/2023/2/PhenOWL/PR1"/>
                                                                                            </rdf:Description>
                                                                                        </rdf:first>
                                                                                        <rdf:rest>
                                                                                            <rdf:Description>
                                                                                                <rdf:type rdf:resource="http://www.w3.org/2003/11/swrl#AtomList"/>
                                                                                                <rdf:first>
                                                                                                    <rdf:Description>
                                                                                                        <rdf:type rdf:resource="http://www.w3.org/2003/11/swrl#IndividualPropertyAtom"/>
                                                                                                        <swrl:propertyPredicate rdf:resource="https://w3id.org/def/propaphen#hasTimeInterval"/>
                                                                                                        <swrl:argument1 rdf:resource="http://www.semanticweb.org/alencga1/ontologies/2023/2/PhenOWL/PR1"/>
                                                                                                        <swrl:argument2 rdf:resource="http://www.semanticweb.org/alencga1/ontologies/2023/2/PhenOWL/PI2"/>
                                                                                                    </rdf:Description>
                                                                                                </rdf:first>
                                                                                                <rdf:rest>
                                                                                                    <rdf:Description>
                                                                                                        <rdf:type rdf:resource="http://www.w3.org/2003/11/swrl#AtomList"/>
                                                                                                        <rdf:first>
                                                                                                            <rdf:Description>
                                                                                                                <rdf:type rdf:resource="http://www.w3.org/2003/11/swrl#IndividualPropertyAtom"/>
                                                                                                                <swrl:propertyPredicate rdf:resource="http://www.opengis.net/ont/geosparql#rcc8eq"/>
                                                                                                                <swrl:argument1 rdf:resource="http://www.semanticweb.org/alencga1/ontologies/2023/2/PhenOWL/SO2"/>
                                                                                                                <swrl:argument2 rdf:resource="http://www.semanticweb.org/alencga1/ontologies/2023/2/PhenOWL/S1"/>
                                                                                                            </rdf:Description>
                                                                                                        </rdf:first>
                                                                                                        <rdf:rest rdf:resource="http://www.w3.org/1999/02/22-rdf-syntax-ns#nil"/>
                                                                                                    </rdf:Description>
                                                                                                </rdf:rest>
                                                                                            </rdf:Description>
                                                                                        </rdf:rest>
                                                                                    </rdf:Description>
                                                                                </rdf:rest>
                                                                            </rdf:Description>
                                                                        </rdf:rest>
                                                                    </rdf:Description>
                                                                </rdf:rest>
                                                            </rdf:Description>
                                                        </rdf:rest>
                                                    </rdf:Description>
                                                </rdf:rest>
                                            </rdf:Description>
                                        </rdf:rest>
                                    </rdf:Description>
                                </rdf:rest>
                            </rdf:Description>
                        </rdf:rest>
                    </rdf:Description>
                </rdf:rest>
            </rdf:Description>
        </swrl:body>
        <swrl:head>
            <rdf:Description>
                <rdf:type rdf:resource="http://www.w3.org/2003/11/swrl#AtomList"/>
                <rdf:first>
                    <rdf:Description>
                        <rdf:type rdf:resource="http://www.w3.org/2003/11/swrl#IndividualPropertyAtom"/>
                        <swrl:propertyPredicate rdf:resource="https://w3id.org/def/propaphen#observationalPresenceIn"/>
                        <swrl:argument1 rdf:resource="http://www.semanticweb.org/alencga1/ontologies/2023/2/PhenOWL/PR1"/>
                        <swrl:argument2 rdf:resource="http://www.semanticweb.org/alencga1/ontologies/2023/2/PhenOWL/O1"/>
                    </rdf:Description>
                </rdf:first>
                <rdf:rest rdf:resource="http://www.w3.org/1999/02/22-rdf-syntax-ns#nil"/>
            </rdf:Description>
        </swrl:head>
    </rdf:Description>
    <rdf:Description>
        <swrla:isRuleEnabled rdf:datatype="http://www.w3.org/2001/XMLSchema#boolean">true</swrla:isRuleEnabled>
        <rdfs:comment rdf:datatype="http://www.w3.org/2001/XMLSchema#string">Presence of group of Individuals in both node/system and observation (ntpp contains)</rdfs:comment>
        <rdfs:label rdf:datatype="http://www.w3.org/2001/XMLSchema#string">S4.5 - Pr in Obs (nttp contains)</rdfs:label>
        <rdf:type rdf:resource="http://www.w3.org/2003/11/swrl#Imp"/>
        <swrl:body>
            <rdf:Description>
                <rdf:type rdf:resource="http://www.w3.org/2003/11/swrl#AtomList"/>
                <rdf:first>
                    <rdf:Description>
                        <rdf:type rdf:resource="http://www.w3.org/2003/11/swrl#IndividualPropertyAtom"/>
                        <swrl:propertyPredicate rdf:resource="http://www.w3.org/2006/time#intervalContains"/>
                        <swrl:argument1 rdf:resource="http://www.semanticweb.org/alencga1/ontologies/2023/2/PhenOWL/PI1"/>
                        <swrl:argument2 rdf:resource="http://www.semanticweb.org/alencga1/ontologies/2023/2/PhenOWL/PI2"/>
                    </rdf:Description>
                </rdf:first>
                <rdf:rest>
                    <rdf:Description>
                        <rdf:type rdf:resource="http://www.w3.org/2003/11/swrl#AtomList"/>
                        <rdf:first>
                            <rdf:Description>
                                <rdf:type rdf:resource="http://www.w3.org/2003/11/swrl#ClassAtom"/>
                                <swrl:classPredicate rdf:resource="https://w3id.org/def/propaphen#Observation"/>
                                <swrl:argument1 rdf:resource="http://www.semanticweb.org/alencga1/ontologies/2023/2/PhenOWL/O1"/>
                            </rdf:Description>
                        </rdf:first>
                        <rdf:rest>
                            <rdf:Description>
                                <rdf:type rdf:resource="http://www.w3.org/2003/11/swrl#AtomList"/>
                                <rdf:first>
                                    <rdf:Description>
                                        <rdf:type rdf:resource="http://www.w3.org/2003/11/swrl#ClassAtom"/>
                                        <swrl:classPredicate rdf:resource="http://www.opengis.net/ont/geosparql#SpatialObject"/>
                                        <swrl:argument1 rdf:resource="http://www.semanticweb.org/alencga1/ontologies/2023/2/PhenOWL/SO2"/>
                                    </rdf:Description>
                                </rdf:first>
                                <rdf:rest>
                                    <rdf:Description>
                                        <rdf:type rdf:resource="http://www.w3.org/2003/11/swrl#AtomList"/>
                                        <rdf:first>
                                            <rdf:Description>
                                                <rdf:type rdf:resource="http://www.w3.org/2003/11/swrl#ClassAtom"/>
                                                <swrl:classPredicate rdf:resource="http://www.w3.org/2006/time#ProperInterval"/>
                                                <swrl:argument1 rdf:resource="http://www.semanticweb.org/alencga1/ontologies/2023/2/PhenOWL/PI1"/>
                                            </rdf:Description>
                                        </rdf:first>
                                        <rdf:rest>
                                            <rdf:Description>
                                                <rdf:type rdf:resource="http://www.w3.org/2003/11/swrl#AtomList"/>
                                                <rdf:first>
                                                    <rdf:Description>
                                                        <rdf:type rdf:resource="http://www.w3.org/2003/11/swrl#ClassAtom"/>
                                                        <swrl:classPredicate rdf:resource="https://w3id.org/seas/System"/>
                                                        <swrl:argument1 rdf:resource="http://www.semanticweb.org/alencga1/ontologies/2023/2/PhenOWL/S1"/>
                                                    </rdf:Description>
                                                </rdf:first>
                                                <rdf:rest>
                                                    <rdf:Description>
                                                        <rdf:type rdf:resource="http://www.w3.org/2003/11/swrl#AtomList"/>
                                                        <rdf:first>
                                                            <rdf:Description>
                                                                <rdf:type rdf:resource="http://www.w3.org/2003/11/swrl#ClassAtom"/>
                                                                <swrl:classPredicate rdf:resource="http://www.w3.org/2006/time#ProperInterval"/>
                                                                <swrl:argument1 rdf:resource="http://www.semanticweb.org/alencga1/ontologies/2023/2/PhenOWL/PI2"/>
                                                            </rdf:Description>
                                                        </rdf:first>
                                                        <rdf:rest>
                                                            <rdf:Description>
                                                                <rdf:type rdf:resource="http://www.w3.org/2003/11/swrl#AtomList"/>
                                                                <rdf:first>
                                                                    <rdf:Description>
                                                                        <rdf:type rdf:resource="http://www.w3.org/2003/11/swrl#IndividualPropertyAtom"/>
                                                                        <swrl:propertyPredicate rdf:resource="http://www.opengis.net/ont/geosparql#rcc8ntpp"/>
                                                                        <swrl:argument1 rdf:resource="http://www.semanticweb.org/alencga1/ontologies/2023/2/PhenOWL/SO2"/>
                                                                        <swrl:argument2 rdf:resource="http://www.semanticweb.org/alencga1/ontologies/2023/2/PhenOWL/S1"/>
                                                                    </rdf:Description>
                                                                </rdf:first>
                                                                <rdf:rest>
                                                                    <rdf:Description>
                                                                        <rdf:type rdf:resource="http://www.w3.org/2003/11/swrl#AtomList"/>
                                                                        <rdf:first>
                                                                            <rdf:Description>
                                                                                <rdf:type rdf:resource="http://www.w3.org/2003/11/swrl#IndividualPropertyAtom"/>
                                                                                <swrl:propertyPredicate rdf:resource="https://w3id.org/def/propaphen#hasTimeInterval"/>
                                                                                <swrl:argument1 rdf:resource="http://www.semanticweb.org/alencga1/ontologies/2023/2/PhenOWL/O1"/>
                                                                                <swrl:argument2 rdf:resource="http://www.semanticweb.org/alencga1/ontologies/2023/2/PhenOWL/PI1"/>
                                                                            </rdf:Description>
                                                                        </rdf:first>
                                                                        <rdf:rest>
                                                                            <rdf:Description>
                                                                                <rdf:type rdf:resource="http://www.w3.org/2003/11/swrl#AtomList"/>
                                                                                <rdf:first>
                                                                                    <rdf:Description>
                                                                                        <rdf:type rdf:resource="http://www.w3.org/2003/11/swrl#IndividualPropertyAtom"/>
                                                                                        <swrl:propertyPredicate rdf:resource="https://w3id.org/def/propaphen#happensIn"/>
                                                                                        <swrl:argument1 rdf:resource="http://www.semanticweb.org/alencga1/ontologies/2023/2/PhenOWL/O1"/>
                                                                                        <swrl:argument2 rdf:resource="http://www.semanticweb.org/alencga1/ontologies/2023/2/PhenOWL/S1"/>
                                                                                    </rdf:Description>
                                                                                </rdf:first>
                                                                                <rdf:rest>
                                                                                    <rdf:Description>
                                                                                        <rdf:type rdf:resource="http://www.w3.org/2003/11/swrl#AtomList"/>
                                                                                        <rdf:first>
                                                                                            <rdf:Description>
                                                                                                <rdf:type rdf:resource="http://www.w3.org/2003/11/swrl#IndividualPropertyAtom"/>
                                                                                                <swrl:propertyPredicate rdf:resource="https://w3id.org/def/propaphen#spatialPresenceIn"/>
                                                                                                <swrl:argument1 rdf:resource="http://www.semanticweb.org/alencga1/ontologies/2023/2/PhenOWL/PR1"/>
                                                                                                <swrl:argument2 rdf:resource="http://www.semanticweb.org/alencga1/ontologies/2023/2/PhenOWL/SO2"/>
                                                                                            </rdf:Description>
                                                                                        </rdf:first>
                                                                                        <rdf:rest>
                                                                                            <rdf:Description>
                                                                                                <rdf:type rdf:resource="http://www.w3.org/2003/11/swrl#AtomList"/>
                                                                                                <rdf:first>
                                                                                                    <rdf:Description>
                                                                                                        <rdf:type rdf:resource="http://www.w3.org/2003/11/swrl#ClassAtom"/>
                                                                                                        <swrl:classPredicate rdf:resource="https://w3id.org/def/propaphen#Presence"/>
                                                                                                        <swrl:argument1 rdf:resource="http://www.semanticweb.org/alencga1/ontologies/2023/2/PhenOWL/PR1"/>
                                                                                                    </rdf:Description>
                                                                                                </rdf:first>
                                                                                                <rdf:rest>
                                                                                                    <rdf:Description>
                                                                                                        <rdf:type rdf:resource="http://www.w3.org/2003/11/swrl#AtomList"/>
                                                                                                        <rdf:first>
                                                                                                            <rdf:Description>
                                                                                                                <rdf:type rdf:resource="http://www.w3.org/2003/11/swrl#IndividualPropertyAtom"/>
                                                                                                                <swrl:propertyPredicate rdf:resource="https://w3id.org/def/propaphen#hasTimeInterval"/>
                                                                                                                <swrl:argument1 rdf:resource="http://www.semanticweb.org/alencga1/ontologies/2023/2/PhenOWL/PR1"/>
                                                                                                                <swrl:argument2 rdf:resource="http://www.semanticweb.org/alencga1/ontologies/2023/2/PhenOWL/PI2"/>
                                                                                                            </rdf:Description>
                                                                                                        </rdf:first>
                                                                                                        <rdf:rest rdf:resource="http://www.w3.org/1999/02/22-rdf-syntax-ns#nil"/>
                                                                                                    </rdf:Description>
                                                                                                </rdf:rest>
                                                                                            </rdf:Description>
                                                                                        </rdf:rest>
                                                                                    </rdf:Description>
                                                                                </rdf:rest>
                                                                            </rdf:Description>
                                                                        </rdf:rest>
                                                                    </rdf:Description>
                                                                </rdf:rest>
                                                            </rdf:Description>
                                                        </rdf:rest>
                                                    </rdf:Description>
                                                </rdf:rest>
                                            </rdf:Description>
                                        </rdf:rest>
                                    </rdf:Description>
                                </rdf:rest>
                            </rdf:Description>
                        </rdf:rest>
                    </rdf:Description>
                </rdf:rest>
            </rdf:Description>
        </swrl:body>
        <swrl:head>
            <rdf:Description>
                <rdf:type rdf:resource="http://www.w3.org/2003/11/swrl#AtomList"/>
                <rdf:first>
                    <rdf:Description>
                        <rdf:type rdf:resource="http://www.w3.org/2003/11/swrl#IndividualPropertyAtom"/>
                        <swrl:propertyPredicate rdf:resource="https://w3id.org/def/propaphen#observationalPresenceIn"/>
                        <swrl:argument1 rdf:resource="http://www.semanticweb.org/alencga1/ontologies/2023/2/PhenOWL/PR1"/>
                        <swrl:argument2 rdf:resource="http://www.semanticweb.org/alencga1/ontologies/2023/2/PhenOWL/O1"/>
                    </rdf:Description>
                </rdf:first>
                <rdf:rest rdf:resource="http://www.w3.org/1999/02/22-rdf-syntax-ns#nil"/>
            </rdf:Description>
        </swrl:head>
    </rdf:Description>
    <rdf:Description>
        <swrla:isRuleEnabled rdf:datatype="http://www.w3.org/2001/XMLSchema#boolean">true</swrla:isRuleEnabled>
        <rdfs:comment rdf:datatype="http://www.w3.org/2001/XMLSchema#string">Presence of group of Individuals in both node/system and observation (ntpp equals)</rdfs:comment>
        <rdfs:label rdf:datatype="http://www.w3.org/2001/XMLSchema#string">S4.2 - Pr in Obs (nttp equals)</rdfs:label>
        <rdf:type rdf:resource="http://www.w3.org/2003/11/swrl#Imp"/>
        <swrl:body>
            <rdf:Description>
                <rdf:type rdf:resource="http://www.w3.org/2003/11/swrl#AtomList"/>
                <rdf:first>
                    <rdf:Description>
                        <rdf:type rdf:resource="http://www.w3.org/2003/11/swrl#IndividualPropertyAtom"/>
                        <swrl:propertyPredicate rdf:resource="http://www.w3.org/2006/time#intervalEquals"/>
                        <swrl:argument1 rdf:resource="http://www.semanticweb.org/alencga1/ontologies/2023/2/PhenOWL/PI1"/>
                        <swrl:argument2 rdf:resource="http://www.semanticweb.org/alencga1/ontologies/2023/2/PhenOWL/PI2"/>
                    </rdf:Description>
                </rdf:first>
                <rdf:rest>
                    <rdf:Description>
                        <rdf:type rdf:resource="http://www.w3.org/2003/11/swrl#AtomList"/>
                        <rdf:first>
                            <rdf:Description>
                                <rdf:type rdf:resource="http://www.w3.org/2003/11/swrl#ClassAtom"/>
                                <swrl:classPredicate rdf:resource="https://w3id.org/def/propaphen#Observation"/>
                                <swrl:argument1 rdf:resource="http://www.semanticweb.org/alencga1/ontologies/2023/2/PhenOWL/O1"/>
                            </rdf:Description>
                        </rdf:first>
                        <rdf:rest>
                            <rdf:Description>
                                <rdf:type rdf:resource="http://www.w3.org/2003/11/swrl#AtomList"/>
                                <rdf:first>
                                    <rdf:Description>
                                        <rdf:type rdf:resource="http://www.w3.org/2003/11/swrl#ClassAtom"/>
                                        <swrl:classPredicate rdf:resource="http://www.opengis.net/ont/geosparql#SpatialObject"/>
                                        <swrl:argument1 rdf:resource="http://www.semanticweb.org/alencga1/ontologies/2023/2/PhenOWL/SO2"/>
                                    </rdf:Description>
                                </rdf:first>
                                <rdf:rest>
                                    <rdf:Description>
                                        <rdf:type rdf:resource="http://www.w3.org/2003/11/swrl#AtomList"/>
                                        <rdf:first>
                                            <rdf:Description>
                                                <rdf:type rdf:resource="http://www.w3.org/2003/11/swrl#ClassAtom"/>
                                                <swrl:classPredicate rdf:resource="http://www.w3.org/2006/time#ProperInterval"/>
                                                <swrl:argument1 rdf:resource="http://www.semanticweb.org/alencga1/ontologies/2023/2/PhenOWL/PI1"/>
                                            </rdf:Description>
                                        </rdf:first>
                                        <rdf:rest>
                                            <rdf:Description>
                                                <rdf:type rdf:resource="http://www.w3.org/2003/11/swrl#AtomList"/>
                                                <rdf:first>
                                                    <rdf:Description>
                                                        <rdf:type rdf:resource="http://www.w3.org/2003/11/swrl#ClassAtom"/>
                                                        <swrl:classPredicate rdf:resource="https://w3id.org/seas/System"/>
                                                        <swrl:argument1 rdf:resource="http://www.semanticweb.org/alencga1/ontologies/2023/2/PhenOWL/S1"/>
                                                    </rdf:Description>
                                                </rdf:first>
                                                <rdf:rest>
                                                    <rdf:Description>
                                                        <rdf:type rdf:resource="http://www.w3.org/2003/11/swrl#AtomList"/>
                                                        <rdf:first>
                                                            <rdf:Description>
                                                                <rdf:type rdf:resource="http://www.w3.org/2003/11/swrl#ClassAtom"/>
                                                                <swrl:classPredicate rdf:resource="http://www.w3.org/2006/time#ProperInterval"/>
                                                                <swrl:argument1 rdf:resource="http://www.semanticweb.org/alencga1/ontologies/2023/2/PhenOWL/PI2"/>
                                                            </rdf:Description>
                                                        </rdf:first>
                                                        <rdf:rest>
                                                            <rdf:Description>
                                                                <rdf:type rdf:resource="http://www.w3.org/2003/11/swrl#AtomList"/>
                                                                <rdf:first>
                                                                    <rdf:Description>
                                                                        <rdf:type rdf:resource="http://www.w3.org/2003/11/swrl#IndividualPropertyAtom"/>
                                                                        <swrl:propertyPredicate rdf:resource="http://www.opengis.net/ont/geosparql#rcc8ntpp"/>
                                                                        <swrl:argument1 rdf:resource="http://www.semanticweb.org/alencga1/ontologies/2023/2/PhenOWL/SO2"/>
                                                                        <swrl:argument2 rdf:resource="http://www.semanticweb.org/alencga1/ontologies/2023/2/PhenOWL/S1"/>
                                                                    </rdf:Description>
                                                                </rdf:first>
                                                                <rdf:rest>
                                                                    <rdf:Description>
                                                                        <rdf:type rdf:resource="http://www.w3.org/2003/11/swrl#AtomList"/>
                                                                        <rdf:first>
                                                                            <rdf:Description>
                                                                                <rdf:type rdf:resource="http://www.w3.org/2003/11/swrl#IndividualPropertyAtom"/>
                                                                                <swrl:propertyPredicate rdf:resource="https://w3id.org/def/propaphen#hasTimeInterval"/>
                                                                                <swrl:argument1 rdf:resource="http://www.semanticweb.org/alencga1/ontologies/2023/2/PhenOWL/O1"/>
                                                                                <swrl:argument2 rdf:resource="http://www.semanticweb.org/alencga1/ontologies/2023/2/PhenOWL/PI1"/>
                                                                            </rdf:Description>
                                                                        </rdf:first>
                                                                        <rdf:rest>
                                                                            <rdf:Description>
                                                                                <rdf:type rdf:resource="http://www.w3.org/2003/11/swrl#AtomList"/>
                                                                                <rdf:first>
                                                                                    <rdf:Description>
                                                                                        <rdf:type rdf:resource="http://www.w3.org/2003/11/swrl#IndividualPropertyAtom"/>
                                                                                        <swrl:propertyPredicate rdf:resource="https://w3id.org/def/propaphen#happensIn"/>
                                                                                        <swrl:argument1 rdf:resource="http://www.semanticweb.org/alencga1/ontologies/2023/2/PhenOWL/O1"/>
                                                                                        <swrl:argument2 rdf:resource="http://www.semanticweb.org/alencga1/ontologies/2023/2/PhenOWL/S1"/>
                                                                                    </rdf:Description>
                                                                                </rdf:first>
                                                                                <rdf:rest>
                                                                                    <rdf:Description>
                                                                                        <rdf:type rdf:resource="http://www.w3.org/2003/11/swrl#AtomList"/>
                                                                                        <rdf:first>
                                                                                            <rdf:Description>
                                                                                                <rdf:type rdf:resource="http://www.w3.org/2003/11/swrl#IndividualPropertyAtom"/>
                                                                                                <swrl:propertyPredicate rdf:resource="https://w3id.org/def/propaphen#spatialPresenceIn"/>
                                                                                                <swrl:argument1 rdf:resource="http://www.semanticweb.org/alencga1/ontologies/2023/2/PhenOWL/PR1"/>
                                                                                                <swrl:argument2 rdf:resource="http://www.semanticweb.org/alencga1/ontologies/2023/2/PhenOWL/SO2"/>
                                                                                            </rdf:Description>
                                                                                        </rdf:first>
                                                                                        <rdf:rest>
                                                                                            <rdf:Description>
                                                                                                <rdf:type rdf:resource="http://www.w3.org/2003/11/swrl#AtomList"/>
                                                                                                <rdf:first>
                                                                                                    <rdf:Description>
                                                                                                        <rdf:type rdf:resource="http://www.w3.org/2003/11/swrl#ClassAtom"/>
                                                                                                        <swrl:classPredicate rdf:resource="https://w3id.org/def/propaphen#Presence"/>
                                                                                                        <swrl:argument1 rdf:resource="http://www.semanticweb.org/alencga1/ontologies/2023/2/PhenOWL/PR1"/>
                                                                                                    </rdf:Description>
                                                                                                </rdf:first>
                                                                                                <rdf:rest>
                                                                                                    <rdf:Description>
                                                                                                        <rdf:type rdf:resource="http://www.w3.org/2003/11/swrl#AtomList"/>
                                                                                                        <rdf:first>
                                                                                                            <rdf:Description>
                                                                                                                <rdf:type rdf:resource="http://www.w3.org/2003/11/swrl#IndividualPropertyAtom"/>
                                                                                                                <swrl:propertyPredicate rdf:resource="https://w3id.org/def/propaphen#hasTimeInterval"/>
                                                                                                                <swrl:argument1 rdf:resource="http://www.semanticweb.org/alencga1/ontologies/2023/2/PhenOWL/PR1"/>
                                                                                                                <swrl:argument2 rdf:resource="http://www.semanticweb.org/alencga1/ontologies/2023/2/PhenOWL/PI2"/>
                                                                                                            </rdf:Description>
                                                                                                        </rdf:first>
                                                                                                        <rdf:rest rdf:resource="http://www.w3.org/1999/02/22-rdf-syntax-ns#nil"/>
                                                                                                    </rdf:Description>
                                                                                                </rdf:rest>
                                                                                            </rdf:Description>
                                                                                        </rdf:rest>
                                                                                    </rdf:Description>
                                                                                </rdf:rest>
                                                                            </rdf:Description>
                                                                        </rdf:rest>
                                                                    </rdf:Description>
                                                                </rdf:rest>
                                                            </rdf:Description>
                                                        </rdf:rest>
                                                    </rdf:Description>
                                                </rdf:rest>
                                            </rdf:Description>
                                        </rdf:rest>
                                    </rdf:Description>
                                </rdf:rest>
                            </rdf:Description>
                        </rdf:rest>
                    </rdf:Description>
                </rdf:rest>
            </rdf:Description>
        </swrl:body>
        <swrl:head>
            <rdf:Description>
                <rdf:type rdf:resource="http://www.w3.org/2003/11/swrl#AtomList"/>
                <rdf:first>
                    <rdf:Description>
                        <rdf:type rdf:resource="http://www.w3.org/2003/11/swrl#IndividualPropertyAtom"/>
                        <swrl:propertyPredicate rdf:resource="https://w3id.org/def/propaphen#observationalPresenceIn"/>
                        <swrl:argument1 rdf:resource="http://www.semanticweb.org/alencga1/ontologies/2023/2/PhenOWL/PR1"/>
                        <swrl:argument2 rdf:resource="http://www.semanticweb.org/alencga1/ontologies/2023/2/PhenOWL/O1"/>
                    </rdf:Description>
                </rdf:first>
                <rdf:rest rdf:resource="http://www.w3.org/1999/02/22-rdf-syntax-ns#nil"/>
            </rdf:Description>
        </swrl:head>
    </rdf:Description>
    <rdf:Description>
        <swrla:isRuleEnabled rdf:datatype="http://www.w3.org/2001/XMLSchema#boolean">true</swrla:isRuleEnabled>
        <rdfs:comment rdf:datatype="http://www.w3.org/2001/XMLSchema#string">Presence of group of Individuals in both node/system and observation (tpp contains)</rdfs:comment>
        <rdfs:label rdf:datatype="http://www.w3.org/2001/XMLSchema#string">S4.4 - Pr in Obs (ttp contains)</rdfs:label>
        <rdf:type rdf:resource="http://www.w3.org/2003/11/swrl#Imp"/>
        <swrl:body>
            <rdf:Description>
                <rdf:type rdf:resource="http://www.w3.org/2003/11/swrl#AtomList"/>
                <rdf:first>
                    <rdf:Description>
                        <rdf:type rdf:resource="http://www.w3.org/2003/11/swrl#IndividualPropertyAtom"/>
                        <swrl:propertyPredicate rdf:resource="http://www.w3.org/2006/time#intervalContains"/>
                        <swrl:argument1 rdf:resource="http://www.semanticweb.org/alencga1/ontologies/2023/2/PhenOWL/PI1"/>
                        <swrl:argument2 rdf:resource="http://www.semanticweb.org/alencga1/ontologies/2023/2/PhenOWL/PI2"/>
                    </rdf:Description>
                </rdf:first>
                <rdf:rest>
                    <rdf:Description>
                        <rdf:type rdf:resource="http://www.w3.org/2003/11/swrl#AtomList"/>
                        <rdf:first>
                            <rdf:Description>
                                <rdf:type rdf:resource="http://www.w3.org/2003/11/swrl#IndividualPropertyAtom"/>
                                <swrl:propertyPredicate rdf:resource="http://www.opengis.net/ont/geosparql#rcc8tpp"/>
                                <swrl:argument1 rdf:resource="http://www.semanticweb.org/alencga1/ontologies/2023/2/PhenOWL/SO2"/>
                                <swrl:argument2 rdf:resource="http://www.semanticweb.org/alencga1/ontologies/2023/2/PhenOWL/S1"/>
                            </rdf:Description>
                        </rdf:first>
                        <rdf:rest>
                            <rdf:Description>
                                <rdf:type rdf:resource="http://www.w3.org/2003/11/swrl#AtomList"/>
                                <rdf:first>
                                    <rdf:Description>
                                        <rdf:type rdf:resource="http://www.w3.org/2003/11/swrl#ClassAtom"/>
                                        <swrl:classPredicate rdf:resource="https://w3id.org/def/propaphen#Observation"/>
                                        <swrl:argument1 rdf:resource="http://www.semanticweb.org/alencga1/ontologies/2023/2/PhenOWL/O1"/>
                                    </rdf:Description>
                                </rdf:first>
                                <rdf:rest>
                                    <rdf:Description>
                                        <rdf:type rdf:resource="http://www.w3.org/2003/11/swrl#AtomList"/>
                                        <rdf:first>
                                            <rdf:Description>
                                                <rdf:type rdf:resource="http://www.w3.org/2003/11/swrl#ClassAtom"/>
                                                <swrl:classPredicate rdf:resource="http://www.opengis.net/ont/geosparql#SpatialObject"/>
                                                <swrl:argument1 rdf:resource="http://www.semanticweb.org/alencga1/ontologies/2023/2/PhenOWL/SO2"/>
                                            </rdf:Description>
                                        </rdf:first>
                                        <rdf:rest>
                                            <rdf:Description>
                                                <rdf:type rdf:resource="http://www.w3.org/2003/11/swrl#AtomList"/>
                                                <rdf:first>
                                                    <rdf:Description>
                                                        <rdf:type rdf:resource="http://www.w3.org/2003/11/swrl#ClassAtom"/>
                                                        <swrl:classPredicate rdf:resource="http://www.w3.org/2006/time#ProperInterval"/>
                                                        <swrl:argument1 rdf:resource="http://www.semanticweb.org/alencga1/ontologies/2023/2/PhenOWL/PI1"/>
                                                    </rdf:Description>
                                                </rdf:first>
                                                <rdf:rest>
                                                    <rdf:Description>
                                                        <rdf:type rdf:resource="http://www.w3.org/2003/11/swrl#AtomList"/>
                                                        <rdf:first>
                                                            <rdf:Description>
                                                                <rdf:type rdf:resource="http://www.w3.org/2003/11/swrl#ClassAtom"/>
                                                                <swrl:classPredicate rdf:resource="https://w3id.org/seas/System"/>
                                                                <swrl:argument1 rdf:resource="http://www.semanticweb.org/alencga1/ontologies/2023/2/PhenOWL/S1"/>
                                                            </rdf:Description>
                                                        </rdf:first>
                                                        <rdf:rest>
                                                            <rdf:Description>
                                                                <rdf:type rdf:resource="http://www.w3.org/2003/11/swrl#AtomList"/>
                                                                <rdf:first>
                                                                    <rdf:Description>
                                                                        <rdf:type rdf:resource="http://www.w3.org/2003/11/swrl#ClassAtom"/>
                                                                        <swrl:classPredicate rdf:resource="http://www.w3.org/2006/time#ProperInterval"/>
                                                                        <swrl:argument1 rdf:resource="http://www.semanticweb.org/alencga1/ontologies/2023/2/PhenOWL/PI2"/>
                                                                    </rdf:Description>
                                                                </rdf:first>
                                                                <rdf:rest>
                                                                    <rdf:Description>
                                                                        <rdf:type rdf:resource="http://www.w3.org/2003/11/swrl#AtomList"/>
                                                                        <rdf:first>
                                                                            <rdf:Description>
                                                                                <rdf:type rdf:resource="http://www.w3.org/2003/11/swrl#IndividualPropertyAtom"/>
                                                                                <swrl:propertyPredicate rdf:resource="https://w3id.org/def/propaphen#hasTimeInterval"/>
                                                                                <swrl:argument1 rdf:resource="http://www.semanticweb.org/alencga1/ontologies/2023/2/PhenOWL/O1"/>
                                                                                <swrl:argument2 rdf:resource="http://www.semanticweb.org/alencga1/ontologies/2023/2/PhenOWL/PI1"/>
                                                                            </rdf:Description>
                                                                        </rdf:first>
                                                                        <rdf:rest>
                                                                            <rdf:Description>
                                                                                <rdf:type rdf:resource="http://www.w3.org/2003/11/swrl#AtomList"/>
                                                                                <rdf:first>
                                                                                    <rdf:Description>
                                                                                        <rdf:type rdf:resource="http://www.w3.org/2003/11/swrl#IndividualPropertyAtom"/>
                                                                                        <swrl:propertyPredicate rdf:resource="https://w3id.org/def/propaphen#happensIn"/>
                                                                                        <swrl:argument1 rdf:resource="http://www.semanticweb.org/alencga1/ontologies/2023/2/PhenOWL/O1"/>
                                                                                        <swrl:argument2 rdf:resource="http://www.semanticweb.org/alencga1/ontologies/2023/2/PhenOWL/S1"/>
                                                                                    </rdf:Description>
                                                                                </rdf:first>
                                                                                <rdf:rest>
                                                                                    <rdf:Description>
                                                                                        <rdf:type rdf:resource="http://www.w3.org/2003/11/swrl#AtomList"/>
                                                                                        <rdf:first>
                                                                                            <rdf:Description>
                                                                                                <rdf:type rdf:resource="http://www.w3.org/2003/11/swrl#IndividualPropertyAtom"/>
                                                                                                <swrl:propertyPredicate rdf:resource="https://w3id.org/def/propaphen#spatialPresenceIn"/>
                                                                                                <swrl:argument1 rdf:resource="http://www.semanticweb.org/alencga1/ontologies/2023/2/PhenOWL/PR1"/>
                                                                                                <swrl:argument2 rdf:resource="http://www.semanticweb.org/alencga1/ontologies/2023/2/PhenOWL/SO2"/>
                                                                                            </rdf:Description>
                                                                                        </rdf:first>
                                                                                        <rdf:rest>
                                                                                            <rdf:Description>
                                                                                                <rdf:type rdf:resource="http://www.w3.org/2003/11/swrl#AtomList"/>
                                                                                                <rdf:first>
                                                                                                    <rdf:Description>
                                                                                                        <rdf:type rdf:resource="http://www.w3.org/2003/11/swrl#ClassAtom"/>
                                                                                                        <swrl:classPredicate rdf:resource="https://w3id.org/def/propaphen#Presence"/>
                                                                                                        <swrl:argument1 rdf:resource="http://www.semanticweb.org/alencga1/ontologies/2023/2/PhenOWL/PR1"/>
                                                                                                    </rdf:Description>
                                                                                                </rdf:first>
                                                                                                <rdf:rest>
                                                                                                    <rdf:Description>
                                                                                                        <rdf:type rdf:resource="http://www.w3.org/2003/11/swrl#AtomList"/>
                                                                                                        <rdf:first>
                                                                                                            <rdf:Description>
                                                                                                                <rdf:type rdf:resource="http://www.w3.org/2003/11/swrl#IndividualPropertyAtom"/>
                                                                                                                <swrl:propertyPredicate rdf:resource="https://w3id.org/def/propaphen#hasTimeInterval"/>
                                                                                                                <swrl:argument1 rdf:resource="http://www.semanticweb.org/alencga1/ontologies/2023/2/PhenOWL/PR1"/>
                                                                                                                <swrl:argument2 rdf:resource="http://www.semanticweb.org/alencga1/ontologies/2023/2/PhenOWL/PI2"/>
                                                                                                            </rdf:Description>
                                                                                                        </rdf:first>
                                                                                                        <rdf:rest rdf:resource="http://www.w3.org/1999/02/22-rdf-syntax-ns#nil"/>
                                                                                                    </rdf:Description>
                                                                                                </rdf:rest>
                                                                                            </rdf:Description>
                                                                                        </rdf:rest>
                                                                                    </rdf:Description>
                                                                                </rdf:rest>
                                                                            </rdf:Description>
                                                                        </rdf:rest>
                                                                    </rdf:Description>
                                                                </rdf:rest>
                                                            </rdf:Description>
                                                        </rdf:rest>
                                                    </rdf:Description>
                                                </rdf:rest>
                                            </rdf:Description>
                                        </rdf:rest>
                                    </rdf:Description>
                                </rdf:rest>
                            </rdf:Description>
                        </rdf:rest>
                    </rdf:Description>
                </rdf:rest>
            </rdf:Description>
        </swrl:body>
        <swrl:head>
            <rdf:Description>
                <rdf:type rdf:resource="http://www.w3.org/2003/11/swrl#AtomList"/>
                <rdf:first>
                    <rdf:Description>
                        <rdf:type rdf:resource="http://www.w3.org/2003/11/swrl#IndividualPropertyAtom"/>
                        <swrl:propertyPredicate rdf:resource="https://w3id.org/def/propaphen#observationalPresenceIn"/>
                        <swrl:argument1 rdf:resource="http://www.semanticweb.org/alencga1/ontologies/2023/2/PhenOWL/PR1"/>
                        <swrl:argument2 rdf:resource="http://www.semanticweb.org/alencga1/ontologies/2023/2/PhenOWL/O1"/>
                    </rdf:Description>
                </rdf:first>
                <rdf:rest rdf:resource="http://www.w3.org/1999/02/22-rdf-syntax-ns#nil"/>
            </rdf:Description>
        </swrl:head>
    </rdf:Description>
    <rdf:Description>
        <swrla:isRuleEnabled rdf:datatype="http://www.w3.org/2001/XMLSchema#boolean">true</swrla:isRuleEnabled>
        <rdfs:comment rdf:datatype="http://www.w3.org/2001/XMLSchema#string">Presence of group of Individuals in both node/system and observation (tpp equals)</rdfs:comment>
        <rdfs:label rdf:datatype="http://www.w3.org/2001/XMLSchema#string">S4.1 - Pr in Obs (ttp equals)</rdfs:label>
        <rdf:type rdf:resource="http://www.w3.org/2003/11/swrl#Imp"/>
        <swrl:body>
            <rdf:Description>
                <rdf:type rdf:resource="http://www.w3.org/2003/11/swrl#AtomList"/>
                <rdf:first>
                    <rdf:Description>
                        <rdf:type rdf:resource="http://www.w3.org/2003/11/swrl#IndividualPropertyAtom"/>
                        <swrl:propertyPredicate rdf:resource="http://www.w3.org/2006/time#intervalEquals"/>
                        <swrl:argument1 rdf:resource="http://www.semanticweb.org/alencga1/ontologies/2023/2/PhenOWL/PI1"/>
                        <swrl:argument2 rdf:resource="http://www.semanticweb.org/alencga1/ontologies/2023/2/PhenOWL/PI2"/>
                    </rdf:Description>
                </rdf:first>
                <rdf:rest>
                    <rdf:Description>
                        <rdf:type rdf:resource="http://www.w3.org/2003/11/swrl#AtomList"/>
                        <rdf:first>
                            <rdf:Description>
                                <rdf:type rdf:resource="http://www.w3.org/2003/11/swrl#IndividualPropertyAtom"/>
                                <swrl:propertyPredicate rdf:resource="http://www.opengis.net/ont/geosparql#rcc8tpp"/>
                                <swrl:argument1 rdf:resource="http://www.semanticweb.org/alencga1/ontologies/2023/2/PhenOWL/SO2"/>
                                <swrl:argument2 rdf:resource="http://www.semanticweb.org/alencga1/ontologies/2023/2/PhenOWL/S1"/>
                            </rdf:Description>
                        </rdf:first>
                        <rdf:rest>
                            <rdf:Description>
                                <rdf:type rdf:resource="http://www.w3.org/2003/11/swrl#AtomList"/>
                                <rdf:first>
                                    <rdf:Description>
                                        <rdf:type rdf:resource="http://www.w3.org/2003/11/swrl#ClassAtom"/>
                                        <swrl:classPredicate rdf:resource="https://w3id.org/def/propaphen#Observation"/>
                                        <swrl:argument1 rdf:resource="http://www.semanticweb.org/alencga1/ontologies/2023/2/PhenOWL/O1"/>
                                    </rdf:Description>
                                </rdf:first>
                                <rdf:rest>
                                    <rdf:Description>
                                        <rdf:type rdf:resource="http://www.w3.org/2003/11/swrl#AtomList"/>
                                        <rdf:first>
                                            <rdf:Description>
                                                <rdf:type rdf:resource="http://www.w3.org/2003/11/swrl#ClassAtom"/>
                                                <swrl:classPredicate rdf:resource="http://www.opengis.net/ont/geosparql#SpatialObject"/>
                                                <swrl:argument1 rdf:resource="http://www.semanticweb.org/alencga1/ontologies/2023/2/PhenOWL/SO2"/>
                                            </rdf:Description>
                                        </rdf:first>
                                        <rdf:rest>
                                            <rdf:Description>
                                                <rdf:type rdf:resource="http://www.w3.org/2003/11/swrl#AtomList"/>
                                                <rdf:first>
                                                    <rdf:Description>
                                                        <rdf:type rdf:resource="http://www.w3.org/2003/11/swrl#ClassAtom"/>
                                                        <swrl:classPredicate rdf:resource="http://www.w3.org/2006/time#ProperInterval"/>
                                                        <swrl:argument1 rdf:resource="http://www.semanticweb.org/alencga1/ontologies/2023/2/PhenOWL/PI1"/>
                                                    </rdf:Description>
                                                </rdf:first>
                                                <rdf:rest>
                                                    <rdf:Description>
                                                        <rdf:type rdf:resource="http://www.w3.org/2003/11/swrl#AtomList"/>
                                                        <rdf:first>
                                                            <rdf:Description>
                                                                <rdf:type rdf:resource="http://www.w3.org/2003/11/swrl#ClassAtom"/>
                                                                <swrl:classPredicate rdf:resource="https://w3id.org/seas/System"/>
                                                                <swrl:argument1 rdf:resource="http://www.semanticweb.org/alencga1/ontologies/2023/2/PhenOWL/S1"/>
                                                            </rdf:Description>
                                                        </rdf:first>
                                                        <rdf:rest>
                                                            <rdf:Description>
                                                                <rdf:type rdf:resource="http://www.w3.org/2003/11/swrl#AtomList"/>
                                                                <rdf:first>
                                                                    <rdf:Description>
                                                                        <rdf:type rdf:resource="http://www.w3.org/2003/11/swrl#ClassAtom"/>
                                                                        <swrl:classPredicate rdf:resource="http://www.w3.org/2006/time#ProperInterval"/>
                                                                        <swrl:argument1 rdf:resource="http://www.semanticweb.org/alencga1/ontologies/2023/2/PhenOWL/PI2"/>
                                                                    </rdf:Description>
                                                                </rdf:first>
                                                                <rdf:rest>
                                                                    <rdf:Description>
                                                                        <rdf:type rdf:resource="http://www.w3.org/2003/11/swrl#AtomList"/>
                                                                        <rdf:first>
                                                                            <rdf:Description>
                                                                                <rdf:type rdf:resource="http://www.w3.org/2003/11/swrl#IndividualPropertyAtom"/>
                                                                                <swrl:propertyPredicate rdf:resource="https://w3id.org/def/propaphen#hasTimeInterval"/>
                                                                                <swrl:argument1 rdf:resource="http://www.semanticweb.org/alencga1/ontologies/2023/2/PhenOWL/O1"/>
                                                                                <swrl:argument2 rdf:resource="http://www.semanticweb.org/alencga1/ontologies/2023/2/PhenOWL/PI1"/>
                                                                            </rdf:Description>
                                                                        </rdf:first>
                                                                        <rdf:rest>
                                                                            <rdf:Description>
                                                                                <rdf:type rdf:resource="http://www.w3.org/2003/11/swrl#AtomList"/>
                                                                                <rdf:first>
                                                                                    <rdf:Description>
                                                                                        <rdf:type rdf:resource="http://www.w3.org/2003/11/swrl#IndividualPropertyAtom"/>
                                                                                        <swrl:propertyPredicate rdf:resource="https://w3id.org/def/propaphen#happensIn"/>
                                                                                        <swrl:argument1 rdf:resource="http://www.semanticweb.org/alencga1/ontologies/2023/2/PhenOWL/O1"/>
                                                                                        <swrl:argument2 rdf:resource="http://www.semanticweb.org/alencga1/ontologies/2023/2/PhenOWL/S1"/>
                                                                                    </rdf:Description>
                                                                                </rdf:first>
                                                                                <rdf:rest>
                                                                                    <rdf:Description>
                                                                                        <rdf:type rdf:resource="http://www.w3.org/2003/11/swrl#AtomList"/>
                                                                                        <rdf:first>
                                                                                            <rdf:Description>
                                                                                                <rdf:type rdf:resource="http://www.w3.org/2003/11/swrl#IndividualPropertyAtom"/>
                                                                                                <swrl:propertyPredicate rdf:resource="https://w3id.org/def/propaphen#spatialPresenceIn"/>
                                                                                                <swrl:argument1 rdf:resource="http://www.semanticweb.org/alencga1/ontologies/2023/2/PhenOWL/PR1"/>
                                                                                                <swrl:argument2 rdf:resource="http://www.semanticweb.org/alencga1/ontologies/2023/2/PhenOWL/SO2"/>
                                                                                            </rdf:Description>
                                                                                        </rdf:first>
                                                                                        <rdf:rest>
                                                                                            <rdf:Description>
                                                                                                <rdf:type rdf:resource="http://www.w3.org/2003/11/swrl#AtomList"/>
                                                                                                <rdf:first>
                                                                                                    <rdf:Description>
                                                                                                        <rdf:type rdf:resource="http://www.w3.org/2003/11/swrl#ClassAtom"/>
                                                                                                        <swrl:classPredicate rdf:resource="https://w3id.org/def/propaphen#Presence"/>
                                                                                                        <swrl:argument1 rdf:resource="http://www.semanticweb.org/alencga1/ontologies/2023/2/PhenOWL/PR1"/>
                                                                                                    </rdf:Description>
                                                                                                </rdf:first>
                                                                                                <rdf:rest>
                                                                                                    <rdf:Description>
                                                                                                        <rdf:type rdf:resource="http://www.w3.org/2003/11/swrl#AtomList"/>
                                                                                                        <rdf:first>
                                                                                                            <rdf:Description>
                                                                                                                <rdf:type rdf:resource="http://www.w3.org/2003/11/swrl#IndividualPropertyAtom"/>
                                                                                                                <swrl:propertyPredicate rdf:resource="https://w3id.org/def/propaphen#hasTimeInterval"/>
                                                                                                                <swrl:argument1 rdf:resource="http://www.semanticweb.org/alencga1/ontologies/2023/2/PhenOWL/PR1"/>
                                                                                                                <swrl:argument2 rdf:resource="http://www.semanticweb.org/alencga1/ontologies/2023/2/PhenOWL/PI2"/>
                                                                                                            </rdf:Description>
                                                                                                        </rdf:first>
                                                                                                        <rdf:rest rdf:resource="http://www.w3.org/1999/02/22-rdf-syntax-ns#nil"/>
                                                                                                    </rdf:Description>
                                                                                                </rdf:rest>
                                                                                            </rdf:Description>
                                                                                        </rdf:rest>
                                                                                    </rdf:Description>
                                                                                </rdf:rest>
                                                                            </rdf:Description>
                                                                        </rdf:rest>
                                                                    </rdf:Description>
                                                                </rdf:rest>
                                                            </rdf:Description>
                                                        </rdf:rest>
                                                    </rdf:Description>
                                                </rdf:rest>
                                            </rdf:Description>
                                        </rdf:rest>
                                    </rdf:Description>
                                </rdf:rest>
                            </rdf:Description>
                        </rdf:rest>
                    </rdf:Description>
                </rdf:rest>
            </rdf:Description>
        </swrl:body>
        <swrl:head>
            <rdf:Description>
                <rdf:type rdf:resource="http://www.w3.org/2003/11/swrl#AtomList"/>
                <rdf:first>
                    <rdf:Description>
                        <rdf:type rdf:resource="http://www.w3.org/2003/11/swrl#IndividualPropertyAtom"/>
                        <swrl:propertyPredicate rdf:resource="https://w3id.org/def/propaphen#observationalPresenceIn"/>
                        <swrl:argument1 rdf:resource="http://www.semanticweb.org/alencga1/ontologies/2023/2/PhenOWL/PR1"/>
                        <swrl:argument2 rdf:resource="http://www.semanticweb.org/alencga1/ontologies/2023/2/PhenOWL/O1"/>
                    </rdf:Description>
                </rdf:first>
                <rdf:rest rdf:resource="http://www.w3.org/1999/02/22-rdf-syntax-ns#nil"/>
            </rdf:Description>
        </swrl:head>
    </rdf:Description>
    <rdf:Description>
        <swrla:isRuleEnabled rdf:datatype="http://www.w3.org/2001/XMLSchema#boolean">true</swrla:isRuleEnabled>
        <rdfs:comment rdf:datatype="http://www.w3.org/2001/XMLSchema#string">Valid ST Path from gufo begin point</rdfs:comment>
        <rdfs:label rdf:datatype="http://www.w3.org/2001/XMLSchema#string">S5.1 - Valid ST Path from gufo</rdfs:label>
        <rdf:type rdf:resource="http://www.w3.org/2003/11/swrl#Imp"/>
        <swrl:body>
            <rdf:Description>
                <rdf:type rdf:resource="http://www.w3.org/2003/11/swrl#AtomList"/>
                <rdf:first>
                    <rdf:Description>
                        <rdf:type rdf:resource="http://www.w3.org/2003/11/swrl#ClassAtom"/>
                        <swrl:classPredicate rdf:resource="https://w3id.org/seas/System"/>
                        <swrl:argument1 rdf:resource="http://www.semanticweb.org/alencga1/ontologies/2023/2/PhenOWL/S2"/>
                    </rdf:Description>
                </rdf:first>
                <rdf:rest>
                    <rdf:Description>
                        <rdf:type rdf:resource="http://www.w3.org/2003/11/swrl#AtomList"/>
                        <rdf:first>
                            <rdf:Description>
                                <rdf:type rdf:resource="http://www.w3.org/2003/11/swrl#IndividualPropertyAtom"/>
                                <swrl:propertyPredicate rdf:resource="https://w3id.org/def/propaphen#fromPhenomenon"/>
                                <swrl:argument1 rdf:resource="http://www.semanticweb.org/alencga1/ontologies/2023/2/PhenOWL/OP1"/>
                                <swrl:argument2 rdf:resource="http://www.semanticweb.org/alencga1/ontologies/2023/2/PhenOWL/P1"/>
                            </rdf:Description>
                        </rdf:first>
                        <rdf:rest>
                            <rdf:Description>
                                <rdf:type rdf:resource="http://www.w3.org/2003/11/swrl#AtomList"/>
                                <rdf:first>
                                    <rdf:Description>
                                        <rdf:type rdf:resource="http://www.w3.org/2003/11/swrl#ClassAtom"/>
                                        <swrl:classPredicate rdf:resource="http://www.w3.org/2006/time#Instant"/>
                                        <swrl:argument1 rdf:resource="http://www.semanticweb.org/alencga1/ontologies/2023/2/PhenOWL/t1"/>
                                    </rdf:Description>
                                </rdf:first>
                                <rdf:rest>
                                    <rdf:Description>
                                        <rdf:type rdf:resource="http://www.w3.org/2003/11/swrl#AtomList"/>
                                        <rdf:first>
                                            <rdf:Description>
                                                <rdf:type rdf:resource="http://www.w3.org/2003/11/swrl#IndividualPropertyAtom"/>
                                                <swrl:propertyPredicate rdf:resource="http://www.w3.org/2006/time#after"/>
                                                <swrl:argument1 rdf:resource="http://www.semanticweb.org/alencga1/ontologies/2023/2/PhenOWL/t2"/>
                                                <swrl:argument2 rdf:resource="http://www.semanticweb.org/alencga1/ontologies/2023/2/PhenOWL/t1"/>
                                            </rdf:Description>
                                        </rdf:first>
                                        <rdf:rest>
                                            <rdf:Description>
                                                <rdf:type rdf:resource="http://www.w3.org/2003/11/swrl#AtomList"/>
                                                <rdf:first>
                                                    <rdf:Description>
                                                        <rdf:type rdf:resource="http://www.w3.org/2003/11/swrl#IndividualPropertyAtom"/>
                                                        <swrl:propertyPredicate rdf:resource="https://w3id.org/def/propaphen#fromPhenomenon"/>
                                                        <swrl:argument1 rdf:resource="http://www.semanticweb.org/alencga1/ontologies/2023/2/PhenOWL/OP2"/>
                                                        <swrl:argument2 rdf:resource="http://www.semanticweb.org/alencga1/ontologies/2023/2/PhenOWL/P1"/>
                                                    </rdf:Description>
                                                </rdf:first>
                                                <rdf:rest>
                                                    <rdf:Description>
                                                        <rdf:type rdf:resource="http://www.w3.org/2003/11/swrl#AtomList"/>
                                                        <rdf:first>
                                                            <rdf:Description>
                                                                <rdf:type rdf:resource="http://www.w3.org/2003/11/swrl#ClassAtom"/>
                                                                <swrl:classPredicate rdf:resource="https://w3id.org/seas/System"/>
                                                                <swrl:argument1 rdf:resource="http://www.semanticweb.org/alencga1/ontologies/2023/2/PhenOWL/S1"/>
                                                            </rdf:Description>
                                                        </rdf:first>
                                                        <rdf:rest>
                                                            <rdf:Description>
                                                                <rdf:type rdf:resource="http://www.w3.org/2003/11/swrl#AtomList"/>
                                                                <rdf:first>
                                                                    <rdf:Description>
                                                                        <rdf:type rdf:resource="http://www.w3.org/2003/11/swrl#IndividualPropertyAtom"/>
                                                                        <swrl:propertyPredicate rdf:resource="https://w3id.org/seas/connectedTo"/>
                                                                        <swrl:argument1 rdf:resource="http://www.semanticweb.org/alencga1/ontologies/2023/2/PhenOWL/S1"/>
                                                                        <swrl:argument2 rdf:resource="http://www.semanticweb.org/alencga1/ontologies/2023/2/PhenOWL/S2"/>
                                                                    </rdf:Description>
                                                                </rdf:first>
                                                                <rdf:rest>
                                                                    <rdf:Description>
                                                                        <rdf:type rdf:resource="http://www.w3.org/2003/11/swrl#AtomList"/>
                                                                        <rdf:first>
                                                                            <rdf:Description>
                                                                                <rdf:type rdf:resource="http://www.w3.org/2003/11/swrl#ClassAtom"/>
                                                                                <swrl:classPredicate rdf:resource="http://www.w3.org/2006/time#Instant"/>
                                                                                <swrl:argument1 rdf:resource="http://www.semanticweb.org/alencga1/ontologies/2023/2/PhenOWL/t2"/>
                                                                            </rdf:Description>
                                                                        </rdf:first>
                                                                        <rdf:rest>
                                                                            <rdf:Description>
                                                                                <rdf:type rdf:resource="http://www.w3.org/2003/11/swrl#AtomList"/>
                                                                                <rdf:first>
                                                                                    <rdf:Description>
                                                                                        <rdf:type rdf:resource="http://www.w3.org/2003/11/swrl#IndividualPropertyAtom"/>
                                                                                        <swrl:propertyPredicate rdf:resource="https://w3id.org/def/propaphen#happensIn"/>
                                                                                        <swrl:argument1 rdf:resource="http://www.semanticweb.org/alencga1/ontologies/2023/2/PhenOWL/O1"/>
                                                                                        <swrl:argument2 rdf:resource="http://www.semanticweb.org/alencga1/ontologies/2023/2/PhenOWL/S1"/>
                                                                                    </rdf:Description>
                                                                                </rdf:first>
                                                                                <rdf:rest>
                                                                                    <rdf:Description>
                                                                                        <rdf:type rdf:resource="http://www.w3.org/2003/11/swrl#AtomList"/>
                                                                                        <rdf:first>
                                                                                            <rdf:Description>
                                                                                                <rdf:type rdf:resource="http://www.w3.org/2003/11/swrl#IndividualPropertyAtom"/>
                                                                                                <swrl:propertyPredicate rdf:resource="https://w3id.org/def/propaphen#happensIn"/>
                                                                                                <swrl:argument1 rdf:resource="http://www.semanticweb.org/alencga1/ontologies/2023/2/PhenOWL/O2"/>
                                                                                                <swrl:argument2 rdf:resource="http://www.semanticweb.org/alencga1/ontologies/2023/2/PhenOWL/S2"/>
                                                                                            </rdf:Description>
                                                                                        </rdf:first>
                                                                                        <rdf:rest>
                                                                                            <rdf:Description>
                                                                                                <rdf:type rdf:resource="http://www.w3.org/2003/11/swrl#AtomList"/>
                                                                                                <rdf:first>
                                                                                                    <rdf:Description>
                                                                                                        <rdf:type rdf:resource="http://www.w3.org/2003/11/swrl#IndividualPropertyAtom"/>
                                                                                                        <swrl:propertyPredicate rdf:resource="https://w3id.org/def/propaphen#observationOf"/>
                                                                                                        <swrl:argument1 rdf:resource="http://www.semanticweb.org/alencga1/ontologies/2023/2/PhenOWL/O1"/>
                                                                                                        <swrl:argument2 rdf:resource="http://www.semanticweb.org/alencga1/ontologies/2023/2/PhenOWL/OP1"/>
                                                                                                    </rdf:Description>
                                                                                                </rdf:first>
                                                                                                <rdf:rest>
                                                                                                    <rdf:Description>
                                                                                                        <rdf:type rdf:resource="http://www.w3.org/2003/11/swrl#AtomList"/>
                                                                                                        <rdf:first>
                                                                                                            <rdf:Description>
                                                                                                                <rdf:type rdf:resource="http://www.w3.org/2003/11/swrl#IndividualPropertyAtom"/>
                                                                                                                <swrl:propertyPredicate rdf:resource="https://w3id.org/def/propaphen#observationOf"/>
                                                                                                                <swrl:argument1 rdf:resource="http://www.semanticweb.org/alencga1/ontologies/2023/2/PhenOWL/O2"/>
                                                                                                                <swrl:argument2 rdf:resource="http://www.semanticweb.org/alencga1/ontologies/2023/2/PhenOWL/OP2"/>
                                                                                                            </rdf:Description>
                                                                                                        </rdf:first>
                                                                                                        <rdf:rest>
                                                                                                            <rdf:Description>
                                                                                                                <rdf:type rdf:resource="http://www.w3.org/2003/11/swrl#AtomList"/>
                                                                                                                <rdf:first>
                                                                                                                    <rdf:Description>
                                                                                                                        <rdf:type rdf:resource="http://www.w3.org/2003/11/swrl#ClassAtom"/>
                                                                                                                        <swrl:classPredicate rdf:resource="https://w3id.org/def/propaphen#Phenomenon"/>
                                                                                                                        <swrl:argument1 rdf:resource="http://www.semanticweb.org/alencga1/ontologies/2023/2/PhenOWL/P1"/>
                                                                                                                    </rdf:Description>
                                                                                                                </rdf:first>
                                                                                                                <rdf:rest>
                                                                                                                    <rdf:Description>
                                                                                                                        <rdf:type rdf:resource="http://www.w3.org/2003/11/swrl#AtomList"/>
                                                                                                                        <rdf:first>
                                                                                                                            <rdf:Description>
                                                                                                                                <rdf:type rdf:resource="http://www.w3.org/2003/11/swrl#ClassAtom"/>
                                                                                                                                <swrl:classPredicate rdf:resource="https://w3id.org/def/propaphen#Observation"/>
                                                                                                                                <swrl:argument1 rdf:resource="http://www.semanticweb.org/alencga1/ontologies/2023/2/PhenOWL/O1"/>
                                                                                                                            </rdf:Description>
                                                                                                                        </rdf:first>
                                                                                                                        <rdf:rest>
                                                                                                                            <rdf:Description>
                                                                                                                                <rdf:type rdf:resource="http://www.w3.org/2003/11/swrl#AtomList"/>
                                                                                                                                <rdf:first>
                                                                                                                                    <rdf:Description>
                                                                                                                                        <rdf:type rdf:resource="http://www.w3.org/2003/11/swrl#ClassAtom"/>
                                                                                                                                        <swrl:classPredicate rdf:resource="https://w3id.org/def/propaphen#Observation"/>
                                                                                                                                        <swrl:argument1 rdf:resource="http://www.semanticweb.org/alencga1/ontologies/2023/2/PhenOWL/O2"/>
                                                                                                                                    </rdf:Description>
                                                                                                                                </rdf:first>
                                                                                                                                <rdf:rest>
                                                                                                                                    <rdf:Description>
                                                                                                                                        <rdf:type rdf:resource="http://www.w3.org/2003/11/swrl#AtomList"/>
                                                                                                                                        <rdf:first>
                                                                                                                                            <rdf:Description>
                                                                                                                                                <rdf:type rdf:resource="http://www.w3.org/2003/11/swrl#IndividualPropertyAtom"/>
                                                                                                                                                <swrl:propertyPredicate rdf:resource="http://purl.org/nemo/gufo#hasBeginPoint"/>
                                                                                                                                                <swrl:argument1 rdf:resource="http://www.semanticweb.org/alencga1/ontologies/2023/2/PhenOWL/O1"/>
                                                                                                                                                <swrl:argument2 rdf:resource="http://www.semanticweb.org/alencga1/ontologies/2023/2/PhenOWL/t1"/>
                                                                                                                                            </rdf:Description>
                                                                                                                                        </rdf:first>
                                                                                                                                        <rdf:rest>
                                                                                                                                            <rdf:Description>
                                                                                                                                                <rdf:type rdf:resource="http://www.w3.org/2003/11/swrl#AtomList"/>
                                                                                                                                                <rdf:first>
                                                                                                                                                    <rdf:Description>
                                                                                                                                                        <rdf:type rdf:resource="http://www.w3.org/2003/11/swrl#IndividualPropertyAtom"/>
                                                                                                                                                        <swrl:propertyPredicate rdf:resource="http://purl.org/nemo/gufo#hasBeginPoint"/>
                                                                                                                                                        <swrl:argument1 rdf:resource="http://www.semanticweb.org/alencga1/ontologies/2023/2/PhenOWL/O2"/>
                                                                                                                                                        <swrl:argument2 rdf:resource="http://www.semanticweb.org/alencga1/ontologies/2023/2/PhenOWL/t2"/>
                                                                                                                                                    </rdf:Description>
                                                                                                                                                </rdf:first>
                                                                                                                                                <rdf:rest>
                                                                                                                                                    <rdf:Description>
                                                                                                                                                        <rdf:type rdf:resource="http://www.w3.org/2003/11/swrl#AtomList"/>
                                                                                                                                                        <rdf:first>
                                                                                                                                                            <rdf:Description>
                                                                                                                                                                <rdf:type rdf:resource="http://www.w3.org/2003/11/swrl#ClassAtom"/>
                                                                                                                                                                <swrl:classPredicate rdf:resource="https://w3id.org/def/propaphen#PhenomenonOccurrence"/>
                                                                                                                                                                <swrl:argument1 rdf:resource="http://www.semanticweb.org/alencga1/ontologies/2023/2/PhenOWL/OP2"/>
                                                                                                                                                            </rdf:Description>
                                                                                                                                                        </rdf:first>
                                                                                                                                                        <rdf:rest>
                                                                                                                                                            <rdf:Description>
                                                                                                                                                                <rdf:type rdf:resource="http://www.w3.org/2003/11/swrl#AtomList"/>
                                                                                                                                                                <rdf:first>
                                                                                                                                                                    <rdf:Description>
                                                                                                                                                                        <rdf:type rdf:resource="http://www.w3.org/2003/11/swrl#ClassAtom"/>
                                                                                                                                                                        <swrl:classPredicate rdf:resource="https://w3id.org/def/propaphen#PhenomenonOccurrence"/>
                                                                                                                                                                        <swrl:argument1 rdf:resource="http://www.semanticweb.org/alencga1/ontologies/2023/2/PhenOWL/OP1"/>
                                                                                                                                                                    </rdf:Description>
                                                                                                                                                                </rdf:first>
                                                                                                                                                                <rdf:rest rdf:resource="http://www.w3.org/1999/02/22-rdf-syntax-ns#nil"/>
                                                                                                                                                            </rdf:Description>
                                                                                                                                                        </rdf:rest>
                                                                                                                                                    </rdf:Description>
                                                                                                                                                </rdf:rest>
                                                                                                                                            </rdf:Description>
                                                                                                                                        </rdf:rest>
                                                                                                                                    </rdf:Description>
                                                                                                                                </rdf:rest>
                                                                                                                            </rdf:Description>
                                                                                                                        </rdf:rest>
                                                                                                                    </rdf:Description>
                                                                                                                </rdf:rest>
                                                                                                            </rdf:Description>
                                                                                                        </rdf:rest>
                                                                                                    </rdf:Description>
                                                                                                </rdf:rest>
                                                                                            </rdf:Description>
                                                                                        </rdf:rest>
                                                                                    </rdf:Description>
                                                                                </rdf:rest>
                                                                            </rdf:Description>
                                                                        </rdf:rest>
                                                                    </rdf:Description>
                                                                </rdf:rest>
                                                            </rdf:Description>
                                                        </rdf:rest>
                                                    </rdf:Description>
                                                </rdf:rest>
                                            </rdf:Description>
                                        </rdf:rest>
                                    </rdf:Description>
                                </rdf:rest>
                            </rdf:Description>
                        </rdf:rest>
                    </rdf:Description>
                </rdf:rest>
            </rdf:Description>
        </swrl:body>
        <swrl:head>
            <rdf:Description>
                <rdf:type rdf:resource="http://www.w3.org/2003/11/swrl#AtomList"/>
                <rdf:first>
                    <rdf:Description>
                        <rdf:type rdf:resource="http://www.w3.org/2003/11/swrl#IndividualPropertyAtom"/>
                        <swrl:propertyPredicate rdf:resource="https://w3id.org/def/propaphen#hasSTValidPath"/>
                        <swrl:argument1 rdf:resource="http://www.semanticweb.org/alencga1/ontologies/2023/2/PhenOWL/O1"/>
                        <swrl:argument2 rdf:resource="http://www.semanticweb.org/alencga1/ontologies/2023/2/PhenOWL/O2"/>
                    </rdf:Description>
                </rdf:first>
                <rdf:rest rdf:resource="http://www.w3.org/1999/02/22-rdf-syntax-ns#nil"/>
            </rdf:Description>
        </swrl:head>
    </rdf:Description>
    <rdf:Description>
        <swrla:isRuleEnabled rdf:datatype="http://www.w3.org/2001/XMLSchema#boolean">true</swrla:isRuleEnabled>
        <rdfs:comment rdf:datatype="http://www.w3.org/2001/XMLSchema#string">If phenomenon happens in one system, it must also happen in its super-system</rdfs:comment>
        <rdfs:label rdf:datatype="http://www.w3.org/2001/XMLSchema#string">S2 - Observation in System</rdfs:label>
        <rdf:type rdf:resource="http://www.w3.org/2003/11/swrl#Imp"/>
        <swrl:body>
            <rdf:Description>
                <rdf:type rdf:resource="http://www.w3.org/2003/11/swrl#AtomList"/>
                <rdf:first>
                    <rdf:Description>
                        <rdf:type rdf:resource="http://www.w3.org/2003/11/swrl#ClassAtom"/>
                        <swrl:classPredicate rdf:resource="https://w3id.org/seas/System"/>
                        <swrl:argument1 rdf:resource="http://www.semanticweb.org/alencga1/ontologies/2023/2/PhenOWL/S2"/>
                    </rdf:Description>
                </rdf:first>
                <rdf:rest>
                    <rdf:Description>
                        <rdf:type rdf:resource="http://www.w3.org/2003/11/swrl#AtomList"/>
                        <rdf:first>
                            <rdf:Description>
                                <rdf:type rdf:resource="http://www.w3.org/2003/11/swrl#ClassAtom"/>
                                <swrl:classPredicate rdf:resource="https://w3id.org/def/propaphen#Observation"/>
                                <swrl:argument1 rdf:resource="http://www.semanticweb.org/alencga1/ontologies/2023/2/PhenOWL/O1"/>
                            </rdf:Description>
                        </rdf:first>
                        <rdf:rest>
                            <rdf:Description>
                                <rdf:type rdf:resource="http://www.w3.org/2003/11/swrl#AtomList"/>
                                <rdf:first>
                                    <rdf:Description>
                                        <rdf:type rdf:resource="http://www.w3.org/2003/11/swrl#ClassAtom"/>
                                        <swrl:classPredicate rdf:resource="https://w3id.org/seas/System"/>
                                        <swrl:argument1 rdf:resource="http://www.semanticweb.org/alencga1/ontologies/2023/2/PhenOWL/S1"/>
                                    </rdf:Description>
                                </rdf:first>
                                <rdf:rest>
                                    <rdf:Description>
                                        <rdf:type rdf:resource="http://www.w3.org/2003/11/swrl#AtomList"/>
                                        <rdf:first>
                                            <rdf:Description>
                                                <rdf:type rdf:resource="http://www.w3.org/2003/11/swrl#IndividualPropertyAtom"/>
                                                <swrl:propertyPredicate rdf:resource="https://w3id.org/def/propaphen#happensIn"/>
                                                <swrl:argument1 rdf:resource="http://www.semanticweb.org/alencga1/ontologies/2023/2/PhenOWL/O1"/>
                                                <swrl:argument2 rdf:resource="http://www.semanticweb.org/alencga1/ontologies/2023/2/PhenOWL/S1"/>
                                            </rdf:Description>
                                        </rdf:first>
                                        <rdf:rest>
                                            <rdf:Description>
                                                <rdf:type rdf:resource="http://www.w3.org/2003/11/swrl#AtomList"/>
                                                <rdf:first>
                                                    <rdf:Description>
                                                        <rdf:type rdf:resource="http://www.w3.org/2003/11/swrl#IndividualPropertyAtom"/>
                                                        <swrl:propertyPredicate rdf:resource="https://w3id.org/seas/hasSubSystem"/>
                                                        <swrl:argument1 rdf:resource="http://www.semanticweb.org/alencga1/ontologies/2023/2/PhenOWL/S2"/>
                                                        <swrl:argument2 rdf:resource="http://www.semanticweb.org/alencga1/ontologies/2023/2/PhenOWL/S1"/>
                                                    </rdf:Description>
                                                </rdf:first>
                                                <rdf:rest rdf:resource="http://www.w3.org/1999/02/22-rdf-syntax-ns#nil"/>
                                            </rdf:Description>
                                        </rdf:rest>
                                    </rdf:Description>
                                </rdf:rest>
                            </rdf:Description>
                        </rdf:rest>
                    </rdf:Description>
                </rdf:rest>
            </rdf:Description>
        </swrl:body>
        <swrl:head>
            <rdf:Description>
                <rdf:type rdf:resource="http://www.w3.org/2003/11/swrl#AtomList"/>
                <rdf:first>
                    <rdf:Description>
                        <rdf:type rdf:resource="http://www.w3.org/2003/11/swrl#IndividualPropertyAtom"/>
                        <swrl:propertyPredicate rdf:resource="https://w3id.org/def/propaphen#happensIn"/>
                        <swrl:argument1 rdf:resource="http://www.semanticweb.org/alencga1/ontologies/2023/2/PhenOWL/O1"/>
                        <swrl:argument2 rdf:resource="http://www.semanticweb.org/alencga1/ontologies/2023/2/PhenOWL/S2"/>
                    </rdf:Description>
                </rdf:first>
                <rdf:rest rdf:resource="http://www.w3.org/1999/02/22-rdf-syntax-ns#nil"/>
            </rdf:Description>
        </swrl:head>
    </rdf:Description>
</rdf:RDF>



<!-- Generated by the OWL API (version 4.5.9.2019-02-01T07:24:44Z) https://github.com/owlcs/owlapi -->

